<?xml version="1.0" encoding="UTF-8"?>
<!DOCTYPE rdf:RDF [
  <!ENTITY Economy "http://reliant.teknowledge.com/DAML/Economy.owl#">
  <!ENTITY Economy.owl "http://reliant.teknowledge.com/DAML/Economy.owl">
  <!ENTITY Government "http://reliant.teknowledge.com/DAML/Government.owl#">
  <!ENTITY Mid-level-ontology "http://reliant.teknowledge.com/DAML/Mid-level-ontology.owl#">
  <!ENTITY SUMO "http://reliant.teknowledge.com/DAML/SUMO.owl#">
  <!ENTITY owl "http://www.w3.org/2002/07/owl#">
  <!ENTITY rdf "http://www.w3.org/1999/02/22-rdf-syntax-ns#">
  <!ENTITY rdfs "http://www.w3.org/2000/01/rdf-schema#">
  <!ENTITY xsd "http://www.w3.org/2001/XMLSchema#">
]>
<rdf:RDF xml:base="&Economy.owl;"
         xmlns:Economy="&Economy;"
         xmlns:Government="&Government;"
         xmlns:Mid-level-ontology="&Mid-level-ontology;"
         xmlns:SUMO="&SUMO;"
         xmlns:owl="&owl;"
         xmlns:rdf="&rdf;"
         xmlns:rdfs="&rdfs;">

<!-- Ontology Information -->
  <owl:Ontology rdf:about=""/>

<!-- Classes -->
  <SUMO:UnitOfMeasure rdf:about="#AfghanAfghani">
    <rdf:type rdf:resource="&owl;Class"/>
    <rdfs:comment>AfghanAfghani represents the basic unit of 

currency of Afghanistan.</rdfs:comment>
    <rdfs:subClassOf rdf:resource="&SUMO;CurrencyMeasure"/>
  </SUMO:UnitOfMeasure>

  <owl:Class rdf:about="#AgriculturalProduct">
    <rdfs:comment>AgriculturalProduct is the 

subclass of Product that comprises the products of agricultural 

activity.</rdfs:comment>
    <rdfs:subClassOf rdf:resource="&SUMO;OrganicObject"/>
    <rdfs:subClassOf rdf:resource="&SUMO;Product"/>
    <owl:disjointWith rdf:resource="#CapitalGood"/>
    <owl:disjointWith rdf:resource="#FoodProduct"/>
    <owl:disjointWith rdf:resource="#ForestProduct"/>
    <owl:disjointWith rdf:resource="#HandicraftProduct"/>
    <owl:disjointWith rdf:resource="#ManufacturedProduct"/>
    <owl:disjointWith rdf:resource="#MiningProduct"/>
    <owl:disjointWith rdf:resource="#PackagedBeverageProduct"/>
    <owl:disjointWith rdf:resource="#PackagedFoodProduct"/>
    <owl:disjointWith rdf:resource="&Mid-level-ontology;Fodder"/>
  </owl:Class>

  <owl:Class rdf:about="#Alfalfa">
    <rdfs:subClassOf rdf:resource="#PlantAgriculturalProduct"/>
    <rdfs:subClassOf rdf:resource="&Mid-level-ontology;Fodder"/>
    <rdfs:subClassOf rdf:resource="&SUMO;Plant"/>
  </owl:Class>

  <owl:Class rdf:about="#AlmondNut">
    <rdfs:subClassOf rdf:resource="#EdibleNut"/>
  </owl:Class>

  <owl:Class rdf:about="#Aloes">
    <rdfs:comment>Aloes is the class of 

PlantAgriculturalProducts that are dried juice of 

the Aloe plant.</rdfs:comment>
    <rdfs:subClassOf rdf:resource="#PlantAgriculturalProduct"/>
  </owl:Class>

  <owl:Class rdf:about="#Alumina">
    <rdf:type rdf:resource="&owl;Thing"/>
    <rdfs:comment>Alumina is the naturally occurring oxide 

of aluminum which is found in corundum and bauxite.</rdfs:comment>
    <rdfs:label>alumina</rdfs:label>
    <rdfs:label>aluminum oxide</rdfs:label>
    <rdfs:subClassOf rdf:resource="&SUMO;CompoundSubstance"/>
  </owl:Class>

  <owl:Class rdf:about="#AluminumMetal">
    <SUMO:relatedInternalConcept rdf:resource="http://reliant.teknowledge.com/DAML/elements.owl#Aluminum"/>
    <rdf:type rdf:resource="&owl;Thing"/>
    <rdfs:subClassOf rdf:resource="#MetalProduct"/>
  </owl:Class>

  <owl:Class rdf:about="#AnimalAgriculturalProduct">
    <rdfs:comment>AnimalAgriculturalProduct is the class of AgriculturalProducts 

that are animal in nature, including meat, fish, dairy products, 

hides, furs, animal fats and oils, etc.</rdfs:comment>
    <rdfs:subClassOf rdf:resource="#AgriculturalProduct"/>
    <owl:disjointWith rdf:resource="#PlantAgriculturalProduct"/>
  </owl:Class>

  <owl:Class rdf:about="#AnimalSkin">
    <rdfs:comment>AnimalSkin is the subclass of 

BodyCovering that includes the skins, or parts of skins, 

of animals.</rdfs:comment>
    <rdfs:subClassOf rdf:resource="&SUMO;BodyCovering"/>
  </owl:Class>

  <owl:Class rdf:about="#Apple">
    <rdfs:subClassOf rdf:resource="#Fruit"/>
    <rdfs:subClassOf rdf:resource="#GroceryProduce"/>
  </owl:Class>

  <owl:Class rdf:about="#Asphalt">
    <rdf:type rdf:resource="&owl;Thing"/>
    <rdfs:comment>Asphalt is the subclass of 

RefinedPetroleumProducts that are asphalts.</rdfs:comment>
    <rdfs:subClassOf rdf:resource="#RefinedPetroleumProduct"/>
  </owl:Class>

  <owl:Class rdf:about="#BalsaWood">
    <rdfs:subClassOf rdf:resource="#WoodProduct"/>
  </owl:Class>

  <owl:Class rdf:about="#Banana">
    <rdfs:subClassOf rdf:resource="#GroceryProduce"/>
    <rdfs:subClassOf rdf:resource="#TropicalFruit"/>
  </owl:Class>

  <owl:Class rdf:about="#BarleyGrain">
    <rdf:type rdf:resource="&owl;Thing"/>
    <rdfs:subClassOf rdf:resource="&Mid-level-ontology;CerealGrain"/>
  </owl:Class>

  <owl:Class rdf:about="#Bean">
    <rdfs:subClassOf rdf:resource="#Legume"/>
  </owl:Class>

  <owl:Class rdf:about="#Berry">
    <rdfs:subClassOf rdf:resource="#Fruit"/>
    <rdfs:subClassOf rdf:resource="#GroceryProduce"/>
  </owl:Class>

  <owl:Class rdf:about="#BeverageProduct">
    <rdfs:comment>BeverageProduct is the class of products 

that are Beverages, packaged or unpackaged.</rdfs:comment>
    <rdfs:subClassOf rdf:resource="&SUMO;Product"/>
    <owl:disjointWith rdf:resource="#CapitalGood"/>
    <owl:disjointWith rdf:resource="#FoodProduct"/>
    <owl:disjointWith rdf:resource="#ForestProduct"/>
    <owl:disjointWith rdf:resource="#HandicraftProduct"/>
    <owl:disjointWith rdf:resource="#ManufacturedProduct"/>
    <owl:disjointWith rdf:resource="#MiningProduct"/>
    <owl:disjointWith rdf:resource="#PackagedBeverageProduct"/>
    <owl:disjointWith rdf:resource="#PackagedFoodProduct"/>
  </owl:Class>

  <owl:Class rdf:about="#BlackPepper">
    <rdfs:subClassOf rdf:resource="#Spice"/>
  </owl:Class>

  <owl:Class rdf:about="#Breadfruit">
    <rdfs:subClassOf rdf:resource="#GroceryProduce"/>
    <rdfs:subClassOf rdf:resource="#TropicalFruit"/>
  </owl:Class>

  <SUMO:UnitOfMeasure rdf:about="#BritishPound">
    <rdf:type rdf:resource="&owl;Class"/>
    <rdfs:comment>BritishPound represents the basic unit of 

currency of the UnitedKingdomOfGreatBritainAndNorthernIreland.</rdfs:comment>
    <rdfs:subClassOf rdf:resource="&SUMO;CurrencyMeasure"/>
  </SUMO:UnitOfMeasure>

  <owl:Class rdf:about="#Cabbage">
    <rdfs:subClassOf rdf:resource="#GroceryProduce"/>
    <rdfs:subClassOf rdf:resource="#Vegetable"/>
  </owl:Class>

  <owl:Class rdf:about="#Camel">
    <rdfs:subClassOf rdf:resource="#Livestock"/>
    <rdfs:subClassOf rdf:resource="&SUMO;Mammal"/>
  </owl:Class>

  <SUMO:UnitOfMeasure rdf:about="#CanadianDollar">
    <rdf:type rdf:resource="&owl;Class"/>
    <rdfs:comment>CanadianDollar represents the basic unit of 

currency of Canada.</rdfs:comment>
    <rdfs:subClassOf rdf:resource="&SUMO;CurrencyMeasure"/>
  </SUMO:UnitOfMeasure>

  <owl:Class rdf:about="#Cannabis">
    <rdfs:subClassOf rdf:resource="#PlantAgriculturalProduct"/>
  </owl:Class>

  <owl:Class rdf:about="#CapitalGood">
    <rdfs:comment>CapitalGoods are those that are used 

in the production of other Products.  For example, raw materials 

from which end products are manufactured, or machines and other 

structures used in the production process.</rdfs:comment>
    <rdfs:subClassOf rdf:resource="&SUMO;Product"/>
    <owl:disjointWith rdf:resource="#AgriculturalProduct"/>
    <owl:disjointWith rdf:resource="#BeverageProduct"/>
    <owl:disjointWith rdf:resource="#FoodProduct"/>
    <owl:disjointWith rdf:resource="#ForestProduct"/>
    <owl:disjointWith rdf:resource="#HandicraftProduct"/>
    <owl:disjointWith rdf:resource="#ManufacturedProduct"/>
    <owl:disjointWith rdf:resource="#MiningProduct"/>
    <owl:disjointWith rdf:resource="#PackagedBeverageProduct"/>
    <owl:disjointWith rdf:resource="#PackagedFoodProduct"/>
  </owl:Class>

  <owl:Class rdf:about="#Cardamom">
    <rdfs:subClassOf rdf:resource="#Spice"/>
  </owl:Class>

  <owl:Class rdf:about="#Carrot">
    <rdfs:subClassOf rdf:resource="#GroceryProduce"/>
    <rdfs:subClassOf rdf:resource="#RootVegetable"/>
  </owl:Class>

  <owl:Class rdf:about="#CashewNut">
    <rdfs:subClassOf rdf:resource="#EdibleNut"/>
  </owl:Class>

  <owl:Class rdf:about="#Cassava">
    <rdfs:label>cassava</rdfs:label>
    <rdfs:label>manioc</rdfs:label>
    <rdfs:label>tapioca</rdfs:label>
    <rdfs:subClassOf rdf:resource="#GroceryProduce"/>
    <rdfs:subClassOf rdf:resource="#RootVegetable"/>
  </owl:Class>

  <owl:Class rdf:about="#Cattle">
    <rdf:type rdf:resource="&owl;Thing"/>
    <rdfs:subClassOf rdf:resource="#Livestock"/>
    <rdfs:subClassOf rdf:resource="&SUMO;HoofedMammal"/>
  </owl:Class>

  <owl:Class rdf:about="#Cauliflower">
    <rdfs:subClassOf rdf:resource="#GroceryProduce"/>
    <rdfs:subClassOf rdf:resource="#Vegetable"/>
  </owl:Class>

  <owl:Class rdf:about="#Caviar">
    <rdfs:subClassOf rdf:resource="#FishRoe"/>
  </owl:Class>

  <owl:Class rdf:about="#CerealGrass">
    <rdfs:subClassOf rdf:resource="&Mid-level-ontology;Grass"/>
  </owl:Class>

  <owl:Class rdf:about="#Cheese">
    <rdfs:subClassOf rdf:resource="#DairyProduct"/>
  </owl:Class>

  <owl:Class rdf:about="#ChemicalProduct">
    <rdf:type rdf:resource="&owl;Thing"/>
    <rdfs:comment>ChemicalProduct is the subclass 

of Product comprising all chemical compounds that are end products 

or industrial products used in the manufacture of end products.</rdfs:comment>
    <rdfs:subClassOf rdf:resource="#ManufacturedProduct"/>
    <rdfs:subClassOf rdf:resource="&SUMO;CompoundSubstance"/>
  </owl:Class>

  <owl:Class rdf:about="#Chrysanthemum">
    <SUMO:relatedInternalConcept rdf:resource="#Pyrethrum"/>
    <rdf:type rdf:resource="&owl;Thing"/>
    <rdfs:subClassOf rdf:resource="#PlantAgriculturalProduct"/>
    <rdfs:subClassOf rdf:resource="&SUMO;FloweringPlant"/>
  </owl:Class>

  <owl:Class rdf:about="#Cinnamon">
    <rdfs:subClassOf rdf:resource="#Spice"/>
  </owl:Class>

  <owl:Class rdf:about="#CitrusFruit">
    <rdfs:subClassOf rdf:resource="#Fruit"/>
    <rdfs:subClassOf rdf:resource="#GroceryProduce"/>
  </owl:Class>

  <owl:Class rdf:about="#ClothesDrier">
    <rdfs:comment>ClothesDrier is the class of automatic clothes 

driers.</rdfs:comment>
    <rdfs:subClassOf rdf:resource="#MajorAppliance"/>
  </owl:Class>

  <owl:Class rdf:about="#ClothesWashingMachine">
    <rdfs:comment>ClothesWashingMachine is the class of 

washing machines.</rdfs:comment>
    <rdfs:subClassOf rdf:resource="#MajorAppliance"/>
  </owl:Class>

  <owl:Class rdf:about="#Clove">
    <rdfs:subClassOf rdf:resource="#Spice"/>
  </owl:Class>

  <owl:Class rdf:about="#Clover">
    <rdfs:subClassOf rdf:resource="#PlantAgriculturalProduct"/>
    <rdfs:subClassOf rdf:resource="&Mid-level-ontology;Fodder"/>
    <rdfs:subClassOf rdf:resource="&SUMO;Plant"/>
  </owl:Class>

  <owl:Class rdf:about="#Coca">
    <rdfs:comment>Coca is the class of 

PlantAgriculturalProducts consisting of the parts, 

especially leaves, of the coca plant.  Coca leaves 

are the source of Cocaine.</rdfs:comment>
    <rdfs:subClassOf rdf:resource="#PlantAgriculturalProduct"/>
  </owl:Class>

  <owl:Class rdf:about="#Cocaine">
    <rdfs:subClassOf rdf:resource="#PlantAgriculturalProduct"/>
    <rdfs:subClassOf rdf:resource="&Mid-level-ontology;Narcotic"/>
  </owl:Class>

  <owl:Class rdf:about="#Cocoa">
    <rdf:type rdf:resource="&owl;Thing"/>
    <rdfs:comment>Cocoa is the class of powdered 

PlantAgriculturalProduct derived from cacao beans.</rdfs:comment>
    <rdfs:subClassOf rdf:resource="#PlantAgriculturalProduct"/>
    <rdfs:subClassOf rdf:resource="&SUMO;FruitOrVegetable"/>
  </owl:Class>

  <owl:Class rdf:about="#CocoaBean">
    <SUMO:relatedInternalConcept rdf:resource="#Cocoa"/>
    <rdf:type rdf:resource="&owl;Thing"/>
    <rdfs:subClassOf rdf:resource="#PlantAgriculturalProduct"/>
    <rdfs:subClassOf rdf:resource="&SUMO;FruitOrVegetable"/>
  </owl:Class>

  <owl:Class rdf:about="#Coconut">
    <rdfs:subClassOf rdf:resource="#GroceryProduce"/>
    <rdfs:subClassOf rdf:resource="#TropicalFruit"/>
  </owl:Class>

  <owl:Class rdf:about="#CoffeeBean">
    <rdfs:subClassOf rdf:resource="#PlantAgriculturalProduct"/>
    <rdfs:subClassOf rdf:resource="&SUMO;FruitOrVegetable"/>
  </owl:Class>

  <owl:Class rdf:about="#ConsumerGood">
    <SUMO:disjoint rdf:resource="#DurableGood"/>
    <rdf:type rdf:resource="&owl;Thing"/>
    <rdfs:comment>ConsumerGood is the subclass of 

ManufacturedProducts that are intended for immediate or short-term 

consumption.</rdfs:comment>
    <rdfs:subClassOf rdf:resource="#ManufacturedProduct"/>
  </owl:Class>

  <owl:Class rdf:about="#CookingOven">
    <rdfs:comment>CookingOven is the class of ovens for cooking.</rdfs:comment>
    <rdfs:subClassOf rdf:resource="#MajorAppliance"/>
  </owl:Class>

  <owl:Class rdf:about="#CookingRange">
    <rdfs:comment>CookingRange is the class of cooktops or 

ranges.</rdfs:comment>
    <rdfs:subClassOf rdf:resource="#MajorAppliance"/>
  </owl:Class>

  <owl:Class rdf:about="#CopperOre">
    <rdf:type rdf:resource="&owl;Thing"/>
    <rdfs:subClassOf rdf:resource="#MiningProduct"/>
    <rdfs:subClassOf rdf:resource="&SUMO;Mineral"/>
  </owl:Class>

  <owl:Class rdf:about="#Copra">
    <SUMO:relatedInternalConcept rdf:resource="#VegetableOil"/>
    <rdf:type rdf:resource="&owl;Thing"/>
    <rdfs:comment>Copra is the class of dried coconut 

meat valued for the extracted coconut oil.</rdfs:comment>
    <rdfs:subClassOf rdf:resource="#PlantAgriculturalProduct"/>
  </owl:Class>

  <owl:Class rdf:about="#Corn">
    <SUMO:relatedInternalConcept rdf:resource="#MaizeGrain"/>
    <rdf:type rdf:resource="&owl;Thing"/>
    <rdfs:subClassOf rdf:resource="#GroceryProduce"/>
    <rdfs:subClassOf rdf:resource="#Vegetable"/>
  </owl:Class>

  <owl:Class rdf:about="#CottonFiber">
    <rdf:type rdf:resource="&owl;Thing"/>
    <rdfs:subClassOf rdf:resource="#PlantAgriculturalProduct"/>
  </owl:Class>

  <owl:Class rdf:about="#CowPea">
    <rdfs:subClassOf rdf:resource="#Legume"/>
  </owl:Class>

  <owl:Class rdf:about="#Crayfish">
    <rdfs:subClassOf rdf:resource="#Shellfish"/>
  </owl:Class>

  <Economy:IndustryAttribute rdf:about="#CropProduction">
    <Mid-level-ontology:industryProductType rdf:resource="&SUMO;Plant"/>
    <SUMO:subAttribute rdf:resource="#AgriculturalSector"/>
    <rdf:type rdf:resource="&owl;Class"/>
    <rdfs:comment>CropProduction is the IndustryAttribute 

that describes crop farming operations.</rdfs:comment>
  </Economy:IndustryAttribute>

  <owl:Class rdf:about="#Cucumber">
    <rdfs:subClassOf rdf:resource="#GroceryProduce"/>
    <rdfs:subClassOf rdf:resource="#Vegetable"/>
  </owl:Class>

  <owl:Class rdf:about="#CutFlower">
    <SUMO:relatedInternalConcept rdf:resource="&SUMO;FloweringPlant"/>
    <rdf:type rdf:resource="&owl;Thing"/>
    <rdfs:subClassOf rdf:resource="#PlantAgriculturalProduct"/>
  </owl:Class>

  <owl:Class rdf:about="#DairyProduct">
    <rdfs:subClassOf rdf:resource="#AnimalAgriculturalProduct"/>
  </owl:Class>

  <owl:Class rdf:about="#Deer">
    <rdfs:subClassOf rdf:resource="#Livestock"/>
    <rdfs:subClassOf rdf:resource="&SUMO;HoofedMammal"/>
  </owl:Class>

  <owl:Class rdf:about="#Dishwasher">
    <rdfs:comment>Dishwasher is the class of automatic dishwashers.</rdfs:comment>
    <rdfs:subClassOf rdf:resource="#MajorAppliance"/>
  </owl:Class>

  <owl:Class rdf:about="#Duck">
    <rdfs:subClassOf rdf:resource="#Poultry"/>
  </owl:Class>

  <owl:Class rdf:about="#DurableGood">
    <rdf:type rdf:resource="&owl;Thing"/>
    <rdfs:comment>DurableGood is the subclass of 

ManufacturedProducts which are designed to last for three years 

or more.</rdfs:comment>
    <rdfs:subClassOf rdf:resource="#ManufacturedProduct"/>
  </owl:Class>

  <owl:Class rdf:about="#EconomicDevelopmentLevel">
    <rdfs:comment>EconomicDevelopmentLevel is a subclass of EconomicAttribute  

containing terms used to describe the economic development level of a 

Nation or GeopoliticalArea.  This class is further subdivided into 

different scales devised or used by different agencies.</rdfs:comment>
    <rdfs:subClassOf rdf:resource="&Mid-level-ontology;EconomicAttribute"/>
  </owl:Class>

  <owl:Class rdf:about="#EconomicSector">
    <rdfs:comment>EconomicSector is the subclass of 

IndustryAttributes that describe broad characterizations of different 

kinds of business activities; e.g., manufacturing; services; retail trade; 

wholesale trade; finance, insurance, and real estate; transportation and 

utilities; construction; mining; agriculture, forestry, and fishing.</rdfs:comment>
    <rdfs:subClassOf rdf:resource="#IndustryAttribute"/>
  </owl:Class>

  <owl:Class rdf:about="#EdibleNut">
    <rdf:type rdf:resource="&owl;Thing"/>
    <rdfs:subClassOf rdf:resource="#GroceryProduce"/>
    <rdfs:subClassOf rdf:resource="&SUMO;FruitOrVegetable"/>
  </owl:Class>

  <owl:Class rdf:about="#EdibleTuber">
    <rdfs:subClassOf rdf:resource="#PlantAgriculturalProduct"/>
    <rdfs:subClassOf rdf:resource="#RootVegetable"/>
  </owl:Class>

  <owl:Class rdf:about="#Eggplant">
    <rdfs:subClassOf rdf:resource="#GroceryProduce"/>
    <rdfs:subClassOf rdf:resource="#Vegetable"/>
  </owl:Class>

  <owl:Class rdf:about="#ElectricalPowerGeneration">
    <Mid-level-ontology:industryProductType rdf:resource="#Electricity"/>
    <rdf:type rdf:resource="&owl;Thing"/>
    <rdfs:comment>ElectricalPowerGeneration is 

the subclass of PowerGeneration processes in which electricity is 

generated.</rdfs:comment>
    <rdfs:subClassOf rdf:resource="#PowerGeneration"/>
  </owl:Class>

  <owl:Class rdf:about="#Electricity">
    <rdf:type rdf:resource="&owl;Thing"/>
    <rdfs:subClassOf rdf:resource="&SUMO;Substance"/>
  </owl:Class>

  <owl:Class rdf:about="#Fertilizer">
    <SUMO:relatedInternalConcept rdf:resource="#PhosphoricAcid"/>
    <SUMO:relatedInternalConcept rdf:resource="http://reliant.teknowledge.com/DAML/Geography.owl#Potash"/>
    <SUMO:relatedInternalConcept rdf:resource="&Mid-level-ontology;Nitrogen"/>
    <rdf:type rdf:resource="&owl;Thing"/>
    <rdfs:comment>Fertilizer is the subclass of ChemicalProducts 

that are used in Agriculture to enrich soils to produce more or better 

quality crop yields.</rdfs:comment>
    <rdfs:subClassOf rdf:resource="#ChemicalProduct"/>
    <rdfs:subClassOf rdf:resource="&SUMO;Mixture"/>
  </owl:Class>

  <owl:Class rdf:about="#FinancialSectorAttribute">
    <rdfs:comment>FinancialSectorAttribute is 

a class of Attributes that are used to indicate which financial sectors 

are most important in the economy of a Nation or GeopoliticalArea.  

These terms classify nations (or areas) according to the concentration of 

their economy into one or more EconomicSectors.  See also EconomicSector 

and IndustryAttribute, which classify business organizations into sectors.</rdfs:comment>
    <rdfs:subClassOf rdf:resource="&Mid-level-ontology;EconomicAttribute"/>
  </owl:Class>

  <owl:Class rdf:about="#FishProduct">
    <SUMO:relatedInternalConcept rdf:resource="#FoodFish"/>
    <rdf:type rdf:resource="&owl;Thing"/>
    <rdfs:comment>FishProduct is the subclass of 

AnimalAgriculturalProduct that comprises products derived  

from fish.</rdfs:comment>
    <rdfs:subClassOf rdf:resource="#AnimalAgriculturalProduct"/>
  </owl:Class>

  <owl:Class rdf:about="#FishRoe">
    <rdfs:subClassOf rdf:resource="#FishProduct"/>
  </owl:Class>

  <owl:Class rdf:about="#FlaxFiber">
    <rdfs:subClassOf rdf:resource="#PlantAgriculturalProduct"/>
  </owl:Class>

  <owl:Class rdf:about="#FoodEgg">
    <rdfs:subClassOf rdf:resource="#AnimalAgriculturalProduct"/>
  </owl:Class>

  <owl:Class rdf:about="#FoodFish">
    <rdf:type rdf:resource="&owl;Thing"/>
    <rdfs:subClassOf rdf:resource="#Seafood"/>
  </owl:Class>

  <owl:Class rdf:about="#FoodProduct">
    <rdf:type rdf:resource="&owl;Thing"/>
    <rdfs:comment>FoodProduct is the class of food 

products, packaged or unpackaged.</rdfs:comment>
    <rdfs:subClassOf rdf:resource="&SUMO;Product"/>
    <owl:disjointWith rdf:resource="#AgriculturalProduct"/>
    <owl:disjointWith rdf:resource="#BeverageProduct"/>
    <owl:disjointWith rdf:resource="#CapitalGood"/>
    <owl:disjointWith rdf:resource="#ForestProduct"/>
    <owl:disjointWith rdf:resource="#HandicraftProduct"/>
    <owl:disjointWith rdf:resource="#ManufacturedProduct"/>
    <owl:disjointWith rdf:resource="#MiningProduct"/>
    <owl:disjointWith rdf:resource="#PackagedBeverageProduct"/>
    <owl:disjointWith rdf:resource="#PackagedFoodProduct"/>
  </owl:Class>

  <owl:Class rdf:about="#Footwear">
    <rdf:type rdf:resource="&owl;Thing"/>
    <rdfs:comment>Footwear is the subclass of Clothing that 

includes shoes, boots, slippers, and other clothing designed to be worn 

on feet.</rdfs:comment>
    <rdfs:subClassOf rdf:resource="&SUMO;Clothing"/>
  </owl:Class>

  <owl:Class rdf:about="#ForageCrop">
    <rdfs:subClassOf rdf:resource="#PlantAgriculturalProduct"/>
    <rdfs:subClassOf rdf:resource="&Mid-level-ontology;Fodder"/>
    <rdfs:subClassOf rdf:resource="&SUMO;Plant"/>
  </owl:Class>

  <owl:Class rdf:about="#ForestProduct">
    <rdf:type rdf:resource="&owl;Thing"/>
    <rdfs:subClassOf rdf:resource="&SUMO;Product"/>
    <owl:disjointWith rdf:resource="#AgriculturalProduct"/>
    <owl:disjointWith rdf:resource="#BeverageProduct"/>
    <owl:disjointWith rdf:resource="#CapitalGood"/>
    <owl:disjointWith rdf:resource="#FoodProduct"/>
    <owl:disjointWith rdf:resource="#HandicraftProduct"/>
    <owl:disjointWith rdf:resource="#ManufacturedProduct"/>
    <owl:disjointWith rdf:resource="#MiningProduct"/>
    <owl:disjointWith rdf:resource="#PackagedBeverageProduct"/>
    <owl:disjointWith rdf:resource="#PackagedFoodProduct"/>
  </owl:Class>

  <owl:Class rdf:about="#Freezer">
    <rdf:type rdf:resource="&owl;Thing"/>
    <rdfs:comment>Freezer is the class of household freezers.</rdfs:comment>
    <rdfs:subClassOf rdf:resource="#MajorAppliance"/>
  </owl:Class>

  <SUMO:UnitOfMeasure rdf:about="#FrenchFranc">
    <rdf:type rdf:resource="&owl;Class"/>
    <rdfs:comment>FrenchFranc represents the basic unit of 

currency of France.</rdfs:comment>
    <rdfs:subClassOf rdf:resource="&SUMO;CurrencyMeasure"/>
  </SUMO:UnitOfMeasure>

  <owl:Class rdf:about="#Fruit">
    <rdf:type rdf:resource="&owl;Thing"/>
    <rdfs:subClassOf rdf:resource="&SUMO;FruitOrVegetable"/>
    <owl:disjointWith rdf:resource="#GroceryProduce"/>
    <owl:disjointWith rdf:resource="#RootStarch"/>
    <owl:disjointWith rdf:resource="#RootVegetable"/>
  </owl:Class>

  <owl:Class rdf:about="#Gemstone">
    <rdfs:comment>Gemstone is the subclass of Minerals or 

petrified organic substances that are especially valued for use in 

jewelry and other decorative items; some Gemstones are also valuable 

for mechanical or industrial applications.</rdfs:comment>
    <rdfs:subClassOf rdf:resource="&SUMO;Object"/>
  </owl:Class>

  <SUMO:UnitOfMeasure rdf:about="#GermanMark">
    <rdf:type rdf:resource="&owl;Class"/>
    <rdfs:comment>GermanMark represents the basic unit of 

currency of Germany.</rdfs:comment>
    <rdfs:subClassOf rdf:resource="&SUMO;CurrencyMeasure"/>
  </SUMO:UnitOfMeasure>

  <owl:Class rdf:about="#Ginger">
    <rdfs:subClassOf rdf:resource="#Spice"/>
    <rdfs:subClassOf rdf:resource="#Vegetable"/>
  </owl:Class>

  <owl:Class rdf:about="#Goose">
    <rdfs:subClassOf rdf:resource="#Poultry"/>
  </owl:Class>

  <owl:Class rdf:about="#Grape">
    <rdf:type rdf:resource="&owl;Thing"/>
    <rdfs:subClassOf rdf:resource="#Fruit"/>
    <rdfs:subClassOf rdf:resource="#GroceryProduce"/>
  </owl:Class>

  <owl:Class rdf:about="#GreenPepper">
    <rdfs:subClassOf rdf:resource="#GroceryProduce"/>
    <rdfs:subClassOf rdf:resource="#Vegetable"/>
  </owl:Class>

  <owl:Class rdf:about="#GroceryProduce">
    <rdfs:subClassOf rdf:resource="#PlantAgriculturalProduct"/>
    <rdfs:subClassOf rdf:resource="&SUMO;FruitOrVegetable"/>
    <owl:disjointWith rdf:resource="#Fruit"/>
    <owl:disjointWith rdf:resource="#RootStarch"/>
    <owl:disjointWith rdf:resource="#RootVegetable"/>
    <owl:disjointWith rdf:resource="#Spice"/>
    <owl:disjointWith rdf:resource="#TeaPlantAerialPart"/>
    <owl:disjointWith rdf:resource="#Vegetable"/>
    <owl:disjointWith rdf:resource="&SUMO;Seed"/>
  </owl:Class>

  <owl:Class rdf:about="#Groundnut">
    <rdfs:subClassOf rdf:resource="#EdibleTuber"/>
    <rdfs:subClassOf rdf:resource="#GroceryProduce"/>
    <rdfs:subClassOf rdf:resource="&SUMO;FruitOrVegetable"/>
  </owl:Class>

  <owl:Class rdf:about="#GuernseyCattle">
    <rdfs:subClassOf rdf:resource="#Cattle"/>
  </owl:Class>

  <owl:Class rdf:about="#GumArabic">
    <rdfs:subClassOf rdf:resource="#PlantAgriculturalProduct"/>
    <rdfs:subClassOf rdf:resource="&SUMO;Substance"/>
  </owl:Class>

  <owl:Class rdf:about="#HandicraftProduct">
    <rdfs:comment>HandicraftProduct is the class of 

Products that are manufactured by hand with a special skill.</rdfs:comment>
    <rdfs:subClassOf rdf:resource="&SUMO;Product"/>
    <owl:disjointWith rdf:resource="#AgriculturalProduct"/>
    <owl:disjointWith rdf:resource="#BeverageProduct"/>
    <owl:disjointWith rdf:resource="#CapitalGood"/>
    <owl:disjointWith rdf:resource="#FoodProduct"/>
    <owl:disjointWith rdf:resource="#ForestProduct"/>
    <owl:disjointWith rdf:resource="#ManufacturedProduct"/>
    <owl:disjointWith rdf:resource="#MiningProduct"/>
    <owl:disjointWith rdf:resource="#PackagedBeverageProduct"/>
    <owl:disjointWith rdf:resource="#PackagedFoodProduct"/>
  </owl:Class>

  <owl:Class rdf:about="#HandwovenCarpet">
    <rdf:type rdf:resource="&owl;Thing"/>
    <rdfs:comment>HandwovenCarpet is the class of carpets 

that are woven, tied, knitted, or otherwise manufactured by hand.</rdfs:comment>
    <rdfs:subClassOf rdf:resource="#HandicraftProduct"/>
    <rdfs:subClassOf rdf:resource="#TextileProduct"/>
  </owl:Class>

  <owl:Class rdf:about="#Hardwood">
    <rdfs:subClassOf rdf:resource="#WoodProduct"/>
  </owl:Class>

  <owl:Class rdf:about="#HempFiber">
    <rdfs:subClassOf rdf:resource="#PlantAgriculturalProduct"/>
  </owl:Class>

  <owl:Class rdf:about="#HotWaterHeater">
    <rdfs:comment>HotWaterHeater is the class of hot water 

heaters.</rdfs:comment>
    <rdfs:subClassOf rdf:resource="#MajorAppliance"/>
  </owl:Class>

  <owl:Class rdf:about="#IMFDevelopmentLevel">
    <rdfs:comment>IMFDevelopmentLevel is a 

collection of Attributes representing economic development levels 

used by the InternationalMonetaryFund (IMF) to characterize national 

economies.  The hierarchy of IMF levels includes: AdvancedEconomy, 

CountryInTransition, and DevelopingCountry.  There is some, but not  

complete, overlap with concepts used by UnitedNations agencies.  

See</rdfs:comment>
    <rdfs:subClassOf rdf:resource="#EconomicDevelopmentLevel"/>
  </owl:Class>

  <owl:Class rdf:about="#IndustrialRawMaterial">
    <rdfs:comment>IndustrialRawMaterial is the 

subclass of objects or substances that are used as inputs to manufacturing 

or other industrial processes.  IndustrialRawMaterials are resources 

and as such are consumed in the process for which they are used.</rdfs:comment>
    <rdfs:subClassOf rdf:resource="#CapitalGood"/>
  </owl:Class>

  <owl:Class rdf:about="#IndustrialSupply">
    <rdfs:comment>IndustrialSupply is the class of 

products that are used in industry but which are not raw materials 

for products being manufactured.  IndustrialSupply includes maintenance, 

repair, and operation (MRO) supplies, including janitorial, electrical, 

bearings, tools, machinery, accessories, fire and safety equipment, and 

other industrial items.</rdfs:comment>
    <rdfs:subClassOf rdf:resource="#CapitalGood"/>
    <rdfs:subClassOf rdf:resource="#ManufacturedProduct"/>
  </owl:Class>

  <owl:Class rdf:about="#IndustryAttribute">
    <rdfs:comment>IndustryAttribute is a class of 

Attributes which identify an Organization as belonging to a particular 

industry type.  For example, the company Hallmark has the attribute 

of GreetingCardPublishers.</rdfs:comment>
    <rdfs:subClassOf rdf:resource="&SUMO;RelationalAttribute"/>
  </owl:Class>

  <owl:Class rdf:about="#IronMetal">
    <SUMO:relatedInternalConcept rdf:resource="&Mid-level-ontology;Iron"/>
    <rdf:type rdf:resource="&owl;Thing"/>
    <rdfs:subClassOf rdf:resource="#MetalProduct"/>
  </owl:Class>

  <SUMO:UnitOfMeasure rdf:about="#ItalianLire">
    <rdf:type rdf:resource="&owl;Class"/>
    <rdfs:comment>ItalianLire represents the basic unit of 

currency of Italy.</rdfs:comment>
    <rdfs:subClassOf rdf:resource="&SUMO;CurrencyMeasure"/>
  </SUMO:UnitOfMeasure>

  <SUMO:UnitOfMeasure rdf:about="#JapaneseYen">
    <rdf:type rdf:resource="&owl;Class"/>
    <rdfs:comment>JapaneseYen represents the basic unit of 

currency of Japan.</rdfs:comment>
    <rdfs:subClassOf rdf:resource="&SUMO;CurrencyMeasure"/>
  </SUMO:UnitOfMeasure>

  <owl:Class rdf:about="#Jewelry">
    <rdfs:comment>Jewelry is the subclass of WearableItems 

that are worn primarily for decorative purposes (sometimes with social 

significance, e.g., wedding rings).  Jewelry may be made of metals 

(especially precious metals), gems, or other materials.</rdfs:comment>
    <rdfs:subClassOf rdf:resource="#WearableItem"/>
  </owl:Class>

  <owl:Class rdf:about="#JuteFiber">
    <rdfs:subClassOf rdf:resource="#PlantAgriculturalProduct"/>
  </owl:Class>

  <owl:Class rdf:about="#KentiaPalmSeed">
    <rdfs:subClassOf rdf:resource="#PlantAgriculturalProduct"/>
    <rdfs:subClassOf rdf:resource="&SUMO;Seed"/>
  </owl:Class>

  <owl:Class rdf:about="#Khat">
    <rdfs:comment>Khat is the class of PlantAgriculturalProducts 

made from the leaves and buds of the staff tree, which 

are chewed or brewed as a stimulating tea.</rdfs:comment>
    <rdfs:label>khat</rdfs:label>
    <rdfs:label>qat</rdfs:label>
    <rdfs:subClassOf rdf:resource="#PlantAgriculturalProduct"/>
  </owl:Class>

  <owl:Class rdf:about="#LambMeat">
    <rdfs:subClassOf rdf:resource="#MeatOfLandAnimal"/>
  </owl:Class>

  <owl:Class rdf:about="#Lambskin">
    <rdfs:subClassOf rdf:resource="#Pelt"/>
  </owl:Class>

  <owl:Class rdf:about="#LeadMetal">
    <SUMO:relatedInternalConcept rdf:resource="&Mid-level-ontology;Lead"/>
    <rdf:type rdf:resource="&owl;Thing"/>
    <rdfs:subClassOf rdf:resource="#MetalProduct"/>
  </owl:Class>

  <owl:Class rdf:about="#LeadOre">
    <rdf:type rdf:resource="&owl;Thing"/>
    <rdfs:subClassOf rdf:resource="#MiningProduct"/>
    <rdfs:subClassOf rdf:resource="&SUMO;Mineral"/>
  </owl:Class>

  <owl:Class rdf:about="#LeadProduct">
    <rdf:type rdf:resource="&owl;Thing"/>
    <rdfs:subClassOf rdf:resource="#LeadMetal"/>
    <rdfs:subClassOf rdf:resource="#ManufacturedProduct"/>
  </owl:Class>

  <owl:Class rdf:about="#Leaf">
    <rdfs:subClassOf rdf:resource="&SUMO;AnatomicalStructure"/>
  </owl:Class>

  <owl:Class rdf:about="#LeafyGreenVegetable">
    <rdfs:subClassOf rdf:resource="#GroceryProduce"/>
    <rdfs:subClassOf rdf:resource="#Vegetable"/>
  </owl:Class>

  <owl:Class rdf:about="#Legume">
    <rdfs:subClassOf rdf:resource="#PlantAgriculturalProduct"/>
    <rdfs:subClassOf rdf:resource="#Vegetable"/>
  </owl:Class>

  <owl:Class rdf:about="#Lemon">
    <rdfs:subClassOf rdf:resource="#CitrusFruit"/>
  </owl:Class>

  <owl:Class rdf:about="#Lentil">
    <rdfs:subClassOf rdf:resource="#Legume"/>
  </owl:Class>

  <owl:Class rdf:about="#Lime">
    <rdfs:subClassOf rdf:resource="#CitrusFruit"/>
  </owl:Class>

  <owl:Class rdf:about="#Livestock">
    <rdfs:comment>Livestock is the class of live animals 

raised as AgriculturalProducts.</rdfs:comment>
    <rdfs:subClassOf rdf:resource="#AnimalAgriculturalProduct"/>
  </owl:Class>

  <owl:Class rdf:about="#Lumber">
    <rdfs:subClassOf rdf:resource="#DurableGood"/>
    <rdfs:subClassOf rdf:resource="#ForestProduct"/>
    <rdfs:subClassOf rdf:resource="#ManufacturedProduct"/>
  </owl:Class>

  <owl:Class rdf:about="#MacademiaNut">
    <rdfs:subClassOf rdf:resource="#EdibleNut"/>
  </owl:Class>

  <owl:Class rdf:about="#Mace">
    <rdfs:subClassOf rdf:resource="#Spice"/>
  </owl:Class>

  <owl:Class rdf:about="#MachineTool">
    <rdf:type rdf:resource="&owl;Thing"/>
    <rdfs:subClassOf rdf:resource="#Machinery"/>
  </owl:Class>

  <owl:Class rdf:about="#Machinery">
    <rdf:type rdf:resource="&owl;Thing"/>
    <rdfs:comment>Machinery is the class of products 

that includes Machines, tools, and machine parts used in industrial 

or other commercial processes.</rdfs:comment>
    <rdfs:subClassOf rdf:resource="#DurableGood"/>
    <rdfs:subClassOf rdf:resource="#IndustrialSupply"/>
    <rdfs:subClassOf rdf:resource="&SUMO;Device"/>
  </owl:Class>

  <owl:Class rdf:about="#MaizeGrain">
    <rdf:type rdf:resource="&owl;Thing"/>
    <rdfs:label>corn</rdfs:label>
    <rdfs:label>maize</rdfs:label>
    <rdfs:subClassOf rdf:resource="&Mid-level-ontology;CerealGrain"/>
  </owl:Class>

  <owl:Class rdf:about="#MajorAppliance">
    <rdf:type rdf:resource="&owl;Thing"/>
    <rdfs:comment>MajorAppliance is the subclass of 

ElectricDevices that are large DurableGoods manufactured for use 

in household tasks.</rdfs:comment>
    <rdfs:subClassOf rdf:resource="#DurableGood"/>
    <rdfs:subClassOf rdf:resource="&Mid-level-ontology;ElectricDevice"/>
  </owl:Class>

  <owl:Class rdf:about="#Mango">
    <rdfs:subClassOf rdf:resource="#GroceryProduce"/>
    <rdfs:subClassOf rdf:resource="#TropicalFruit"/>
  </owl:Class>

  <owl:Class rdf:about="#ManufacturedProduct">
    <rdfs:comment>ManufacturedProduct is 

the subclass of Product that includes goods that are produced 

or assembled in factories or other manufacturing processes, 

in contrast to AgriculturalProducts.</rdfs:comment>
    <rdfs:subClassOf rdf:resource="&SUMO;Product"/>
    <owl:disjointWith rdf:resource="#AgriculturalProduct"/>
    <owl:disjointWith rdf:resource="#BeverageProduct"/>
    <owl:disjointWith rdf:resource="#CapitalGood"/>
    <owl:disjointWith rdf:resource="#FoodProduct"/>
    <owl:disjointWith rdf:resource="#ForestProduct"/>
    <owl:disjointWith rdf:resource="#HandicraftProduct"/>
    <owl:disjointWith rdf:resource="#MiningProduct"/>
    <owl:disjointWith rdf:resource="#PackagedBeverageProduct"/>
    <owl:disjointWith rdf:resource="#PackagedFoodProduct"/>
  </owl:Class>

  <owl:Class rdf:about="#MeatOfLandAnimal">
    <rdfs:subClassOf rdf:resource="&SUMO;Meat"/>
  </owl:Class>

  <owl:Class rdf:about="#Melon">
    <rdfs:subClassOf rdf:resource="#Fruit"/>
    <rdfs:subClassOf rdf:resource="#GroceryProduce"/>
  </owl:Class>

  <owl:Class rdf:about="#MetalProduct">
    <SUMO:relatedInternalConcept rdf:resource="&SUMO;Metal"/>
    <rdf:type rdf:resource="&owl;Thing"/>
    <rdfs:subClassOf rdf:resource="#DurableGood"/>
    <rdfs:subClassOf rdf:resource="#ManufacturedProduct"/>
  </owl:Class>

  <owl:Class rdf:about="#MilletGrain">
    <rdf:type rdf:resource="&owl;Thing"/>
    <rdfs:subClassOf rdf:resource="&Mid-level-ontology;CerealGrain"/>
  </owl:Class>

  <owl:Class rdf:about="#MiningProduct">
    <rdfs:comment>MiningProduct is the class of things 

that are produced from the earth for human use by mining or another form 

of extraction.  This includes metal ores, petroleum, and other products.</rdfs:comment>
    <rdfs:subClassOf rdf:resource="&SUMO;Product"/>
    <owl:disjointWith rdf:resource="#AgriculturalProduct"/>
    <owl:disjointWith rdf:resource="#BeverageProduct"/>
    <owl:disjointWith rdf:resource="#CapitalGood"/>
    <owl:disjointWith rdf:resource="#FoodProduct"/>
    <owl:disjointWith rdf:resource="#ForestProduct"/>
    <owl:disjointWith rdf:resource="#HandicraftProduct"/>
    <owl:disjointWith rdf:resource="#ManufacturedProduct"/>
    <owl:disjointWith rdf:resource="#PackagedBeverageProduct"/>
    <owl:disjointWith rdf:resource="#PackagedFoodProduct"/>
  </owl:Class>

  <owl:Class rdf:about="#MotorOil">
    <rdfs:comment>MotorOil is the subclass of PetroleumLubricants 

that are used to lubricate motors.</rdfs:comment>
    <rdfs:subClassOf rdf:resource="#PetroleumLubricant"/>
  </owl:Class>

  <owl:Class rdf:about="#MulberryLeaf">
    <rdfs:subClassOf rdf:resource="#Leaf"/>
    <rdfs:subClassOf rdf:resource="#PlantAgriculturalProduct"/>
    <rdfs:subClassOf rdf:resource="&Mid-level-ontology;Fodder"/>
  </owl:Class>

  <owl:Class rdf:about="#Mutton">
    <rdfs:subClassOf rdf:resource="#MeatOfLandAnimal"/>
  </owl:Class>

  <owl:Class rdf:about="#NaturalRubber">
    <rdfs:comment>NaturalRubber is the subclass of 

PlantAgriculturalProducts made from the sap of plant species 

which produce natural polymers.</rdfs:comment>
    <rdfs:subClassOf rdf:resource="#PlantAgriculturalProduct"/>
  </owl:Class>

  <owl:Class rdf:about="#NickelOre">
    <rdf:type rdf:resource="&owl;Thing"/>
    <rdfs:subClassOf rdf:resource="#MiningProduct"/>
    <rdfs:subClassOf rdf:resource="&SUMO;Mineral"/>
  </owl:Class>

  <owl:Class rdf:about="#NorfolkIslandPineSeed">
    <rdfs:subClassOf rdf:resource="#PlantAgriculturalProduct"/>
    <rdfs:subClassOf rdf:resource="&SUMO;Seed"/>
  </owl:Class>

  <owl:Class rdf:about="#Nut">
    <rdfs:subClassOf rdf:resource="#PlantAgriculturalProduct"/>
    <rdfs:subClassOf rdf:resource="&SUMO;ReproductiveBody"/>
  </owl:Class>

  <owl:Class rdf:about="#Nutmeg">
    <rdfs:subClassOf rdf:resource="#Spice"/>
  </owl:Class>

  <owl:Class rdf:about="#OatGrain">
    <rdf:type rdf:resource="&owl;Thing"/>
    <rdfs:subClassOf rdf:resource="&Mid-level-ontology;CerealGrain"/>
  </owl:Class>

  <owl:Class rdf:about="#Oilseed">
    <rdfs:subClassOf rdf:resource="#PlantAgriculturalProduct"/>
    <rdfs:subClassOf rdf:resource="&SUMO;Seed"/>
  </owl:Class>

  <owl:Class rdf:about="#Okoume">
    <rdfs:comment>Okoume (Aucoumea klaineana), also called 

'gaboon', is a wood of West African origin.</rdfs:comment>
    <rdfs:subClassOf rdf:resource="#Hardwood"/>
  </owl:Class>

  <SUMO:UnitOfMeasure rdf:about="#OldTajikSomoni">
    <rdf:type rdf:resource="&owl;Class"/>
    <rdfs:comment>OldTajikSomoni represents a former unit of 

currency of Tajikistan.</rdfs:comment>
    <rdfs:subClassOf rdf:resource="&SUMO;CurrencyMeasure"/>
  </SUMO:UnitOfMeasure>

  <owl:Class rdf:about="#Olive">
    <rdfs:subClassOf rdf:resource="#Fruit"/>
    <rdfs:subClassOf rdf:resource="#GroceryProduce"/>
  </owl:Class>

  <owl:Class rdf:about="#OliveOil">
    <rdfs:subClassOf rdf:resource="#VegetableOil"/>
  </owl:Class>

  <owl:Class rdf:about="#OpiumPoppy">
    <rdf:type rdf:resource="&owl;Thing"/>
    <rdfs:subClassOf rdf:resource="#PlantAgriculturalProduct"/>
    <rdfs:subClassOf rdf:resource="&SUMO;FloweringPlant"/>
  </owl:Class>

  <owl:Class rdf:about="#OpiumPoppyFarming">
    <Mid-level-ontology:industryProductType rdf:resource="#OpiumPoppy"/>
    <rdf:type rdf:resource="&owl;Thing"/>
    <rdfs:comment>OpiumPoppyFarming is the specification 

of CropProduction that describes OpiumPoppy farming operations.</rdfs:comment>
    <rdfs:subClassOf rdf:resource="#CropProduction"/>
  </owl:Class>

  <owl:Class rdf:about="#Orchid">
    <rdfs:subClassOf rdf:resource="#PlantAgriculturalProduct"/>
    <rdfs:subClassOf rdf:resource="&SUMO;FloweringPlant"/>
  </owl:Class>

  <owl:Class rdf:about="#OrnamentalFish">
    <rdfs:subClassOf rdf:resource="#AnimalAgriculturalProduct"/>
    <rdfs:subClassOf rdf:resource="&SUMO;Fish"/>
  </owl:Class>

  <owl:Class rdf:about="#PPPBasedEconomicValuation">
    <rdfs:comment>PPPBasedEconomicValuation 

is a class of relations used to state international economic information 

in U.S. dollar amounts.  The U.S. dollar amounts are derived from Purchasing 

Power Parity conversions of economic totals (e.g., GDP)  given in local 

currency.  This contrasts with a method of conversion based on currency 

exchange rates.  The PPP method is used by the CIA World Fact Book for 

the purpose of presenting economic data for all countries covered.  Their 

basis for PPP dollar price weights is the UN International Comparison Program 

(UNICP) and the work of Professors Robert Summers and Alan Heston of the 

University of Pennsylvania.</rdfs:comment>
    <rdfs:subClassOf rdf:resource="&SUMO;Relation"/>
  </owl:Class>

  <owl:Class rdf:about="#PackagedBeverageProduct">
    <rdfs:comment>PackagedBeverageProduct is the 

class of Products that consist of a BeverageProduct in some kind of 

packaging, including cups and bottles.</rdfs:comment>
    <rdfs:subClassOf rdf:resource="&SUMO;Product"/>
    <owl:disjointWith rdf:resource="#AgriculturalProduct"/>
    <owl:disjointWith rdf:resource="#BeverageProduct"/>
    <owl:disjointWith rdf:resource="#CapitalGood"/>
    <owl:disjointWith rdf:resource="#FoodProduct"/>
    <owl:disjointWith rdf:resource="#ForestProduct"/>
    <owl:disjointWith rdf:resource="#HandicraftProduct"/>
    <owl:disjointWith rdf:resource="#ManufacturedProduct"/>
    <owl:disjointWith rdf:resource="#MiningProduct"/>
    <owl:disjointWith rdf:resource="#PackagedFoodProduct"/>
  </owl:Class>

  <owl:Class rdf:about="#PackagedFoodProduct">
    <rdfs:comment>PackagedFoodProduct is the 

class of Products that consist of a FoodProduct in a package.</rdfs:comment>
    <rdfs:subClassOf rdf:resource="&SUMO;Product"/>
    <owl:disjointWith rdf:resource="#AgriculturalProduct"/>
    <owl:disjointWith rdf:resource="#BeverageProduct"/>
    <owl:disjointWith rdf:resource="#CapitalGood"/>
    <owl:disjointWith rdf:resource="#FoodProduct"/>
    <owl:disjointWith rdf:resource="#ForestProduct"/>
    <owl:disjointWith rdf:resource="#HandicraftProduct"/>
    <owl:disjointWith rdf:resource="#ManufacturedProduct"/>
    <owl:disjointWith rdf:resource="#MiningProduct"/>
    <owl:disjointWith rdf:resource="#PackagedBeverageProduct"/>
  </owl:Class>

  <owl:Class rdf:about="#PaddyRice">
    <rdfs:subClassOf rdf:resource="#CerealGrass"/>
  </owl:Class>

  <owl:Class rdf:about="#PalmKernel">
    <SUMO:relatedInternalConcept rdf:resource="#PalmOilNut"/>
    <rdf:type rdf:resource="&owl;Thing"/>
    <rdfs:subClassOf rdf:resource="#PlantAgriculturalProduct"/>
  </owl:Class>

  <owl:Class rdf:about="#PalmOil">
    <rdfs:subClassOf rdf:resource="#VegetableOil"/>
  </owl:Class>

  <owl:Class rdf:about="#PalmOilNut">
    <rdf:type rdf:resource="&owl;Thing"/>
    <rdfs:label>coquilla nut</rdfs:label>
    <rdfs:label>palm oil nut</rdfs:label>
    <rdfs:subClassOf rdf:resource="#Nut"/>
    <rdfs:subClassOf rdf:resource="#PlantAgriculturalProduct"/>
  </owl:Class>

  <owl:Class rdf:about="#Papaw">
    <rdfs:label>papaw</rdfs:label>
    <rdfs:label>pawpaw</rdfs:label>
    <rdfs:subClassOf rdf:resource="#GroceryProduce"/>
    <rdfs:subClassOf rdf:resource="#TropicalFruit"/>
  </owl:Class>

  <owl:Class rdf:about="#Papaya">
    <rdfs:subClassOf rdf:resource="#GroceryProduce"/>
    <rdfs:subClassOf rdf:resource="#TropicalFruit"/>
  </owl:Class>

  <owl:Class rdf:about="#PassionFruit">
    <rdfs:subClassOf rdf:resource="#GroceryProduce"/>
    <rdfs:subClassOf rdf:resource="#TropicalFruit"/>
  </owl:Class>

  <owl:Class rdf:about="#Pea">
    <rdfs:subClassOf rdf:resource="#Legume"/>
  </owl:Class>

  <owl:Class rdf:about="#Peanut">
    <rdf:type rdf:resource="&owl;Thing"/>
    <rdfs:subClassOf rdf:resource="#EdibleNut"/>
    <rdfs:subClassOf rdf:resource="#GroceryProduce"/>
  </owl:Class>

  <owl:Class rdf:about="#Pearl"
             rdfs:comment="Pearl is a subclass of Gemstone.">
    <rdfs:subClassOf rdf:resource="http://reliant.teknowledge.com/DAML/Geography.owl#SemipreciousGemstone"/>
  </owl:Class>

  <owl:Class rdf:about="#PecanNut">
    <rdfs:subClassOf rdf:resource="#EdibleNut"/>
  </owl:Class>

  <owl:Class rdf:about="#Pelt">
    <rdfs:comment>Pelt is the subclass of AnimalSkin 

that comprises the pelts or hides of animals that are used in 

the manufacture of wearable or household items.</rdfs:comment>
    <rdfs:label>hide</rdfs:label>
    <rdfs:label>pelt</rdfs:label>
    <rdfs:subClassOf rdf:resource="#AnimalAgriculturalProduct"/>
    <rdfs:subClassOf rdf:resource="#AnimalSkin"/>
  </owl:Class>

  <owl:Class rdf:about="#PerfumeEssence">
    <rdfs:subClassOf rdf:resource="#PlantAgriculturalProduct"/>
  </owl:Class>

  <owl:Class rdf:about="#PetroleumLubricant">
    <rdfs:comment>PetroleumLubricant is the subclass of 

RefinedPetroleumProducts that are lubricants.</rdfs:comment>
    <rdfs:subClassOf rdf:resource="#RefinedPetroleumProduct"/>
  </owl:Class>

  <owl:Class rdf:about="#PetroleumProduct">
    <rdf:type rdf:resource="&owl;Thing"/>
    <rdfs:comment>PetroleumProduct is a broad class that 

includes both crude oil (Petroleum) and RefinedPetroleumProducts.</rdfs:comment>
    <rdfs:subClassOf rdf:resource="#MiningProduct"/>
    <rdfs:subClassOf rdf:resource="&SUMO;CompoundSubstance"/>
  </owl:Class>

  <owl:Class rdf:about="#PharmaceuticalProduct">
    <rdf:type rdf:resource="&owl;Thing"/>
    <rdfs:comment>PharmaceuticalProduct is the 

subclass of ChemicalProducts that are BiologicallyActiveSubstances 

used in treating disorders and diseases in humans and other animals.</rdfs:comment>
    <rdfs:subClassOf rdf:resource="#ChemicalProduct"/>
    <rdfs:subClassOf rdf:resource="#ManufacturedProduct"/>
    <rdfs:subClassOf rdf:resource="&SUMO;BiologicallyActiveSubstance"/>
    <owl:disjointWith rdf:resource="#Pyrethrum"/>
  </owl:Class>

  <owl:Class rdf:about="#PhosphoricAcid">
    <SUMO:relatedInternalConcept rdf:resource="http://reliant.teknowledge.com/DAML/elements.owl#Phosphorus"/>
    <rdf:type rdf:resource="&owl;Thing"/>
    <rdfs:comment>PhosphoricAcid represents phosphoric acid.</rdfs:comment>
    <rdfs:subClassOf rdf:resource="&SUMO;CompoundSubstance"/>
  </owl:Class>

  <owl:Class rdf:about="#Pineapple">
    <rdfs:subClassOf rdf:resource="#GroceryProduce"/>
    <rdfs:subClassOf rdf:resource="#TropicalFruit"/>
  </owl:Class>

  <owl:Class rdf:about="#PlantAgriculturalProduct">
    <rdf:type rdf:resource="&owl;Thing"/>
    <rdfs:comment>PlantAgriculturalProduct 

is the class of AgriculturalProducts that are vegetable in nature, 

in the widest sense, e.g., fruits, grains, green vegetables, cotton, 

linen, flowers, wine grapes, hops.</rdfs:comment>
    <rdfs:subClassOf rdf:resource="#AgriculturalProduct"/>
    <owl:disjointWith rdf:resource="#AnimalAgriculturalProduct"/>
  </owl:Class>

  <owl:Class rdf:about="#Plantain">
    <rdfs:subClassOf rdf:resource="#GroceryProduce"/>
    <rdfs:subClassOf rdf:resource="#TropicalFruit"/>
  </owl:Class>

  <owl:Class rdf:about="#Plastic">
    <rdfs:subClassOf rdf:resource="#ManufacturedProduct"/>
  </owl:Class>

  <owl:Class rdf:about="#Pork">
    <rdf:type rdf:resource="&owl;Thing"/>
    <rdfs:subClassOf rdf:resource="#MeatOfLandAnimal"/>
  </owl:Class>

  <owl:Class rdf:about="#PotatoTuber">
    <rdf:type rdf:resource="&owl;Thing"/>
    <rdfs:comment>PotatoTuber represents the edible tubrous part 

of the potato plant.</rdfs:comment>
    <rdfs:subClassOf rdf:resource="#EdibleTuber"/>
    <rdfs:subClassOf rdf:resource="#GroceryProduce"/>
  </owl:Class>

  <owl:Class rdf:about="#Poultry">
    <rdfs:subClassOf rdf:resource="#Livestock"/>
    <rdfs:subClassOf rdf:resource="&SUMO;Bird"/>
  </owl:Class>

  <owl:Class rdf:about="#PowerGeneration">
    <rdfs:comment>PowerGeneration is the class of 

Processes in which some kind of power is generated either for immediate 

use in a Device or to be stored for future use.</rdfs:comment>
    <rdfs:subClassOf rdf:resource="&SUMO;Process"/>
  </owl:Class>

  <owl:Class rdf:about="#ProductPackage">
    <rdfs:comment>ProductPackage is the class of objects 

designed to contain Products for shipping and sale.</rdfs:comment>
    <rdfs:subClassOf rdf:resource="&SUMO;Object"/>
  </owl:Class>

  <owl:Class rdf:about="#Pyrethrum">
    <rdf:type rdf:resource="&owl;Thing"/>
    <rdfs:comment>Pyrethrum is the subclass of 

BiologicallyActiveSubstance consisting of insecticidal 

derivations from the flower heads of Chrysanthemums.</rdfs:comment>
    <rdfs:subClassOf rdf:resource="#PlantAgriculturalProduct"/>
    <rdfs:subClassOf rdf:resource="&SUMO;BiologicallyActiveSubstance"/>
    <owl:disjointWith rdf:resource="#PharmaceuticalProduct"/>
    <owl:disjointWith rdf:resource="&Mid-level-ontology;ControlledSubstance"/>
  </owl:Class>

  <owl:Class rdf:about="#Quinine">
    <rdfs:subClassOf rdf:resource="#PlantAgriculturalProduct"/>
  </owl:Class>

  <owl:Class rdf:about="#ReadyMixConcrete">
    <rdfs:subClassOf rdf:resource="&Mid-level-ontology;Concrete"/>
  </owl:Class>

  <owl:Class rdf:about="#RefinedPetroleumProduct">
    <rdfs:comment>RefinedPetroleumProduct is the 

subclass of PetroleumProducts that are refined from Petroleum (crude oil).</rdfs:comment>
    <rdfs:subClassOf rdf:resource="#PetroleumProduct"/>
  </owl:Class>

  <owl:Class rdf:about="#Refrigerator">
    <rdf:type rdf:resource="&owl;Thing"/>
    <rdfs:comment>Refrigerator is the class of refrigerators.</rdfs:comment>
    <rdfs:subClassOf rdf:resource="#MajorAppliance"/>
  </owl:Class>

  <owl:Class rdf:about="#Reindeer">
    <rdfs:subClassOf rdf:resource="#Livestock"/>
    <rdfs:subClassOf rdf:resource="&SUMO;HoofedMammal"/>
  </owl:Class>

  <owl:Class rdf:about="#RiceGrain">
    <rdf:type rdf:resource="&owl;Thing"/>
    <rdfs:subClassOf rdf:resource="&Mid-level-ontology;CerealGrain"/>
  </owl:Class>

  <owl:Class rdf:about="#RootStarch">
    <SUMO:relatedInternalConcept rdf:resource="#RootVegetable"/>
    <rdf:type rdf:resource="&owl;Thing"/>
    <rdfs:subClassOf rdf:resource="#PlantAgriculturalProduct"/>
    <rdfs:subClassOf rdf:resource="&SUMO;FruitOrVegetable"/>
    <owl:disjointWith rdf:resource="#Fruit"/>
    <owl:disjointWith rdf:resource="#GroceryProduce"/>
    <owl:disjointWith rdf:resource="#Spice"/>
    <owl:disjointWith rdf:resource="#TeaPlantAerialPart"/>
    <owl:disjointWith rdf:resource="#Vegetable"/>
    <owl:disjointWith rdf:resource="&SUMO;Seed"/>
  </owl:Class>

  <owl:Class rdf:about="#RootVegetable">
    <rdf:type rdf:resource="&owl;Thing"/>
    <rdfs:label>root crop</rdfs:label>
    <rdfs:label>root vegetable</rdfs:label>
    <rdfs:subClassOf rdf:resource="#PlantAgriculturalProduct"/>
    <rdfs:subClassOf rdf:resource="&SUMO;FruitOrVegetable"/>
    <owl:disjointWith rdf:resource="#Fruit"/>
    <owl:disjointWith rdf:resource="#GroceryProduce"/>
    <owl:disjointWith rdf:resource="#Spice"/>
    <owl:disjointWith rdf:resource="#TeaPlantAerialPart"/>
    <owl:disjointWith rdf:resource="#Vegetable"/>
    <owl:disjointWith rdf:resource="&SUMO;Seed"/>
  </owl:Class>

  <owl:Class rdf:about="#RyeGrain">
    <rdf:type rdf:resource="&owl;Thing"/>
    <rdfs:subClassOf rdf:resource="&Mid-level-ontology;CerealGrain"/>
  </owl:Class>

  <owl:Class rdf:about="#Salmon">
    <rdfs:subClassOf rdf:resource="#FoodFish"/>
  </owl:Class>

  <owl:Class rdf:about="#Seafood">
    <rdfs:subClassOf rdf:resource="&SUMO;Meat"/>
  </owl:Class>

  <owl:Class rdf:about="#SenepolCattle">
    <rdfs:subClassOf rdf:resource="#Cattle"/>
  </owl:Class>

  <owl:Class rdf:about="#Sesame">
    <rdfs:subClassOf rdf:resource="#PlantAgriculturalProduct"/>
  </owl:Class>

  <owl:Class rdf:about="#SheaNut">
    <rdfs:subClassOf rdf:resource="#EdibleNut"/>
  </owl:Class>

  <owl:Class rdf:about="#Sheepskin">
    <rdfs:subClassOf rdf:resource="#Pelt"/>
  </owl:Class>

  <owl:Class rdf:about="#Shellfish">
    <rdfs:subClassOf rdf:resource="#Seafood"/>
  </owl:Class>

  <owl:Class rdf:about="#Shrimp">
    <rdfs:subClassOf rdf:resource="#Shellfish"/>
  </owl:Class>

  <owl:Class rdf:about="#SisalFiber">
    <rdfs:subClassOf rdf:resource="#PlantAgriculturalProduct"/>
  </owl:Class>

  <owl:Class rdf:about="#Soap">
    <rdfs:comment>Soap is the class of cleaning agents based on fatty 

acids.</rdfs:comment>
    <rdfs:subClassOf rdf:resource="&Mid-level-ontology;Detergent"/>
  </owl:Class>

  <owl:Class rdf:about="#Sorghum">
    <rdfs:subClassOf rdf:resource="#CerealGrass"/>
  </owl:Class>

  <owl:Class rdf:about="#SorghumGrain">
    <rdf:type rdf:resource="&owl;Thing"/>
    <rdfs:subClassOf rdf:resource="&Mid-level-ontology;CerealGrain"/>
  </owl:Class>

  <owl:Class rdf:about="#Soya">
    <SUMO:relatedInternalConcept rdf:resource="#Soybean"/>
    <rdf:type rdf:resource="&owl;Thing"/>
    <rdfs:subClassOf rdf:resource="#PlantAgriculturalProduct"/>
  </owl:Class>

  <owl:Class rdf:about="#Soybean">
    <rdf:type rdf:resource="&owl;Thing"/>
    <rdfs:subClassOf rdf:resource="#Bean"/>
  </owl:Class>

  <owl:Class rdf:about="#Spice">
    <rdfs:subClassOf rdf:resource="#PlantAgriculturalProduct"/>
    <rdfs:subClassOf rdf:resource="&SUMO;FruitOrVegetable"/>
    <owl:disjointWith rdf:resource="#GroceryProduce"/>
    <owl:disjointWith rdf:resource="#RootStarch"/>
    <owl:disjointWith rdf:resource="#RootVegetable"/>
    <owl:disjointWith rdf:resource="#TeaPlantAerialPart"/>
    <owl:disjointWith rdf:resource="#Vegetable"/>
    <owl:disjointWith rdf:resource="&SUMO;Seed"/>
  </owl:Class>

  <owl:Class rdf:about="#SpicePepper">
    <rdfs:subClassOf rdf:resource="#Spice"/>
  </owl:Class>

  <owl:Class rdf:about="#Squash">
    <rdfs:subClassOf rdf:resource="#GroceryProduce"/>
    <rdfs:subClassOf rdf:resource="#Vegetable"/>
  </owl:Class>

  <owl:Class rdf:about="#SugarBeet">
    <rdf:type rdf:resource="&owl;Thing"/>
    <rdfs:subClassOf rdf:resource="#Vegetable"/>
  </owl:Class>

  <owl:Class rdf:about="#SugarCane">
    <rdfs:subClassOf rdf:resource="#GroceryProduce"/>
    <rdfs:subClassOf rdf:resource="#Vegetable"/>
  </owl:Class>

  <owl:Class rdf:about="#Sunflower">
    <rdfs:subClassOf rdf:resource="#PlantAgriculturalProduct"/>
    <rdfs:subClassOf rdf:resource="&SUMO;FloweringPlant"/>
  </owl:Class>

  <owl:Class rdf:about="#SunflowerSeed">
    <rdfs:subClassOf rdf:resource="#PlantAgriculturalProduct"/>
    <rdfs:subClassOf rdf:resource="&SUMO;Seed"/>
  </owl:Class>

  <owl:Class rdf:about="#SweetPepper">
    <rdfs:subClassOf rdf:resource="#GroceryProduce"/>
    <rdfs:subClassOf rdf:resource="#Vegetable"/>
  </owl:Class>

  <owl:Class rdf:about="#SweetPotatoTuber">
    <rdfs:subClassOf rdf:resource="#EdibleTuber"/>
    <rdfs:subClassOf rdf:resource="#GroceryProduce"/>
  </owl:Class>

  <SUMO:UnitOfMeasure rdf:about="#TajikSomoni">
    <rdf:type rdf:resource="&owl;Class"/>
    <rdfs:comment>TajikSomoni represents the basic unit of 

currency of Tajikistan.</rdfs:comment>
    <rdfs:subClassOf rdf:resource="&SUMO;CurrencyMeasure"/>
  </SUMO:UnitOfMeasure>

  <owl:Class rdf:about="#TaroTuber">
    <rdfs:subClassOf rdf:resource="#EdibleTuber"/>
    <rdfs:subClassOf rdf:resource="#GroceryProduce"/>
  </owl:Class>

  <owl:Class rdf:about="#TeaLeaf">
    <rdfs:subClassOf rdf:resource="#TeaPlantAerialPart"/>
  </owl:Class>

  <owl:Class rdf:about="#TeaPlantAerialPart">
    <rdfs:comment>TeaPlantAerialPart is the 

class of all parts of the tea plant from which tea may be made, 

including leaves, stems, and twigs.</rdfs:comment>
    <rdfs:subClassOf rdf:resource="&SUMO;FruitOrVegetable"/>
    <owl:disjointWith rdf:resource="#GroceryProduce"/>
    <owl:disjointWith rdf:resource="#RootStarch"/>
    <owl:disjointWith rdf:resource="#RootVegetable"/>
    <owl:disjointWith rdf:resource="#Spice"/>
    <owl:disjointWith rdf:resource="#Vegetable"/>
    <owl:disjointWith rdf:resource="&SUMO;Seed"/>
  </owl:Class>

  <owl:Class rdf:about="#TextileProduct">
    <rdf:type rdf:resource="&owl;Thing"/>
    <rdfs:comment>TextileProduct is the subclass of 

ManufacturedProducts consisting of Fabrics or finished fabric items 

(e.g., linens), excluding Clothing.</rdfs:comment>
    <rdfs:subClassOf rdf:resource="#ManufacturedProduct"/>
  </owl:Class>

  <owl:Class rdf:about="#Tobacco">
    <rdfs:subClassOf rdf:resource="#PlantAgriculturalProduct"/>
  </owl:Class>

  <owl:Class rdf:about="#Tomato">
    <rdfs:subClassOf rdf:resource="#Fruit"/>
    <rdfs:subClassOf rdf:resource="#GroceryProduce"/>
  </owl:Class>

  <owl:Class rdf:about="#TropicalFruit">
    <rdfs:subClassOf rdf:resource="#Fruit"/>
    <rdfs:subClassOf rdf:resource="#GroceryProduce"/>
  </owl:Class>

  <Government:IndependentState rdf:about="#Turkey"
                               rdfs:label="Turkey">
    <Mid-level-ontology:economyType rdf:resource="#DevelopedCountry"/>
    <Mid-level-ontology:economyType rdf:resource="#DevelopingCountry"/>
    <Mid-level-ontology:economyType rdf:resource="#LessDevelopedCountry"/>
    <SUMO:geographicSubregion rdf:resource="http://reliant.teknowledge.com/DAML/Geography.owl#SoutheasternEurope"/>
    <rdf:type rdf:resource="&SUMO;Nation"/>
    <rdf:type rdf:resource="&owl;Class"/>
    <rdfs:subClassOf rdf:resource="#Poultry"/>
  </Government:IndependentState>

  <owl:Class rdf:about="#TurkeyMeat">
    <rdfs:subClassOf rdf:resource="#MeatOfLandAnimal"/>
  </owl:Class>

  <owl:Class rdf:about="#Turnip">
    <rdfs:subClassOf rdf:resource="#GroceryProduce"/>
    <rdfs:subClassOf rdf:resource="#RootVegetable"/>
  </owl:Class>

  <owl:Class rdf:about="#Turtle">
    <rdfs:subClassOf rdf:resource="#Livestock"/>
    <rdfs:subClassOf rdf:resource="&SUMO;Reptile"/>
  </owl:Class>

  <owl:Class rdf:about="#UNEconomicDevelopmentLevel">
    <rdfs:comment>UNEconomicDevelopmentLevel 

is a subclass of EconomicDevelopmentLevel containing terms used to 

represent economic development classifications used by UnitedNations 

agencies.  The top level of this classification scheme includes the 

concepts of DevelopedCountry, FormerSovietOrEasternEuropeanCountry, 

and LessDevelopedCountry.</rdfs:comment>
    <rdfs:subClassOf rdf:resource="#EconomicDevelopmentLevel"/>
  </owl:Class>

  <owl:Class rdf:about="#Vanilla">
    <rdfs:subClassOf rdf:resource="#Spice"/>
  </owl:Class>

  <owl:Class rdf:about="#Veal">
    <rdfs:subClassOf rdf:resource="#MeatOfLandAnimal"/>
  </owl:Class>

  <owl:Class rdf:about="#Vegetable">
    <rdf:type rdf:resource="&owl;Thing"/>
    <rdfs:subClassOf rdf:resource="&SUMO;FruitOrVegetable"/>
    <owl:disjointWith rdf:resource="#GroceryProduce"/>
    <owl:disjointWith rdf:resource="#RootStarch"/>
    <owl:disjointWith rdf:resource="#RootVegetable"/>
    <owl:disjointWith rdf:resource="#Spice"/>
    <owl:disjointWith rdf:resource="#TeaPlantAerialPart"/>
    <owl:disjointWith rdf:resource="&SUMO;Seed"/>
  </owl:Class>

  <owl:Class rdf:about="#VegetableOil">
    <rdf:type rdf:resource="&owl;Thing"/>
    <rdfs:subClassOf rdf:resource="#PlantAgriculturalProduct"/>
  </owl:Class>

  <owl:Class rdf:about="#Walnut">
    <rdfs:subClassOf rdf:resource="#EdibleNut"/>
  </owl:Class>

  <owl:Class rdf:about="#WaterBuffalo">
    <rdfs:subClassOf rdf:resource="#Livestock"/>
    <rdfs:subClassOf rdf:resource="&SUMO;HoofedMammal"/>
  </owl:Class>

  <owl:Class rdf:about="#WaterBuffaloMeat">
    <rdfs:subClassOf rdf:resource="#MeatOfLandAnimal"/>
  </owl:Class>

  <owl:Class rdf:about="#Watermelon">
    <rdfs:subClassOf rdf:resource="#Melon"/>
  </owl:Class>

  <owl:Class rdf:about="#WearableItem">
    <rdfs:comment>WearableItem is the subclass of 

Artifacts that are made to be worn on the body, including Clothing, 

Footwear, and Jewelry.</rdfs:comment>
    <rdfs:subClassOf rdf:resource="&SUMO;Artifact"/>
  </owl:Class>

  <owl:Class rdf:about="#WheatGrain">
    <rdf:type rdf:resource="&owl;Thing"/>
    <rdfs:subClassOf rdf:resource="&Mid-level-ontology;CerealGrain"/>
  </owl:Class>

  <owl:Class rdf:about="#WineGrape">
    <rdf:type rdf:resource="&owl;Thing"/>
    <rdfs:subClassOf rdf:resource="#PlantAgriculturalProduct"/>
  </owl:Class>

  <owl:Class rdf:about="#WoodProduct">
    <rdf:type rdf:resource="&owl;Thing"/>
    <rdfs:subClassOf rdf:resource="#ForestProduct"/>
  </owl:Class>

  <owl:Class rdf:about="#WoolFiber">
    <rdfs:subClassOf rdf:resource="#AnimalAgriculturalProduct"/>
  </owl:Class>

  <owl:Class rdf:about="#WorldBankGNIPerCapitaLevel">
    <rdfs:comment>WorldBankGNIPerCapitaLevel 

is the subclass of EconomicDevelopmentLevel containing attributes 

that characterize countries according to their per capita gross national 

income (GNI), as determined by the WorldBankGroup.  The World Bank 

uses the Atlas method for making cross-country comparisons of national 

income.</rdfs:comment>
    <rdfs:label>GNI per capita</rdfs:label>
    <rdfs:label>gross national income per capita</rdfs:label>
    <rdfs:subClassOf rdf:resource="#EconomicDevelopmentLevel"/>
  </owl:Class>

  <owl:Class rdf:about="#YamTuber">
    <rdfs:subClassOf rdf:resource="#EdibleTuber"/>
    <rdfs:subClassOf rdf:resource="#GroceryProduce"/>
  </owl:Class>

  <owl:Class rdf:about="#YlangYlang">
    <rdfs:subClassOf rdf:resource="#PerfumeEssence"/>
  </owl:Class>

  <owl:Class rdf:about="#ZincOre">
    <rdf:type rdf:resource="&owl;Thing"/>
    <rdfs:subClassOf rdf:resource="#MiningProduct"/>
    <rdfs:subClassOf rdf:resource="&SUMO;Mineral"/>
  </owl:Class>

  <owl:Class rdf:about="#ZincProduct">
    <rdf:type rdf:resource="&owl;Thing"/>
    <rdfs:subClassOf rdf:resource="#ManufacturedProduct"/>
    <rdfs:subClassOf rdf:resource="#MetalProduct"/>
  </owl:Class>

  <owl:Class rdf:about="http://reliant.teknowledge.com/DAML/Geography.owl#Bauxite"
             rdfs:label="bauxite">
    <rdfs:subClassOf rdf:resource="#MiningProduct"/>
    <rdfs:subClassOf rdf:resource="&SUMO;Mixture"/>
  </owl:Class>

  <owl:Class rdf:about="http://reliant.teknowledge.com/DAML/Geography.owl#IronOre"
             rdfs:label="iron ore">
    <rdf:type rdf:resource="&owl;Thing"/>
    <rdfs:subClassOf rdf:resource="#MiningProduct"/>
    <rdfs:subClassOf rdf:resource="&SUMO;Mineral"/>
  </owl:Class>

  <owl:Class rdf:about="http://reliant.teknowledge.com/DAML/Geography.owl#Petroleum">
    <rdfs:label>crude oil</rdfs:label>
    <rdfs:label>petroleum</rdfs:label>
    <rdfs:subClassOf rdf:resource="#PetroleumProduct"/>
  </owl:Class>

  <owl:Class rdf:about="http://reliant.teknowledge.com/DAML/Geography.owl#PreciousGemstone">
    <rdfs:comment>PreciousGemstone is the subclass of 

Gemstones that bring the highest prices.</rdfs:comment>
    <rdfs:subClassOf rdf:resource="#Gemstone"/>
    <rdfs:subClassOf rdf:resource="#MiningProduct"/>
  </owl:Class>

  <owl:Class rdf:about="http://reliant.teknowledge.com/DAML/Geography.owl#SemipreciousGemstone">
    <rdfs:comment>SemipreciousGemstone is the subclass 

of Gemstones that are valuable but not as much as PreciousGemstones.</rdfs:comment>
    <rdfs:subClassOf rdf:resource="#Gemstone"/>
    <rdfs:subClassOf rdf:resource="#MiningProduct"/>
  </owl:Class>

  <owl:Class rdf:about="http://reliant.teknowledge.com/DAML/Geography.owl#Timber"
             rdfs:label="timber">
    <rdf:type rdf:resource="&owl;Thing"/>
    <rdfs:subClassOf rdf:resource="#ForestProduct"/>
  </owl:Class>

  <owl:Class rdf:about="&Government;IndependentState"/>
  <owl:Class rdf:about="&Mid-level-ontology;Automobile">
    <rdf:type rdf:resource="&owl;Thing"/>
    <rdfs:subClassOf rdf:resource="#DurableGood"/>
  </owl:Class>

  <owl:Class rdf:about="&Mid-level-ontology;Avocado">
    <rdfs:subClassOf rdf:resource="#GroceryProduce"/>
    <rdfs:subClassOf rdf:resource="#TropicalFruit"/>
  </owl:Class>

  <owl:Class rdf:about="&Mid-level-ontology;Beef">
    <rdfs:subClassOf rdf:resource="#MeatOfLandAnimal"/>
  </owl:Class>

  <owl:Class rdf:about="&Mid-level-ontology;Cement">
    <rdf:type rdf:resource="&owl;Thing"/>
    <rdfs:comment>Cement is a subclass of CompoundSubstance 

whose instances may contain various minerals or ores, prepared by 

heating and pulverizing, and used in binding Concrete or in laying 

brick or stone.</rdfs:comment>
    <rdfs:subClassOf rdf:resource="#ManufacturedProduct"/>
    <rdfs:subClassOf rdf:resource="&SUMO;CompoundSubstance"/>
  </owl:Class>

  <owl:Class rdf:about="&Mid-level-ontology;CerealGrain">
    <rdf:type rdf:resource="&owl;Thing"/>
    <rdfs:subClassOf rdf:resource="#PlantAgriculturalProduct"/>
    <rdfs:subClassOf rdf:resource="#Vegetable"/>
  </owl:Class>

  <owl:Class rdf:about="&Mid-level-ontology;Chicken">
    <rdfs:subClassOf rdf:resource="#Poultry"/>
  </owl:Class>

  <owl:Class rdf:about="&Mid-level-ontology;ChickenMeat">
    <rdfs:subClassOf rdf:resource="#MeatOfLandAnimal"/>
  </owl:Class>

  <owl:Class rdf:about="&Mid-level-ontology;Concrete">
    <rdfs:comment>Concrete is a class of CompoundSubstances 

used as building materials.  Concrete is made up of Mineral pieces 

(sand or gravel) and a Cement material used to bind them together.</rdfs:comment>
    <rdfs:subClassOf rdf:resource="#ManufacturedProduct"/>
    <rdfs:subClassOf rdf:resource="&SUMO;Mixture"/>
  </owl:Class>

  <owl:Class rdf:about="&Mid-level-ontology;ControlledSubstance">
    <rdfs:comment>ControlledSubstance is 

the subclass of BiologicallyActiveSubstances whose distribution 

and use is controlled by government regulation.</rdfs:comment>
    <rdfs:subClassOf rdf:resource="&SUMO;BiologicallyActiveSubstance"/>
    <owl:disjointWith rdf:resource="#Pyrethrum"/>
  </owl:Class>

  <owl:Class rdf:about="&Mid-level-ontology;DateFruit">
    <rdfs:subClassOf rdf:resource="#GroceryProduce"/>
    <rdfs:subClassOf rdf:resource="#TropicalFruit"/>
  </owl:Class>

  <owl:Class rdf:about="&Mid-level-ontology;Detergent">
    <rdf:type rdf:resource="&owl;Thing"/>
    <rdfs:comment>Detergent is the class of cleaning agents, 

including both Soap and synthetic cleaning solutions.</rdfs:comment>
    <rdfs:subClassOf rdf:resource="&SUMO;CompoundSubstance"/>
  </owl:Class>

  <owl:Class rdf:about="&Mid-level-ontology;DieselFuel">
    <rdfs:comment>DieselFuel is the subclass of 

RefinedPetroleumProducts that are fuels for diesel engines.</rdfs:comment>
    <rdfs:subClassOf rdf:resource="#RefinedPetroleumProduct"/>
  </owl:Class>

  <owl:Class rdf:about="&Mid-level-ontology;Donkey">
    <rdfs:subClassOf rdf:resource="#Livestock"/>
    <rdfs:subClassOf rdf:resource="&SUMO;HoofedMammal"/>
  </owl:Class>

  <owl:Class rdf:about="&Mid-level-ontology;EconomicAttribute">
    <rdfs:comment>EconomicAttribute is the class 

of terms including all Attributes used to characterize the 

economic systems or development levels of Nations or dependent 

GeopoliticalAreas.</rdfs:comment>
    <rdfs:subClassOf rdf:resource="&SUMO;RelationalAttribute"/>
  </owl:Class>

  <owl:Class rdf:about="&Mid-level-ontology;EconomicSystemAttribute">
    <rdfs:comment>EconomicSystemAttribute 

is the class of Attributes that describe the type of economic 

system that a country or area has.  For example, CapitalistEconomy 

or SocialistEconomy.</rdfs:comment>
    <rdfs:subClassOf rdf:resource="&Mid-level-ontology;EconomicAttribute"/>
  </owl:Class>

  <owl:Class rdf:about="&Mid-level-ontology;ElectricDevice">
    <rdf:type rdf:resource="&owl;Thing"/>
  </owl:Class>

  <owl:Class rdf:about="&Mid-level-ontology;Exporting">
    <rdfs:comment>Exporting is the class of actions in 

which there is a ChangeOfPossession of goods shipped from a 

provider in one Nation to a destination in another Nation. 

Typically, there are Selling and Buying events associated 

with an Exporting.  Either the seller or the exporting country 

may be considered the origin of Exporting.</rdfs:comment>
    <rdfs:subClassOf rdf:resource="&SUMO;ChangeOfPossession"/>
    <rdfs:subClassOf rdf:resource="&SUMO;FinancialTransaction"/>
  </owl:Class>

  <owl:Class rdf:about="&Mid-level-ontology;Fodder">
    <rdfs:comment>Fodder is the class of OrganicObjects that 

are used as food for domesticated animals.</rdfs:comment>
    <rdfs:subClassOf rdf:resource="&SUMO;OrganicObject"/>
    <owl:disjointWith rdf:resource="#AgriculturalProduct"/>
  </owl:Class>

  <owl:Class rdf:about="&Mid-level-ontology;Furniture">
    <rdf:type rdf:resource="&owl;Thing"/>
    <rdfs:subClassOf rdf:resource="#DurableGood"/>
  </owl:Class>

  <owl:Class rdf:about="&Mid-level-ontology;Gasoline">
    <rdfs:comment>Gasoline is the subclass of 

RefinedPetroleumProducts that are fuels for internal combustion engines.</rdfs:comment>
    <rdfs:subClassOf rdf:resource="#RefinedPetroleumProduct"/>
  </owl:Class>

  <owl:Class rdf:about="&Mid-level-ontology;Goat">
    <rdf:type rdf:resource="&owl;Thing"/>
    <rdfs:subClassOf rdf:resource="#Livestock"/>
    <rdfs:subClassOf rdf:resource="&SUMO;HoofedMammal"/>
  </owl:Class>

  <owl:Class rdf:about="&Mid-level-ontology;Grass"/>
  <owl:Class rdf:about="&Mid-level-ontology;Honey">
    <rdfs:subClassOf rdf:resource="#AnimalAgriculturalProduct"/>
  </owl:Class>

  <owl:Class rdf:about="&Mid-level-ontology;Horse">
    <rdfs:subClassOf rdf:resource="#Livestock"/>
    <rdfs:subClassOf rdf:resource="&SUMO;HoofedMammal"/>
  </owl:Class>

  <owl:Class rdf:about="&Mid-level-ontology;IndustryAttribute"/>
  <SUMO:UnitOfMeasure rdf:about="&Mid-level-ontology;KilowattHour">
    <rdf:type rdf:resource="&owl;Class"/>
    <rdfs:comment>KilowattHour is a UnitOfMeasure for 

energy that represents 1000 Watts (1 kW) of power expended over one 

hour (1 h) of time.  This is the unit commonly used in commercial 

power contexts.  It is equivalent to 3,600,000 Joules.</rdfs:comment>
    <rdfs:subClassOf rdf:resource="&SUMO;FunctionQuantity"/>
  </SUMO:UnitOfMeasure>

  <owl:Class rdf:about="&Mid-level-ontology;Milk">
    <rdfs:subClassOf rdf:resource="#DairyProduct"/>
  </owl:Class>

  <owl:Class rdf:about="&Mid-level-ontology;Narcotic">
    <rdfs:comment>Narcotic is a subclass of addictive 

BiologicallyActiveSubstances that have damping effects on the 

nervous system and may be fatal in large doses.</rdfs:comment>
    <rdfs:subClassOf rdf:resource="&Mid-level-ontology;ControlledSubstance"/>
  </owl:Class>

  <owl:Class rdf:about="&Mid-level-ontology;Opium">
    <rdfs:subClassOf rdf:resource="#PlantAgriculturalProduct"/>
    <rdfs:subClassOf rdf:resource="&Mid-level-ontology;Narcotic"/>
  </owl:Class>

  <owl:Class rdf:about="&Mid-level-ontology;Pig">
    <rdfs:subClassOf rdf:resource="#Livestock"/>
    <rdfs:subClassOf rdf:resource="&SUMO;HoofedMammal"/>
  </owl:Class>

  <owl:Class rdf:about="&Mid-level-ontology;Sheep">
    <rdf:type rdf:resource="&owl;Thing"/>
    <rdfs:subClassOf rdf:resource="#Livestock"/>
    <rdfs:subClassOf rdf:resource="&SUMO;HoofedMammal"/>
  </owl:Class>

  <owl:Class rdf:about="&Mid-level-ontology;Steel">
    <SUMO:relatedInternalConcept rdf:resource="&Mid-level-ontology;Iron"/>
    <rdf:type rdf:resource="&owl;Thing"/>
    <rdfs:subClassOf rdf:resource="#MetalProduct"/>
  </owl:Class>

  <owl:Class rdf:about="&Mid-level-ontology;Sugar">
    <rdfs:subClassOf rdf:resource="#PlantAgriculturalProduct"/>
    <rdfs:subClassOf rdf:resource="&SUMO;Substance"/>
  </owl:Class>

  <owl:Class rdf:about="&Mid-level-ontology;Wine">
    <rdfs:subClassOf rdf:resource="#PlantAgriculturalProduct"/>
    <rdfs:subClassOf rdf:resource="&SUMO;Beverage"/>
  </owl:Class>

  <owl:Class rdf:about="&SUMO;Agent"/>
  <owl:Class rdf:about="&SUMO;AnatomicalStructure"/>
  <owl:Class rdf:about="&SUMO;Artifact">
    <rdf:type rdf:resource="&owl;Thing"/>
  </owl:Class>

  <owl:Class rdf:about="&SUMO;Beverage"/>
  <owl:Class rdf:about="&SUMO;BinaryPredicate"/>
  <owl:Class rdf:about="&SUMO;BiologicallyActiveSubstance"/>
  <owl:Class rdf:about="&SUMO;Bird"/>
  <owl:Class rdf:about="&SUMO;BodyCovering"/>
  <owl:Class rdf:about="&SUMO;ChangeOfPossession"/>
  <owl:Class rdf:about="&SUMO;Clothing">
    <SUMO:disjoint rdf:resource="#TextileProduct"/>
    <rdf:type rdf:resource="&owl;Thing"/>
    <rdfs:subClassOf rdf:resource="#WearableItem"/>
  </owl:Class>

  <owl:Class rdf:about="&SUMO;CompoundSubstance"/>
  <owl:Class rdf:about="&SUMO;CurrencyMeasure"/>
  <owl:Class rdf:about="&SUMO;Device"/>
  <SUMO:UnitOfMeasure rdf:about="&SUMO;EuroDollar">
    <rdf:type rdf:resource="&owl;Class"/>
    <rdfs:comment>EuroDollar represents the basic unit of 

currency of the EuropeanUnion.</rdfs:comment>
    <rdfs:subClassOf rdf:resource="&SUMO;CurrencyMeasure"/>
  </SUMO:UnitOfMeasure>

  <owl:Class rdf:about="&SUMO;Fabric">
    <rdf:type rdf:resource="&owl;Thing"/>
    <rdfs:subClassOf rdf:resource="#TextileProduct"/>
  </owl:Class>

  <owl:Class rdf:about="&SUMO;FinancialTransaction"/>
  <owl:Class rdf:about="&SUMO;Fish"/>
  <owl:Class rdf:about="&SUMO;FloweringPlant">
    <rdf:type rdf:resource="&owl;Thing"/>
  </owl:Class>

  <owl:Class rdf:about="&SUMO;FruitOrVegetable"/>
  <owl:Class rdf:about="&SUMO;FunctionQuantity"/>
  <owl:Class rdf:about="&SUMO;GeopoliticalArea"/>
  <owl:Class rdf:about="&SUMO;HoofedMammal">
    <rdfs:comment>HoofedMammal is the subclass of Livestock

that are hoofed animals.</rdfs:comment>
    <rdfs:subClassOf rdf:resource="#AnimalAgriculturalProduct"/>
    <rdfs:subClassOf rdf:resource="#Livestock"/>
  </owl:Class>

  <owl:Class rdf:about="&SUMO;IntentionalProcess"/>
  <owl:Class rdf:about="&SUMO;IrreflexiveRelation"/>
  <owl:Class rdf:about="&SUMO;Machine">
    <rdfs:subClassOf rdf:resource="#Machinery"/>
  </owl:Class>

  <owl:Class rdf:about="&SUMO;Mammal"/>
  <owl:Class rdf:about="&SUMO;Meat">
    <rdfs:subClassOf rdf:resource="#AnimalAgriculturalProduct"/>
  </owl:Class>

  <owl:Class rdf:about="&SUMO;Mineral"/>
  <owl:Class rdf:about="&SUMO;Mixture"/>
  <owl:Class rdf:about="&SUMO;Nation"/>
  <owl:Class rdf:about="&SUMO;Object"/>
  <owl:Class rdf:about="&SUMO;OrganicObject"/>
  <owl:Class rdf:about="&SUMO;Organization"/>
  <owl:Class rdf:about="&SUMO;PhysicalQuantity"/>
  <owl:Class rdf:about="&SUMO;Plant">
    <rdf:type rdf:resource="&owl;Thing"/>
  </owl:Class>

  <owl:Class rdf:about="&SUMO;Process"/>
  <owl:Class rdf:about="&SUMO;Product"/>
  <owl:Class rdf:about="&SUMO;Relation"/>
  <owl:Class rdf:about="&SUMO;RelationalAttribute"/>
  <owl:Class rdf:about="&SUMO;ReproductiveBody"/>
  <owl:Class rdf:about="&SUMO;Reptile"/>
  <owl:Class rdf:about="&SUMO;Seed">
    <rdfs:subClassOf rdf:resource="&SUMO;FruitOrVegetable"/>
    <owl:disjointWith rdf:resource="#GroceryProduce"/>
    <owl:disjointWith rdf:resource="#RootStarch"/>
    <owl:disjointWith rdf:resource="#RootVegetable"/>
    <owl:disjointWith rdf:resource="#Spice"/>
    <owl:disjointWith rdf:resource="#TeaPlantAerialPart"/>
    <owl:disjointWith rdf:resource="#Vegetable"/>
  </owl:Class>

  <owl:Class rdf:about="&SUMO;Substance"/>
  <owl:Class rdf:about="&SUMO;SymbolicString"/>
  <owl:Class rdf:about="&SUMO;TernaryPredicate"/>
  <owl:Class rdf:about="&SUMO;UnaryFunction"/>
  <owl:Class rdf:about="&SUMO;UnitOfMeasure"/>

<!-- Annotation Properties -->
  <owl:AnnotationProperty rdf:about="&rdfs;comment"/>
  <owl:AnnotationProperty rdf:about="&rdfs;label"/>

<!-- Datatype Properties -->
  <SUMO:BinaryPredicate rdf:about="#highestDecileShareOfHouseholdIncome">
    <rdf:type rdf:resource="&owl;DatatypeProperty"/>
    <rdfs:comment>(highestDecileShareOfHouseholdIncome ?AREA ?FRACTION) means that 

in the GeopoliticalArea ?AREA, the highest decile (90-100%) of 

households with respect to household income (or consumption) had 

?FRACTION amount of the total household income (or consumption).  

Data from different countries may not be directly comparable due to 

variation in the basis of the data (e.g., based on income versus 

based on consumption).</rdfs:comment>
    <rdfs:domain rdf:resource="&SUMO;GeopoliticalArea"/>
  </SUMO:BinaryPredicate>

  <SUMO:BinaryPredicate rdf:about="#incomeDistributionByGiniIndex">
    <rdf:type rdf:resource="&owl;DatatypeProperty"/>
    <rdfs:comment>(incomeDistributionByGiniIndex ?AREA ?INDEX) means that in the 

GeopoliticalArea ?AREA, the distribution of family income is ?INDEX, 

as measured by the Gini index for family income distribution.</rdfs:comment>
    <rdfs:domain rdf:resource="&SUMO;GeopoliticalArea"/>
  </SUMO:BinaryPredicate>

  <SUMO:BinaryPredicate rdf:about="#industrialProductionGrowthRate">
    <rdf:type rdf:resource="&owl;DatatypeProperty"/>
    <rdfs:comment>(industrialProductionGrowthRate ?AREA ?RATE) means that in 

the GeopoliticalArea ?AREA, the annual percentage increase in 

industrial production is ?RATE.</rdfs:comment>
    <rdfs:domain rdf:resource="&SUMO;GeopoliticalArea"/>
  </SUMO:BinaryPredicate>

  <SUMO:BinaryPredicate rdf:about="#inflationRateOfConsumerPrices">
    <rdf:type rdf:resource="&owl;DatatypeProperty"/>
    <rdfs:comment>(inflationRateOfConsumerPrices ?AREA ?FRACTION) means that in the 

GeopoliticalArea ?AREA, the annual change in consumer prices was 

?FRACTION, compared with prices from the previous year.</rdfs:comment>
    <rdfs:domain rdf:resource="&SUMO;GeopoliticalArea"/>
  </SUMO:BinaryPredicate>

  <SUMO:BinaryPredicate rdf:about="#laborForceTotal">
    <rdf:type rdf:resource="&owl;DatatypeProperty"/>
    <rdfs:comment>(laborForceTotal ?AREA ?AMOUNT) means that the total labor 

force of the GeopoliticalArea ?AREA is ?AMOUNT. This includes 

unemployed workers.</rdfs:comment>
    <rdfs:domain rdf:resource="&SUMO;GeopoliticalArea"/>
  </SUMO:BinaryPredicate>

  <SUMO:BinaryPredicate rdf:about="#lowestDecileShareOfHouseholdIncome">
    <rdf:type rdf:resource="&owl;DatatypeProperty"/>
    <rdfs:comment>(lowestDecileShareOfHouseholdIncome ?AREA ?FRACTION) means that 

in the GeopoliticalArea ?AREA, the lowest decile (0-10%) of 

households with respect to household income (or consumption) had 

?FRACTION amount of the total household income (or consumption).  

Data from different countries may not be directly comparable due to 

variation in the basis of the data (e.g., based on income versus based 

on consumption).</rdfs:comment>
    <rdfs:domain rdf:resource="&SUMO;GeopoliticalArea"/>
  </SUMO:BinaryPredicate>

  <SUMO:BinaryPredicate rdf:about="#populationFractionBelowPovertyLine">
    <rdf:type rdf:resource="&owl;DatatypeProperty"/>
    <rdfs:comment>(populationFractionBelowPovertyLine ?AREA ?FRACTION) means that in 

the GeopoliticalArea ?AREA, the segment of the population living 

below the (locally defined) poverty line is ?FRACTION.  Note that the 

definition of the poverty line varies internationally.</rdfs:comment>
    <rdfs:domain rdf:resource="&SUMO;GeopoliticalArea"/>
  </SUMO:BinaryPredicate>

  <Economy:PPPBasedEconomicValuation rdf:about="#realGrowthRateOfGDP">
    <rdf:type rdf:resource="&SUMO;BinaryPredicate"/>
    <rdf:type rdf:resource="&owl;DatatypeProperty"/>
    <rdfs:comment>(realGrowthRateOfGDP ?AREA ?RATE) 

means that the annual rate of growth in the Gross Domestic Product (GDP) 

for the GeopoliticalArea ?AREA is the fraction ?RATE, adjusted for 

inflation, with GDP calculated on a purchasing power parity basis.  

See PPPBasedEconomicValuation.</rdfs:comment>
    <rdfs:domain rdf:resource="&SUMO;GeopoliticalArea"/>
  </Economy:PPPBasedEconomicValuation>

<!-- Object Properties -->
  <SUMO:UnaryFunction rdf:about="#AgricultureFn">
    <SUMO:rangeSubclass rdf:resource="&Mid-level-ontology;Agriculture"/>
    <rdf:type rdf:resource="&owl;ObjectProperty"/>
    <rdfs:comment>(AgricultureFn ?PRODUCT) denotes the 

subclass of Agriculture processes in which the AgriculturalProduct 

?PRODUCT is cultivated.</rdfs:comment>
    <rdfs:domain rdf:resource="#AgriculturalProduct"/>
  </SUMO:UnaryFunction>

  <SUMO:UnaryFunction rdf:about="#FiscalYearFn">
    <rdf:type rdf:resource="&owl;ObjectProperty"/>
    <rdfs:comment>(FiscalYearFn ?PLACE) denotes the subclass 

of TimeIntervals that are fiscalYearPeriods of the Organization or 

GeopoliticalArea ?PLACE.</rdfs:comment>
    <rdfs:domain rdf:resource="&SUMO;Agent"/>
  </SUMO:UnaryFunction>

  <SUMO:BinaryPredicate rdf:about="#agriculturalProductType">
    <rdf:type rdf:resource="&owl;ObjectProperty"/>
    <rdfs:comment>(agriculturalProductType ?AREA ?TYPE) means that the 

GeopoliticalArea ?AREA produces a crop or other 

agricultural product of ?TYPE.</rdfs:comment>
    <rdfs:domain rdf:resource="&SUMO;GeopoliticalArea"/>
    <rdfs:range rdf:resource="&SUMO;Object"/>
  </SUMO:BinaryPredicate>

  <SUMO:BinaryPredicate rdf:about="#annualElectricityConsumption">
    <rdf:type rdf:resource="&owl;ObjectProperty"/>
    <rdfs:comment>(annualElectricityConsumption ?AREA ?AMOUNT) means that the 

GeopoliticalArea ?AREA uses ?AMOUNT of electricity (measured in 

KilowattHours) annually.</rdfs:comment>
    <rdfs:domain rdf:resource="&SUMO;GeopoliticalArea"/>
    <rdfs:range rdf:resource="&SUMO;PhysicalQuantity"/>
  </SUMO:BinaryPredicate>

  <SUMO:BinaryPredicate rdf:about="#annualElectricityExport">
    <rdf:type rdf:resource="&owl;ObjectProperty"/>
    <rdfs:comment>(annualElectricityExport ?AREA ?AMOUNT) means that the 

GeopoliticalArea ?AREA exported the total ?AMOUNT of 

electricity (measured in KilowattHours) annually.</rdfs:comment>
    <rdfs:domain rdf:resource="&SUMO;GeopoliticalArea"/>
    <rdfs:range rdf:resource="&SUMO;PhysicalQuantity"/>
  </SUMO:BinaryPredicate>

  <SUMO:BinaryPredicate rdf:about="#annualElectricityImport">
    <rdf:type rdf:resource="&owl;ObjectProperty"/>
    <rdfs:comment>(annualElectricityImport ?AREA ?AMOUNT) means that the 

GeopoliticalArea ?AREA imported the total ?AMOUNT of 

electricity (measured in KilowattHours) annually.</rdfs:comment>
    <rdfs:domain rdf:resource="&SUMO;GeopoliticalArea"/>
    <rdfs:range rdf:resource="&SUMO;PhysicalQuantity"/>
  </SUMO:BinaryPredicate>

  <SUMO:BinaryPredicate rdf:about="#annualElectricityProduction">
    <rdf:type rdf:resource="&owl;ObjectProperty"/>
    <rdfs:comment>(annualElectricityProduction ?AREA ?AMOUNT) means that the amount of 

electricity generated annually in the GeographicalArea ?AREA is 

?AMOUNT, measured in KilowattHours.</rdfs:comment>
    <rdfs:domain rdf:resource="&SUMO;GeopoliticalArea"/>
    <rdfs:range rdf:resource="&SUMO;PhysicalQuantity"/>
  </SUMO:BinaryPredicate>

  <SUMO:BinaryPredicate rdf:about="#annualExpenditures">
    <rdf:type rdf:resource="&owl;ObjectProperty"/>
    <rdfs:comment>(annualExpenditures ?AGENT ?AMOUNT) means that the annual 

budgetary expenditures of the Agent ?AGENT are ?AMOUNT.</rdfs:comment>
    <rdfs:domain rdf:resource="&SUMO;Agent"/>
    <rdfs:range rdf:resource="&SUMO;CurrencyMeasure"/>
  </SUMO:BinaryPredicate>

  <SUMO:BinaryPredicate rdf:about="#annualExpendituresOfArea">
    <rdf:type rdf:resource="&owl;ObjectProperty"/>
    <rdfs:comment>(annualExpendituresOfArea ?AREA ?AMOUNT) means that the annual 

budgetary expenditures of the GeopoliticalArea ?AREA are ?AMOUNT, 

calculated in U.S. dollars according  to the currency exchange rate 

method.</rdfs:comment>
    <rdfs:domain rdf:resource="&SUMO;GeopoliticalArea"/>
    <rdfs:range rdf:resource="&SUMO;CurrencyMeasure"/>
    <rdfs:subPropertyOf rdf:resource="#annualExpenditures"/>
  </SUMO:BinaryPredicate>

  <SUMO:BinaryPredicate rdf:about="#annualExportTotal">
    <rdf:type rdf:resource="&owl;ObjectProperty"/>
    <rdfs:comment>(annualExportTotal ?AREA ?AMOUNT) means that the total 

value of exports from the GeopoliticalArea ?AREA is ?AMOUNT 

(in UnitedStatesDollars) annually.  Export value is calculated 

on a Free on Board (F.O.B.) basis.</rdfs:comment>
    <rdfs:domain rdf:resource="&SUMO;GeopoliticalArea"/>
    <rdfs:range rdf:resource="&SUMO;CurrencyMeasure"/>
  </SUMO:BinaryPredicate>

  <SUMO:BinaryPredicate rdf:about="#annualImportTotal">
    <rdf:type rdf:resource="&owl;ObjectProperty"/>
    <rdfs:comment>(annualImportTotal ?AREA ?AMOUNT) means that the total 

value of imports to the GeopoliticalArea ?AREA is ?AMOUNT (in 

UnitedStatesDollars) annually.  Import value is calculated on a Cost, 

Insurance, and Freight (C.I.F.) or a Free on Board (F.O.B.) basis.</rdfs:comment>
    <rdfs:domain rdf:resource="&SUMO;GeopoliticalArea"/>
    <rdfs:range rdf:resource="&SUMO;CurrencyMeasure"/>
  </SUMO:BinaryPredicate>

  <SUMO:BinaryPredicate rdf:about="#annualRevenues">
    <rdf:type rdf:resource="&owl;ObjectProperty"/>
    <rdfs:comment>(annualRevenues ?AGENT ?AMOUNT) means that the annual budgetary 

revenues of the Agent ?AGENT are ?AMOUNT.</rdfs:comment>
    <rdfs:domain rdf:resource="&SUMO;Agent"/>
    <rdfs:range rdf:resource="&SUMO;CurrencyMeasure"/>
  </SUMO:BinaryPredicate>

  <SUMO:BinaryPredicate rdf:about="#annualRevenuesOfArea">
    <rdf:type rdf:resource="&owl;ObjectProperty"/>
    <rdfs:comment>(annualRevenuesOfArea ?AREA ?AMOUNT) means that the annual budgetary 

revenues of the GeopoliticalArea ?AREA are ?AMOUNT, calculated in U.S. 

dollars according  to the currency exchange rate method.</rdfs:comment>
    <rdfs:domain rdf:resource="&SUMO;GeopoliticalArea"/>
    <rdfs:range rdf:resource="&SUMO;CurrencyMeasure"/>
    <rdfs:subPropertyOf rdf:resource="#annualRevenues"/>
  </SUMO:BinaryPredicate>

  <SUMO:BinaryPredicate rdf:about="#capitalExpenditures">
    <rdf:type rdf:resource="&owl;ObjectProperty"/>
    <rdfs:comment>(capitalExpenditures ?AGENT ?AMOUNT) means that the annual capital 

expenditures of the Agent ?AGENT are ?AMOUNT.</rdfs:comment>
    <rdfs:domain rdf:resource="&SUMO;Agent"/>
    <rdfs:range rdf:resource="&SUMO;CurrencyMeasure"/>
  </SUMO:BinaryPredicate>

  <SUMO:BinaryPredicate rdf:about="#capitalExpendituresOfArea">
    <rdf:type rdf:resource="&owl;ObjectProperty"/>
    <rdfs:comment>(capitalExpendituresOfArea ?AREA ?AMOUNT) means that the annual 

capital expenditures of the GeopoliticalArea ?AREA are ?AMOUNT, 

calculated in U.S. dollars according to the currency exchange rate 

method.  This figure is a portion of the annualExpendituresOfArea 

for ?AREA.</rdfs:comment>
    <rdfs:domain rdf:resource="&SUMO;GeopoliticalArea"/>
    <rdfs:range rdf:resource="&SUMO;CurrencyMeasure"/>
    <rdfs:subPropertyOf rdf:resource="#capitalExpenditures"/>
  </SUMO:BinaryPredicate>

  <SUMO:BinaryPredicate rdf:about="#currencyCode">
    <rdf:type rdf:resource="&owl;ObjectProperty"/>
    <rdfs:comment>(currencyCode ?CODE ?UNIT) means 

that ?CODE is the InternationalOrganizationForStandardization 

(ISO) 4217 alphabetic currency code for the national 

CurrencyMeasure ?UNIT.</rdfs:comment>
    <rdfs:domain rdf:resource="&SUMO;SymbolicString"/>
    <rdfs:range rdf:resource="&SUMO;CurrencyMeasure"/>
    <rdfs:range rdf:resource="&SUMO;UnitOfMeasure"/>
  </SUMO:BinaryPredicate>

  <SUMO:BinaryPredicate rdf:about="#currencyExchangePerUSDollar">
    <rdf:type rdf:resource="&owl;ObjectProperty"/>
    <rdfs:comment>(currencyExchangePerUSDollar ?AMOUNT ?PERIOD) means that one 

UnitedStatesDollar is worth ?AMOUNT (in a non-U.S. CurrencyMeasure), 

during the TimeInterval indicated by ?PERIOD.  The rate of exchange may 

be based either on international market forces or official fiat.</rdfs:comment>
    <rdfs:domain rdf:resource="&SUMO;CurrencyMeasure"/>
  </SUMO:BinaryPredicate>

  <SUMO:BinaryPredicate rdf:about="#currencyExchangeRate">
    <rdf:type rdf:resource="&owl;ObjectProperty"/>
    <rdfs:comment>(currencyExchangeRate ?UNIT ?AMOUNT) means that the currency 

denomination ?UNIT is worth ?AMOUNT (which is in another 

CurrencyMeasure).</rdfs:comment>
    <rdfs:domain rdf:resource="&SUMO;CurrencyMeasure"/>
    <rdfs:domain rdf:resource="&SUMO;UnitOfMeasure"/>
    <rdfs:range rdf:resource="&SUMO;CurrencyMeasure"/>
  </SUMO:BinaryPredicate>

  <SUMO:BinaryPredicate rdf:about="#economicAidDonated">
    <rdf:type rdf:resource="&owl;ObjectProperty"/>
    <rdfs:comment>(economicAidDonated ?AGENT ?AMOUNT) means that the GeopoliticalArea 

?AREA donated ?AMOUNT of aid (valued in U.S. dollars) to developing 

countries and multilateral organizations.  This figure covers 'net 

official development assistance' (ODA), which is net financial assistance 

from nations belonging to the 

OrganizationForEconomicCooperationAndDevelopment (OECD), with the main 

goal of promoting economic development and welfare.  Such aid contains a 

grant element of at least 25%.  This statistic does not cover private 

flows of assistance or other official flows (OOF).</rdfs:comment>
    <rdfs:domain rdf:resource="&SUMO;GeopoliticalArea"/>
    <rdfs:range rdf:resource="&SUMO;CurrencyMeasure"/>
  </SUMO:BinaryPredicate>

  <SUMO:BinaryPredicate rdf:about="#economicAidReceivedNet">
    <rdf:type rdf:resource="&owl;ObjectProperty"/>
    <rdfs:comment>(economicAidReceivedNet ?AREA ?AMOUNT) means that the 

GeopoliticalArea ?AREA had a net inflow of Official Development Finance 

(ODF) of ?AMOUNT.  ODF includes funds from the World Bank, the IMF, other 

international organizations, and individual donor nations, including both 

grants and loans.  The figure includes formal commitments of aid not yet 

disbursed.  The figure is the net amount of inflow after deducting 

repayments, valued in U.S. dollars.</rdfs:comment>
    <rdfs:domain rdf:resource="&SUMO;GeopoliticalArea"/>
    <rdfs:range rdf:resource="&SUMO;CurrencyMeasure"/>
  </SUMO:BinaryPredicate>

  <SUMO:BinaryPredicate rdf:about="#exportCommodityType">
    <rdf:type rdf:resource="&owl;ObjectProperty"/>
    <rdfs:comment>(exportCommodityType ?AREA ?TYPE) means that the GeopoliticalArea 

?AREA exports the commodity ?TYPE.</rdfs:comment>
    <rdfs:domain rdf:resource="&SUMO;GeopoliticalArea"/>
    <rdfs:range rdf:resource="&SUMO;Object"/>
  </SUMO:BinaryPredicate>

  <SUMO:BinaryPredicate rdf:about="#exportPartner">
    <rdf:type rdf:resource="&SUMO;IrreflexiveRelation"/>
    <rdf:type rdf:resource="&owl;ObjectProperty"/>
    <rdfs:comment>(exportPartner ?AGENT1 ?AGENT2) 

means that the Agent ?AGENT1 exports goods to the Agent 

?AGENT2.</rdfs:comment>
    <rdfs:domain rdf:resource="&SUMO;Agent"/>
    <rdfs:range rdf:resource="&SUMO;Agent"/>
  </SUMO:BinaryPredicate>

  <SUMO:IrreflexiveRelation rdf:about="#exportPartnerInPeriod">
    <rdf:type rdf:resource="&SUMO;TernaryPredicate"/>
    <rdf:type rdf:resource="&owl;ObjectProperty"/>
    <rdfs:comment>(exportPartnerInPeriod ?AGENT1 ?AGENT2 ?PERIOD) means that the Agent 

?AGENT1 exports goods to the Agent ?AGENT2 during the TimeInterval 

indicated by ?PERIOD.</rdfs:comment>
    <rdfs:domain rdf:resource="&SUMO;Agent"/>
    <rdfs:range rdf:resource="&SUMO;Agent"/>
  </SUMO:IrreflexiveRelation>

  <SUMO:BinaryPredicate rdf:about="#externalDebt">
    <rdf:type rdf:resource="&owl;ObjectProperty"/>
    <rdfs:comment>(externalDebt ?COUNTRY ?AMOUNT) means 

that the GeopoliticalArea ?COUNTRY owes the total sum ?AMOUNT of debt 

(public and private) to nonresidents.  The amount is valued in U.S. 

dollars but may be repayable in foreign currency, goods, or services.</rdfs:comment>
    <rdfs:domain rdf:resource="&SUMO;GeopoliticalArea"/>
    <rdfs:range rdf:resource="&SUMO;CurrencyMeasure"/>
  </SUMO:BinaryPredicate>

  <SUMO:BinaryPredicate rdf:about="#importCommodityType">
    <rdf:type rdf:resource="&owl;ObjectProperty"/>
    <rdfs:comment>(importCommodityType ?AREA ?TYPE) means that the GeopoliticalArea 

?AREA imports the commodity ?TYPE.</rdfs:comment>
    <rdfs:domain rdf:resource="&SUMO;GeopoliticalArea"/>
    <rdfs:range rdf:resource="&SUMO;Object"/>
  </SUMO:BinaryPredicate>

  <SUMO:BinaryPredicate rdf:about="#importPartner">
    <rdf:type rdf:resource="&SUMO;IrreflexiveRelation"/>
    <rdf:type rdf:resource="&owl;ObjectProperty"/>
    <rdfs:comment>(importPartner ?AGENT1 ?AGENT2) means 

that the Agent ?AGENT1 imports goods from the Agent ?AGENT2.</rdfs:comment>
    <rdfs:domain rdf:resource="&SUMO;Agent"/>
    <rdfs:range rdf:resource="&SUMO;Agent"/>
  </SUMO:BinaryPredicate>

  <SUMO:IrreflexiveRelation rdf:about="#importPartnerInPeriod">
    <rdf:type rdf:resource="&SUMO;TernaryPredicate"/>
    <rdf:type rdf:resource="&owl;ObjectProperty"/>
    <rdfs:comment>(importPartnerInPeriod ?AGENT1 ?AGENT2 ?PERIOD) means that the Agent 

?AGENT1 imports goods from the Agent ?AGENT2 during the TimeInterval 

indicated by ?PERIOD.</rdfs:comment>
    <rdfs:domain rdf:resource="&SUMO;Agent"/>
    <rdfs:range rdf:resource="&SUMO;Agent"/>
  </SUMO:IrreflexiveRelation>

  <SUMO:BinaryPredicate rdf:about="#industryServiceType">
    <rdf:type rdf:resource="&owl;ObjectProperty"/>
    <rdfs:comment>(industryServiceType ?INDUSTRY ?TYPE) means that organizations with 

the IndustryAttribute ?INDUSTRY provide services of the kind ?TYPE.</rdfs:comment>
    <rdfs:domain rdf:resource="&Mid-level-ontology;IndustryAttribute"/>
    <rdfs:range rdf:resource="&SUMO;IntentionalProcess"/>
  </SUMO:BinaryPredicate>

  <SUMO:BinaryPredicate rdf:about="#organizationProductType">
    <rdf:type rdf:resource="&owl;ObjectProperty"/>
    <rdfs:comment>(organizationProductType ?BUSINESS ?TYPE) means that the Organization 

?BUSINESS produces products of the kind ?TYPE.</rdfs:comment>
    <rdfs:domain rdf:resource="&SUMO;Organization"/>
    <rdfs:range rdf:resource="&SUMO;Object"/>
  </SUMO:BinaryPredicate>

  <SUMO:BinaryPredicate rdf:about="#organizationServiceType">
    <rdf:type rdf:resource="&owl;ObjectProperty"/>
    <rdfs:comment>(organizationServiceType ?BUSINESS ?TYPE) means that the Organization 

?BUSINESS provides services of the kind ?TYPE.</rdfs:comment>
    <rdfs:domain rdf:resource="&SUMO;Organization"/>
    <rdfs:range rdf:resource="&SUMO;IntentionalProcess"/>
  </SUMO:BinaryPredicate>

  <Economy:PPPBasedEconomicValuation rdf:about="#perCapitaGDP">
    <rdf:type rdf:resource="&SUMO;BinaryPredicate"/>
    <rdf:type rdf:resource="&owl;ObjectProperty"/>
    <rdfs:comment>(perCapitaGDP ?AREA ?AMOUNT) means 

that the Gross Domestic Product, on a per capita basis, for the 

GeopoliticalArea ?AREA is ?AMOUNT, calculated in U.S. dollars on a 

purchasing power parity basis.  See PPPBasedEconomicValuation.</rdfs:comment>
    <rdfs:domain rdf:resource="&SUMO;GeopoliticalArea"/>
    <rdfs:range rdf:resource="&SUMO;CurrencyMeasure"/>
  </Economy:PPPBasedEconomicValuation>

  <SUMO:BinaryPredicate rdf:about="#resultType">
    <rdf:type rdf:resource="&owl;ObjectProperty"/>
    <rdfs:comment>(resultType ?PROCESS ?TYPE) means that 

the Process ?PROCESS produces some result(s) of the type ?TYPE.</rdfs:comment>
    <rdfs:domain rdf:resource="&SUMO;Process"/>
    <rdfs:range rdf:resource="&SUMO;Object"/>
  </SUMO:BinaryPredicate>

  <SUMO:BinaryPredicate rdf:about="&Mid-level-ontology;currencyType">
    <rdf:type rdf:resource="&owl;ObjectProperty"/>
    <rdfs:comment>(currencyType ?AREA ?UNIT) means 

that the official currency used in the GeopoliticalArea ?AREA 

is the UnitOfMeasure ?UNIT.</rdfs:comment>
    <rdfs:domain rdf:resource="&SUMO;GeopoliticalArea"/>
    <rdfs:range rdf:resource="&SUMO;CurrencyMeasure"/>
    <rdfs:range rdf:resource="&SUMO;UnitOfMeasure"/>
  </SUMO:BinaryPredicate>

  <SUMO:BinaryPredicate rdf:about="&Mid-level-ontology;economyType">
    <rdf:type rdf:resource="&owl;ObjectProperty"/>
    <rdfs:comment>(economyType ?POLITY ?TYPE) means that the 

GeopoliticalArea ?POLITY has an economic system of TYPE.</rdfs:comment>
    <rdfs:domain rdf:resource="&SUMO;Agent"/>
    <rdfs:range rdf:resource="&Mid-level-ontology;EconomicAttribute"/>
  </SUMO:BinaryPredicate>

  <SUMO:BinaryPredicate rdf:about="&Mid-level-ontology;fiscalYearPeriod">
    <rdf:type rdf:resource="&owl;ObjectProperty"/>
    <rdfs:comment>The predicate fiscalYearPeriod 

indicates the period that an Agent or Organization uses as its 

12-month accounting period.  (fiscalYearPeriod ?AGENT Year) means 

that ?AGENT observes its 12-month accounting period during the 

regular calendar year (CY), from January to December.  For 

fiscal years with other beginning and ending months (FYs), use 

(fiscalYearPeriod ?AGENT (RecurrentTimeIntervalFn ?STARTMONTH ?ENDMONTH)).  

For example, (fiscalYearPeriod (GovernmentFn UnitedStates) 

(RecurrentTimeIntervalFn October September)).  For FYs that begin 

or end mid-month, days may be specified within RecurrentTimeIntervalFn.</rdfs:comment>
    <rdfs:domain rdf:resource="&SUMO;Agent"/>
  </SUMO:BinaryPredicate>

  <SUMO:BinaryPredicate rdf:about="&Mid-level-ontology;industryOfArea">
    <rdf:type rdf:resource="&owl;ObjectProperty"/>
    <rdfs:comment>(industryOfArea ?AREA ?SECTOR) 

means that the GeopoliticalArea ?AREA produces goods or services 

in the economic area ?SECTOR.</rdfs:comment>
    <rdfs:domain rdf:resource="&SUMO;GeopoliticalArea"/>
    <rdfs:range rdf:resource="#IndustryAttribute"/>
  </SUMO:BinaryPredicate>

  <SUMO:BinaryPredicate rdf:about="&Mid-level-ontology;industryProductType">
    <rdf:type rdf:resource="&owl;ObjectProperty"/>
    <rdfs:comment>(industryProductType ?INDUSTRY ?TYPE) means that organizations with 

the IndustryAttribute ?INDUSTRY produce products of the kind ?TYPE.</rdfs:comment>
    <rdfs:domain rdf:resource="&Mid-level-ontology;IndustryAttribute"/>
    <rdfs:range rdf:resource="&SUMO;Object"/>
  </SUMO:BinaryPredicate>

  <Economy:PPPBasedEconomicValuation rdf:about="&Mid-level-ontology;totalGDP">
    <rdf:type rdf:resource="&SUMO;BinaryPredicate"/>
    <rdf:type rdf:resource="&owl;ObjectProperty"/>
    <rdfs:comment>(totalGDP ?AREA ?AMOUNT) means that the value 

of all final goods and services produced within the GeopoliticalArea 

?AREA is ?AMOUNT, in U.S. dollars, calculated on a purchasing power parity 

basis.  This represents Gross Domestic Product (GDP).  See 

PPPBasedEconomicValuation.</rdfs:comment>
    <rdfs:domain rdf:resource="&SUMO;GeopoliticalArea"/>
    <rdfs:range rdf:resource="&SUMO;CurrencyMeasure"/>
  </Economy:PPPBasedEconomicValuation>

  <owl:ObjectProperty rdf:about="&SUMO;contraryAttribute"/>
  <owl:ObjectProperty rdf:about="&SUMO;disjoint"/>
  <owl:ObjectProperty rdf:about="&SUMO;geographicSubregion"/>
  <owl:ObjectProperty rdf:about="&SUMO;rangeSubclass"/>
  <owl:ObjectProperty rdf:about="&SUMO;relatedInternalConcept"/>
  <owl:ObjectProperty rdf:about="&SUMO;subAttribute"/>
  <owl:ObjectProperty rdf:about="&SUMO;successorAttribute"/>

<!-- Instances -->
  <Economy:EconomicDevelopmentLevel rdf:about="#AdvancedDevelopingCountry"
                                    rdfs:label="Advanced Developing Country">
    <SUMO:subAttribute rdf:resource="#LessDevelopedCountry"/>
    <rdfs:comment>AdvancedDevelopingCountry 

is an Attribute used to describe a LessDevelopedCountry (LDC) 

that is undergoing rapid industrial development.  Also called 'newly 

industrializing economy' (or 'country').</rdfs:comment>
  </Economy:EconomicDevelopmentLevel>

  <Economy:IMFDevelopmentLevel rdf:about="#AdvancedEconomy">
    <rdfs:comment>AdvancedEconomy is an Attribute 

used to represent the InternationalMonetaryFund's top category of 

development levels (AdvancedEconomy,, countries in transition, and 

developing countries.  Generally (but not exactly) corresponds with 

DevelopedCountry classification used by UnitedNations agencies.</rdfs:comment>
  </Economy:IMFDevelopmentLevel>

  <owl:Thing rdf:about="#AerospaceIndustry">
    <SUMO:subAttribute rdf:resource="#TransportationEquipmentIndustry"/>
    <rdfs:comment>AerospaceIndustry is the Attribute 

of an Organization whose primary business involves manufacturing 

aerospace products.</rdfs:comment>
  </owl:Thing>

  <owl:Thing rdf:about="#Afghanistan">
    <Mid-level-ontology:economyType rdf:resource="#DevelopingCountry"/>
    <Mid-level-ontology:economyType rdf:resource="#LessDevelopedCountry"/>
  </owl:Thing>

  <Economy:EconomicSector rdf:about="#AgriculturalSector">
    <rdfs:comment>AgriculturalSector is an attribute 

that describes commercial organizations or agents whose business is in 

the agricultural sector of the economy.</rdfs:comment>
  </Economy:EconomicSector>

  <Economy:FinancialSectorAttribute rdf:about="#AgricultureBasedEconomy">
    <rdfs:comment>AgricultureBasedEconomy is 

the Attribute of an economy that is based primarily or significantly 

on AgriculturalSector businesses.</rdfs:comment>
  </Economy:FinancialSectorAttribute>

  <owl:Thing rdf:about="#AircraftManufacturing">
    <Mid-level-ontology:industryProductType rdf:resource="&Mid-level-ontology;Aircraft"/>
    <SUMO:subAttribute rdf:resource="#AerospaceIndustry"/>
    <rdfs:comment>AircraftManufacturing is the 

Attribute of an Organization whose primary business involves 

designing or manufacturing Aircraft or aircraft parts.</rdfs:comment>
  </owl:Thing>

  <owl:Thing rdf:about="#Albania">
    <Mid-level-ontology:economyType rdf:resource="#CountryInTransition"/>
  </owl:Thing>

  <owl:Thing rdf:about="#Algeria">
    <Mid-level-ontology:economyType rdf:resource="#DevelopingCountry"/>
    <Mid-level-ontology:economyType rdf:resource="#LessDevelopedCountry"/>
  </owl:Thing>

  <owl:Thing rdf:about="#AluminaAndAluminumIndustry">
    <Mid-level-ontology:industryProductType rdf:resource="#Alumina"/>
    <Mid-level-ontology:industryProductType rdf:resource="#AluminumMetal"/>
    <SUMO:subAttribute rdf:resource="#PrimaryMetalManufacturing"/>
    <rdfs:comment>AluminaAndAluminumIndustry is the Attribute of an Organization whose 

primary business involves processing or producing alumina or aluminum.</rdfs:comment>
  </owl:Thing>

  <owl:Thing rdf:about="#Andorra">
    <Mid-level-ontology:economyType rdf:resource="#DevelopedCountry"/>
  </owl:Thing>

  <owl:Thing rdf:about="#Angola">
    <Mid-level-ontology:economyType rdf:resource="#DevelopingCountry"/>
    <Mid-level-ontology:economyType rdf:resource="#LessDevelopedCountry"/>
  </owl:Thing>

  <Economy:IndustryAttribute rdf:about="#AnimalProduction">
    <Mid-level-ontology:industryProductType rdf:resource="&SUMO;Animal"/>
    <SUMO:subAttribute rdf:resource="#AgriculturalSector"/>
    <rdfs:comment>AnimalProduction is the IndustryAttribute that describes animal 

agriculture operations.</rdfs:comment>
  </Economy:IndustryAttribute>

  <owl:Thing rdf:about="#AntiguaAndBarbuda">
    <Mid-level-ontology:economyType rdf:resource="#DevelopingCountry"/>
    <Mid-level-ontology:economyType rdf:resource="#LessDevelopedCountry"/>
  </owl:Thing>

  <owl:Thing rdf:about="#Argentina">
    <Mid-level-ontology:economyType rdf:resource="#DevelopingCountry"/>
    <Mid-level-ontology:economyType rdf:resource="#LessDevelopedCountry"/>
  </owl:Thing>

  <owl:Thing rdf:about="#Armenia">
    <Mid-level-ontology:economyType rdf:resource="#CountryInTransition"/>
  </owl:Thing>

  <owl:Thing rdf:about="#Aruba">
    <Mid-level-ontology:economyType rdf:resource="#DevelopingCountry"/>
    <Mid-level-ontology:economyType rdf:resource="#LessDevelopedCountry"/>
  </owl:Thing>

  <owl:Thing rdf:about="#AsphaltMaterialsIndustry">
    <Mid-level-ontology:industryProductType rdf:resource="#Asphalt"/>
    <SUMO:subAttribute rdf:resource="#PetroleumIndustry"/>
    <rdfs:comment>AsphaltMaterialsIndustry is the 

Attribute of an Organization whose primary business involves 

manufacturing Asphalt materials.</rdfs:comment>
  </owl:Thing>

  <owl:Thing rdf:about="#Australia">
    <Mid-level-ontology:economyType rdf:resource="#AdvancedEconomy"/>
    <Mid-level-ontology:economyType rdf:resource="#DevelopedCountry"/>
  </owl:Thing>

  <owl:Thing rdf:about="#Austria">
    <Mid-level-ontology:economyType rdf:resource="#AdvancedEconomy"/>
    <Mid-level-ontology:economyType rdf:resource="#DevelopedCountry"/>
  </owl:Thing>

  <owl:Thing rdf:about="#AutomobileIndustry">
    <Mid-level-ontology:industryProductType rdf:resource="&Mid-level-ontology;Automobile"/>
    <SUMO:subAttribute rdf:resource="#TransportationEquipmentIndustry"/>
    <rdfs:comment>AutomobileIndustry is an Attribute 

of an Organization whose primary business involves manufacturing 

light duty motor vehicles (including Automobiles, LightTrucks and 

SUVs).</rdfs:comment>
  </owl:Thing>

  <owl:Thing rdf:about="#Azerbaijan">
    <Mid-level-ontology:economyType rdf:resource="#CountryInTransition"/>
  </owl:Thing>

  <owl:Thing rdf:about="#Bahrain">
    <Mid-level-ontology:economyType rdf:resource="#DevelopingCountry"/>
    <Mid-level-ontology:economyType rdf:resource="#LessDevelopedCountry"/>
  </owl:Thing>

  <owl:Thing rdf:about="#Bangladesh">
    <Mid-level-ontology:economyType rdf:resource="#DevelopingCountry"/>
    <Mid-level-ontology:economyType rdf:resource="#LessDevelopedCountry"/>
  </owl:Thing>

  <owl:Thing rdf:about="#Barbados">
    <Mid-level-ontology:economyType rdf:resource="#DevelopingCountry"/>
    <Mid-level-ontology:economyType rdf:resource="#LessDevelopedCountry"/>
  </owl:Thing>

  <Economy:IndustryAttribute rdf:about="#BarleyFarming">
    <Mid-level-ontology:industryProductType rdf:resource="#BarleyGrain"/>
    <SUMO:subAttribute rdf:resource="#CerealGrainFarming"/>
    <rdfs:comment>BarleyFarming is the IndustryAttribute that describes barley farming operations.</rdfs:comment>
  </Economy:IndustryAttribute>

  <owl:Thing rdf:about="#Belarus">
    <Mid-level-ontology:economyType rdf:resource="#CountryInTransition"/>
  </owl:Thing>

  <owl:Thing rdf:about="#Belgium">
    <Mid-level-ontology:economyType rdf:resource="#AdvancedEconomy"/>
    <Mid-level-ontology:economyType rdf:resource="#DevelopedCountry"/>
  </owl:Thing>

  <owl:Thing rdf:about="#Belize">
    <Mid-level-ontology:economyType rdf:resource="#DevelopingCountry"/>
    <Mid-level-ontology:economyType rdf:resource="#LessDevelopedCountry"/>
  </owl:Thing>

  <owl:Thing rdf:about="#Bermuda">
    <Mid-level-ontology:economyType rdf:resource="#DevelopedCountry"/>
  </owl:Thing>

  <owl:Thing rdf:about="#BosniaAndHerzegovina">
    <Mid-level-ontology:economyType rdf:resource="#CountryInTransition"/>
  </owl:Thing>

  <owl:Thing rdf:about="#Bulgaria">
    <Mid-level-ontology:economyType rdf:resource="#CountryInTransition"/>
  </owl:Thing>

  <owl:Thing rdf:about="#Burundi">
    <Mid-level-ontology:economyType rdf:resource="#DevelopingCountry"/>
    <Mid-level-ontology:economyType rdf:resource="#LessDevelopedCountry"/>
  </owl:Thing>

  <owl:Thing rdf:about="#Cambodia">
    <Mid-level-ontology:economyType rdf:resource="#DevelopingCountry"/>
    <Mid-level-ontology:economyType rdf:resource="#LessDevelopedCountry"/>
  </owl:Thing>

  <owl:Thing rdf:about="#Cameroon">
    <Mid-level-ontology:economyType rdf:resource="#DevelopingCountry"/>
    <Mid-level-ontology:economyType rdf:resource="#LessDevelopedCountry"/>
  </owl:Thing>

  <owl:Thing rdf:about="#CapeVerde">
    <Mid-level-ontology:economyType rdf:resource="#DevelopingCountry"/>
    <Mid-level-ontology:economyType rdf:resource="#LessDevelopedCountry"/>
  </owl:Thing>

  <owl:Thing rdf:about="#CattleRanchingAndFarming">
    <Mid-level-ontology:industryProductType rdf:resource="#Cattle"/>
    <SUMO:subAttribute rdf:resource="#AnimalProduction"/>
    <rdfs:comment>CattleRanchingAndFarming is 

the specification of AnimalProduction that describes cattle 

ranching and farming operations.</rdfs:comment>
  </owl:Thing>

  <Economy:IndustryAttribute rdf:about="#CementManufacturing">
    <Mid-level-ontology:industryProductType rdf:resource="&Mid-level-ontology;Cement"/>
    <SUMO:subAttribute rdf:resource="#IndustrialSector"/>
    <rdfs:comment>CementManufacturing is an 

Attribute of an Organization whose primary business involves 

manufacturing Cement.</rdfs:comment>
  </Economy:IndustryAttribute>

  <owl:Thing rdf:about="#CentralAfricanRepublic">
    <Mid-level-ontology:economyType rdf:resource="#DevelopingCountry"/>
    <Mid-level-ontology:economyType rdf:resource="#LessDevelopedCountry"/>
  </owl:Thing>

  <Economy:IndustryAttribute rdf:about="#CerealGrainFarming">
    <Mid-level-ontology:industryProductType rdf:resource="&Mid-level-ontology;CerealGrain"/>
    <SUMO:subAttribute rdf:resource="#CropProduction"/>
    <rdfs:comment>CerealGrainFarming is the IndustryAttribute that describes cereal 

grain farming operations.</rdfs:comment>
  </Economy:IndustryAttribute>

  <owl:Thing rdf:about="#Chad">
    <Mid-level-ontology:economyType rdf:resource="#DevelopingCountry"/>
    <Mid-level-ontology:economyType rdf:resource="#LessDevelopedCountry"/>
  </owl:Thing>

  <Economy:IndustryAttribute rdf:about="#ChemicalManufacturing">
    <Mid-level-ontology:industryProductType rdf:resource="#ChemicalProduct"/>
    <SUMO:subAttribute rdf:resource="#IndustrialSector"/>
    <rdfs:comment>ChemicalManufacturing is an 

Attribute of an Organization whose primary business involves the 

manufacture of chemicals.</rdfs:comment>
  </Economy:IndustryAttribute>

  <owl:Thing rdf:about="#Chile">
    <Mid-level-ontology:economyType rdf:resource="#DevelopingCountry"/>
    <Mid-level-ontology:economyType rdf:resource="#LessDevelopedCountry"/>
  </owl:Thing>

  <owl:Thing rdf:about="#China">
    <Mid-level-ontology:economyType rdf:resource="#DevelopingCountry"/>
    <Mid-level-ontology:economyType rdf:resource="#LessDevelopedCountry"/>
  </owl:Thing>

  <Economy:IndustryAttribute rdf:about="#ClothingIndustry">
    <SUMO:relatedInternalConcept rdf:resource="#FootwearIndustry"/>
    <SUMO:subAttribute rdf:resource="#IndustrialSector"/>
    <rdfs:comment>ClothingIndustry is the Attribute 

of an Organization whose primary business involves manufacturing 

Clothing.</rdfs:comment>
  </Economy:IndustryAttribute>

  <Economy:IndustryAttribute rdf:about="#CoalIndustry">
    <Mid-level-ontology:industryProductType rdf:resource="http://reliant.teknowledge.com/DAML/Geography.owl#Coal"/>
    <SUMO:subAttribute rdf:resource="#IndustrialSector"/>
    <rdfs:comment>CoalIndustry is the Attribute 

of an Organization whose primary business involves producing  

Coal and coal products.</rdfs:comment>
  </Economy:IndustryAttribute>

  <owl:Thing rdf:about="#CoalMining">
    <Mid-level-ontology:industryProductType rdf:resource="http://reliant.teknowledge.com/DAML/Geography.owl#Coal"/>
    <SUMO:subAttribute rdf:resource="#CoalIndustry"/>
    <SUMO:subAttribute rdf:resource="#MiningIndustry"/>
    <rdfs:comment>CoalMining is the Attribute of an 

Organization whose primary business is mining  Coal.</rdfs:comment>
  </owl:Thing>

  <owl:Thing rdf:about="#Colombia">
    <Mid-level-ontology:economyType rdf:resource="#DevelopingCountry"/>
    <Mid-level-ontology:economyType rdf:resource="#LessDevelopedCountry"/>
  </owl:Thing>

  <Mid-level-ontology:EconomicSystemAttribute rdf:about="#CommunalLandOwnershipEconomy">
    <SUMO:subAttribute rdf:resource="&Mid-level-ontology;SocialistEconomy"/>
    <rdfs:comment>CommunalLandOwnershipEconomy is an Attribute that describes an economy 

in which all or most of the land is communally owned.</rdfs:comment>
  </Mid-level-ontology:EconomicSystemAttribute>

  <owl:Thing rdf:about="#Comoros">
    <Mid-level-ontology:economyType rdf:resource="#DevelopingCountry"/>
    <Mid-level-ontology:economyType rdf:resource="#LessDevelopedCountry"/>
  </owl:Thing>

  <Economy:IndustryAttribute rdf:about="#ConsumerGoodsIndustry">
    <Mid-level-ontology:industryProductType rdf:resource="#ConsumerGood"/>
    <SUMO:subAttribute rdf:resource="#IndustrialSector"/>
    <rdfs:comment>ConsumerGoodsIndustry is the 

Attribute of an Organization whose primary business is the production  

of consumer goods.</rdfs:comment>
  </Economy:IndustryAttribute>

  <Economy:FinancialSectorAttribute rdf:about="#ControlledLaborMarketEconomy">
    <rdfs:comment>ControlledLaborMarketEconomy 

is the Attribute of an area whose economy has a labor market with wages 

and working conditions controlled by government policies or laws.</rdfs:comment>
  </Economy:FinancialSectorAttribute>

  <Economy:IndustryAttribute rdf:about="#CopperIndustry">
    <SUMO:subAttribute rdf:resource="#PrimaryMetalManufacturing"/>
    <rdfs:comment>CopperIndustry is the Attribute of 

an Organization whose primary business involves mining, smelting, 

rolling, drawing, extruding, or alloying Copper.</rdfs:comment>
  </Economy:IndustryAttribute>

  <owl:Thing rdf:about="#CopperOreMining">
    <Mid-level-ontology:industryProductType rdf:resource="#CopperOre"/>
    <SUMO:subAttribute rdf:resource="#CopperIndustry"/>
    <SUMO:subAttribute rdf:resource="#MetalOreMining"/>
    <rdfs:comment>CopperOreMining is the Attribute of 

an Organization whose primary business involves mining CopperOre.</rdfs:comment>
  </owl:Thing>

  <Economy:IndustryAttribute rdf:about="#CornFarming">
    <Mid-level-ontology:industryProductType rdf:resource="#MaizeGrain"/>
    <SUMO:subAttribute rdf:resource="#CerealGrainFarming"/>
    <rdfs:comment>CornFarming is the IndustryAttribute that 

describes corn or maize farming operations.</rdfs:comment>
  </Economy:IndustryAttribute>

  <owl:Thing rdf:about="#CostaRica">
    <Mid-level-ontology:economyType rdf:resource="#DevelopingCountry"/>
    <Mid-level-ontology:economyType rdf:resource="#LessDevelopedCountry"/>
  </owl:Thing>

  <owl:Thing rdf:about="#CoteDIvoire">
    <Mid-level-ontology:economyType rdf:resource="#DevelopingCountry"/>
    <Mid-level-ontology:economyType rdf:resource="#LessDevelopedCountry"/>
  </owl:Thing>

  <owl:Thing rdf:about="#CottonFarming">
    <Mid-level-ontology:industryProductType rdf:resource="#CottonFiber"/>
    <SUMO:subAttribute rdf:resource="#CropProduction"/>
    <rdfs:comment>CottonFarming is the specification of 

CropProductionthat describes cotton farming operations.</rdfs:comment>
  </owl:Thing>

  <Economy:IMFDevelopmentLevel rdf:about="#CountryInTransition">
    <SUMO:successorAttribute rdf:resource="#AdvancedEconomy"/>
    <rdfs:comment>CountryInTransition is a term 

used by the InternationalMonetaryFund (IMF) to describe the middle 

group in its hierarchy of advanced countries, countries in transition, 

and developing countries.  Most of the countries with this attribute 

are former USSR or Eastern European countries.  Generally corresponds 

with FormerSovietOrEasternEuropeanCountry classification used by 

UnitedNations agencies.</rdfs:comment>
  </Economy:IMFDevelopmentLevel>

  <owl:Thing rdf:about="#Croatia">
    <Mid-level-ontology:economyType rdf:resource="#CountryInTransition"/>
  </owl:Thing>

  <owl:Thing rdf:about="#Cyprus">
    <Mid-level-ontology:economyType rdf:resource="#DevelopingCountry"/>
    <Mid-level-ontology:economyType rdf:resource="#LessDevelopedCountry"/>
  </owl:Thing>

  <owl:Thing rdf:about="#CzechRepublic">
    <Mid-level-ontology:economyType rdf:resource="#CountryInTransition"/>
  </owl:Thing>

  <owl:Thing rdf:about="#DemocraticRepublicOfTheCongo">
    <Mid-level-ontology:economyType rdf:resource="#DevelopingCountry"/>
    <Mid-level-ontology:economyType rdf:resource="#LessDevelopedCountry"/>
  </owl:Thing>

  <owl:Thing rdf:about="#Denmark">
    <Mid-level-ontology:economyType rdf:resource="#AdvancedEconomy"/>
    <Mid-level-ontology:economyType rdf:resource="#DevelopedCountry"/>
  </owl:Thing>

  <Economy:UNEconomicDevelopmentLevel rdf:about="#DevelopedCountry">
    <rdfs:comment>DevelopedCountry (DC) is a term used to describe members of the top 

group in the UNEconomicDevelopmentLevels.  DevelopedCountry includes 

market-oriented economies of mainly democratic nations, including members 

of the OrganizationForEconomicCooperationAndDevelopment (OECD).  DCs 

are also known as First World countries, 'the North', and industrial 

countries.  Developed countries generally have high incomes (high per 

capita GDP or GNI), but there are exceptions to DC membership both above 

and below that standard.  There is significant overlap, but not perfect 

congruence, between the UN category DevelopedCountry and the IMF 

category AdvancedEconomy.</rdfs:comment>
    <rdfs:label>Developed Country</rdfs:label>
    <rdfs:label>industrial country</rdfs:label>
    <rdfs:label>the North</rdfs:label>
  </Economy:UNEconomicDevelopmentLevel>

  <Economy:IMFDevelopmentLevel rdf:about="#DevelopingCountry">
    <SUMO:successorAttribute rdf:resource="#CountryInTransition"/>
    <rdfs:comment>DevelopingCountry is a term 

used by the InternationalMonetaryFund (IMF) for the bottom group 

in its hierarchy of advanced countries, countries in transition, 

and developing countries. Generally corresponds to the attribute 

LessDevelopedCountry used by UnitedNations agencies.  Not to 

be confused with DevelopedCountry.</rdfs:comment>
  </Economy:IMFDevelopmentLevel>

  <Economy:FinancialSectorAttribute rdf:about="#DiversifiedEconomy">
    <rdfs:comment>DiversifiedEconomy is the Attribute 

of an area whose economy is based on significant activities in more than 

one economic sector.</rdfs:comment>
  </Economy:FinancialSectorAttribute>

  <owl:Thing rdf:about="#Djibouti">
    <Mid-level-ontology:economyType rdf:resource="#DevelopingCountry"/>
    <Mid-level-ontology:economyType rdf:resource="#LessDevelopedCountry"/>
  </owl:Thing>

  <owl:Thing rdf:about="#Dominica">
    <Mid-level-ontology:economyType rdf:resource="#DevelopingCountry"/>
    <Mid-level-ontology:economyType rdf:resource="#LessDevelopedCountry"/>
  </owl:Thing>

  <owl:Thing rdf:about="#DominicanRepublic">
    <Mid-level-ontology:economyType rdf:resource="#DevelopingCountry"/>
    <Mid-level-ontology:economyType rdf:resource="#LessDevelopedCountry"/>
  </owl:Thing>

  <owl:Thing rdf:about="#Ecuador">
    <Mid-level-ontology:economyType rdf:resource="#DevelopingCountry"/>
    <Mid-level-ontology:economyType rdf:resource="#LessDevelopedCountry"/>
  </owl:Thing>

  <owl:Thing rdf:about="#Egypt">
    <Mid-level-ontology:economyType rdf:resource="#DevelopingCountry"/>
    <Mid-level-ontology:economyType rdf:resource="#LessDevelopedCountry"/>
  </owl:Thing>

  <owl:Thing rdf:about="#ElSalvador">
    <Mid-level-ontology:economyType rdf:resource="#DevelopingCountry"/>
    <Mid-level-ontology:economyType rdf:resource="#LessDevelopedCountry"/>
  </owl:Thing>

  <Economy:IndustryAttribute rdf:about="#ElectronicsIndustry">
    <Mid-level-ontology:industryProductType rdf:resource="&Mid-level-ontology;ElectricDevice"/>
    <SUMO:subAttribute rdf:resource="#IndustrialSector"/>
    <rdfs:comment>ElectronicsIndustry is the 

Attribute of an Organization whose primary business involves 

electronics manufacturing (including but not limited to Computers).</rdfs:comment>
  </Economy:IndustryAttribute>

  <owl:Thing rdf:about="#EquatorialGuinea">
    <Mid-level-ontology:economyType rdf:resource="#DevelopingCountry"/>
    <Mid-level-ontology:economyType rdf:resource="#LessDevelopedCountry"/>
  </owl:Thing>

  <owl:Thing rdf:about="#Estonia">
    <Mid-level-ontology:economyType rdf:resource="#CountryInTransition"/>
  </owl:Thing>

  <owl:Thing rdf:about="#Ethiopia">
    <Mid-level-ontology:economyType rdf:resource="#DevelopingCountry"/>
    <Mid-level-ontology:economyType rdf:resource="#LessDevelopedCountry"/>
  </owl:Thing>

  <owl:Thing rdf:about="#FaroeIslands">
    <Mid-level-ontology:economyType rdf:resource="#DevelopedCountry"/>
  </owl:Thing>

  <Economy:IndustryAttribute rdf:about="#FertilizerIndustry">
    <Mid-level-ontology:industryProductType rdf:resource="#Fertilizer"/>
    <SUMO:subAttribute rdf:resource="#ChemicalManufacturing"/>
    <rdfs:comment>FertilizerIndustry is the 

Attribute of an Organization whose primary business involves 

manufacturing Fertilizer.</rdfs:comment>
  </Economy:IndustryAttribute>

  <owl:Thing rdf:about="#Fiji">
    <Mid-level-ontology:economyType rdf:resource="#DevelopingCountry"/>
    <Mid-level-ontology:economyType rdf:resource="#LessDevelopedCountry"/>
  </owl:Thing>

  <owl:Thing rdf:about="#Finland">
    <Mid-level-ontology:economyType rdf:resource="#AdvancedEconomy"/>
    <Mid-level-ontology:economyType rdf:resource="#DevelopedCountry"/>
  </owl:Thing>

  <Economy:IndustryAttribute rdf:about="#FoodManufacturing">
    <Mid-level-ontology:industryProductType rdf:resource="#FoodProduct"/>
    <Mid-level-ontology:industryProductType rdf:resource="&SUMO;Food"/>
    <SUMO:subAttribute rdf:resource="#AgriculturalSector"/>
    <rdfs:comment>FoodManufacturing is the 

Attribute of an Organization whose primary business involves 

manufacturing Food.</rdfs:comment>
  </Economy:IndustryAttribute>

  <Economy:IndustryAttribute rdf:about="#FootwearIndustry">
    <Mid-level-ontology:industryProductType rdf:resource="#Footwear"/>
    <SUMO:subAttribute rdf:resource="#IndustrialSector"/>
    <rdfs:comment>FootwearIndustry is the Attribute 

of an Organization whose primary business involves manufacture of 

Footwear.</rdfs:comment>
  </Economy:IndustryAttribute>

  <owl:Thing rdf:about="#ForestryAndLogging">
    <Mid-level-ontology:industryProductType rdf:resource="#ForestProduct"/>
    <Mid-level-ontology:industryProductType rdf:resource="http://reliant.teknowledge.com/DAML/Geography.owl#Timber"/>
    <SUMO:subAttribute rdf:resource="#LumberIndustry"/>
    <rdfs:comment>ForestryAndLogging is the Attribute 

of an Organization whose primary business involves manufacturing 

Timber.</rdfs:comment>
  </owl:Thing>

  <Economy:UNEconomicDevelopmentLevel rdf:about="#FormerSovietOrEasternEuropeanCountry">
    <SUMO:successorAttribute rdf:resource="#DevelopedCountry"/>
    <rdfs:comment>FormerSovietOrEasternEuropeanCountry (former USSR-EE) is an  

Attribute that characterizes countries that were part of the former 

Soviet Union or its sphere of influence in Eastern Europe.  This level 

occupies a middle position between DevelopedCountry (DC) and 

LessDevelopedCountry (LDC) in UNEconomicDevelopmentLevels. 

Previously, former USSR-EE countries had a CentrallyPlannedEconomy and 

were Marxist-Leninist states.  Many are now evolving away from command 

economies to market economic systems.  During the 1980's, the group 

included Albania, Bulgaria, Cambodia, China, Cuba, Czechoslovakia, the 

German Democratic Republic (East Germany), Hungary, North Korea, Laos, 

Mongolia, Poland, Romania, the USSR, Vietnam and Yugoslavia.</rdfs:comment>
    <rdfs:label>Former Eastern European</rdfs:label>
    <rdfs:label>Former Soviet</rdfs:label>
    <rdfs:label>Former Soviet or Eastern European Country</rdfs:label>
  </Economy:UNEconomicDevelopmentLevel>

  <Economy:PowerGeneration rdf:about="#FossilFuelPowerGeneration"/>
  <Economy:EconomicDevelopmentLevel rdf:about="#FourDragonsEconomy">
    <rdfs:comment>FourDragonsEconomy describes four 

small Asian countries that achieved rapid economic growth in the 1990s. 

Some systems of EconomicDevelopmentLevel place them as a 

LessDevelopedCountry, but the IMF includes them in AdvancedEconomy.</rdfs:comment>
    <rdfs:label>Four Dragons</rdfs:label>
    <rdfs:label>Four Tigers</rdfs:label>
  </Economy:EconomicDevelopmentLevel>

  <Economy:IndustryAttribute rdf:about="#FruitAndTreeNutFarming">
    <Mid-level-ontology:industryProductType rdf:resource="#PlantAgriculturalProduct"/>
    <SUMO:subAttribute rdf:resource="#CropProduction"/>
    <rdfs:comment>FruitAndTreeNutFarming is the IndustryAttribute that describes 

fruit and tree nut farming operations.</rdfs:comment>
  </Economy:IndustryAttribute>

  <Economy:IndustryAttribute rdf:about="#FruitFarming">
    <Mid-level-ontology:industryProductType rdf:resource="#Fruit"/>
    <SUMO:subAttribute rdf:resource="#FruitAndTreeNutFarming"/>
    <rdfs:comment>FruitFarming is the specification of 

FruitAndTreeNutFarming that describes fruit farming operations.</rdfs:comment>
  </Economy:IndustryAttribute>

  <Economy:IndustryAttribute rdf:about="#FurnitureIndustry">
    <Mid-level-ontology:industryProductType rdf:resource="&Mid-level-ontology;Furniture"/>
    <SUMO:subAttribute rdf:resource="#IndustrialSector"/>
    <rdfs:comment>FurnitureIndustry is the Attribute 

of an Organization whose primary business involves manufacture of 

Furniture.</rdfs:comment>
  </Economy:IndustryAttribute>

  <owl:Thing rdf:about="#Gabon">
    <Mid-level-ontology:economyType rdf:resource="#DevelopingCountry"/>
    <Mid-level-ontology:economyType rdf:resource="#LessDevelopedCountry"/>
  </owl:Thing>

  <owl:Thing rdf:about="#Gambia">
    <Mid-level-ontology:economyType rdf:resource="#DevelopingCountry"/>
    <Mid-level-ontology:economyType rdf:resource="#LessDevelopedCountry"/>
  </owl:Thing>

  <owl:Thing rdf:about="#Ghana">
    <Mid-level-ontology:economyType rdf:resource="#DevelopingCountry"/>
    <Mid-level-ontology:economyType rdf:resource="#LessDevelopedCountry"/>
  </owl:Thing>

  <owl:Thing rdf:about="#GoatFarming">
    <Mid-level-ontology:industryProductType rdf:resource="&Mid-level-ontology;Goat"/>
    <SUMO:subAttribute rdf:resource="#AnimalProduction"/>
    <rdfs:comment>GoatFarming is the specification of 

AnimalProduction that describes goat farming operations.</rdfs:comment>
  </owl:Thing>

  <owl:Thing rdf:about="#GrapeFarming">
    <Mid-level-ontology:industryProductType rdf:resource="#Grape"/>
    <SUMO:subAttribute rdf:resource="#FruitFarming"/>
    <rdfs:comment>GrapeFarming is the specification of 

FruitFarming that describes Grape farming operations.</rdfs:comment>
  </owl:Thing>

  <owl:Thing rdf:about="#Grenada">
    <Mid-level-ontology:economyType rdf:resource="#DevelopingCountry"/>
    <Mid-level-ontology:economyType rdf:resource="#LessDevelopedCountry"/>
  </owl:Thing>

  <owl:Thing rdf:about="#Guatemala">
    <Mid-level-ontology:economyType rdf:resource="#DevelopingCountry"/>
    <Mid-level-ontology:economyType rdf:resource="#LessDevelopedCountry"/>
  </owl:Thing>

  <owl:Thing rdf:about="#Guinea">
    <Mid-level-ontology:economyType rdf:resource="#DevelopingCountry"/>
    <Mid-level-ontology:economyType rdf:resource="#LessDevelopedCountry"/>
  </owl:Thing>

  <owl:Thing rdf:about="#GuineaBissau">
    <Mid-level-ontology:economyType rdf:resource="#DevelopingCountry"/>
    <Mid-level-ontology:economyType rdf:resource="#LessDevelopedCountry"/>
  </owl:Thing>

  <owl:Thing rdf:about="#Guyana">
    <Mid-level-ontology:economyType rdf:resource="#DevelopingCountry"/>
    <Mid-level-ontology:economyType rdf:resource="#LessDevelopedCountry"/>
  </owl:Thing>

  <owl:Thing rdf:about="#Haiti">
    <Mid-level-ontology:economyType rdf:resource="#DevelopingCountry"/>
    <Mid-level-ontology:economyType rdf:resource="#LessDevelopedCountry"/>
  </owl:Thing>

  <Economy:IndustryAttribute rdf:about="#HandicraftIndustry">
    <Mid-level-ontology:industryProductType rdf:resource="&SUMO;Artifact"/>
    <SUMO:subAttribute rdf:resource="#IndustrialSector"/>
    <rdfs:comment>HandicraftIndustry is the Attribute 

of an Organization whose primary business involves manufacturing items 

by hand.</rdfs:comment>
  </Economy:IndustryAttribute>

  <owl:Thing rdf:about="#HandwovenCarpetManufacturing">
    <Mid-level-ontology:industryProductType rdf:resource="#HandwovenCarpet"/>
    <SUMO:subAttribute rdf:resource="#HandicraftIndustry"/>
    <rdfs:comment>HandwovenCarpetManufacturing 

is the Attribute of an Organization whose primary business involves 

manufacturing HandwovenCarpets.</rdfs:comment>
  </owl:Thing>

  <owl:Thing rdf:about="#HeavyDutyTruckIndustry">
    <Mid-level-ontology:industryProductType rdf:resource="&Mid-level-ontology;Truck"/>
    <SUMO:subAttribute rdf:resource="#MotorVehicleIndustry"/>
    <rdfs:comment>HeavyDutyTruckIndustry 

is the Attribute of an Organization whose primary business is 

manufacturing heavy duty trucks.</rdfs:comment>
  </owl:Thing>

  <Economy:WorldBankGNIPerCapitaLevel rdf:about="#HighIncomeCountry">
    <rdfs:comment>HighIncomeCountry is an Attribute representing the World Bank 

classification for any country where the per capita GNI is 

equal to or greater than 9,266 in UnitedStatesDollars.</rdfs:comment>
  </Economy:WorldBankGNIPerCapitaLevel>

  <Economy:EconomicDevelopmentLevel rdf:about="#HighTechIndustrialEconomy">
    <rdfs:comment>HighTechIndustrialEconomy 

is an Attribute used to describe industrialized countries whose 

infrastructure uses the most advanced kinds of technology.</rdfs:comment>
  </Economy:EconomicDevelopmentLevel>

  <owl:Thing rdf:about="#HogAndPigFarming">
    <Mid-level-ontology:industryProductType rdf:resource="#Pork"/>
    <SUMO:subAttribute rdf:resource="#AnimalProduction"/>
    <rdfs:comment>HogAndPigFarming is the specification of 

AnimalProduction that describes hog and pig farming operations.</rdfs:comment>
  </owl:Thing>

  <owl:Thing rdf:about="#HolySee">
    <Mid-level-ontology:economyType rdf:resource="#DevelopedCountry"/>
  </owl:Thing>

  <owl:Thing rdf:about="#Honduras">
    <Mid-level-ontology:economyType rdf:resource="#DevelopingCountry"/>
    <Mid-level-ontology:economyType rdf:resource="#LessDevelopedCountry"/>
  </owl:Thing>

  <owl:Thing rdf:about="#HongKong">
    <Mid-level-ontology:economyType rdf:resource="#AdvancedEconomy"/>
    <Mid-level-ontology:economyType rdf:resource="#FourDragonsEconomy"/>
  </owl:Thing>

  <Economy:IndustryAttribute rdf:about="#HouseholdApplianceManufacturing">
    <Mid-level-ontology:industryProductType rdf:resource="&Mid-level-ontology;ElectricDevice"/>
    <SUMO:subAttribute rdf:resource="#IndustrialSector"/>
    <rdfs:comment>HouseholdApplianceManufacturing is the Attribute of an Organization 

whose primary business involves manufacturing electrical household appliances.</rdfs:comment>
  </Economy:IndustryAttribute>

  <owl:Thing rdf:about="#Hungary">
    <Mid-level-ontology:economyType rdf:resource="#CountryInTransition"/>
  </owl:Thing>

  <Economy:ElectricalPowerGeneration rdf:about="#HydroElectricPowerGeneration"/>
  <owl:Thing rdf:about="#Iceland">
    <Mid-level-ontology:economyType rdf:resource="#AdvancedEconomy"/>
    <Mid-level-ontology:economyType rdf:resource="#DevelopedCountry"/>
  </owl:Thing>

  <owl:Thing rdf:about="#India">
    <Mid-level-ontology:economyType rdf:resource="#DevelopingCountry"/>
    <Mid-level-ontology:economyType rdf:resource="#LessDevelopedCountry"/>
  </owl:Thing>

  <owl:Thing rdf:about="#Indonesia">
    <Mid-level-ontology:economyType rdf:resource="#DevelopingCountry"/>
    <Mid-level-ontology:economyType rdf:resource="#LessDevelopedCountry"/>
  </owl:Thing>

  <owl:Thing rdf:about="#IndustrialSandMining">
    <Mid-level-ontology:industryProductType rdf:resource="&Mid-level-ontology;Sand"/>
    <SUMO:subAttribute rdf:resource="#MiningIndustry"/>
    <rdfs:comment>IndustrialSandMining is the 

Attribute of an Organization whose primary business is mining 

industrial-quality Sand.</rdfs:comment>
  </owl:Thing>

  <Economy:EconomicSector rdf:about="#IndustrialSector">
    <rdfs:comment>IndustrialSector is an attribute 

that describes commercial organizations or agents whose business is in 

the industrial sector of the economy.</rdfs:comment>
  </Economy:EconomicSector>

  <owl:Thing rdf:about="#Iran">
    <Mid-level-ontology:economyType rdf:resource="#DevelopingCountry"/>
    <Mid-level-ontology:economyType rdf:resource="#LessDevelopedCountry"/>
  </owl:Thing>

  <owl:Thing rdf:about="#Iraq">
    <Mid-level-ontology:economyType rdf:resource="#DevelopingCountry"/>
    <Mid-level-ontology:economyType rdf:resource="#LessDevelopedCountry"/>
  </owl:Thing>

  <owl:Thing rdf:about="#IronMills">
    <Mid-level-ontology:industryProductType rdf:resource="#IronMetal"/>
    <Mid-level-ontology:industryProductType rdf:resource="&Mid-level-ontology;Iron"/>
    <SUMO:subAttribute rdf:resource="#PrimaryMetalManufacturing"/>
    <rdfs:comment>IronMills is the Attribute of 

an Organization whose primary business is manufacturing iron.</rdfs:comment>
  </owl:Thing>

  <owl:Thing rdf:about="#IronOreMining">
    <Mid-level-ontology:industryProductType rdf:resource="http://reliant.teknowledge.com/DAML/Geography.owl#IronOre"/>
    <SUMO:subAttribute rdf:resource="#MiningIndustry"/>
    <rdfs:comment>IronOreMining is the Attribute of an 

Organization whose primary business is mining IronOre.</rdfs:comment>
  </owl:Thing>

  <owl:Thing rdf:about="#Israel">
    <Mid-level-ontology:economyType rdf:resource="#AdvancedEconomy"/>
    <Mid-level-ontology:economyType rdf:resource="#DevelopedCountry"/>
  </owl:Thing>

  <owl:Thing rdf:about="#Jamaica">
    <Mid-level-ontology:economyType rdf:resource="#DevelopingCountry"/>
    <Mid-level-ontology:economyType rdf:resource="#LessDevelopedCountry"/>
  </owl:Thing>

  <owl:Thing rdf:about="#Jordan">
    <Mid-level-ontology:economyType rdf:resource="#DevelopingCountry"/>
    <Mid-level-ontology:economyType rdf:resource="#LessDevelopedCountry"/>
  </owl:Thing>

  <owl:Thing rdf:about="#KaolinAndBallClayMining">
    <Mid-level-ontology:industryProductType rdf:resource="&Mid-level-ontology;Clay"/>
    <SUMO:subAttribute rdf:resource="#MiningIndustry"/>
    <rdfs:comment>KaolinAndBallClayMining is 

the Attribute of an Organization whose primary business is mining 

Clay.</rdfs:comment>
  </owl:Thing>

  <owl:Thing rdf:about="#Kazakhstan">
    <Mid-level-ontology:economyType rdf:resource="#CountryInTransition"/>
  </owl:Thing>

  <owl:Thing rdf:about="#Kenya">
    <Mid-level-ontology:economyType rdf:resource="#DevelopingCountry"/>
    <Mid-level-ontology:economyType rdf:resource="#LessDevelopedCountry"/>
  </owl:Thing>

  <owl:Thing rdf:about="#Kiribati">
    <Mid-level-ontology:economyType rdf:resource="#DevelopingCountry"/>
    <Mid-level-ontology:economyType rdf:resource="#LessDevelopedCountry"/>
  </owl:Thing>

  <owl:Thing rdf:about="#Kuwait">
    <Mid-level-ontology:economyType rdf:resource="#DevelopingCountry"/>
    <Mid-level-ontology:economyType rdf:resource="#LessDevelopedCountry"/>
  </owl:Thing>

  <owl:Thing rdf:about="#Kyrgyzstan">
    <Mid-level-ontology:economyType rdf:resource="#CountryInTransition"/>
  </owl:Thing>

  <owl:Thing rdf:about="#Latvia">
    <Mid-level-ontology:economyType rdf:resource="#CountryInTransition"/>
  </owl:Thing>

  <Economy:IndustryAttribute rdf:about="#LeadIndustry">
    <Mid-level-ontology:industryProductType rdf:resource="&Mid-level-ontology;Lead"/>
    <SUMO:subAttribute rdf:resource="#IndustrialSector"/>
    <rdfs:comment>LeadIndustry is the Attribute of an 

Organization whose primary business involves mining or manufacturing 

lead.</rdfs:comment>
  </Economy:IndustryAttribute>

  <Economy:IndustryAttribute rdf:about="#LeadManufacturing">
    <Mid-level-ontology:industryProductType rdf:resource="#LeadProduct"/>
    <SUMO:subAttribute rdf:resource="#LeadIndustry"/>
    <SUMO:subAttribute rdf:resource="#PrimaryMetalManufacturing"/>
    <rdfs:comment>LeadManufacturing is the Attribute 

of an Organization whose primary business involves manufacturing 

LeadProducts.</rdfs:comment>
  </Economy:IndustryAttribute>

  <owl:Thing rdf:about="#LeadOreMining">
    <Mid-level-ontology:industryProductType rdf:resource="#LeadOre"/>
    <SUMO:subAttribute rdf:resource="#LeadIndustry"/>
    <SUMO:subAttribute rdf:resource="#MetalOreMining"/>
    <rdfs:comment>LeadOreMining is the Attribute of an 

Organization whose primary business involves mining LeadOre.</rdfs:comment>
  </owl:Thing>

  <Economy:EconomicDevelopmentLevel rdf:about="#LeastDevelopedCountry">
    <SUMO:subAttribute rdf:resource="#LessDevelopedCountry"/>
    <rdfs:comment>LeastDevelopedCountry 

is a sub-classification of LessDevelopedCountry characterizing

those countries that have no significant economic growth, a per 

capita GDP of less than $1,000 UnitedStatesDollars, and low 

literacy.  Also known as 'undeveloped countries'.</rdfs:comment>
    <rdfs:label>Least Developed Countries</rdfs:label>
    <rdfs:label>Undeveloped Country</rdfs:label>
    <rdfs:label>Undeveloped Economy</rdfs:label>
  </Economy:EconomicDevelopmentLevel>

  <owl:Thing rdf:about="#Lebanon">
    <Mid-level-ontology:economyType rdf:resource="#DevelopingCountry"/>
    <Mid-level-ontology:economyType rdf:resource="#LessDevelopedCountry"/>
  </owl:Thing>

  <owl:Thing rdf:about="#Lesotho">
    <Mid-level-ontology:economyType rdf:resource="#DevelopingCountry"/>
    <Mid-level-ontology:economyType rdf:resource="#LessDevelopedCountry"/>
  </owl:Thing>

  <Economy:UNEconomicDevelopmentLevel rdf:about="#LessDevelopedCountry">
    <SUMO:successorAttribute rdf:resource="#FormerSovietOrEasternEuropeanCountry"/>
    <rdfs:comment>LessDevelopedCountry (LDC) is 

the Attribute used to describe the bottom group in the hierarchy 

of UNEconomicDevelopmentLevels. Less developed countries are countries 

or dependent areas with low levels of production, living standards, 

and technology.  Per capita GDP (perCapitaGDPInPeriod), or GDI 

(Gross Domestic Income), is generally less than $5,000 and often 

below $1,500.  Subgroups of LDC, however, include countries that have 

higher per capita incomes, as well as advanced technology, and rapid rates 

of growth.  Subgroups of LDC include: advanced developing countries, 

the Four Dragons (also known as Four Tigers), LeastDevelopedCountry 

(LLDCs), low-income countries, middle-income countries, newly 

industrializing economies (NIEs), the South (from the location of 

most LDC countries, relative to Northern developed countries), Third 

World (obsolete), UnderdevelopedCountry, UndevelopedCountry.</rdfs:comment>
    <rdfs:label>Less Developed Country</rdfs:label>
    <rdfs:label>the South</rdfs:label>
  </Economy:UNEconomicDevelopmentLevel>

  <owl:Thing rdf:about="#Liberia">
    <Mid-level-ontology:economyType rdf:resource="#DevelopingCountry"/>
    <Mid-level-ontology:economyType rdf:resource="#LessDevelopedCountry"/>
  </owl:Thing>

  <owl:Thing rdf:about="#Libya">
    <Mid-level-ontology:economyType rdf:resource="#DevelopingCountry"/>
    <Mid-level-ontology:economyType rdf:resource="#LessDevelopedCountry"/>
  </owl:Thing>

  <owl:Thing rdf:about="#Liechtenstein">
    <Mid-level-ontology:economyType rdf:resource="#DevelopedCountry"/>
  </owl:Thing>

  <owl:Thing rdf:about="#Lithuania">
    <Mid-level-ontology:economyType rdf:resource="#CountryInTransition"/>
  </owl:Thing>

  <Economy:WorldBankGNIPerCapitaLevel rdf:about="#LowIncomeCountry">
    <SUMO:successorAttribute rdf:resource="#LowerMiddleIncomeCountry"/>
    <rdfs:comment>LowIncomeCountry is an 

Attribute representing the World Bank classification for any country 

where the per capita GNI is $755 or below in UnitedStatesDollars.</rdfs:comment>
  </Economy:WorldBankGNIPerCapitaLevel>

  <Economy:WorldBankGNIPerCapitaLevel rdf:about="#LowerMiddleIncomeCountry">
    <SUMO:successorAttribute rdf:resource="#UpperMiddleIncomeCountry"/>
    <rdfs:comment>LowerMiddleIncomeCountry is an Attribute representing the World 

Bank classification for any country where the per capita GNI is 

between $756 and $2,995 (inclusive) in UnitedStatesDollars.</rdfs:comment>
  </Economy:WorldBankGNIPerCapitaLevel>

  <Economy:IndustryAttribute rdf:about="#LumberIndustry">
    <Mid-level-ontology:industryProductType rdf:resource="#ForestProduct"/>
    <SUMO:subAttribute rdf:resource="#AgriculturalSector"/>
    <rdfs:comment>LumberIndustry is the Attribute 

of an Organization whose primary business involves logging, 

manufacturing lumber, or making other wood products.</rdfs:comment>
  </Economy:IndustryAttribute>

  <owl:Thing rdf:about="#Luxembourg">
    <Mid-level-ontology:economyType rdf:resource="#AdvancedEconomy"/>
    <Mid-level-ontology:economyType rdf:resource="#DevelopedCountry"/>
  </owl:Thing>

  <owl:Thing rdf:about="#Macedonia">
    <Mid-level-ontology:economyType rdf:resource="#CountryInTransition"/>
  </owl:Thing>

  <Economy:IndustryAttribute rdf:about="#MachineryManufacturing">
    <Mid-level-ontology:industryProductType rdf:resource="#Machinery"/>
    <SUMO:subAttribute rdf:resource="#IndustrialSector"/>
    <rdfs:comment>MachineryManufacturing is 

the Attribute of an Organization whose primary business involves 

manufacturing Machinery.</rdfs:comment>
  </Economy:IndustryAttribute>

  <owl:Thing rdf:about="#Madagascar">
    <Mid-level-ontology:economyType rdf:resource="#DevelopingCountry"/>
    <Mid-level-ontology:economyType rdf:resource="#LessDevelopedCountry"/>
  </owl:Thing>

  <owl:Thing rdf:about="#MajorApplianceManufacturing">
    <Mid-level-ontology:industryProductType rdf:resource="#MajorAppliance"/>
    <SUMO:subAttribute rdf:resource="#HouseholdApplianceManufacturing"/>
    <rdfs:comment>MajorApplianceManufacturing 

is the Attribute of an Organization whose primary business involves 

manufacturing MajorAppliances.</rdfs:comment>
  </owl:Thing>

  <Economy:EconomicDevelopmentLevel rdf:about="#MajorIndustrialEconomy">
    <rdfs:comment>MajorIndustrialEconomy is an 

Attribute used to describe countries with the largest, industrialized, 

non-communist economies in the world.</rdfs:comment>
  </Economy:EconomicDevelopmentLevel>

  <owl:Thing rdf:about="#Malawi">
    <Mid-level-ontology:economyType rdf:resource="#DevelopingCountry"/>
    <Mid-level-ontology:economyType rdf:resource="#LessDevelopedCountry"/>
  </owl:Thing>

  <owl:Thing rdf:about="#Malaysia">
    <Mid-level-ontology:economyType rdf:resource="#DevelopingCountry"/>
    <Mid-level-ontology:economyType rdf:resource="#LessDevelopedCountry"/>
  </owl:Thing>

  <owl:Thing rdf:about="#Maldives">
    <Mid-level-ontology:economyType rdf:resource="#DevelopingCountry"/>
    <Mid-level-ontology:economyType rdf:resource="#LessDevelopedCountry"/>
  </owl:Thing>

  <owl:Thing rdf:about="#Mali">
    <Mid-level-ontology:economyType rdf:resource="#DevelopingCountry"/>
    <Mid-level-ontology:economyType rdf:resource="#LessDevelopedCountry"/>
  </owl:Thing>

  <owl:Thing rdf:about="#Malta">
    <Mid-level-ontology:economyType rdf:resource="#DevelopedCountry"/>
    <Mid-level-ontology:economyType rdf:resource="#DevelopingCountry"/>
    <Mid-level-ontology:economyType rdf:resource="#LessDevelopedCountry"/>
  </owl:Thing>

  <Economy:FinancialSectorAttribute rdf:about="#ManufacturingBasedEconomy">
    <rdfs:comment>ManufacturingBasedEconomy is the 

Attribute of an area whose economy is based primarily on activities in 

the manufacturing sector.</rdfs:comment>
  </Economy:FinancialSectorAttribute>

  <Mid-level-ontology:EconomicSystemAttribute rdf:about="#MarketSocialism">
    <SUMO:subAttribute rdf:resource="#PartialMarketEconomy"/>
    <rdfs:comment>MarketSocialism is an Attribute that 

describes an economy that has some socialistic institutions and some 

limited sectors in which markets operate.</rdfs:comment>
  </Mid-level-ontology:EconomicSystemAttribute>

  <owl:Thing rdf:about="#MarshallIslands">
    <Mid-level-ontology:economyType rdf:resource="#DevelopingCountry"/>
    <Mid-level-ontology:economyType rdf:resource="#LessDevelopedCountry"/>
  </owl:Thing>

  <owl:Thing rdf:about="#Mauritania">
    <Mid-level-ontology:economyType rdf:resource="#DevelopingCountry"/>
    <Mid-level-ontology:economyType rdf:resource="#LessDevelopedCountry"/>
  </owl:Thing>

  <owl:Thing rdf:about="#Mauritius">
    <Mid-level-ontology:economyType rdf:resource="#DevelopingCountry"/>
    <Mid-level-ontology:economyType rdf:resource="#LessDevelopedCountry"/>
  </owl:Thing>

  <owl:Thing rdf:about="#MetalOreMining">
    <Mid-level-ontology:industryProductType rdf:resource="&SUMO;Metal"/>
    <SUMO:subAttribute rdf:resource="#MiningIndustry"/>
    <rdfs:comment>MetalOreMining is the Attribute of an 

Organization whose primary business is mining metallic ore.</rdfs:comment>
  </owl:Thing>

  <Economy:IndustryAttribute rdf:about="#MetallurgyIndustry">
    <Mid-level-ontology:industryProductType rdf:resource="&SUMO;Metal"/>
    <SUMO:subAttribute rdf:resource="#IndustrialSector"/>
  </Economy:IndustryAttribute>

  <owl:Thing rdf:about="#MetalworkingMachineryManufacturing">
    <Mid-level-ontology:industryProductType rdf:resource="#MachineTool"/>
    <SUMO:subAttribute rdf:resource="#MachineryManufacturing"/>
    <rdfs:comment>MetalworkingMachineryManufacturing is the Attribute of an 

Organization whose primary business is manufacturing MachineTools.</rdfs:comment>
  </owl:Thing>

  <Economy:IndustryAttribute rdf:about="#MilletFarming">
    <Mid-level-ontology:industryProductType rdf:resource="#MilletGrain"/>
    <SUMO:subAttribute rdf:resource="#CerealGrainFarming"/>
    <rdfs:comment>MilletFarming is the IndustryAttribute that describes millet farming operations.</rdfs:comment>
  </Economy:IndustryAttribute>

  <Economy:IndustryAttribute rdf:about="#MiningIndustry">
    <SUMO:subAttribute rdf:resource="#IndustrialSector"/>
    <rdfs:comment>MiningIndustry is an Attribute of an 

Organization whose primary business involves mining.</rdfs:comment>
  </Economy:IndustryAttribute>

  <owl:Thing rdf:about="#Moldova">
    <Mid-level-ontology:economyType rdf:resource="#CountryInTransition"/>
  </owl:Thing>

  <owl:Thing rdf:about="#Monaco">
    <Mid-level-ontology:economyType rdf:resource="#DevelopedCountry"/>
  </owl:Thing>

  <owl:Thing rdf:about="#Mongolia">
    <Mid-level-ontology:economyType rdf:resource="#CountryInTransition"/>
  </owl:Thing>

  <owl:Thing rdf:about="#Morocco">
    <Mid-level-ontology:economyType rdf:resource="#DevelopingCountry"/>
    <Mid-level-ontology:economyType rdf:resource="#LessDevelopedCountry"/>
  </owl:Thing>

  <Economy:IndustryAttribute rdf:about="#MotorVehicleIndustry">
    <Mid-level-ontology:industryProductType rdf:resource="&Mid-level-ontology;RoadVehicle"/>
    <SUMO:subAttribute rdf:resource="#TransportationEquipmentIndustry"/>
    <rdfs:comment>MotorVehicleIndustry 

is the Attribute of an Organization whose primary business is 

manufacturing motor vehicles.</rdfs:comment>
  </Economy:IndustryAttribute>

  <owl:Thing rdf:about="#Mozambique">
    <Mid-level-ontology:economyType rdf:resource="#DevelopingCountry"/>
    <Mid-level-ontology:economyType rdf:resource="#LessDevelopedCountry"/>
  </owl:Thing>

  <owl:Thing rdf:about="#Namibia">
    <Mid-level-ontology:economyType rdf:resource="#DevelopingCountry"/>
    <Mid-level-ontology:economyType rdf:resource="#LessDevelopedCountry"/>
  </owl:Thing>

  <Economy:IndustryAttribute rdf:about="#NaturalGasIndustry">
    <Mid-level-ontology:industryProductType rdf:resource="http://reliant.teknowledge.com/DAML/Geography.owl#NaturalGas"/>
    <SUMO:subAttribute rdf:resource="#MiningIndustry"/>
    <rdfs:comment>NaturalGasIndustry is the Attribute 

of an Organization whose primary business is producing NaturalGas.</rdfs:comment>
  </Economy:IndustryAttribute>

  <owl:Thing rdf:about="#Nepal">
    <Mid-level-ontology:economyType rdf:resource="#DevelopingCountry"/>
    <Mid-level-ontology:economyType rdf:resource="#LessDevelopedCountry"/>
  </owl:Thing>

  <owl:Thing rdf:about="#Netherlands">
    <Mid-level-ontology:economyType rdf:resource="#AdvancedEconomy"/>
    <Mid-level-ontology:economyType rdf:resource="#DevelopedCountry"/>
  </owl:Thing>

  <owl:Thing rdf:about="#NetherlandsAntilles">
    <Mid-level-ontology:economyType rdf:resource="#DevelopingCountry"/>
    <Mid-level-ontology:economyType rdf:resource="#LessDevelopedCountry"/>
  </owl:Thing>

  <owl:Thing rdf:about="#NewZealand">
    <Mid-level-ontology:economyType rdf:resource="#AdvancedEconomy"/>
    <Mid-level-ontology:economyType rdf:resource="#DevelopedCountry"/>
  </owl:Thing>

  <Economy:EconomicDevelopmentLevel rdf:about="#NewlyIndustrializingEconomy"
                                    rdfs:label="Newly Industrializing Economies">
    <rdfs:comment>NewlyIndustrializingEconomy is an Attribute used to describe a 

LessDevelopedCountry (LDC) that is undergoing rapid industrial 

development.  Also called 'newly industrializing economy' (or 

'country').</rdfs:comment>
  </Economy:EconomicDevelopmentLevel>

  <owl:Thing rdf:about="#Nicaragua">
    <Mid-level-ontology:economyType rdf:resource="#DevelopingCountry"/>
    <Mid-level-ontology:economyType rdf:resource="#LessDevelopedCountry"/>
  </owl:Thing>

  <owl:Thing rdf:about="#NickelOreMining">
    <Mid-level-ontology:industryProductType rdf:resource="#NickelOre"/>
    <SUMO:subAttribute rdf:resource="#MiningIndustry"/>
    <rdfs:comment>NickelOreMining is the Attribute of 

an Organization whose primary business involves mining NickelOre.</rdfs:comment>
  </owl:Thing>

  <owl:Thing rdf:about="#Niger">
    <Mid-level-ontology:economyType rdf:resource="#DevelopingCountry"/>
    <Mid-level-ontology:economyType rdf:resource="#LessDevelopedCountry"/>
  </owl:Thing>

  <owl:Thing rdf:about="#Nigeria">
    <Mid-level-ontology:economyType rdf:resource="#DevelopingCountry"/>
    <Mid-level-ontology:economyType rdf:resource="#LessDevelopedCountry"/>
  </owl:Thing>

  <owl:Thing rdf:about="#Norway">
    <Mid-level-ontology:economyType rdf:resource="#AdvancedEconomy"/>
    <Mid-level-ontology:economyType rdf:resource="#DevelopedCountry"/>
  </owl:Thing>

  <Economy:PowerGeneration rdf:about="#NuclearPowerGeneration"/>
  <Economy:IndustryAttribute rdf:about="#OatFarming">
    <Mid-level-ontology:industryProductType rdf:resource="#OatGrain"/>
    <SUMO:subAttribute rdf:resource="#CerealGrainFarming"/>
    <rdfs:comment>OatFarming is the IndustryAttribute that describes oat farming operations.</rdfs:comment>
  </Economy:IndustryAttribute>

  <owl:Thing rdf:about="#OffshoreBankingSectorEconomy">
    <SUMO:subAttribute rdf:resource="#OffshoreFinancialSectorEconomy"/>
    <rdfs:comment>OffshoreBankingSectorEconomy 

is the sub-type of OffshoreFinancialSectorEconomy, describing an area 

whose economy is based primarily or significantly on its offshore banking 

services.</rdfs:comment>
  </owl:Thing>

  <Economy:FinancialSectorAttribute rdf:about="#OffshoreFinancialSectorEconomy">
    <rdfs:comment>OffshoreFinancialSectorEconomy is the Attribute of an area whose 

economy is based primarily or significantly on its offshore financial 

services, which attract overseas investments or deposits.</rdfs:comment>
  </Economy:FinancialSectorAttribute>

  <owl:Thing rdf:about="#Oman">
    <Mid-level-ontology:economyType rdf:resource="#DevelopingCountry"/>
    <Mid-level-ontology:economyType rdf:resource="#LessDevelopedCountry"/>
  </owl:Thing>

  <Economy:PowerGeneration rdf:about="#OtherSourcePowerGeneration">
    <rdfs:comment>OtherSourcePowerGeneration 

represents all non-fossil fuel, non-hydroelectric, and non-nuclear power 

generation processes, e.g., wind power generation.</rdfs:comment>
  </Economy:PowerGeneration>

  <owl:Thing rdf:about="#Pakistan">
    <Mid-level-ontology:economyType rdf:resource="#DevelopingCountry"/>
    <Mid-level-ontology:economyType rdf:resource="#LessDevelopedCountry"/>
  </owl:Thing>

  <owl:Thing rdf:about="#Panama">
    <Mid-level-ontology:economyType rdf:resource="#DevelopingCountry"/>
    <Mid-level-ontology:economyType rdf:resource="#LessDevelopedCountry"/>
  </owl:Thing>

  <owl:Thing rdf:about="#PapuaNewGuinea">
    <Mid-level-ontology:economyType rdf:resource="#DevelopingCountry"/>
    <Mid-level-ontology:economyType rdf:resource="#LessDevelopedCountry"/>
  </owl:Thing>

  <owl:Thing rdf:about="#Paraguay">
    <Mid-level-ontology:economyType rdf:resource="#DevelopingCountry"/>
    <Mid-level-ontology:economyType rdf:resource="#LessDevelopedCountry"/>
  </owl:Thing>

  <Mid-level-ontology:EconomicSystemAttribute rdf:about="#PartialMarketEconomy">
    <SUMO:subAttribute rdf:resource="&Mid-level-ontology;MixedEconomy"/>
    <rdfs:comment>PartialMarketEconomy is the 

Attribute of any MixedEconomy which operates partially with market 

mechanisms.</rdfs:comment>
  </Mid-level-ontology:EconomicSystemAttribute>

  <owl:Thing rdf:about="#PeanutFarming">
    <Mid-level-ontology:industryProductType rdf:resource="#Peanut"/>
    <SUMO:subAttribute rdf:resource="#CropProduction"/>
    <rdfs:comment>PeanutFarming is the specification of 

CropProduction that describes peanut farming operations.</rdfs:comment>
  </owl:Thing>

  <owl:Thing rdf:about="#Peru">
    <Mid-level-ontology:economyType rdf:resource="#DevelopingCountry"/>
    <Mid-level-ontology:economyType rdf:resource="#LessDevelopedCountry"/>
  </owl:Thing>

  <Economy:FinancialSectorAttribute rdf:about="#PetroleumBasedEconomy">
    <rdfs:comment>PetroleumBasedEconomy is the 

Attribute of an area whose economy is based primarily on activities in 

the petroleum industry.</rdfs:comment>
  </Economy:FinancialSectorAttribute>

  <Economy:IndustryAttribute rdf:about="#PetroleumIndustry">
    <Mid-level-ontology:industryProductType rdf:resource="#PetroleumProduct"/>
    <SUMO:subAttribute rdf:resource="#IndustrialSector"/>
    <rdfs:comment>PetroleumIndustry is the Attribute of 

an Organization whose primary business involves drilling, extracting, or 

further processing of crude petroleum or petroleum products.</rdfs:comment>
  </Economy:IndustryAttribute>

  <Economy:IndustryAttribute rdf:about="#PharmaceuticalPreparationManufacturing">
    <Mid-level-ontology:industryProductType rdf:resource="#PharmaceuticalProduct"/>
    <SUMO:subAttribute rdf:resource="#IndustrialSector"/>
    <rdfs:comment>PharmaceuticalPreparationManufacturing is the Attribute of an 

Organization whose primary business involves manufacturing drugs.</rdfs:comment>
  </Economy:IndustryAttribute>

  <owl:Thing rdf:about="#Philippines">
    <Mid-level-ontology:economyType rdf:resource="#DevelopingCountry"/>
    <Mid-level-ontology:economyType rdf:resource="#LessDevelopedCountry"/>
  </owl:Thing>

  <owl:Thing rdf:about="#Portugal">
    <Mid-level-ontology:economyType rdf:resource="#AdvancedEconomy"/>
    <Mid-level-ontology:economyType rdf:resource="#DevelopedCountry"/>
  </owl:Thing>

  <owl:Thing rdf:about="#PotatoFarming">
    <Mid-level-ontology:industryProductType rdf:resource="#PotatoTuber"/>
    <SUMO:subAttribute rdf:resource="#VegetableFarming"/>
    <rdfs:comment>PotatoFarming is the specification of 

VegetableFarming that describes potato farming operations.</rdfs:comment>
  </owl:Thing>

  <Economy:IndustryAttribute rdf:about="#PrimaryMetalManufacturing">
    <Mid-level-ontology:industryProductType rdf:resource="&SUMO;Metal"/>
    <SUMO:subAttribute rdf:resource="#MetallurgyIndustry"/>
    <rdfs:comment>PrimaryMetalManufacturing is 

an Attribute of an Organization whose primary business involves the 

smelting or refining of ferrous or non-ferrous metals from ore or scrap 

to produce forgings or castings; in particular iron, aluminum, copper, 

lead, zinc, or nickel manufacturing.</rdfs:comment>
  </Economy:IndustryAttribute>

  <owl:Thing rdf:about="#Qatar">
    <Mid-level-ontology:economyType rdf:resource="#DevelopingCountry"/>
    <Mid-level-ontology:economyType rdf:resource="#LessDevelopedCountry"/>
  </owl:Thing>

  <owl:Thing rdf:about="#RefrigeratorAndFreezerIndustry">
    <Mid-level-ontology:industryProductType rdf:resource="#Freezer"/>
    <Mid-level-ontology:industryProductType rdf:resource="#Refrigerator"/>
    <SUMO:subAttribute rdf:resource="#MajorApplianceManufacturing"/>
    <rdfs:comment>RefrigeratorAndFreezerIndustry is the Attribute of an Organization 

whose primary business involves manufacturing refrigerators or freezers.</rdfs:comment>
  </owl:Thing>

  <owl:Thing rdf:about="#RepublicOfTheCongo">
    <Mid-level-ontology:economyType rdf:resource="#DevelopingCountry"/>
    <Mid-level-ontology:economyType rdf:resource="#LessDevelopedCountry"/>
  </owl:Thing>

  <Economy:IndustryAttribute rdf:about="#RiceFarming">
    <Mid-level-ontology:industryProductType rdf:resource="#RiceGrain"/>
    <SUMO:subAttribute rdf:resource="#CerealGrainFarming"/>
    <rdfs:comment>RiceFarming is the IndustryAttribute 

that describes rice farming operations.</rdfs:comment>
  </Economy:IndustryAttribute>

  <owl:Thing rdf:about="#Romania">
    <Mid-level-ontology:economyType rdf:resource="#CountryInTransition"/>
  </owl:Thing>

  <owl:Thing rdf:about="#Rwanda">
    <Mid-level-ontology:economyType rdf:resource="#DevelopingCountry"/>
    <Mid-level-ontology:economyType rdf:resource="#LessDevelopedCountry"/>
  </owl:Thing>

  <Economy:IndustryAttribute rdf:about="#RyeFarming">
    <Mid-level-ontology:industryProductType rdf:resource="#RyeGrain"/>
    <SUMO:subAttribute rdf:resource="#CerealGrainFarming"/>
    <rdfs:comment>RyeFarming is the IndustryAttribute that describes rye farming operations.</rdfs:comment>
  </Economy:IndustryAttribute>

  <owl:Thing rdf:about="#SaintKittsAndNevis">
    <Mid-level-ontology:economyType rdf:resource="#DevelopingCountry"/>
    <Mid-level-ontology:economyType rdf:resource="#LessDevelopedCountry"/>
  </owl:Thing>

  <owl:Thing rdf:about="#SaintLucia">
    <Mid-level-ontology:economyType rdf:resource="#DevelopingCountry"/>
    <Mid-level-ontology:economyType rdf:resource="#LessDevelopedCountry"/>
  </owl:Thing>

  <owl:Thing rdf:about="#SaintVincentAndTheGrenadines">
    <Mid-level-ontology:economyType rdf:resource="#DevelopingCountry"/>
    <Mid-level-ontology:economyType rdf:resource="#LessDevelopedCountry"/>
  </owl:Thing>

  <owl:Thing rdf:about="#Samoa">
    <Mid-level-ontology:economyType rdf:resource="#DevelopingCountry"/>
    <Mid-level-ontology:economyType rdf:resource="#LessDevelopedCountry"/>
  </owl:Thing>

  <owl:Thing rdf:about="#SanMarino">
    <Mid-level-ontology:economyType rdf:resource="#DevelopedCountry"/>
  </owl:Thing>

  <owl:Thing rdf:about="#SaoTomeAndPrincipe">
    <Mid-level-ontology:economyType rdf:resource="#DevelopingCountry"/>
    <Mid-level-ontology:economyType rdf:resource="#LessDevelopedCountry"/>
  </owl:Thing>

  <owl:Thing rdf:about="#SaudiArabia">
    <Mid-level-ontology:economyType rdf:resource="#DevelopingCountry"/>
    <Mid-level-ontology:economyType rdf:resource="#LessDevelopedCountry"/>
  </owl:Thing>

  <owl:Thing rdf:about="#Senegal">
    <Mid-level-ontology:economyType rdf:resource="#DevelopingCountry"/>
    <Mid-level-ontology:economyType rdf:resource="#LessDevelopedCountry"/>
  </owl:Thing>

  <Economy:FinancialSectorAttribute rdf:about="#ServiceBasedEconomy">
    <rdfs:comment>ServiceBasedEconomy is the 

Attribute of an economy that is based primarily or significantly 

on ServiceSector businesses.</rdfs:comment>
  </Economy:FinancialSectorAttribute>

  <Economy:EconomicSector rdf:about="#ServiceSector">
    <rdfs:comment>ServiceSector is an attribute 

that describes commercial organizations or agents whose business is in 

the service sector of the economy.</rdfs:comment>
  </Economy:EconomicSector>

  <owl:Thing rdf:about="#Seychelles">
    <Mid-level-ontology:economyType rdf:resource="#DevelopingCountry"/>
    <Mid-level-ontology:economyType rdf:resource="#LessDevelopedCountry"/>
  </owl:Thing>

  <owl:Thing rdf:about="#SheepFarming">
    <Mid-level-ontology:industryProductType rdf:resource="&Mid-level-ontology;Sheep"/>
    <SUMO:subAttribute rdf:resource="#AnimalProduction"/>
    <rdfs:comment>SheepFarming is the specification of 

AnimalProduction that describes sheep farming operations.</rdfs:comment>
  </owl:Thing>

  <owl:Thing rdf:about="#SierraLeone">
    <Mid-level-ontology:economyType rdf:resource="#DevelopingCountry"/>
    <Mid-level-ontology:economyType rdf:resource="#LessDevelopedCountry"/>
  </owl:Thing>

  <owl:Thing rdf:about="#Singapore">
    <Mid-level-ontology:economyType rdf:resource="#AdvancedEconomy"/>
    <Mid-level-ontology:economyType rdf:resource="#FourDragonsEconomy"/>
  </owl:Thing>

  <owl:Thing rdf:about="#Slovakia">
    <Mid-level-ontology:economyType rdf:resource="#CountryInTransition"/>
  </owl:Thing>

  <owl:Thing rdf:about="#Slovenia">
    <Mid-level-ontology:economyType rdf:resource="#CountryInTransition"/>
  </owl:Thing>

  <owl:Thing rdf:about="#SmallElectricalApplianceManufacturing">
    <Mid-level-ontology:industryProductType rdf:resource="&Mid-level-ontology;ElectricDevice"/>
    <SUMO:subAttribute rdf:resource="#HouseholdApplianceManufacturing"/>
    <rdfs:comment>SmallElectricalApplianceManufacturing is the Attribute of an 

Organization whose primary business involves manufacturing small 

electrical household appliances.</rdfs:comment>
  </owl:Thing>

  <Economy:IndustryAttribute rdf:about="#SoapIndustry">
    <Mid-level-ontology:industryProductType rdf:resource="&Mid-level-ontology;Detergent"/>
    <SUMO:subAttribute rdf:resource="#IndustrialSector"/>
    <rdfs:comment>SoapIndustry is the Attribute of an 

Organization whose primary business involves manufacturing detergents.</rdfs:comment>
  </Economy:IndustryAttribute>

  <owl:Thing rdf:about="#Somalia">
    <Mid-level-ontology:economyType rdf:resource="#DevelopingCountry"/>
    <Mid-level-ontology:economyType rdf:resource="#LessDevelopedCountry"/>
  </owl:Thing>

  <Economy:IndustryAttribute rdf:about="#SorghumFarming">
    <Mid-level-ontology:industryProductType rdf:resource="#SorghumGrain"/>
    <SUMO:subAttribute rdf:resource="#CerealGrainFarming"/>
    <rdfs:comment>SorghumFarming is the IndustryAttribute that describes sorghum farming operations.</rdfs:comment>
  </Economy:IndustryAttribute>

  <owl:Thing rdf:about="#SouthAfrica">
    <Mid-level-ontology:economyType rdf:resource="#DevelopedCountry"/>
    <Mid-level-ontology:economyType rdf:resource="#DevelopingCountry"/>
    <Mid-level-ontology:economyType rdf:resource="#LessDevelopedCountry"/>
  </owl:Thing>

  <owl:Thing rdf:about="#SouthKorea">
    <Mid-level-ontology:economyType rdf:resource="#AdvancedEconomy"/>
    <Mid-level-ontology:economyType rdf:resource="#FourDragonsEconomy"/>
  </owl:Thing>

  <owl:Thing rdf:about="#Spain">
    <Mid-level-ontology:economyType rdf:resource="#AdvancedEconomy"/>
    <Mid-level-ontology:economyType rdf:resource="#DevelopedCountry"/>
  </owl:Thing>

  <owl:Thing rdf:about="#SriLanka">
    <Mid-level-ontology:economyType rdf:resource="#DevelopingCountry"/>
    <Mid-level-ontology:economyType rdf:resource="#LessDevelopedCountry"/>
  </owl:Thing>

  <Economy:IndustryAttribute rdf:about="#SteelIndustry">
    <Mid-level-ontology:industryProductType rdf:resource="&Mid-level-ontology;Steel"/>
    <SUMO:subAttribute rdf:resource="#PrimaryMetalManufacturing"/>
    <rdfs:comment>SteelIndustry is the Attribute of an 

Organization whose primary business involves manufacturing steel or 

steel products.</rdfs:comment>
  </Economy:IndustryAttribute>

  <owl:Thing rdf:about="#SteelMills">
    <Mid-level-ontology:industryProductType rdf:resource="&Mid-level-ontology;Steel"/>
    <SUMO:subAttribute rdf:resource="#SteelIndustry"/>
    <rdfs:comment>SteelMills is the Attribute of 

an Organization whose primary business involves manufacturing steel.</rdfs:comment>
  </owl:Thing>

  <owl:Thing rdf:about="#StoneMiningAndQuarrying">
    <Mid-level-ontology:industryProductType rdf:resource="&Mid-level-ontology;Rock"/>
    <SUMO:subAttribute rdf:resource="#MiningIndustry"/>
    <rdfs:comment>StoneMiningAndQuarrying is the 

Attribute of an Organization whose primary business involves quarrying 

or mining stone.</rdfs:comment>
  </owl:Thing>

  <Economy:FinancialSectorAttribute rdf:about="#SubsistenceAgricultureEconomy">
    <SUMO:subAttribute rdf:resource="#AgricultureBasedEconomy"/>
    <rdfs:comment>SubsistenceAgricultureEconomy is the Attribute of an economy that is 

based primarily or significantly on AgriculturalSector activities that 

operate merely at the subsistence level.</rdfs:comment>
  </Economy:FinancialSectorAttribute>

  <owl:Thing rdf:about="#Sudan">
    <Mid-level-ontology:economyType rdf:resource="#DevelopingCountry"/>
    <Mid-level-ontology:economyType rdf:resource="#LessDevelopedCountry"/>
  </owl:Thing>

  <owl:Thing rdf:about="#SugarBeetFarming">
    <Mid-level-ontology:industryProductType rdf:resource="#SugarBeet"/>
    <SUMO:subAttribute rdf:resource="#CropProduction"/>
    <rdfs:comment>SugarBeetFarming is the specification 

of CropProduction that describes sugar beet farming operations.</rdfs:comment>
  </owl:Thing>

  <owl:Thing rdf:about="#Suriname">
    <Mid-level-ontology:economyType rdf:resource="#DevelopingCountry"/>
    <Mid-level-ontology:economyType rdf:resource="#LessDevelopedCountry"/>
  </owl:Thing>

  <owl:Thing rdf:about="#Swaziland">
    <Mid-level-ontology:economyType rdf:resource="#DevelopingCountry"/>
    <Mid-level-ontology:economyType rdf:resource="#LessDevelopedCountry"/>
  </owl:Thing>

  <owl:Thing rdf:about="#Syria">
    <Mid-level-ontology:economyType rdf:resource="#DevelopingCountry"/>
    <Mid-level-ontology:economyType rdf:resource="#LessDevelopedCountry"/>
  </owl:Thing>

  <owl:Thing rdf:about="#Taiwan">
    <Mid-level-ontology:economyType rdf:resource="#AdvancedEconomy"/>
    <Mid-level-ontology:economyType rdf:resource="#FourDragonsEconomy"/>
  </owl:Thing>

  <owl:Thing rdf:about="#Tajikistan">
    <Mid-level-ontology:economyType rdf:resource="#CountryInTransition"/>
  </owl:Thing>

  <owl:Thing rdf:about="#Tanzania">
    <Mid-level-ontology:economyType rdf:resource="#DevelopingCountry"/>
    <Mid-level-ontology:economyType rdf:resource="#LessDevelopedCountry"/>
  </owl:Thing>

  <Economy:IndustryAttribute rdf:about="#TelecommunicationsIndustry">
    <Economy:industryServiceType rdf:resource="&SUMO;Communication"/>
    <SUMO:subAttribute rdf:resource="#ServiceSector"/>
    <rdfs:comment>TelecommunicationsIndustry 

is the Attribute of an Organization whose primary business involves 

telecommunications.</rdfs:comment>
  </Economy:IndustryAttribute>

  <Economy:IndustryAttribute rdf:about="#TextileIndustry">
    <Mid-level-ontology:industryProductType rdf:resource="#TextileProduct"/>
    <Mid-level-ontology:industryProductType rdf:resource="&SUMO;Fabric"/>
    <SUMO:subAttribute rdf:resource="#IndustrialSector"/>
    <rdfs:comment>TextileIndustry is the Attribute of 

an Organization whose primary business is making TextileProducts.</rdfs:comment>
  </Economy:IndustryAttribute>

  <owl:Thing rdf:about="#Thailand">
    <Mid-level-ontology:economyType rdf:resource="#DevelopingCountry"/>
    <Mid-level-ontology:economyType rdf:resource="#LessDevelopedCountry"/>
  </owl:Thing>

  <owl:Thing rdf:about="#Togo">
    <Mid-level-ontology:economyType rdf:resource="#DevelopingCountry"/>
    <Mid-level-ontology:economyType rdf:resource="#LessDevelopedCountry"/>
  </owl:Thing>

  <Economy:FinancialSectorAttribute rdf:about="#TourismBasedEconomy">
    <rdfs:comment>TourismBasedEconomy is the 

Attribute of an area whose economy is based primarily on activities in 

the tourist industry.</rdfs:comment>
  </Economy:FinancialSectorAttribute>

  <Economy:IndustryAttribute rdf:about="#TourismIndustry">
    <Economy:industryServiceType rdf:resource="&SUMO;RecreationOrExercise"/>
    <SUMO:subAttribute rdf:resource="#ServiceSector"/>
    <rdfs:comment>TourismIndustry is an Attribute that 

describes organizations that provide services or products for travellers 

who stay temporarily in a region to experience local attractions.  There 

is an overlap (but not subsumption) between TourismIndustry and each of 

the following industries: travel services and accommodations, entertainment 

and recreation, and arts and museums or historical sites.</rdfs:comment>
  </Economy:IndustryAttribute>

  <Economy:FinancialSectorAttribute rdf:about="#TradeBasedEconomy">
    <rdfs:comment>TradeBasedEconomy is the 

Attribute of an area whose economy is based primarily on activities in 

the trade sector.</rdfs:comment>
  </Economy:FinancialSectorAttribute>

  <Economy:IndustryAttribute rdf:about="#TransportationEquipmentIndustry">
    <Mid-level-ontology:industryProductType rdf:resource="&SUMO;TransportationDevice"/>
    <SUMO:subAttribute rdf:resource="#IndustrialSector"/>
    <rdfs:comment>TransportationEquipmentIndustry  is an Attribute of an 

Organization whose primary business involves the manufacturing of 

TransportationDevices.</rdfs:comment>
  </Economy:IndustryAttribute>

  <owl:Thing rdf:about="#TreeNutFarming">
    <Mid-level-ontology:industryProductType rdf:resource="#EdibleNut"/>
    <SUMO:subAttribute rdf:resource="#FruitAndTreeNutFarming"/>
    <rdfs:comment>TreeNutFarming is the specification of 

FruitAndTreeNutFarming that describes tree nut farming operations.</rdfs:comment>
  </owl:Thing>

  <owl:Thing rdf:about="#TrinidadAndTobago">
    <Mid-level-ontology:economyType rdf:resource="#DevelopingCountry"/>
    <Mid-level-ontology:economyType rdf:resource="#LessDevelopedCountry"/>
  </owl:Thing>

  <owl:Thing rdf:about="#Tunisia">
    <Mid-level-ontology:economyType rdf:resource="#DevelopingCountry"/>
    <Mid-level-ontology:economyType rdf:resource="#LessDevelopedCountry"/>
  </owl:Thing>

  <owl:Thing rdf:about="#Turkmenistan">
    <Mid-level-ontology:economyType rdf:resource="#CountryInTransition"/>
  </owl:Thing>

  <Economy:FinancialSectorAttribute rdf:about="#TwoTierLaborMarketEconomy">
    <rdfs:comment>TwoTierLaborMarketEconomy is 

the Attribute of an area whose economy has a labor market characterized 

by a division between highly paid professional workers and low-paid 

unskilled labor.  Such economies may provide cheap labor pools for 

overseas manufacturing.</rdfs:comment>
  </Economy:FinancialSectorAttribute>

  <owl:Thing rdf:about="#Uganda">
    <Mid-level-ontology:economyType rdf:resource="#DevelopingCountry"/>
    <Mid-level-ontology:economyType rdf:resource="#LessDevelopedCountry"/>
  </owl:Thing>

  <owl:Thing rdf:about="#Ukraine">
    <Mid-level-ontology:economyType rdf:resource="#CountryInTransition"/>
  </owl:Thing>

  <Economy:EconomicDevelopmentLevel rdf:about="#UnderdevelopedCountry">
    <SUMO:subAttribute rdf:resource="#LessDevelopedCountry"/>
    <rdfs:comment>UnderdevelopedCountry is an 

Attribute describing less developed countries that have potential 

for above-average economic growth.  See also LessDevelopedCountry.</rdfs:comment>
  </Economy:EconomicDevelopmentLevel>

  <owl:Thing rdf:about="#UnitedArabEmirates">
    <Mid-level-ontology:economyType rdf:resource="#DevelopingCountry"/>
    <Mid-level-ontology:economyType rdf:resource="#LessDevelopedCountry"/>
  </owl:Thing>

  <Economy:WorldBankGNIPerCapitaLevel rdf:about="#UpperMiddleIncomeCountry">
    <SUMO:successorAttribute rdf:resource="#HighIncomeCountry"/>
    <rdfs:comment>LowerMiddleIncomeCountry is an Attribute representing the World Bank 

classification for any country where the per capita GNI is 

between $2,996 and $9,266 (inclusive) in UnitedStatesDollars.</rdfs:comment>
  </Economy:WorldBankGNIPerCapitaLevel>

  <owl:Thing rdf:about="#Uruguay">
    <Mid-level-ontology:economyType rdf:resource="#DevelopingCountry"/>
    <Mid-level-ontology:economyType rdf:resource="#LessDevelopedCountry"/>
  </owl:Thing>

  <owl:Thing rdf:about="#Uzbekistan">
    <Mid-level-ontology:economyType rdf:resource="#CountryInTransition"/>
  </owl:Thing>

  <owl:Thing rdf:about="#Vanuatu">
    <Mid-level-ontology:economyType rdf:resource="#DevelopingCountry"/>
    <Mid-level-ontology:economyType rdf:resource="#LessDevelopedCountry"/>
  </owl:Thing>

  <Economy:IndustryAttribute rdf:about="#VegetableAndMelonFarming">
    <Mid-level-ontology:industryProductType rdf:resource="#PlantAgriculturalProduct"/>
    <SUMO:subAttribute rdf:resource="#CropProduction"/>
    <rdfs:comment>VegetableAndMelonFarming is the IndustryAttribute that describes 

vegetable and melon farming operations.</rdfs:comment>
  </Economy:IndustryAttribute>

  <Economy:IndustryAttribute rdf:about="#VegetableFarming">
    <Mid-level-ontology:industryProductType rdf:resource="#Vegetable"/>
    <SUMO:subAttribute rdf:resource="#VegetableAndMelonFarming"/>
    <rdfs:comment>VegetableFarming is the specification of 

VegetableAndMelonFarming that describes vegetable farming operations.</rdfs:comment>
  </Economy:IndustryAttribute>

  <Economy:IndustryAttribute rdf:about="#VegetableOilIndustry">
    <Mid-level-ontology:industryProductType rdf:resource="#VegetableOil"/>
    <SUMO:subAttribute rdf:resource="#AgriculturalSector"/>
    <rdfs:comment>VegetableOilIndustry is the 

Attribute of an Organization whose primary business is manufacturing  

VegetableOil.</rdfs:comment>
  </Economy:IndustryAttribute>

  <owl:Thing rdf:about="#Venezuela">
    <Mid-level-ontology:economyType rdf:resource="#DevelopingCountry"/>
    <Mid-level-ontology:economyType rdf:resource="#LessDevelopedCountry"/>
  </owl:Thing>

  <owl:Thing rdf:about="#Vietnam">
    <Mid-level-ontology:economyType rdf:resource="#DevelopingCountry"/>
    <Mid-level-ontology:economyType rdf:resource="#LessDevelopedCountry"/>
  </owl:Thing>

  <Economy:IndustryAttribute rdf:about="#WheatFarming">
    <Mid-level-ontology:industryProductType rdf:resource="#WheatGrain"/>
    <SUMO:subAttribute rdf:resource="#CerealGrainFarming"/>
    <rdfs:comment>WheatFarming is the IndustryAttribute that describes wheat farming operations.</rdfs:comment>
  </Economy:IndustryAttribute>

  <owl:Thing rdf:about="#WineGrapeFarming">
    <Mid-level-ontology:industryProductType rdf:resource="#WineGrape"/>
    <SUMO:subAttribute rdf:resource="#GrapeFarming"/>
    <rdfs:comment>WineGrapeFarming is the specification 

of GrapeFarming that describes WineGrape farming operations.</rdfs:comment>
  </owl:Thing>

  <owl:Thing rdf:about="#WoodProductManufacturing">
    <Mid-level-ontology:industryProductType rdf:resource="#WoodProduct"/>
    <SUMO:subAttribute rdf:resource="#LumberIndustry"/>
    <rdfs:comment>WoodProductManufacturing is 

the Attribute of an Organization whose primary business involves 

manufacturing WoodProducts.</rdfs:comment>
  </owl:Thing>

  <owl:Thing rdf:about="#Yemen">
    <Mid-level-ontology:economyType rdf:resource="#DevelopingCountry"/>
    <Mid-level-ontology:economyType rdf:resource="#LessDevelopedCountry"/>
  </owl:Thing>

  <owl:Thing rdf:about="#Zambia">
    <Mid-level-ontology:economyType rdf:resource="#DevelopingCountry"/>
    <Mid-level-ontology:economyType rdf:resource="#LessDevelopedCountry"/>
  </owl:Thing>

  <owl:Thing rdf:about="#Zimbabwe">
    <Mid-level-ontology:economyType rdf:resource="#DevelopingCountry"/>
    <Mid-level-ontology:economyType rdf:resource="#LessDevelopedCountry"/>
  </owl:Thing>

  <Economy:IndustryAttribute rdf:about="#ZincIndustry">
    <Mid-level-ontology:industryProductType rdf:resource="&Mid-level-ontology;Zinc"/>
    <SUMO:subAttribute rdf:resource="#IndustrialSector"/>
    <rdfs:comment>ZincIndustry is the Attribute of an 

Organization whose primary business is mining or manufacturing Zinc.</rdfs:comment>
  </Economy:IndustryAttribute>

  <Economy:IndustryAttribute rdf:about="#ZincManufacturing">
    <Mid-level-ontology:industryProductType rdf:resource="#ZincProduct"/>
    <SUMO:subAttribute rdf:resource="#PrimaryMetalManufacturing"/>
    <SUMO:subAttribute rdf:resource="#ZincIndustry"/>
    <rdfs:comment>ZincManufacturing is the Attribute 

of an Organization whose primary business is making ZincProducts.</rdfs:comment>
  </Economy:IndustryAttribute>

  <Economy:IndustryAttribute rdf:about="#ZincOreMining">
    <Mid-level-ontology:industryProductType rdf:resource="#ZincOre"/>
    <SUMO:subAttribute rdf:resource="#MetalOreMining"/>
    <SUMO:subAttribute rdf:resource="#ZincIndustry"/>
    <rdfs:comment>ZincOreMining is the Attribute of an 

Organization whose primary business is mining ZincOre.</rdfs:comment>
  </Economy:IndustryAttribute>

  <owl:Thing rdf:about="http://reliant.teknowledge.com/DAML/Geography.owl#Coal"/>
  <owl:Thing rdf:about="http://reliant.teknowledge.com/DAML/Geography.owl#NaturalGas"/>
  <owl:Thing rdf:about="http://reliant.teknowledge.com/DAML/Geography.owl#Potash"/>
  <owl:Thing rdf:about="http://reliant.teknowledge.com/DAML/Geography.owl#SoutheasternEurope"/>
  <owl:Thing rdf:about="&Mid-level-ontology;Agriculture"/>
  <owl:Thing rdf:about="&Mid-level-ontology;Aircraft"/>
  <owl:Thing rdf:about="&Mid-level-ontology;Canada">
    <Mid-level-ontology:economyType rdf:resource="#AdvancedEconomy"/>
    <Mid-level-ontology:economyType rdf:resource="#DevelopedCountry"/>
  </owl:Thing>

  <Mid-level-ontology:EconomicSystemAttribute rdf:about="&Mid-level-ontology;CapitalistEconomy">
    <rdfs:comment>CapitalistEconomy is the 

Attribute used to characterize a country whose economy is based 

on private ownership of the means of production and distribution, 

and on private accumulation of capital.</rdfs:comment>
  </Mid-level-ontology:EconomicSystemAttribute>

  <Mid-level-ontology:EconomicSystemAttribute rdf:about="&Mid-level-ontology;CentrallyPlannedEconomy">
    <SUMO:subAttribute rdf:resource="&Mid-level-ontology;GovernmentRegulatedEconomy"/>
    <rdfs:comment>CentrallyPlannedEconomy 

is a term used mainly to describe communist or formerly communist 

states, many of which are now evolving away from command economies 

towards market-oriented systems.  Also known as a 'command economy'.</rdfs:comment>
  </Mid-level-ontology:EconomicSystemAttribute>

  <owl:Thing rdf:about="&Mid-level-ontology;Clay"/>
  <Mid-level-ontology:EconomicSystemAttribute rdf:about="&Mid-level-ontology;DemocraticSocialism">
    <SUMO:subAttribute rdf:resource="&Mid-level-ontology;SocialistEconomy"/>
    <rdfs:comment>DemocraticSocialism is an  

Attribute that describes a country in which socialism is promoted 

by a political party or parties within a democratic government. 

Under DemocraticSocialism, the government participates in central 

planning of the economy and may also manage nationalized industries.</rdfs:comment>
  </Mid-level-ontology:EconomicSystemAttribute>

  <owl:Thing rdf:about="&Mid-level-ontology;France">
    <Mid-level-ontology:economyType rdf:resource="#AdvancedEconomy"/>
    <Mid-level-ontology:economyType rdf:resource="#DevelopedCountry"/>
  </owl:Thing>

  <owl:Thing rdf:about="&Mid-level-ontology;Georgia">
    <Mid-level-ontology:economyType rdf:resource="#CountryInTransition"/>
  </owl:Thing>

  <owl:Thing rdf:about="&Mid-level-ontology;Germany">
    <Mid-level-ontology:economyType rdf:resource="#AdvancedEconomy"/>
    <Mid-level-ontology:economyType rdf:resource="#DevelopedCountry"/>
  </owl:Thing>

  <Mid-level-ontology:EconomicSystemAttribute rdf:about="&Mid-level-ontology;GovernmentRegulatedEconomy">
    <rdfs:comment>GovernmentRegulatedEconomy 

is an Attribute that describes the economy of a country in which the 

government determines prices, production, wages, allocation of resources, 

or other economic factors.  An economy that is wholly government planned 

is a CentrallyPlannedEconomy.</rdfs:comment>
  </Mid-level-ontology:EconomicSystemAttribute>

  <Mid-level-ontology:EconomicSystemAttribute rdf:about="&Mid-level-ontology;GovernmentSubsidizedEconomy">
    <rdfs:comment>GovernmentSubsidizedEconomy 

is an Attribute describing an economy in which the government provides 

subsidies to various industries, workers, or other groups as part of its 

economic policy.</rdfs:comment>
  </Mid-level-ontology:EconomicSystemAttribute>

  <owl:Thing rdf:about="&Mid-level-ontology;Greece">
    <Mid-level-ontology:economyType rdf:resource="#AdvancedEconomy"/>
    <Mid-level-ontology:economyType rdf:resource="#DevelopedCountry"/>
  </owl:Thing>

  <owl:Thing rdf:about="&Mid-level-ontology;Ireland">
    <Mid-level-ontology:economyType rdf:resource="#AdvancedEconomy"/>
    <Mid-level-ontology:economyType rdf:resource="#DevelopedCountry"/>
  </owl:Thing>

  <owl:Thing rdf:about="&Mid-level-ontology;Iron"/>
  <owl:Thing rdf:about="&Mid-level-ontology;Italy">
    <Mid-level-ontology:economyType rdf:resource="#AdvancedEconomy"/>
    <Mid-level-ontology:economyType rdf:resource="#DevelopedCountry"/>
  </owl:Thing>

  <owl:Thing rdf:about="&Mid-level-ontology;Japan">
    <Mid-level-ontology:economyType rdf:resource="#AdvancedEconomy"/>
    <Mid-level-ontology:economyType rdf:resource="#DevelopedCountry"/>
  </owl:Thing>

  <owl:Thing rdf:about="&Mid-level-ontology;Laos">
    <Mid-level-ontology:economyType rdf:resource="#DevelopingCountry"/>
    <Mid-level-ontology:economyType rdf:resource="#LessDevelopedCountry"/>
  </owl:Thing>

  <owl:Thing rdf:about="&Mid-level-ontology;Lead"/>
  <Mid-level-ontology:EconomicSystemAttribute rdf:about="&Mid-level-ontology;MarketEconomy">
    <rdfs:comment>MarketEconomy is an Attribute that 

describes an economy in which market forces, specifically supply and 

demand, provide input for privately managed decisions about pricing 

and production of goods.</rdfs:comment>
  </Mid-level-ontology:EconomicSystemAttribute>

  <owl:Thing rdf:about="&Mid-level-ontology;Mexico">
    <Mid-level-ontology:economyType rdf:resource="#DevelopedCountry"/>
    <Mid-level-ontology:economyType rdf:resource="#DevelopingCountry"/>
    <Mid-level-ontology:economyType rdf:resource="#LessDevelopedCountry"/>
  </owl:Thing>

  <Mid-level-ontology:EconomicSystemAttribute rdf:about="&Mid-level-ontology;MixedEconomy">
    <rdfs:comment>MixedEconomy is the Attribute 

of a country whose economy has elements of more than one pure 

economic system, e.g., a market economy with government welfare 

for unemployed workers.  A mixed-economy country may be a 

CountryInTransition, as from a prior communist economy to 

capitalism, but a mixed economy may also be a stable combination 

of different economic approaches in different areas of a national 

economy, e.g., nationally managed health care and education systems 

in an otherwise private-enterprise economy.</rdfs:comment>
  </Mid-level-ontology:EconomicSystemAttribute>

  <Mid-level-ontology:EconomicSystemAttribute rdf:about="&Mid-level-ontology;NationalizedIndustryEconomy">
    <SUMO:subAttribute rdf:resource="&Mid-level-ontology;GovernmentRegulatedEconomy"/>
    <rdfs:comment>NationalizedIndustryEconomy 

is an Attribute describing an economy in which the major industries,  

such as energy and transportation, are owned by the national government.</rdfs:comment>
  </Mid-level-ontology:EconomicSystemAttribute>

  <owl:Thing rdf:about="&Mid-level-ontology;Nitrogen"/>
  <owl:Thing rdf:about="&Mid-level-ontology;Poland">
    <Mid-level-ontology:economyType rdf:resource="#CountryInTransition"/>
  </owl:Thing>

  <Mid-level-ontology:EconomicSystemAttribute rdf:about="&Mid-level-ontology;PrivateEnterpriseEconomy">
    <SUMO:subAttribute rdf:resource="&Mid-level-ontology;CapitalistEconomy"/>
    <rdfs:comment>PrivateEnterpriseEconomy is 

the Attribute used to characterize a country in which private 

enterprise is the main source of economic wealth.</rdfs:comment>
  </Mid-level-ontology:EconomicSystemAttribute>

  <Mid-level-ontology:EconomicSystemAttribute rdf:about="&Mid-level-ontology;PrivatizingEconomy">
    <SUMO:subAttribute rdf:resource="&Mid-level-ontology;MixedEconomy"/>
    <rdfs:comment>PrivatizingEconomy is an 

Attribute that describes a country in which formerly government-

owned industries are being transferred into private holdings.</rdfs:comment>
  </Mid-level-ontology:EconomicSystemAttribute>

  <Mid-level-ontology:EconomicSystemAttribute rdf:about="&Mid-level-ontology;PureCapitalistEconomy">
    <SUMO:contraryAttribute rdf:resource="&Mid-level-ontology;MixedEconomy"/>
    <SUMO:subAttribute rdf:resource="&Mid-level-ontology;CapitalistEconomy"/>
    <rdfs:comment>PureCapitalistEconomy is an 

Attribute representing a capitalist economy that has no admixture of 

socialism.</rdfs:comment>
  </Mid-level-ontology:EconomicSystemAttribute>

  <Mid-level-ontology:EconomicSystemAttribute rdf:about="&Mid-level-ontology;PureSocialistEconomy">
    <SUMO:contraryAttribute rdf:resource="&Mid-level-ontology;MixedEconomy"/>
    <SUMO:contraryAttribute rdf:resource="&Mid-level-ontology;PureCapitalistEconomy"/>
    <SUMO:subAttribute rdf:resource="&Mid-level-ontology;SocialistEconomy"/>
    <rdfs:comment>PureSocialistEconomy is an 

Attribute representing a socialist economy that has no admixture of 

capitalism.</rdfs:comment>
  </Mid-level-ontology:EconomicSystemAttribute>

  <owl:Thing rdf:about="&Mid-level-ontology;RoadVehicle"/>
  <owl:Thing rdf:about="&Mid-level-ontology;Rock"/>
  <owl:Thing rdf:about="&Mid-level-ontology;Russia">
    <Mid-level-ontology:economyType rdf:resource="#CountryInTransition"/>
  </owl:Thing>

  <owl:Thing rdf:about="&Mid-level-ontology;Sand"/>
  <Mid-level-ontology:EconomicSystemAttribute rdf:about="&Mid-level-ontology;SocialistEconomy">
    <rdfs:comment>SocialistEconomy is the Attribute 

used to characterize a country in which there is government ownership 

or direction of the means of production and distribution.</rdfs:comment>
  </Mid-level-ontology:EconomicSystemAttribute>

  <owl:Thing rdf:about="&Mid-level-ontology;Sweden">
    <Mid-level-ontology:economyType rdf:resource="#AdvancedEconomy"/>
    <Mid-level-ontology:economyType rdf:resource="#DevelopedCountry"/>
  </owl:Thing>

  <owl:Thing rdf:about="&Mid-level-ontology;Switzerland">
    <Mid-level-ontology:economyType rdf:resource="#AdvancedEconomy"/>
    <Mid-level-ontology:economyType rdf:resource="#DevelopedCountry"/>
  </owl:Thing>

  <owl:Thing rdf:about="&Mid-level-ontology;Truck"/>
  <owl:Thing rdf:about="&Mid-level-ontology;UnitedKingdomOfGreatBritainAndNorthernIreland">
    <Mid-level-ontology:economyType rdf:resource="#AdvancedEconomy"/>
    <Mid-level-ontology:economyType rdf:resource="#DevelopedCountry"/>
  </owl:Thing>

  <owl:Thing rdf:about="&Mid-level-ontology;UnitedStates">
    <Mid-level-ontology:economyType rdf:resource="#AdvancedEconomy"/>
    <Mid-level-ontology:economyType rdf:resource="#DevelopedCountry"/>
  </owl:Thing>

  <Mid-level-ontology:EconomicSystemAttribute rdf:about="&Mid-level-ontology;WelfareCapitalism">
    <SUMO:subAttribute rdf:resource="&Mid-level-ontology;GovernmentSubsidizedEconomy"/>
    <SUMO:subAttribute rdf:resource="&Mid-level-ontology;MixedEconomy"/>
    <rdfs:comment>WelfareCapitalism is an Attribute 

describing an economy in which the government provides economic subsidies 

to unemployed or disabled individuals.</rdfs:comment>
  </Mid-level-ontology:EconomicSystemAttribute>

  <owl:Thing rdf:about="&Mid-level-ontology;Zinc"/>
  <owl:Thing rdf:about="&SUMO;Animal"/>
  <owl:Thing rdf:about="&SUMO;Communication"/>
  <owl:Thing rdf:about="&SUMO;Food"/>
  <owl:Thing rdf:about="&SUMO;Metal"/>
  <owl:Thing rdf:about="&SUMO;RecreationOrExercise"/>
  <owl:Thing rdf:about="&SUMO;TransportationDevice"/>
  <owl:Thing rdf:about="http://reliant.teknowledge.com/DAML/elements.owl#Aluminum"/>
  <owl:Thing rdf:about="http://reliant.teknowledge.com/DAML/elements.owl#Phosphorus"/>
</rdf:RDF>
