<?xml version="1.0"?>


<!DOCTYPE rdf:RDF [
    <!ENTITY sp "http://spinrdf.org/sp#" >
    <!ENTITY spin "http://spinrdf.org/spin#" >
    <!ENTITY sxml "http://topbraid.org/sxml#" >
    <!ENTITY owl "http://www.w3.org/2002/07/owl#" >
    <!ENTITY parties "http://www.fadyart.com/parties#" >
    <!ENTITY mic "http://www.fadyart.com/markets#" >
    <!ENTITY swrl "http://www.w3.org/2003/11/swrl#" >
    <!ENTITY dc "http://purl.org/dc/elements/1.1/" >
    <!ENTITY swrlb "http://www.w3.org/2003/11/swrlb#" >
    <!ENTITY ctry "http://www.fadyart.com/countries#" >
    <!ENTITY xsd "http://www.w3.org/2001/XMLSchema#" >
    <!ENTITY isic "http://www.fadyart.com/activities#" >
    <!ENTITY owl2xml "http://www.w3.org/2006/12/owl2-xml#" >
    <!ENTITY iso20022 "http://www.fadyart.com/iso20022.owl#" >
    <!ENTITY rdfs "http://www.w3.org/2000/01/rdf-schema#" >
    <!ENTITY rdf "http://www.w3.org/1999/02/22-rdf-syntax-ns#" >
    <!ENTITY fi "http://www.fadyart.com/financialInstruments#" >
    <!ENTITY protege "http://protege.stanford.edu/plugins/owl/protege#" >
    <!ENTITY xsp "http://www.owl-ontologies.com/2005/08/07/xsp.owl#" >
]>


<rdf:RDF xmlns="http://www.fadyart.com/Finance.owl#"
     xml:base="http://www.fadyart.com/Finance.owl"
     xmlns:dc="http://purl.org/dc/elements/1.1/"
     xmlns:protege="http://protege.stanford.edu/plugins/owl/protege#"
     xmlns:sp="http://spinrdf.org/sp#"
     xmlns:xsp="http://www.owl-ontologies.com/2005/08/07/xsp.owl#"
     xmlns:rdfs="http://www.w3.org/2000/01/rdf-schema#"
     xmlns:swrl="http://www.w3.org/2003/11/swrl#"
     xmlns:owl2xml="http://www.w3.org/2006/12/owl2-xml#"
     xmlns:mic="http://www.fadyart.com/markets#"
     xmlns:iso20022="http://www.fadyart.com/iso20022.owl#"
     xmlns:isic="http://www.fadyart.com/activities#"
     xmlns:parties="http://www.fadyart.com/parties#"
     xmlns:fi="http://www.fadyart.com/financialInstruments#"
     xmlns:sxml="http://topbraid.org/sxml#"
     xmlns:swrlb="http://www.w3.org/2003/11/swrlb#"
     xmlns:owl="http://www.w3.org/2002/07/owl#"
     xmlns:xsd="http://www.w3.org/2001/XMLSchema#"
     xmlns:rdf="http://www.w3.org/1999/02/22-rdf-syntax-ns#"
     xmlns:spin="http://spinrdf.org/spin#"
     xmlns:ctry="http://www.fadyart.com/countries#">
    <owl:Ontology rdf:about="http://www.fadyart.com/Finance.owl">
        <rdfs:label rdf:datatype="&xsd;string">Finance</rdfs:label>
        <rdfs:label xml:lang="en">Finance</rdfs:label>
        <dc:rights rdf:datatype="&xsd;string">All rights reserved by Eddy Vanderlinden - Rietlaan 79 - B-8200 Bruges.
Free for non-commercial usage.</dc:rights>
        <rdfs:seeAlso rdf:datatype="&xsd;anyURI">http://fadyart.com/</rdfs:seeAlso>
        <owl:priorVersion xml:lang="en">3.02 Federated ontology with parties as new federation
3.01 Federated ontology including part of iso20022
3.00 Client acceptance processes
2.02 Commented relations
2.01 Referential systems
2.00 Risk monitoring
1.02 Financial instruments including credit rating information.
1.01 Financial instruments including ISO and ISIC codes
1.00 Financial instruments</owl:priorVersion>
        <owl:versionInfo xml:lang="en">3.03 Federated ontology with &apos;financial instruments&apos; as new federation</owl:versionInfo>
        <rdfs:isDefinedBy xml:lang="en">Eddy Vanderlinden
Rietlaan 79
8200 Sint-Michiels (Bruges)
Belgium

info@fadyart.com</rdfs:isDefinedBy>
        <rdfs:comment xml:lang="en">Securities handling ontology.

Construction phase 5: processes and procedures

All rights reserved.
Usage free for non-commercial purposes.</rdfs:comment>
        <owl:imports rdf:resource="http://fadyart.com/financialInstruments"/>
        <owl:imports rdf:resource="http://spinrdf.org/spin"/>
        <owl:imports rdf:resource="http://www.fadyart.com/countries"/>
        <owl:imports rdf:resource="http://www.fadyart.com/currencies"/>
        <owl:imports rdf:resource="http://www.fadyart.com/iso20022.owl"/>
        <owl:imports rdf:resource="http://www.fadyart.com/markets"/>
        <owl:imports rdf:resource="http://www.fadyart.com/parties"/>
        <owl:incompatibleWith rdf:resource="http://www.fadyart.com/ontologies/data/Finance.owl"/>
    </owl:Ontology>
    


    <!-- 
    ///////////////////////////////////////////////////////////////////////////////////////
    //
    // Annotation properties
    //
    ///////////////////////////////////////////////////////////////////////////////////////
     -->

    


    <!-- http://purl.org/dc/elements/1.1/creator -->

    <owl:AnnotationProperty rdf:about="&dc;creator"/>
    


    <!-- http://purl.org/dc/elements/1.1/rights -->

    <owl:AnnotationProperty rdf:about="&dc;rights"/>
    


    <!-- http://purl.org/dc/elements/1.1/source -->

    <owl:AnnotationProperty rdf:about="&dc;source"/>
    


    <!-- 
    ///////////////////////////////////////////////////////////////////////////////////////
    //
    // Object Properties
    //
    ///////////////////////////////////////////////////////////////////////////////////////
     -->

    


    <!-- http://www.fadyart.com/Finance.owl#concernsFinancialInstrument -->

    <owl:ObjectProperty rdf:about="http://www.fadyart.com/Finance.owl#concernsFinancialInstrument">
        <rdfs:comment xml:lang="en">The right side of the relation concerns the financial instrument where-off the position is registered. This is represented through an individual of the class FinancialInstrument</rdfs:comment>
        <rdfs:domain rdf:resource="http://www.fadyart.com/Finance.owl#BalanceSheet"/>
        <rdfs:range rdf:resource="http://www.fadyart.com/Finance.owl#FinancialInstrument"/>
        <rdfs:subPropertyOf rdf:resource="http://www.fadyart.com/Finance.owl#hasPositionRelation"/>
    </owl:ObjectProperty>
    


    <!-- http://www.fadyart.com/Finance.owl#hasAccessToChannel -->

    <owl:ObjectProperty rdf:about="http://www.fadyart.com/Finance.owl#hasAccessToChannel">
        <rdfs:comment xml:lang="en">The organisational entity has access to channels represented by instances of the class ValuePartition - AdministrationChannel</rdfs:comment>
        <rdfs:range rdf:resource="http://www.fadyart.com/Finance.owl#AdministrationChannel"/>
        <rdfs:domain rdf:resource="http://www.fadyart.com/Finance.owl#Organization"/>
    </owl:ObjectProperty>
    


    <!-- http://www.fadyart.com/Finance.owl#hasAccountDomain -->

    <owl:ObjectProperty rdf:about="http://www.fadyart.com/Finance.owl#hasAccountDomain">
        <rdfs:comment xml:lang="en">The left hand side of the relation has individuals of the class Account as role, the right hand side refers to individuals of other classes.</rdfs:comment>
        <rdfs:domain rdf:resource="http://www.fadyart.com/Finance.owl#Account"/>
    </owl:ObjectProperty>
    


    <!-- http://www.fadyart.com/Finance.owl#hasAccountRestrictionReason -->

    <owl:ObjectProperty rdf:about="http://www.fadyart.com/Finance.owl#hasAccountRestrictionReason">
        <rdfs:comment xml:lang="en">Client accounts, Nostro or Vostro accounts as well as the principal&apos;s general ledger accounts can be restricted for many reasons. These possible reasons are found as individuals of the class ValuePartition - AccountValues - ReasonForAccountFreeze</rdfs:comment>
        <rdfs:comment xml:lang="en">The reason for restriction of the account management or disposal of the deposits</rdfs:comment>
        <rdfs:domain rdf:resource="http://www.fadyart.com/Finance.owl#BalanceSheet"/>
        <rdfs:range rdf:resource="http://www.fadyart.com/Finance.owl#ReasonForAccountFreeze"/>
        <rdfs:subPropertyOf rdf:resource="http://www.fadyart.com/Finance.owl#hasAccountDomain"/>
    </owl:ObjectProperty>
    


    <!-- http://www.fadyart.com/Finance.owl#hasAsFiscalResident -->

    <owl:ObjectProperty rdf:about="http://www.fadyart.com/Finance.owl#hasAsFiscalResident">
        <rdf:type rdf:resource="&owl;InverseFunctionalProperty"/>
        <rdfs:range rdf:resource="http://www.fadyart.com/Finance.owl#InvolvedParty"/>
        <rdfs:subPropertyOf rdf:resource="http://www.fadyart.com/Finance.owl#hasValuePartitionDomain"/>
        <rdfs:domain rdf:resource="&ctry;ISO3166-CountryCode"/>
    </owl:ObjectProperty>
    


    <!-- http://www.fadyart.com/Finance.owl#hasAsLegalResident -->

    <owl:ObjectProperty rdf:about="http://www.fadyart.com/Finance.owl#hasAsLegalResident">
        <rdf:type rdf:resource="&owl;InverseFunctionalProperty"/>
        <rdfs:range rdf:resource="http://www.fadyart.com/Finance.owl#InvolvedParty"/>
        <rdfs:subPropertyOf rdf:resource="http://www.fadyart.com/Finance.owl#hasValuePartitionDomain"/>
        <rdfs:domain rdf:resource="&ctry;ISO3166-CountryCode"/>
    </owl:ObjectProperty>
    


    <!-- http://www.fadyart.com/Finance.owl#hasAsNationalBank -->

    <owl:ObjectProperty rdf:about="http://www.fadyart.com/Finance.owl#hasAsNationalBank">
        <rdfs:subPropertyOf rdf:resource="http://www.fadyart.com/Finance.owl#hasValuePartitionDomain"/>
        <rdfs:domain rdf:resource="&ctry;ISO3166-CountryCode"/>
        <rdfs:range rdf:resource="&fi;NationalBank"/>
    </owl:ObjectProperty>
    


    <!-- http://www.fadyart.com/Finance.owl#hasAsPrincipal -->

    <owl:ObjectProperty rdf:about="http://www.fadyart.com/Finance.owl#hasAsPrincipal">
        <rdf:type rdf:resource="&owl;FunctionalProperty"/>
        <rdfs:comment xml:lang="en">A property of the Account class is the principal for whom the accounts are kept. The reference to the possible principals is found in Party-PartyPrincipal.</rdfs:comment>
        <rdfs:comment xml:lang="en">The party for who&apos;s account and eventually in who&apos;s name securities handling services are performed.</rdfs:comment>
        <rdfs:domain rdf:resource="http://www.fadyart.com/Finance.owl#Account"/>
        <rdfs:subPropertyOf rdf:resource="http://www.fadyart.com/Finance.owl#hasAccountDomain"/>
        <rdfs:range rdf:resource="&parties;Party"/>
        <owl:inverseOf rdf:resource="&parties;isPrincipalOf"/>
    </owl:ObjectProperty>
    


    <!-- http://www.fadyart.com/Finance.owl#hasAuthorizedPartyForDisposal -->

    <owl:ObjectProperty rdf:about="http://www.fadyart.com/Finance.owl#hasAuthorizedPartyForDisposal">
        <rdfs:label xml:lang="en">Client Authorization to dispose of the holdings</rdfs:label>
        <rdfs:comment xml:lang="en">Authorization to dispose over the account&apos;s holdings.
The authorized person is allowed to transfer holdings to third party and to his own accounts. 
Only client accounts are involved in thie left side of the relation.
The reference to authorized party individuals is found in class Party - PartyClientArrangement - PartyAuthorizedPerson.</rdfs:comment>
        <rdfs:domain rdf:resource="http://www.fadyart.com/Finance.owl#YearlyAccount"/>
        <rdfs:subPropertyOf rdf:resource="http://www.fadyart.com/Finance.owl#hasAccountDomain"/>
        <rdfs:range rdf:resource="&parties;IndividualPerson"/>
    </owl:ObjectProperty>
    


    <!-- http://www.fadyart.com/Finance.owl#hasAuthorizedPartyForManagement -->

    <owl:ObjectProperty rdf:about="http://www.fadyart.com/Finance.owl#hasAuthorizedPartyForManagement">
        <rdfs:label xml:lang="en">Client organization to manage the holdings</rdfs:label>
        <rdfs:comment xml:lang="en">Authorization to manage the client&apos;s holdings.
The authorized person is not allowed to transfer holdings to third party or to his own accounts.
The involved left hand side can be a client account, a NOSTO or VOSTRO account or a principal&apos;s general ledger account.
The reference to authorized party individuals is found in class Party - PartyClientArrangement - PartyAuthorizedPerson.</rdfs:comment>
        <rdfs:domain rdf:resource="http://www.fadyart.com/Finance.owl#YearlyAccount"/>
        <rdfs:subPropertyOf rdf:resource="http://www.fadyart.com/Finance.owl#hasAccountDomain"/>
        <rdfs:range rdf:resource="&parties;IndividualPerson"/>
    </owl:ObjectProperty>
    


    <!-- http://www.fadyart.com/Finance.owl#hasClientPortfolioBeneficialOwnerCapital -->

    <owl:ObjectProperty rdf:about="http://www.fadyart.com/Finance.owl#hasClientPortfolioBeneficialOwnerCapital">
        <rdfs:comment xml:lang="en">Points to the parties beneficial owners of the capital.</rdfs:comment>
        <rdfs:comment xml:lang="en">The reference to beneficial owners capital of the financial instruments deposited in account is found in the individuals of class Party - PartyClientArrangement - PartyHolder</rdfs:comment>
        <rdfs:domain rdf:resource="http://www.fadyart.com/Finance.owl#ClientPortfolio"/>
        <rdfs:subPropertyOf rdf:resource="http://www.fadyart.com/Finance.owl#hasAccountDomain"/>
        <rdfs:range rdf:resource="&parties;Party"/>
    </owl:ObjectProperty>
    


    <!-- http://www.fadyart.com/Finance.owl#hasClientPortfolioBeneficialOwnerIncome -->

    <owl:ObjectProperty rdf:about="http://www.fadyart.com/Finance.owl#hasClientPortfolioBeneficialOwnerIncome">
        <rdfs:label xml:lang="en">Points to the parties beneficial owner of the income</rdfs:label>
        <rdfs:comment xml:lang="en">In some countries the parents have the legal usufructuary of the income of their children.
The reference to beneficial owners capital of the financial instruments deposited in account is found in the individuals of class Party - PartyClientArrangement - PartyHolder or PartyUsufructuary or PartyLegalRepresentative</rdfs:comment>
        <rdfs:domain rdf:resource="http://www.fadyart.com/Finance.owl#ClientPortfolio"/>
        <rdfs:subPropertyOf rdf:resource="http://www.fadyart.com/Finance.owl#hasAccountDomain"/>
    </owl:ObjectProperty>
    


    <!-- http://www.fadyart.com/Finance.owl#hasContactPerson -->

    <owl:ObjectProperty rdf:about="http://www.fadyart.com/Finance.owl#hasContactPerson">
        <rdfs:label xml:lang="en">Points to the contactperson who&apos;s contact information contains the communication modalities</rdfs:label>
        <rdfs:comment xml:lang="en">The person appointed as contact according the modalities found in the contact class.
The reference to the individual contact persons is found in class Party, any subclass included.</rdfs:comment>
        <rdfs:domain rdf:resource="http://www.fadyart.com/Finance.owl#Account"/>
        <rdfs:range rdf:resource="http://www.fadyart.com/Finance.owl#InvolvedParty"/>
        <rdfs:subPropertyOf rdf:resource="http://www.fadyart.com/Finance.owl#hasAccountDomain"/>
    </owl:ObjectProperty>
    


    <!-- http://www.fadyart.com/Finance.owl#hasPositionRelation -->

    <owl:ObjectProperty rdf:about="http://www.fadyart.com/Finance.owl#hasPositionRelation">
        <rdfs:comment xml:lang="en">The left hand side of the relation has individuals of the classes VostroAccountPosition, ClientAccountPosition and NostroAccountPosition as role, the right hand side refers to individuals of other classes.</rdfs:comment>
        <rdfs:domain rdf:resource="http://www.fadyart.com/Finance.owl#BalanceSheet"/>
        <rdfs:subPropertyOf rdf:resource="http://www.fadyart.com/Finance.owl#hasAccountDomain"/>
    </owl:ObjectProperty>
    


    <!-- http://www.fadyart.com/Finance.owl#hasProfileValidityPeriod -->

    <owl:ObjectProperty rdf:about="http://www.fadyart.com/Finance.owl#hasProfileValidityPeriod">
        <rdfs:label xml:lang="en">The period during which the risk profile is valid</rdfs:label>
        <rdfs:comment xml:lang="en">The period during which the risk profile is valid is found in individuals of class Temporal - ValidTime - ValidPeriod</rdfs:comment>
        <rdfs:domain rdf:resource="http://www.fadyart.com/Finance.owl#RiskProfile"/>
        <rdfs:range rdf:resource="http://www.fadyart.com/Finance.owl#ValidPeriod"/>
        <rdfs:subPropertyOf rdf:resource="http://www.fadyart.com/Finance.owl#hasRiskProfileDomain"/>
    </owl:ObjectProperty>
    


    <!-- http://www.fadyart.com/Finance.owl#hasRestrictionReason -->

    <owl:ObjectProperty rdf:about="http://www.fadyart.com/Finance.owl#hasRestrictionReason">
        <rdfs:label xml:lang="en">Reason for which a position is frozen</rdfs:label>
        <rdfs:comment xml:lang="en">Each position in the principal&apos;s customer account can be frozen for different reasons. Those reasons are found as individuals of the class ValuePartition - ReasonForPositionFreeze</rdfs:comment>
        <rdfs:domain rdf:resource="http://www.fadyart.com/Finance.owl#BalanceSheet"/>
        <rdfs:range rdf:resource="http://www.fadyart.com/Finance.owl#ReasonForPositionFreeze"/>
        <rdfs:subPropertyOf rdf:resource="http://www.fadyart.com/Finance.owl#hasPositionRelation"/>
    </owl:ObjectProperty>
    


    <!-- http://www.fadyart.com/Finance.owl#hasRiskArea -->

    <owl:ObjectProperty rdf:about="http://www.fadyart.com/Finance.owl#hasRiskArea">
        <rdfs:comment xml:lang="en">The area where the risk finds his source through reference to individuals of: parties, countries, activity sectors,...</rdfs:comment>
        <rdfs:domain rdf:resource="http://www.fadyart.com/Finance.owl#RiskProfile"/>
        <rdfs:subPropertyOf rdf:resource="http://www.fadyart.com/Finance.owl#hasRiskProfileDomain"/>
    </owl:ObjectProperty>
    


    <!-- http://www.fadyart.com/Finance.owl#hasRiskImpact -->

    <owl:ObjectProperty rdf:about="http://www.fadyart.com/Finance.owl#hasRiskImpact">
        <rdfs:comment xml:lang="en">The risk impact evaluation of the risk profile through reference to members of class Risk - ExternalRisk - ImpactOfRiskOccurence</rdfs:comment>
        <rdfs:range rdf:resource="http://www.fadyart.com/Finance.owl#ImpactOfRiskOccurence"/>
        <rdfs:domain rdf:resource="http://www.fadyart.com/Finance.owl#RiskProfile"/>
        <rdfs:subPropertyOf rdf:resource="http://www.fadyart.com/Finance.owl#hasRiskProfileDomain"/>
    </owl:ObjectProperty>
    


    <!-- http://www.fadyart.com/Finance.owl#hasRiskProbability -->

    <owl:ObjectProperty rdf:about="http://www.fadyart.com/Finance.owl#hasRiskProbability">
        <rdfs:comment xml:lang="en">The probability of the risk occuring through refence to individuals of class Risk - ExternalRisk - ProbabilityOfiskOccurance</rdfs:comment>
        <rdfs:range rdf:resource="http://www.fadyart.com/Finance.owl#ProbabilityOfRiskOccurence"/>
        <rdfs:domain rdf:resource="http://www.fadyart.com/Finance.owl#RiskProfile"/>
        <rdfs:subPropertyOf rdf:resource="http://www.fadyart.com/Finance.owl#hasRiskProfileDomain"/>
    </owl:ObjectProperty>
    


    <!-- http://www.fadyart.com/Finance.owl#hasRiskProfileDomain -->

    <owl:ObjectProperty rdf:about="http://www.fadyart.com/Finance.owl#hasRiskProfileDomain">
        <rdfs:comment xml:lang="en">The left side of the relations are individuals of class Risk - ExternalRisk - RiskProfile</rdfs:comment>
        <rdfs:domain rdf:resource="http://www.fadyart.com/Finance.owl#RiskProfile"/>
    </owl:ObjectProperty>
    


    <!-- http://www.fadyart.com/Finance.owl#hasRiskSymptom -->

    <owl:ObjectProperty rdf:about="http://www.fadyart.com/Finance.owl#hasRiskSymptom">
        <rdfs:comment xml:lang="en">The symptoms of the existance of the risk through refence to individuals of class Risk - ExternalRisk-RiskSymptom</rdfs:comment>
        <rdfs:domain rdf:resource="http://www.fadyart.com/Finance.owl#RiskProfile"/>
        <rdfs:range rdf:resource="http://www.fadyart.com/Finance.owl#RiskSymptom"/>
        <rdfs:subPropertyOf rdf:resource="http://www.fadyart.com/Finance.owl#hasRiskProfileDomain"/>
    </owl:ObjectProperty>
    


    <!-- http://www.fadyart.com/Finance.owl#hasTemporalDomain -->

    <owl:ObjectProperty rdf:about="http://www.fadyart.com/Finance.owl#hasTemporalDomain">
        <rdfs:comment xml:lang="en">The domain of the underlying relations is Temporal or a subclass of Temporal</rdfs:comment>
        <rdfs:domain rdf:resource="http://www.fadyart.com/Finance.owl#Temporal"/>
    </owl:ObjectProperty>
    


    <!-- http://www.fadyart.com/Finance.owl#hasTemporalRangeRelation -->

    <owl:ObjectProperty rdf:about="http://www.fadyart.com/Finance.owl#hasTemporalRangeRelation">
        <rdfs:comment xml:lang="en">The right hand of the relation has individuals of the class Temporal as role, the left hand side refers to individuals of other classes.</rdfs:comment>
        <rdfs:range rdf:resource="http://www.fadyart.com/Finance.owl#Temporal"/>
    </owl:ObjectProperty>
    


    <!-- http://www.fadyart.com/Finance.owl#hasTimeGranularity -->

    <owl:ObjectProperty rdf:about="http://www.fadyart.com/Finance.owl#hasTimeGranularity">
        <rdfs:comment xml:lang="en">The width of the time slices is found as individuals of class Temporal - Granularity</rdfs:comment>
        <rdfs:range rdf:resource="http://www.fadyart.com/Finance.owl#Granularity"/>
        <rdfs:domain rdf:resource="http://www.fadyart.com/Finance.owl#ValidTime"/>
        <rdfs:subPropertyOf rdf:resource="http://www.fadyart.com/Finance.owl#hasTemporalDomain"/>
    </owl:ObjectProperty>
    


    <!-- http://www.fadyart.com/Finance.owl#hasValidTime -->

    <owl:ObjectProperty rdf:about="http://www.fadyart.com/Finance.owl#hasValidTime">
        <rdfs:domain rdf:resource="http://www.fadyart.com/Finance.owl#ExtendedProposition"/>
        <rdfs:range rdf:resource="http://www.fadyart.com/Finance.owl#ValidTime"/>
        <rdfs:subPropertyOf rdf:resource="http://www.fadyart.com/Finance.owl#hasTemporalDomain"/>
    </owl:ObjectProperty>
    


    <!-- http://www.fadyart.com/Finance.owl#hasValidityInstant -->

    <owl:ObjectProperty rdf:about="http://www.fadyart.com/Finance.owl#hasValidityInstant">
        <rdfs:comment xml:lang="en">The instant at which the information on the individual is valid.
Reference to the validity instant is found in class Temporal - ValidTime - ValidInstant</rdfs:comment>
        <rdfs:range rdf:resource="http://www.fadyart.com/Finance.owl#ValidInstant"/>
        <rdfs:subPropertyOf rdf:resource="http://www.fadyart.com/Finance.owl#hasTemporalRangeRelation"/>
    </owl:ObjectProperty>
    


    <!-- http://www.fadyart.com/Finance.owl#hasValidityPeriod -->

    <owl:ObjectProperty rdf:about="http://www.fadyart.com/Finance.owl#hasValidityPeriod">
        <rdfs:comment xml:lang="en">The period for which the information on the individual is valid.
Reference to the validity period is found in class Temporal - ValidTime - ValidPeriod</rdfs:comment>
        <rdfs:range rdf:resource="http://www.fadyart.com/Finance.owl#ValidPeriod"/>
        <rdfs:subPropertyOf rdf:resource="http://www.fadyart.com/Finance.owl#hasTemporalRangeRelation"/>
    </owl:ObjectProperty>
    


    <!-- http://www.fadyart.com/Finance.owl#hasValuationMarket -->

    <owl:ObjectProperty rdf:about="http://www.fadyart.com/Finance.owl#hasValuationMarket">
        <rdfs:label xml:lang="en">The market on which a valuation took place.</rdfs:label>
        <rdfs:comment xml:lang="en">The market where the valuation occured is referenced by individuals of class ValuePartition - ISO codes - ISO10383-Market IdentifierCodes.</rdfs:comment>
        <rdfs:domain rdf:resource="http://www.fadyart.com/Finance.owl#BalanceSheet"/>
        <rdfs:subPropertyOf rdf:resource="http://www.fadyart.com/Finance.owl#hasPositionRelation"/>
        <rdfs:range rdf:resource="&mic;ISO10383-MarketIdentifierCodes"/>
    </owl:ObjectProperty>
    


    <!-- http://www.fadyart.com/Finance.owl#hasValuationTime -->

    <owl:ObjectProperty rdf:about="http://www.fadyart.com/Finance.owl#hasValuationTime">
        <rdfs:comment xml:lang="en">The time at which the left hand side position is valuated.
Reference is made to individuals of class Temporal - ValidTime - ValidInstant.</rdfs:comment>
        <rdfs:domain rdf:resource="http://www.fadyart.com/Finance.owl#BalanceSheet"/>
        <rdfs:range rdf:resource="http://www.fadyart.com/Finance.owl#ValidInstant"/>
        <rdfs:subPropertyOf rdf:resource="http://www.fadyart.com/Finance.owl#hasPositionRelation"/>
    </owl:ObjectProperty>
    


    <!-- http://www.fadyart.com/Finance.owl#hasValuePartitionDomain -->

    <owl:ObjectProperty rdf:about="http://www.fadyart.com/Finance.owl#hasValuePartitionDomain">
        <rdfs:domain rdf:resource="http://www.fadyart.com/Finance.owl#ValuePartition"/>
    </owl:ObjectProperty>
    


    <!-- http://www.fadyart.com/Finance.owl#hasXNStatus -->

    <owl:ObjectProperty rdf:about="http://www.fadyart.com/Finance.owl#hasXNStatus"/>
    


    <!-- http://www.fadyart.com/Finance.owl#isAccessibleViaChannel -->

    <owl:ObjectProperty rdf:about="http://www.fadyart.com/Finance.owl#isAccessibleViaChannel">
        <rdfs:label xml:lang="en">The channels through which the accounts can be managed</rdfs:label>
        <rdfs:comment xml:lang="en">The accounts are managed through the channels corresponding to the individuals of the class ValuePartition - AdministrationChannel</rdfs:comment>
        <rdfs:domain rdf:resource="http://www.fadyart.com/Finance.owl#Account"/>
        <rdfs:range rdf:resource="http://www.fadyart.com/Finance.owl#AdministrationChannel"/>
        <rdfs:subPropertyOf rdf:resource="http://www.fadyart.com/Finance.owl#hasAccountDomain"/>
    </owl:ObjectProperty>
    


    <!-- http://www.fadyart.com/Finance.owl#isKeptAtCustodian -->

    <owl:ObjectProperty rdf:about="http://www.fadyart.com/Finance.owl#isKeptAtCustodian">
        <rdfs:comment xml:lang="en">The right side of the relation consists of individuals of the class Party - PartyCustodian</rdfs:comment>
        <rdfs:domain rdf:resource="http://www.fadyart.com/Finance.owl#BalanceSheet"/>
        <rdfs:subPropertyOf rdf:resource="http://www.fadyart.com/Finance.owl#hasPositionRelation"/>
        <rdfs:range rdf:resource="&parties;Organisation"/>
    </owl:ObjectProperty>
    


    <!-- http://www.fadyart.com/Finance.owl#isNationalBankFor -->

    <owl:ObjectProperty rdf:about="http://www.fadyart.com/Finance.owl#isNationalBankFor">
        <owl:inverseOf rdf:resource="http://www.fadyart.com/Finance.owl#hasAsNationalBank"/>
        <rdfs:subPropertyOf rdf:resource="http://www.fadyart.com/Finance.owl#hasValuePartitionDomain"/>
        <rdfs:range rdf:resource="&ctry;ISO3166-CountryCode"/>
        <rdfs:domain rdf:resource="&fi;NationalBank"/>
    </owl:ObjectProperty>
    


    <!-- http://www.fadyart.com/Finance.owl#isTriggerFor -->

    <owl:ObjectProperty rdf:about="http://www.fadyart.com/Finance.owl#isTriggerFor">
        <rdfs:comment xml:lang="en">The values are trigger for the procedure steps of pocesses specified on the right side: ProcessAndProcedure</rdfs:comment>
        <rdfs:range rdf:resource="http://www.fadyart.com/Finance.owl#ProcessAndProcedure"/>
        <rdfs:domain rdf:resource="http://www.fadyart.com/Finance.owl#ProcessTrigger"/>
        <rdfs:subPropertyOf rdf:resource="http://www.fadyart.com/Finance.owl#hasValuePartitionDomain"/>
    </owl:ObjectProperty>
    


    <!-- http://www.fadyart.com/parties#isPrincipalOf -->

    <rdf:Description rdf:about="&parties;isPrincipalOf"/>
    


    <!-- 
    ///////////////////////////////////////////////////////////////////////////////////////
    //
    // Data properties
    //
    ///////////////////////////////////////////////////////////////////////////////////////
     -->

    


    <!-- http://www.fadyart.com/Finance.owl#hasAddress -->

    <owl:DatatypeProperty rdf:about="http://www.fadyart.com/Finance.owl#hasAddress">
        <rdfs:comment xml:lang="en">The value of the address.</rdfs:comment>
        <rdfs:subPropertyOf rdf:resource="http://www.fadyart.com/Finance.owl#hasContactDomainForData"/>
        <rdfs:domain rdf:resource="&parties;Contact"/>
    </owl:DatatypeProperty>
    


    <!-- http://www.fadyart.com/Finance.owl#hasContactDomainForData -->

    <owl:DatatypeProperty rdf:about="http://www.fadyart.com/Finance.owl#hasContactDomainForData">
        <rdfs:comment xml:lang="en">The left hand of the relation has individuals of the class Contact as role, the right hand side refers to literal values.</rdfs:comment>
        <rdfs:domain rdf:resource="&parties;Contact"/>
    </owl:DatatypeProperty>
    


    <!-- http://www.fadyart.com/Finance.owl#hasFinishTime -->

    <owl:DatatypeProperty rdf:about="http://www.fadyart.com/Finance.owl#hasFinishTime">
        <rdf:type rdf:resource="&owl;FunctionalProperty"/>
        <rdfs:comment xml:lang="en">The end date and time of the period</rdfs:comment>
        <rdfs:domain rdf:resource="http://www.fadyart.com/Finance.owl#ValidPeriod"/>
        <rdfs:subPropertyOf rdf:resource="http://www.fadyart.com/Finance.owl#hasTemporalDomainForData"/>
        <rdfs:range rdf:resource="&xsd;dateTime"/>
    </owl:DatatypeProperty>
    


    <!-- http://www.fadyart.com/Finance.owl#hasInterval -->

    <owl:DatatypeProperty rdf:about="http://www.fadyart.com/Finance.owl#hasInterval">
        <rdfs:comment xml:lang="en">The interval according which documents are produced and sent to the indicated address. The granularity of the interval is a separate object property, part of contact.</rdfs:comment>
        <rdfs:subPropertyOf rdf:resource="http://www.fadyart.com/Finance.owl#hasContactDomainForData"/>
        <rdfs:domain rdf:resource="&parties;Contact"/>
    </owl:DatatypeProperty>
    


    <!-- http://www.fadyart.com/Finance.owl#hasPositionDomain -->

    <owl:DatatypeProperty rdf:about="http://www.fadyart.com/Finance.owl#hasPositionDomain">
        <rdfs:comment xml:lang="en">The left side of the relations will be Nostro-, Vostro- and  ClientAccountPosition</rdfs:comment>
    </owl:DatatypeProperty>
    


    <!-- http://www.fadyart.com/Finance.owl#hasRiskSymptomSource -->

    <owl:DatatypeProperty rdf:about="http://www.fadyart.com/Finance.owl#hasRiskSymptomSource">
        <rdfs:comment xml:lang="en">The source, communicataion, publication,... on basis of which the existance of the symptom is reported.</rdfs:comment>
        <rdfs:domain rdf:resource="http://www.fadyart.com/Finance.owl#RiskProfile"/>
    </owl:DatatypeProperty>
    


    <!-- http://www.fadyart.com/Finance.owl#hasStartTime -->

    <owl:DatatypeProperty rdf:about="http://www.fadyart.com/Finance.owl#hasStartTime">
        <rdf:type rdf:resource="&owl;FunctionalProperty"/>
        <rdfs:comment xml:lang="en">The start date and time of the period.</rdfs:comment>
        <rdfs:domain rdf:resource="http://www.fadyart.com/Finance.owl#ValidPeriod"/>
        <rdfs:subPropertyOf rdf:resource="http://www.fadyart.com/Finance.owl#hasTemporalDomainForData"/>
        <rdfs:range rdf:resource="&xsd;dateTime"/>
    </owl:DatatypeProperty>
    


    <!-- http://www.fadyart.com/Finance.owl#hasStatisticalReportingCode -->

    <owl:DatatypeProperty rdf:about="http://www.fadyart.com/Finance.owl#hasStatisticalReportingCode">
        <rdf:type rdf:resource="&owl;FunctionalProperty"/>
        <rdfs:comment xml:lang="en">Lots of reporting is done to the national authorities where the principal is situated. Example the National benk for statistical reporting.
The rubriques in the reporting correspond to the present code.</rdfs:comment>
        <rdfs:domain rdf:resource="http://www.fadyart.com/Finance.owl#ClientPortfolio"/>
    </owl:DatatypeProperty>
    


    <!-- http://www.fadyart.com/Finance.owl#hasTemporalDomainForData -->

    <owl:DatatypeProperty rdf:about="http://www.fadyart.com/Finance.owl#hasTemporalDomainForData">
        <rdfs:comment xml:lang="en">Data property relations with Temporal individuals on their left side</rdfs:comment>
        <rdfs:domain rdf:resource="http://www.fadyart.com/Finance.owl#Temporal"/>
    </owl:DatatypeProperty>
    


    <!-- http://www.fadyart.com/Finance.owl#hasTime -->

    <owl:DatatypeProperty rdf:about="http://www.fadyart.com/Finance.owl#hasTime">
        <rdf:type rdf:resource="&owl;FunctionalProperty"/>
        <rdfs:comment xml:lang="en">The date and time identifying the instant.</rdfs:comment>
        <rdfs:domain rdf:resource="http://www.fadyart.com/Finance.owl#ValidInstant"/>
        <rdfs:subPropertyOf rdf:resource="http://www.fadyart.com/Finance.owl#hasTemporalDomainForData"/>
        <rdfs:range rdf:resource="&xsd;dateTime"/>
    </owl:DatatypeProperty>
    


    <!-- 
    ///////////////////////////////////////////////////////////////////////////////////////
    //
    // Classes
    //
    ///////////////////////////////////////////////////////////////////////////////////////
     -->

    


    <!-- http://spinrdf.org/sp#Select -->

    <rdf:Description rdf:about="&sp;Select">
        <spin:constraint rdf:resource="http://www.fadyart.com/Finance.owl#UsedCountriesAsFiscalResidence"/>
    </rdf:Description>
    


    <!-- http://www.fadyart.com/Finance.owl#Account -->

    <owl:Class rdf:about="http://www.fadyart.com/Finance.owl#Account">
        <rdfs:label xml:lang="en">Account</rdfs:label>
        <rdfs:comment xml:lang="en">Register of financial transactions.</rdfs:comment>
    </owl:Class>
    


    <!-- http://www.fadyart.com/Finance.owl#AccountComments -->

    <owl:Class rdf:about="http://www.fadyart.com/Finance.owl#AccountComments">
        <rdfs:label xml:lang="en">Comments to the yearly accounts</rdfs:label>
        <rdfs:subClassOf rdf:resource="http://www.fadyart.com/Finance.owl#YearlyAccount"/>
        <rdfs:comment xml:lang="en">Comments to the yearly accounts are reported by reference to a separate ledger.
In the European normalized sheme, the first digit of an account number corresponds to an accounts class.
The claas reserved for comments is the 0 class.</rdfs:comment>
    </owl:Class>
    


    <!-- http://www.fadyart.com/Finance.owl#AccountValues -->

    <owl:Class rdf:about="http://www.fadyart.com/Finance.owl#AccountValues">
        <rdfs:label xml:lang="en">Account values</rdfs:label>
        <rdfs:subClassOf rdf:resource="http://www.fadyart.com/Finance.owl#ValuePartition"/>
        <rdfs:comment xml:lang="en">Values used in the account concept.</rdfs:comment>
    </owl:Class>
    


    <!-- http://www.fadyart.com/Finance.owl#Accounting -->

    <owl:Class rdf:about="http://www.fadyart.com/Finance.owl#Accounting">
        <rdfs:label xml:lang="en">Accounting</rdfs:label>
        <rdfs:subClassOf rdf:resource="http://www.fadyart.com/Finance.owl#Operations"/>
        <rdfs:comment xml:lang="en">Accounting entities</rdfs:comment>
    </owl:Class>
    


    <!-- http://www.fadyart.com/Finance.owl#AccountsPayable -->

    <owl:Class rdf:about="http://www.fadyart.com/Finance.owl#AccountsPayable">
        <rdfs:label xml:lang="en">Accounts payable</rdfs:label>
        <rdfs:subClassOf rdf:resource="http://www.fadyart.com/Finance.owl#ShortTermLiabilities"/>
        <rdfs:comment xml:lang="en">The total of the balances of suppliers or creditors.
The totals are obtained in the balance sheet:
- by periodic transfer of the totals of the supplier accounts
- through simultaneaous posting of all details in the supplier accounts and the general ledger.(carbon copy posting)
Both methods are representations of the double posting system:in  the general ledger account and in the supplier account.</rdfs:comment>
    </owl:Class>
    


    <!-- http://www.fadyart.com/Finance.owl#AccountsReceivable -->

    <owl:Class rdf:about="http://www.fadyart.com/Finance.owl#AccountsReceivable">
        <rdfs:label xml:lang="en">Accounts receivable</rdfs:label>
        <owl:equivalentClass>
            <owl:Class>
                <owl:unionOf rdf:parseType="Collection">
                    <rdf:Description rdf:about="http://www.fadyart.com/Finance.owl#Customer"/>
                    <rdf:Description rdf:about="http://www.fadyart.com/Finance.owl#NOSTRO"/>
                    <rdf:Description rdf:about="http://www.fadyart.com/Finance.owl#OtherDebtors"/>
                </owl:unionOf>
            </owl:Class>
        </owl:equivalentClass>
        <rdfs:subClassOf rdf:resource="http://www.fadyart.com/Finance.owl#CurrentAssets"/>
        <rdfs:comment xml:lang="en">The total of the balances of customers or debtors.
The totals are obtained in the balance sheet:
- by periodic transfer of the totals of the customer accounts
- through simultaneaous posting of all details in the customer accounts and the general ledger.(carbon copy posting)
Both methods are representations of the double posting system:in  the general ledger account and in the customer account.</rdfs:comment>
    </owl:Class>
    


    <!-- http://www.fadyart.com/Finance.owl#AdministrationChannel -->

    <owl:Class rdf:about="http://www.fadyart.com/Finance.owl#AdministrationChannel">
        <rdfs:label xml:lang="en">Administration channel</rdfs:label>
        <rdfs:subClassOf rdf:resource="http://www.fadyart.com/Finance.owl#ValuePartition"/>
        <rdfs:comment xml:lang="en">Channels through which the accounts can be administered and orders passed.</rdfs:comment>
    </owl:Class>
    


    <!-- http://www.fadyart.com/Finance.owl#AnalyticalAccount -->

    <owl:Class rdf:about="http://www.fadyart.com/Finance.owl#AnalyticalAccount">
        <rdfs:label xml:lang="en">Analytical account</rdfs:label>
        <rdfs:subClassOf rdf:resource="http://www.fadyart.com/Finance.owl#Account"/>
        <rdfs:comment xml:lang="en">Accounts coupled to profit and loss accounts.
In cost-accounting the purpose is to charge the source of costs and profits to so-called cost centers and to allocate the costs and profits to costbearers. Other models of analytical accounting are possible.
In the European normalized sheme, the first digit of an account number corresponds to an accounts class.
Classes 8 and 9 are reserved for analytical accounting..Normally class 8 for the cost centers, class 9 for the class bearers.
Amounts of the profit- and loss accounts are posted simultaneously on a cost bearer. Periodically or directly, the costs are allocated to cost bearers. 
The allocation key is a periodic struggle in many companies, notably in the budgetting fase of the internal departments.</rdfs:comment>
    </owl:Class>
    


    <!-- http://www.fadyart.com/Finance.owl#Assets -->

    <owl:Class rdf:about="http://www.fadyart.com/Finance.owl#Assets">
        <rdfs:label xml:lang="en">Actif</rdfs:label>
        <owl:equivalentClass>
            <owl:Class>
                <owl:unionOf rdf:parseType="Collection">
                    <rdf:Description rdf:about="http://www.fadyart.com/Finance.owl#CurrentAssets"/>
                    <rdf:Description rdf:about="http://www.fadyart.com/Finance.owl#FixedAssets"/>
                </owl:unionOf>
            </owl:Class>
        </owl:equivalentClass>
        <rdfs:subClassOf rdf:resource="http://www.fadyart.com/Finance.owl#BalanceSheet"/>
        <rdfs:comment xml:lang="en">The assets of the entity where-off the accounting is done.</rdfs:comment>
    </owl:Class>
    


    <!-- http://www.fadyart.com/Finance.owl#BalanceSheet -->

    <owl:Class rdf:about="http://www.fadyart.com/Finance.owl#BalanceSheet">
        <rdfs:label xml:lang="en">Balance sheet</rdfs:label>
        <owl:equivalentClass>
            <owl:Class>
                <owl:unionOf rdf:parseType="Collection">
                    <rdf:Description rdf:about="http://www.fadyart.com/Finance.owl#Assets"/>
                    <rdf:Description rdf:about="http://www.fadyart.com/Finance.owl#Liabilities"/>
                </owl:unionOf>
            </owl:Class>
        </owl:equivalentClass>
        <rdfs:subClassOf rdf:resource="http://www.fadyart.com/Finance.owl#YearlyAccount"/>
        <rdfs:comment xml:lang="en">The state of actif and passif. Both are divided into categories depending on the term of immobilisation.
The total of actif and passif should equal: they are in balance.
Classes 1 to 5 contain the balance sheet accounts.</rdfs:comment>
    </owl:Class>
    


    <!-- http://www.fadyart.com/Finance.owl#BeneficialOwnerCapital -->

    <owl:Class rdf:about="http://www.fadyart.com/Finance.owl#BeneficialOwnerCapital">
        <rdfs:label xml:lang="en">Arrangement of capital beneficial owners</rdfs:label>
        <owl:equivalentClass>
            <owl:Class>
                <owl:unionOf rdf:parseType="Collection">
                    <rdf:Description rdf:about="http://www.fadyart.com/Finance.owl#NonResidentCapitalOwner"/>
                    <rdf:Description rdf:about="http://www.fadyart.com/Finance.owl#ResidentCapitalOwner"/>
                </owl:unionOf>
            </owl:Class>
        </owl:equivalentClass>
        <rdfs:subClassOf rdf:resource="http://www.fadyart.com/Finance.owl#ClientPortfolio"/>
        <rdfs:comment xml:lang="en">The members of the arrangement are all beneficial owners of the capital from economical and fiscal viewpoint.
The application of this status is for capital operations, including entitlements linked to the equity capital. Example subsciption rights.</rdfs:comment>
    </owl:Class>
    


    <!-- http://www.fadyart.com/Finance.owl#BeneficialOwnerIncome -->

    <owl:Class rdf:about="http://www.fadyart.com/Finance.owl#BeneficialOwnerIncome">
        <rdfs:label xml:lang="en">Arrangement of income beneficial owners</rdfs:label>
        <owl:equivalentClass>
            <owl:Class>
                <owl:unionOf rdf:parseType="Collection">
                    <rdf:Description rdf:about="http://www.fadyart.com/Finance.owl#NonResidentIncomeOwner"/>
                    <rdf:Description rdf:about="http://www.fadyart.com/Finance.owl#ResidentIncomeOwner"/>
                </owl:unionOf>
            </owl:Class>
        </owl:equivalentClass>
        <rdfs:subClassOf rdf:resource="http://www.fadyart.com/Finance.owl#ClientPortfolio"/>
        <rdfs:comment xml:lang="en">The members of the arrangement are all beneficial owners of the income from economical and fiscal viewpoint.
The application of this status is for interest and dividend operations, including entitlements linked to the income. Example: optional dividends. stock dividends, ...</rdfs:comment>
    </owl:Class>
    


    <!-- http://www.fadyart.com/Finance.owl#CashAccountsAndCards -->

    <owl:Class rdf:about="http://www.fadyart.com/Finance.owl#CashAccountsAndCards">
        <rdfs:label xml:lang="en">Cash accounts and cards</rdfs:label>
        <rdfs:subClassOf rdf:resource="http://www.fadyart.com/Finance.owl#Operations"/>
        <rdfs:comment xml:lang="en">Entities managing the cash accounts and cards.</rdfs:comment>
    </owl:Class>
    


    <!-- http://www.fadyart.com/Finance.owl#ClientAccountPosition -->

    <owl:Class rdf:about="http://www.fadyart.com/Finance.owl#ClientAccountPosition">
        <rdfs:label xml:lang="en">Client account position</rdfs:label>
        <rdfs:subClassOf rdf:resource="http://www.fadyart.com/Finance.owl#ClientSecuritiesAccount"/>
        <rdfs:subClassOf>
            <owl:Restriction>
                <owl:onProperty rdf:resource="http://www.fadyart.com/Finance.owl#hasValidityInstant"/>
                <owl:someValuesFrom rdf:resource="http://www.fadyart.com/Finance.owl#ValidInstant"/>
            </owl:Restriction>
        </rdfs:subClassOf>
        <rdfs:subClassOf>
            <owl:Class>
                <owl:intersectionOf rdf:parseType="Collection">
                    <owl:Restriction>
                        <owl:onProperty rdf:resource="http://www.fadyart.com/Finance.owl#concernsFinancialInstrument"/>
                        <owl:someValuesFrom rdf:resource="http://www.fadyart.com/Finance.owl#FinancialInstrument"/>
                    </owl:Restriction>
                    <owl:Restriction>
                        <owl:onProperty rdf:resource="http://www.fadyart.com/Finance.owl#concernsFinancialInstrument"/>
                        <owl:allValuesFrom rdf:resource="http://www.fadyart.com/Finance.owl#FinancialInstrument"/>
                    </owl:Restriction>
                </owl:intersectionOf>
            </owl:Class>
        </rdfs:subClassOf>
        <rdfs:comment xml:lang="en">The position of financial instruments in the account</rdfs:comment>
    </owl:Class>
    


    <!-- http://www.fadyart.com/Finance.owl#ClientAuthorization -->

    <owl:Class rdf:about="http://www.fadyart.com/Finance.owl#ClientAuthorization">
        <rdfs:label xml:lang="en">Arrangement of authorization holders</rdfs:label>
        <owl:equivalentClass>
            <owl:Class>
                <owl:unionOf rdf:parseType="Collection">
                    <rdf:Description rdf:about="http://www.fadyart.com/Finance.owl#ClientAuthorizationDisposal"/>
                    <rdf:Description rdf:about="http://www.fadyart.com/Finance.owl#ClientAuthorizationManagement"/>
                </owl:unionOf>
            </owl:Class>
        </owl:equivalentClass>
        <rdfs:subClassOf rdf:resource="http://www.fadyart.com/Finance.owl#ClientPortfolio"/>
        <rdfs:comment xml:lang="en">The members of the arrangement are granted rights on the accounts they are linked to.
These rights can be rights of disposal or rights of management of the account-holdings</rdfs:comment>
    </owl:Class>
    


    <!-- http://www.fadyart.com/Finance.owl#ClientAuthorizationDisposal -->

    <owl:Class rdf:about="http://www.fadyart.com/Finance.owl#ClientAuthorizationDisposal">
        <rdfs:label xml:lang="en">Client Authorization to dispose of the holdings</rdfs:label>
        <rdfs:subClassOf rdf:resource="http://www.fadyart.com/Finance.owl#ClientAuthorization"/>
        <rdfs:comment xml:lang="en">Authorization to dispose over the client&apos;s holdings.
The authorized person is allowed to transfer holdings to third party and to his own accounts.</rdfs:comment>
    </owl:Class>
    


    <!-- http://www.fadyart.com/Finance.owl#ClientAuthorizationManagement -->

    <owl:Class rdf:about="http://www.fadyart.com/Finance.owl#ClientAuthorizationManagement">
        <rdfs:label xml:lang="en">Client organization to manage the holdings</rdfs:label>
        <rdfs:subClassOf rdf:resource="http://www.fadyart.com/Finance.owl#ClientAuthorization"/>
        <rdfs:comment xml:lang="en">Authorization to manage the client&apos;s holdings.
The authorized person is not allowed to transfer holdings to third party or to his own accounts.</rdfs:comment>
    </owl:Class>
    


    <!-- http://www.fadyart.com/Finance.owl#ClientCashAccount -->

    <owl:Class rdf:about="http://www.fadyart.com/Finance.owl#ClientCashAccount">
        <rdfs:label xml:lang="en">Client cash deposits</rdfs:label>
        <rdfs:subClassOf rdf:resource="http://www.fadyart.com/Finance.owl#ClientPortfolio"/>
    </owl:Class>
    


    <!-- http://www.fadyart.com/Finance.owl#ClientPortfolio -->

    <owl:Class rdf:about="http://www.fadyart.com/Finance.owl#ClientPortfolio">
        <rdfs:label xml:lang="en">Client accounts</rdfs:label>
        <rdfs:subClassOf rdf:resource="http://www.fadyart.com/Finance.owl#AccountsPayable"/>
        <rdfs:subClassOf>
            <owl:Class>
                <owl:intersectionOf rdf:parseType="Collection">
                    <owl:Restriction>
                        <owl:onProperty rdf:resource="http://www.fadyart.com/Finance.owl#isAccessibleViaChannel"/>
                        <owl:someValuesFrom rdf:resource="http://www.fadyart.com/Finance.owl#AdministrationChannel"/>
                    </owl:Restriction>
                    <owl:Restriction>
                        <owl:onProperty rdf:resource="http://www.fadyart.com/Finance.owl#isAccessibleViaChannel"/>
                        <owl:allValuesFrom rdf:resource="http://www.fadyart.com/Finance.owl#AdministrationChannel"/>
                    </owl:Restriction>
                </owl:intersectionOf>
            </owl:Class>
        </rdfs:subClassOf>
        <rdfs:comment rdf:datatype="&xsd;string">The clients of the financial institution for whom&apos;s account the securities handling operations are performed.</rdfs:comment>
    </owl:Class>
    


    <!-- http://www.fadyart.com/Finance.owl#ClientRiskProfile -->

    <owl:Class rdf:about="http://www.fadyart.com/Finance.owl#ClientRiskProfile">
        <rdfs:label xml:lang="en">Risk profile of the customers</rdfs:label>
        <rdfs:subClassOf rdf:resource="http://www.fadyart.com/Finance.owl#RiskProfile"/>
        <rdfs:subClassOf>
            <owl:Restriction>
                <owl:onProperty rdf:resource="http://www.fadyart.com/Finance.owl#hasRiskSymptom"/>
                <owl:someValuesFrom rdf:resource="http://www.fadyart.com/Finance.owl#ClientRiskSymptom"/>
            </owl:Restriction>
        </rdfs:subClassOf>
        <rdfs:comment xml:lang="en">Examples of risk occurences:

- Customer area
If the customers are subject to purchase power reductions, the consequence is:
-- less sales by the producer
-- less profit by the issuer in the short term
-- less solvability by the issuer in the long term

- Producer area
If the producers are subject to reduced purchase power, the purchases become more expensive:
-- less sales by the producer
-- less profit by the issuer in the short term
-- less solvability by the issuer in the long term

- Issuer area
Reduced purchase power with the issuer means his foreign holders will be more expensive to compensate for the reduced power.
-- less profit by the issuer in the short term
-- less solvability by the issuer in the long term</rdfs:comment>
        <rdfs:comment xml:lang="en">The risk of decreased purchase power.</rdfs:comment>
    </owl:Class>
    


    <!-- http://www.fadyart.com/Finance.owl#ClientRiskSymptom -->

    <owl:Class rdf:about="http://www.fadyart.com/Finance.owl#ClientRiskSymptom">
        <rdfs:label xml:lang="en">Customer risk symptom</rdfs:label>
        <rdfs:subClassOf rdf:resource="http://www.fadyart.com/Finance.owl#RiskSymptom"/>
        <rdfs:comment xml:lang="en">Customer market risks on which a risk profile is based.</rdfs:comment>
    </owl:Class>
    


    <!-- http://www.fadyart.com/Finance.owl#ClientSecuritiesAccount -->

    <owl:Class rdf:about="http://www.fadyart.com/Finance.owl#ClientSecuritiesAccount">
        <rdfs:label xml:lang="en">Client securities deposits</rdfs:label>
        <rdfs:subClassOf rdf:resource="http://www.fadyart.com/Finance.owl#ClientPortfolio"/>
    </owl:Class>
    


    <!-- http://www.fadyart.com/Finance.owl#CommercialBanking -->

    <owl:Class rdf:about="http://www.fadyart.com/Finance.owl#CommercialBanking">
        <rdfs:label xml:lang="en">Commercial banking</rdfs:label>
        <rdfs:subClassOf rdf:resource="http://www.fadyart.com/Finance.owl#MerchantBanking"/>
        <rdfs:comment xml:lang="en">Contact points for small and middle sized incorporated customers</rdfs:comment>
    </owl:Class>
    


    <!-- http://www.fadyart.com/Finance.owl#CommercialNetwork -->

    <owl:Class rdf:about="http://www.fadyart.com/Finance.owl#CommercialNetwork">
        <rdfs:label xml:lang="en">Commercial network</rdfs:label>
        <rdfs:subClassOf rdf:resource="http://www.fadyart.com/Finance.owl#Organization"/>
        <rdfs:subClassOf>
            <owl:Class>
                <owl:intersectionOf rdf:parseType="Collection">
                    <owl:Restriction>
                        <owl:onProperty rdf:resource="http://www.fadyart.com/Finance.owl#hasAccessToChannel"/>
                        <owl:someValuesFrom rdf:resource="http://www.fadyart.com/Finance.owl#AdministrationChannel"/>
                    </owl:Restriction>
                    <owl:Restriction>
                        <owl:onProperty rdf:resource="http://www.fadyart.com/Finance.owl#hasAccessToChannel"/>
                        <owl:allValuesFrom rdf:resource="http://www.fadyart.com/Finance.owl#AdministrationChannel"/>
                    </owl:Restriction>
                </owl:intersectionOf>
            </owl:Class>
        </rdfs:subClassOf>
        <rdfs:comment xml:lang="en">Network of commercial customer contacts</rdfs:comment>
    </owl:Class>
    


    <!-- http://www.fadyart.com/Finance.owl#CommodityCostRiskProfile -->

    <owl:Class rdf:about="http://www.fadyart.com/Finance.owl#CommodityCostRiskProfile">
        <rdfs:label xml:lang="en">Risk profile of commodity costs</rdfs:label>
        <rdfs:subClassOf rdf:resource="http://www.fadyart.com/Finance.owl#RiskProfile"/>
        <rdfs:subClassOf>
            <owl:Restriction>
                <owl:onProperty rdf:resource="http://www.fadyart.com/Finance.owl#hasRiskSymptom"/>
                <owl:someValuesFrom rdf:resource="http://www.fadyart.com/Finance.owl#CommodityCostRiskSymptom"/>
            </owl:Restriction>
        </rdfs:subClassOf>
        <rdfs:comment xml:lang="en">Examples of risk occurences:

- Producer area
If the commodity costs increase, the costs of production are increasing, then:
-- less sales by the producer
-- less profit by the issuer in the short term
-- less solvability by the issuer in the long term

- Issuer area
If the commodity costs decrease, the costs of collaterals increase and the underlying assets of derivatives become less worth, then:
-- less profit by the issuer in the short term
-- less solvability by the issuer in the long term

- Holder area
If the commodity costs decrease, the underlying values become less worth, then:
-- prices, thus valuation is lowered</rdfs:comment>
        <rdfs:comment xml:lang="en">The assumption is, the needed commodity will always be available but the price can reach sky high.
The price increase is proportional to the scarceness.
That way the valuation and related impact measurement is facilitated.</rdfs:comment>
    </owl:Class>
    


    <!-- http://www.fadyart.com/Finance.owl#CommodityCostRiskSymptom -->

    <owl:Class rdf:about="http://www.fadyart.com/Finance.owl#CommodityCostRiskSymptom">
        <rdfs:label xml:lang="en">Commomdity cost risk symptom</rdfs:label>
        <rdfs:subClassOf rdf:resource="http://www.fadyart.com/Finance.owl#RiskSymptom"/>
        <rdfs:comment xml:lang="en">Commodity cost symptoms on which a risk profile is based.</rdfs:comment>
    </owl:Class>
    


    <!-- http://www.fadyart.com/Finance.owl#Compliance -->

    <owl:Class rdf:about="http://www.fadyart.com/Finance.owl#Compliance">
        <rdfs:label xml:lang="en">Compliance entities</rdfs:label>
        <rdfs:subClassOf rdf:resource="http://www.fadyart.com/Finance.owl#Operations"/>
        <rdfs:comment xml:lang="en">Entities which safeguard the compliance with legislation, regulation and reputational risk matthers.</rdfs:comment>
    </owl:Class>
    


    <!-- http://www.fadyart.com/Finance.owl#CorporateAction -->

    <owl:Class rdf:about="http://www.fadyart.com/Finance.owl#CorporateAction">
        <rdfs:label xml:lang="en">Corporate actions</rdfs:label>
        <rdfs:subClassOf rdf:resource="http://www.fadyart.com/Finance.owl#SecuritiesHandling"/>
        <rdfs:comment xml:lang="en">Entity in charge of handling the corporate actions.
These corporate actions include:
- interest payments;
- reimbursements;
- optional-, stock-, cash dividend payments;
- recouponing;
- splits;
- mergers;
- squeeze outs,...</rdfs:comment>
    </owl:Class>
    


    <!-- http://www.fadyart.com/Finance.owl#CorporateBanking -->

    <owl:Class rdf:about="http://www.fadyart.com/Finance.owl#CorporateBanking">
        <rdfs:label xml:lang="en">Corporate banking</rdfs:label>
        <rdfs:subClassOf rdf:resource="http://www.fadyart.com/Finance.owl#MerchantBanking"/>
        <rdfs:comment xml:lang="en">Contactpoints for large corporation customers</rdfs:comment>
    </owl:Class>
    


    <!-- http://www.fadyart.com/Finance.owl#Credit -->

    <owl:Class rdf:about="http://www.fadyart.com/Finance.owl#Credit">
        <rdfs:label xml:lang="en">Credits</rdfs:label>
        <rdfs:subClassOf rdf:resource="http://www.fadyart.com/Finance.owl#Operations"/>
        <rdfs:comment xml:lang="en">Entities managing the credits.</rdfs:comment>
    </owl:Class>
    


    <!-- http://www.fadyart.com/Finance.owl#CurrentAssets -->

    <owl:Class rdf:about="http://www.fadyart.com/Finance.owl#CurrentAssets">
        <rdfs:label xml:lang="en">Short term actif</rdfs:label>
        <rdfs:subClassOf rdf:resource="http://www.fadyart.com/Finance.owl#Assets"/>
        <rdfs:comment xml:lang="en">Assets which are frozen for less than 1 year.</rdfs:comment>
    </owl:Class>
    


    <!-- http://www.fadyart.com/Finance.owl#Customer -->

    <owl:Class rdf:about="http://www.fadyart.com/Finance.owl#Customer">
        <rdfs:label xml:lang="en">Customers</rdfs:label>
        <rdfs:subClassOf rdf:resource="http://www.fadyart.com/Finance.owl#AccountsReceivable"/>
    </owl:Class>
    


    <!-- http://www.fadyart.com/Finance.owl#CustomerReferential -->

    <owl:Class rdf:about="http://www.fadyart.com/Finance.owl#CustomerReferential">
        <rdfs:label xml:lang="en">Customer referentials</rdfs:label>
        <rdfs:subClassOf rdf:resource="http://www.fadyart.com/Finance.owl#Operations"/>
        <rdfs:comment xml:lang="en">Entities managing the customer referential systems</rdfs:comment>
    </owl:Class>
    


    <!-- http://www.fadyart.com/Finance.owl#EconomicSectorRiskProfile -->

    <owl:Class rdf:about="http://www.fadyart.com/Finance.owl#EconomicSectorRiskProfile">
        <rdfs:label xml:lang="en">Risk profile of commodity costs</rdfs:label>
        <rdfs:subClassOf rdf:resource="http://www.fadyart.com/Finance.owl#RiskProfile"/>
        <rdfs:subClassOf>
            <owl:Restriction>
                <owl:onProperty rdf:resource="http://www.fadyart.com/Finance.owl#hasRiskSymptom"/>
                <owl:someValuesFrom rdf:resource="http://www.fadyart.com/Finance.owl#EconomicSectorRiskSymptom"/>
            </owl:Restriction>
        </rdfs:subClassOf>
        <rdfs:comment xml:lang="en">Examples of risk occurences:

- Producer area
If the commodity costs increase, the costs of production are increasing, then:
-- less sales by the producer
-- less profit by the issuer in the short term
-- less solvability by the issuer in the long term

- Issuer area
If the commodity costs decrease, the costs of collaterals increase and the underlying assets of derivatives become less worth, then:
-- less profit by the issuer in the short term
-- less solvability by the issuer in the long term

- Holder area
If the commodity costs decrease, the underlying values become less worth, then:
-- prices, thus valuation is lowered</rdfs:comment>
        <rdfs:comment xml:lang="en">The assumption is, the needed commodity will allways be available but the price can reach skyhigh.
The price increase is proportional to the scarceness.
That way the valuation and related impactmeasurement is facilitated.</rdfs:comment>
    </owl:Class>
    


    <!-- http://www.fadyart.com/Finance.owl#EconomicSectorRiskSymptom -->

    <owl:Class rdf:about="http://www.fadyart.com/Finance.owl#EconomicSectorRiskSymptom">
        <rdfs:label xml:lang="en">Economic sector risk symptom</rdfs:label>
        <rdfs:subClassOf rdf:resource="http://www.fadyart.com/Finance.owl#RiskSymptom"/>
        <rdfs:comment xml:lang="en">Economic sector symptoms on which a risk profile is based.</rdfs:comment>
    </owl:Class>
    


    <!-- http://www.fadyart.com/Finance.owl#EnergyCostRiskProfile -->

    <owl:Class rdf:about="http://www.fadyart.com/Finance.owl#EnergyCostRiskProfile">
        <rdfs:label xml:lang="en">Risk profile of energy costs</rdfs:label>
        <rdfs:subClassOf rdf:resource="http://www.fadyart.com/Finance.owl#RiskProfile"/>
        <rdfs:subClassOf>
            <owl:Restriction>
                <owl:onProperty rdf:resource="http://www.fadyart.com/Finance.owl#hasRiskSymptom"/>
                <owl:someValuesFrom rdf:resource="http://www.fadyart.com/Finance.owl#EnergyCostRiskSymptom"/>
            </owl:Restriction>
        </rdfs:subClassOf>
        <rdfs:comment xml:lang="en">Example of risk occurence:

- Producer area
If the energy costs increase, the costs of production are increasing, then:
-- less sales by the producer
-- less profit by the issuer in the short term
-- less solvability by the issuer in the long term</rdfs:comment>
        <rdfs:comment xml:lang="en">The assumption is, the needed energy will allways be available but the price can reach skyhigh.
The price increase is proportional to the scarceness.
That way the valuation and related impactmeasurement is facilitated.</rdfs:comment>
    </owl:Class>
    


    <!-- http://www.fadyart.com/Finance.owl#EnergyCostRiskSymptom -->

    <owl:Class rdf:about="http://www.fadyart.com/Finance.owl#EnergyCostRiskSymptom">
        <rdfs:label xml:lang="en">Energy cost risk symptom</rdfs:label>
        <rdfs:subClassOf rdf:resource="http://www.fadyart.com/Finance.owl#RiskSymptom"/>
        <rdfs:comment xml:lang="en">Energy cost symptoms on which a risk profile is based.</rdfs:comment>
    </owl:Class>
    


    <!-- http://www.fadyart.com/Finance.owl#ExchangeRateRiskProfile -->

    <owl:Class rdf:about="http://www.fadyart.com/Finance.owl#ExchangeRateRiskProfile">
        <rdfs:label xml:lang="en">Risk profile of exchange rates</rdfs:label>
        <rdfs:subClassOf rdf:resource="http://www.fadyart.com/Finance.owl#RiskProfile"/>
        <rdfs:subClassOf>
            <owl:Restriction>
                <owl:onProperty rdf:resource="http://www.fadyart.com/Finance.owl#hasRiskSymptom"/>
                <owl:someValuesFrom rdf:resource="http://www.fadyart.com/Finance.owl#ExchangeRateRiskSymptom"/>
            </owl:Restriction>
        </rdfs:subClassOf>
        <rdfs:comment xml:lang="en">Examples of risk occurences:

- Customer area
If the value of the customers currency depreciates against the producers currency, this means: 
-- a more expensive product 
-- less sales by the producer
-- less profit by the issuer in the short term
-- less solvability by the issuer in the long term

- Producer area
If the value of the producers currency appreciates against the customers currency, this means :
-- a more expensive product 
-- less sales by the producer
-- less profit by the issuer in the short term
-- less solvability by the issuer in the long term

- Issuer area
If the value of the issuers currency depreciates against the holders currency, this means :
-- less revenues in holders currency
-- lower stock quotes because of the needed rentability uplift

- Holder area
If the value of the holders currency appreciates against the holders currency, this means :
-- less revenues in holders currency
-- lower stock quotes because of the needed rentability uplift</rdfs:comment>
        <rdfs:comment xml:lang="en">The risk that the exchange rates fluctuate globally in a negative direction.</rdfs:comment>
    </owl:Class>
    


    <!-- http://www.fadyart.com/Finance.owl#ExchangeRateRiskSymptom -->

    <owl:Class rdf:about="http://www.fadyart.com/Finance.owl#ExchangeRateRiskSymptom">
        <rdfs:label xml:lang="en">Exchange rate risk symptom</rdfs:label>
        <rdfs:subClassOf rdf:resource="http://www.fadyart.com/Finance.owl#RiskSymptom"/>
        <rdfs:comment xml:lang="en">Exchange rate symptoms on which a risk profile is based.</rdfs:comment>
    </owl:Class>
    


    <!-- http://www.fadyart.com/Finance.owl#ExtendedProposition -->

    <owl:Class rdf:about="http://www.fadyart.com/Finance.owl#ExtendedProposition">
        <rdfs:subClassOf rdf:resource="http://www.fadyart.com/Finance.owl#Proposition"/>
    </owl:Class>
    


    <!-- http://www.fadyart.com/Finance.owl#ExternalRisk -->

    <owl:Class rdf:about="http://www.fadyart.com/Finance.owl#ExternalRisk">
        <owl:equivalentClass>
            <owl:Class>
                <owl:unionOf rdf:parseType="Collection">
                    <rdf:Description rdf:about="http://www.fadyart.com/Finance.owl#ImpactOfRiskOccurence"/>
                    <rdf:Description rdf:about="http://www.fadyart.com/Finance.owl#ProbabilityOfRiskOccurence"/>
                    <rdf:Description rdf:about="http://www.fadyart.com/Finance.owl#RiskProfile"/>
                    <rdf:Description rdf:about="http://www.fadyart.com/Finance.owl#RiskSymptom"/>
                </owl:unionOf>
            </owl:Class>
        </owl:equivalentClass>
        <rdfs:subClassOf rdf:resource="http://www.fadyart.com/Finance.owl#Risk"/>
        <rdfs:comment xml:lang="en">External risk</rdfs:comment>
        <rdfs:comment xml:lang="en">Monitoring of risk external to the handling of securities.
Risk profile class contains the core information.</rdfs:comment>
    </owl:Class>
    


    <!-- http://www.fadyart.com/Finance.owl#FinancialInstrument -->

    <owl:Class rdf:about="http://www.fadyart.com/Finance.owl#FinancialInstrument">
        <rdfs:label xml:lang="en">Financial instrument</rdfs:label>
        <rdfs:comment xml:lang="en">The securities or combination of securities in the scope of this ontology.</rdfs:comment>
    </owl:Class>
    


    <!-- http://www.fadyart.com/Finance.owl#FiscalRiskProfile -->

    <owl:Class rdf:about="http://www.fadyart.com/Finance.owl#FiscalRiskProfile">
        <rdfs:label xml:lang="en">Risk profile of fiscal costs</rdfs:label>
        <rdfs:subClassOf rdf:resource="http://www.fadyart.com/Finance.owl#RiskProfile"/>
        <rdfs:subClassOf>
            <owl:Restriction>
                <owl:onProperty rdf:resource="http://www.fadyart.com/Finance.owl#hasRiskSymptom"/>
                <owl:someValuesFrom rdf:resource="http://www.fadyart.com/Finance.owl#FiscalRiskSymptom"/>
            </owl:Restriction>
        </rdfs:subClassOf>
        <rdfs:comment xml:lang="en">Examples of risk occurences:

- Customer area
If the customer has to pay more taxes, his consumption is reduced with those directly or indirectly :
-- less sales by the producer
-- less profit by the issuer in the short term
-- less solvability by the issuer in the long term

- Producer area
If there are tax increases on the profits of producers, e.g. ruling is abolished:
-- less profit by the producer
-- less profit by the issuer in the short term
-- less solvability by the issuer in the long term

- Issuer area
If there are tax increases on the activities of issuers, e.g. stock market tax:
-- less profit by the issuer in the short term
-- less solvability by the issuer in the long term

- Holder area
If the fiscal pressure on stock increases, e.g. through higher prepaid tax rates, this means:
-- less net profit for the holder
-- less demand for the stock
-- prices, thus valuation falling</rdfs:comment>
        <rdfs:comment xml:lang="en">The risk that the fiscal costs evolve increasingly high.</rdfs:comment>
    </owl:Class>
    


    <!-- http://www.fadyart.com/Finance.owl#FiscalRiskSymptom -->

    <owl:Class rdf:about="http://www.fadyart.com/Finance.owl#FiscalRiskSymptom">
        <rdfs:label xml:lang="en">Fiscal risk symptom</rdfs:label>
        <rdfs:subClassOf rdf:resource="http://www.fadyart.com/Finance.owl#RiskSymptom"/>
        <rdfs:comment xml:lang="en">Fiscal symptoms on which a risk profile is based.</rdfs:comment>
    </owl:Class>
    


    <!-- http://www.fadyart.com/Finance.owl#FixedAssets -->

    <owl:Class rdf:about="http://www.fadyart.com/Finance.owl#FixedAssets">
        <rdfs:label xml:lang="en">Long term actif</rdfs:label>
        <rdfs:subClassOf rdf:resource="http://www.fadyart.com/Finance.owl#Assets"/>
        <rdfs:comment xml:lang="en">Investments which are fixed for 1 year or more.</rdfs:comment>
    </owl:Class>
    


    <!-- http://www.fadyart.com/Finance.owl#ForeignFiscalApplication -->

    <owl:Class rdf:about="http://www.fadyart.com/Finance.owl#ForeignFiscalApplication">
        <rdfs:subClassOf rdf:resource="http://www.fadyart.com/Finance.owl#ClientSecuritiesAccount"/>
        <rdfs:comment xml:lang="en">The application of foreign fiscal tax withholdings</rdfs:comment>
    </owl:Class>
    


    <!-- http://www.fadyart.com/Finance.owl#GlobalMarkets -->

    <owl:Class rdf:about="http://www.fadyart.com/Finance.owl#GlobalMarkets">
        <rdfs:label xml:lang="en">Global markets</rdfs:label>
        <rdfs:subClassOf rdf:resource="http://www.fadyart.com/Finance.owl#Operations"/>
        <rdfs:comment xml:lang="en">Entities managing global market transactions</rdfs:comment>
    </owl:Class>
    


    <!-- http://www.fadyart.com/Finance.owl#Granularity -->

    <owl:Class rdf:about="http://www.fadyart.com/Finance.owl#Granularity">
        <rdfs:label xml:lang="en">Granularity</rdfs:label>
        <rdfs:subClassOf rdf:resource="http://www.fadyart.com/Finance.owl#Temporal"/>
        <rdfs:comment xml:lang="en">Spread of the timeslices</rdfs:comment>
    </owl:Class>
    


    <!-- http://www.fadyart.com/Finance.owl#HighProfitabilityImpact -->

    <owl:Class rdf:about="http://www.fadyart.com/Finance.owl#HighProfitabilityImpact">
        <rdfs:label xml:lang="en">High profitability impact</rdfs:label>
        <rdfs:subClassOf rdf:resource="http://www.fadyart.com/Finance.owl#ProfitabilityImpact"/>
    </owl:Class>
    


    <!-- http://www.fadyart.com/Finance.owl#HighRiskProbability -->

    <owl:Class rdf:about="http://www.fadyart.com/Finance.owl#HighRiskProbability">
        <rdfs:label xml:lang="en">High risk probability</rdfs:label>
        <rdfs:subClassOf rdf:resource="http://www.fadyart.com/Finance.owl#ProbabilityOfRiskOccurence"/>
    </owl:Class>
    


    <!-- http://www.fadyart.com/Finance.owl#HighSolvabilityImpact -->

    <owl:Class rdf:about="http://www.fadyart.com/Finance.owl#HighSolvabilityImpact">
        <rdfs:label xml:lang="en">High solvability impact</rdfs:label>
        <rdfs:subClassOf rdf:resource="http://www.fadyart.com/Finance.owl#SolvabilityImpact"/>
    </owl:Class>
    


    <!-- http://www.fadyart.com/Finance.owl#HighStockPriceImpact -->

    <owl:Class rdf:about="http://www.fadyart.com/Finance.owl#HighStockPriceImpact">
        <rdfs:label xml:lang="en">High impact on the stock price</rdfs:label>
        <rdfs:subClassOf rdf:resource="http://www.fadyart.com/Finance.owl#StockPriceImpact"/>
    </owl:Class>
    


    <!-- http://www.fadyart.com/Finance.owl#ISO20022-UNIFIMessages -->

    <owl:Class rdf:about="http://www.fadyart.com/Finance.owl#ISO20022-UNIFIMessages">
        <rdfs:subClassOf rdf:resource="http://www.fadyart.com/Finance.owl#ISOCodes"/>
    </owl:Class>
    


    <!-- http://www.fadyart.com/Finance.owl#ISOCodes -->

    <owl:Class rdf:about="http://www.fadyart.com/Finance.owl#ISOCodes">
        <rdfs:subClassOf rdf:resource="http://www.fadyart.com/Finance.owl#ValuePartition"/>
        <rdfs:comment xml:lang="en">Different public ISO codes used in the ontology</rdfs:comment>
    </owl:Class>
    


    <!-- http://www.fadyart.com/Finance.owl#ImpactOfRiskOccurence -->

    <owl:Class rdf:about="http://www.fadyart.com/Finance.owl#ImpactOfRiskOccurence">
        <rdfs:label xml:lang="en">Impact of the risk occuring</rdfs:label>
        <owl:equivalentClass>
            <owl:Class>
                <owl:unionOf rdf:parseType="Collection">
                    <rdf:Description rdf:about="http://www.fadyart.com/Finance.owl#ProfitabilityImpact"/>
                    <rdf:Description rdf:about="http://www.fadyart.com/Finance.owl#SolvabilityImpact"/>
                    <rdf:Description rdf:about="http://www.fadyart.com/Finance.owl#StockPriceImpact"/>
                </owl:unionOf>
            </owl:Class>
        </owl:equivalentClass>
        <rdfs:subClassOf rdf:resource="http://www.fadyart.com/Finance.owl#ExternalRisk"/>
        <rdfs:seeAlso xml:lang="en">http://www.fadyart.com/externalrisks.html</rdfs:seeAlso>
    </owl:Class>
    


    <!-- http://www.fadyart.com/Finance.owl#InlandFiscalApplication -->

    <owl:Class rdf:about="http://www.fadyart.com/Finance.owl#InlandFiscalApplication">
        <rdfs:subClassOf rdf:resource="http://www.fadyart.com/Finance.owl#ClientSecuritiesAccount"/>
    </owl:Class>
    


    <!-- http://www.fadyart.com/Finance.owl#InstitutionalBanking -->

    <owl:Class rdf:about="http://www.fadyart.com/Finance.owl#InstitutionalBanking">
        <rdfs:label xml:lang="en">Institutional banking</rdfs:label>
        <rdfs:subClassOf rdf:resource="http://www.fadyart.com/Finance.owl#MerchantBanking"/>
        <rdfs:comment xml:lang="en">Contactpoints for institutional customers</rdfs:comment>
    </owl:Class>
    


    <!-- http://www.fadyart.com/Finance.owl#Insurance -->

    <owl:Class rdf:about="http://www.fadyart.com/Finance.owl#Insurance">
        <rdfs:label xml:lang="en">Insurance</rdfs:label>
        <rdfs:subClassOf rdf:resource="http://www.fadyart.com/Finance.owl#ServiceLinkedToSecuritiesAccount"/>
        <rdfs:comment xml:lang="en">Insurances linked to the holdings in securities account.
Exemple accident insurance which covers an amount in case of death of the valuation in securities account. Eventually wiht a maximum and minimum amount.</rdfs:comment>
    </owl:Class>
    


    <!-- http://www.fadyart.com/Finance.owl#InterestRateRiskProfile -->

    <owl:Class rdf:about="http://www.fadyart.com/Finance.owl#InterestRateRiskProfile">
        <rdfs:label xml:lang="en">Risk profile of interest rate costs</rdfs:label>
        <rdfs:subClassOf rdf:resource="http://www.fadyart.com/Finance.owl#RiskProfile"/>
        <rdfs:subClassOf>
            <owl:Restriction>
                <owl:onProperty rdf:resource="http://www.fadyart.com/Finance.owl#hasRiskSymptom"/>
                <owl:someValuesFrom rdf:resource="http://www.fadyart.com/Finance.owl#InterestRateRiskSymptom"/>
            </owl:Restriction>
        </rdfs:subClassOf>
        <rdfs:comment xml:lang="en">Examples of risk occurences:

- Customer area
If the customer has to pay more interests for credits, his consumption is reduced with direct or indirect :
-- less sales by the producer
-- less profit by the issuer in the short term
-- less solvability by the issuer in the long term

- Producer area
If the producer has to pay more interests for credits, his profitability is reduced, meaning:
-- less profit by the issuer in the short term
-- less solvability by the issuer in the long term

- Issuer area
If the market interests rise in the issuers area, the issuer has to provide a higher rentability too, meaning:
-- less solvability by the issuer in the long term

- Holder area
If the market interests rise in the holders area, the rentability of the current investments lowers.
-- to keep the rentability uplevel, the underlying value is lowered.</rdfs:comment>
        <rdfs:comment xml:lang="en">Risk that the cost for interest increases.</rdfs:comment>
    </owl:Class>
    


    <!-- http://www.fadyart.com/Finance.owl#InterestRateRiskSymptom -->

    <owl:Class rdf:about="http://www.fadyart.com/Finance.owl#InterestRateRiskSymptom">
        <rdfs:label xml:lang="en">Interest rate symptom</rdfs:label>
        <rdfs:subClassOf rdf:resource="http://www.fadyart.com/Finance.owl#RiskSymptom"/>
        <rdfs:comment xml:lang="en">Interest rate symptoms on which a risk profile is based.</rdfs:comment>
    </owl:Class>
    


    <!-- http://www.fadyart.com/Finance.owl#InternalRisk -->

    <owl:Class rdf:about="http://www.fadyart.com/Finance.owl#InternalRisk">
        <rdfs:label xml:lang="en">Internal risk</rdfs:label>
        <rdfs:subClassOf rdf:resource="http://www.fadyart.com/Finance.owl#Risk"/>
        <rdfs:comment xml:lang="en">Monitoring of risk inherent to securities handling.</rdfs:comment>
    </owl:Class>
    


    <!-- http://www.fadyart.com/Finance.owl#InvestmentBanking -->

    <owl:Class rdf:about="http://www.fadyart.com/Finance.owl#InvestmentBanking">
        <rdfs:label xml:lang="en">Investment banking</rdfs:label>
        <rdfs:subClassOf rdf:resource="http://www.fadyart.com/Finance.owl#MerchantBanking"/>
        <rdfs:comment xml:lang="en">Contact points for large investors</rdfs:comment>
    </owl:Class>
    


    <!-- http://www.fadyart.com/Finance.owl#InvolvedParty -->

    <owl:Class rdf:about="http://www.fadyart.com/Finance.owl#InvolvedParty">
        <rdfs:label rdf:datatype="&xsd;string">Involved party</rdfs:label>
        <rdfs:comment rdf:datatype="&xsd;string">Party involved with the conduct of securities handling or other financial transactions</rdfs:comment>
    </owl:Class>
    


    <!-- http://www.fadyart.com/Finance.owl#LegalRestrictionRiskProfile -->

    <owl:Class rdf:about="http://www.fadyart.com/Finance.owl#LegalRestrictionRiskProfile">
        <rdfs:label xml:lang="en">Risk profile of legal restrictions</rdfs:label>
        <rdfs:subClassOf rdf:resource="http://www.fadyart.com/Finance.owl#RiskProfile"/>
        <rdfs:subClassOf>
            <owl:Restriction>
                <owl:onProperty rdf:resource="http://www.fadyart.com/Finance.owl#hasRiskSymptom"/>
                <owl:someValuesFrom rdf:resource="http://www.fadyart.com/Finance.owl#LegalRestrictionRiskSymptom"/>
            </owl:Restriction>
        </rdfs:subClassOf>
        <rdfs:comment xml:lang="en">Examples of risk occurences:

- Customer area
If there are legal restrictions on the purchases by the customers, e.g. alcohol by young persons:
-- less sales by the producer
-- less profit by the issuer in the short term
-- less solvability by the issuer in the long term

- Producer area
If there are legal restrictions on the production by the producers, e.g. cars with high carbon dioxide emission:
-- less sales by the producer
-- less profit by the issuer in the short term
-- less solvability by the issuer in the long term

- Issuer area
If there are legal restrictions on the issuance of stock, e.g. stock with mortgages as collateral are evaluated less than 100%, this means:
-- need more collaterals as guarantee for loans
-- increased costs for borrowing
-- less profit by the issuer in the short term
-- less solvability by the issuer in the long term

- Holder area
If the purchase of stock is legally restricted, e.g. of so-called fiscal paradises, this means:
-- less demand for the stock
-- prices, thus valuation falling</rdfs:comment>
        <rdfs:comment xml:lang="en">Risk that legal restrictions like technical, ecological and cultural measures, will have negative effects.</rdfs:comment>
    </owl:Class>
    


    <!-- http://www.fadyart.com/Finance.owl#LegalRestrictionRiskSymptom -->

    <owl:Class rdf:about="http://www.fadyart.com/Finance.owl#LegalRestrictionRiskSymptom">
        <rdfs:label xml:lang="en">Legal restriction risk symptom</rdfs:label>
        <rdfs:subClassOf rdf:resource="http://www.fadyart.com/Finance.owl#RiskSymptom"/>
        <rdfs:comment xml:lang="en">Legal restriction risk symptom on which a risk profile is based.</rdfs:comment>
    </owl:Class>
    


    <!-- http://www.fadyart.com/Finance.owl#Liabilities -->

    <owl:Class rdf:about="http://www.fadyart.com/Finance.owl#Liabilities">
        <rdfs:label xml:lang="en">Passif</rdfs:label>
        <owl:equivalentClass>
            <owl:Class>
                <owl:unionOf rdf:parseType="Collection">
                    <rdf:Description rdf:about="http://www.fadyart.com/Finance.owl#LongTermLiabilities"/>
                    <rdf:Description rdf:about="http://www.fadyart.com/Finance.owl#ShortTermLiabilities"/>
                </owl:unionOf>
            </owl:Class>
        </owl:equivalentClass>
        <rdfs:subClassOf rdf:resource="http://www.fadyart.com/Finance.owl#BalanceSheet"/>
        <rdfs:comment xml:lang="en">The debts of the entity the accounting is done for.
The equity capital is included since it is considered a debt against the share-holders.</rdfs:comment>
    </owl:Class>
    


    <!-- http://www.fadyart.com/Finance.owl#LiquidityRiskProfile -->

    <owl:Class rdf:about="http://www.fadyart.com/Finance.owl#LiquidityRiskProfile">
        <rdfs:label xml:lang="en">Risk profile of the stock&apos;s liquidity</rdfs:label>
        <rdfs:subClassOf rdf:resource="http://www.fadyart.com/Finance.owl#RiskProfile"/>
        <rdfs:subClassOf>
            <owl:Restriction>
                <owl:onProperty rdf:resource="http://www.fadyart.com/Finance.owl#hasRiskSymptom"/>
                <owl:someValuesFrom rdf:resource="http://www.fadyart.com/Finance.owl#LiquidityRiskSymptom"/>
            </owl:Restriction>
        </rdfs:subClassOf>
        <rdfs:comment xml:lang="en">Example of risk occurence:

- Issuer area
If some capital markets would become unaccessible:
-- less capital gathering possibilities
-- less profit by the issuer in the short term
-- less solvability by the issuer in the long term

- Holder area
Due to stricter regulatory measures, liquidity decreases, with higher risk premiums as consequence:
-- less demand for the stock
-- prices, thus valuation falling</rdfs:comment>
        <rdfs:comment xml:lang="en">The intrinsic risk that the trade in the stock is restricted wether this is due to market circumstances or regulatory measures.</rdfs:comment>
    </owl:Class>
    


    <!-- http://www.fadyart.com/Finance.owl#LiquidityRiskSymptom -->

    <owl:Class rdf:about="http://www.fadyart.com/Finance.owl#LiquidityRiskSymptom">
        <rdfs:label xml:lang="en">Liquidity risk symptom</rdfs:label>
        <rdfs:subClassOf rdf:resource="http://www.fadyart.com/Finance.owl#RiskSymptom"/>
        <rdfs:comment xml:lang="en">Liquidity symptoms on which a risk profile is based.</rdfs:comment>
    </owl:Class>
    


    <!-- http://www.fadyart.com/Finance.owl#LongTermLiabilities -->

    <owl:Class rdf:about="http://www.fadyart.com/Finance.owl#LongTermLiabilities">
        <rdfs:label xml:lang="en">Long term passif</rdfs:label>
        <rdfs:subClassOf rdf:resource="http://www.fadyart.com/Finance.owl#Liabilities"/>
        <rdfs:comment xml:lang="en">Debts which are fixed for more than 1 year, including the equity capital.</rdfs:comment>
    </owl:Class>
    


    <!-- http://www.fadyart.com/Finance.owl#LowProfitabilityImpact -->

    <owl:Class rdf:about="http://www.fadyart.com/Finance.owl#LowProfitabilityImpact">
        <rdfs:label xml:lang="en">Low profitability impact</rdfs:label>
        <rdfs:subClassOf rdf:resource="http://www.fadyart.com/Finance.owl#ProfitabilityImpact"/>
    </owl:Class>
    


    <!-- http://www.fadyart.com/Finance.owl#LowRiskProbability -->

    <owl:Class rdf:about="http://www.fadyart.com/Finance.owl#LowRiskProbability">
        <rdfs:label xml:lang="en">Low risk probability</rdfs:label>
        <rdfs:subClassOf rdf:resource="http://www.fadyart.com/Finance.owl#ProbabilityOfRiskOccurence"/>
    </owl:Class>
    


    <!-- http://www.fadyart.com/Finance.owl#LowSolvabilityImpact -->

    <owl:Class rdf:about="http://www.fadyart.com/Finance.owl#LowSolvabilityImpact">
        <rdfs:label xml:lang="en">Low solvability impact</rdfs:label>
        <rdfs:subClassOf rdf:resource="http://www.fadyart.com/Finance.owl#SolvabilityImpact"/>
    </owl:Class>
    


    <!-- http://www.fadyart.com/Finance.owl#LowStockPriceImpact -->

    <owl:Class rdf:about="http://www.fadyart.com/Finance.owl#LowStockPriceImpact">
        <rdfs:label xml:lang="en">Low impact on the stock price</rdfs:label>
        <rdfs:subClassOf rdf:resource="http://www.fadyart.com/Finance.owl#StockPriceImpact"/>
    </owl:Class>
    


    <!-- http://www.fadyart.com/Finance.owl#ManagementFee -->

    <owl:Class rdf:about="http://www.fadyart.com/Finance.owl#ManagementFee">
        <rdfs:label xml:lang="en">Maagement fee</rdfs:label>
        <rdfs:subClassOf rdf:resource="http://www.fadyart.com/Finance.owl#ServiceLinkedToClientPortolio"/>
        <rdfs:comment xml:lang="en">The services rendered in the field of portfolio management.
- advisory 
- discretionary</rdfs:comment>
    </owl:Class>
    


    <!-- http://www.fadyart.com/Finance.owl#ManagementRiskProfile -->

    <owl:Class rdf:about="http://www.fadyart.com/Finance.owl#ManagementRiskProfile">
        <rdfs:label xml:lang="en">Risk profile of the management</rdfs:label>
        <rdfs:subClassOf rdf:resource="http://www.fadyart.com/Finance.owl#RiskProfile"/>
        <rdfs:subClassOf>
            <owl:Restriction>
                <owl:onProperty rdf:resource="http://www.fadyart.com/Finance.owl#hasRiskSymptom"/>
                <owl:someValuesFrom rdf:resource="http://www.fadyart.com/Finance.owl#ManagementRiskSymptom"/>
            </owl:Restriction>
        </rdfs:subClassOf>
        <rdfs:comment xml:lang="en">Examples of management risks

- Issuer and producer areas
Management errors are a risk factor for the issuer.

Signs of dangerous management behaviour are (from empiric studies):
-- the management did not learn from errors in the past since there were no errors commitet
-- the management decides from the stomac
-- only successes lived in the past

with as result:
-- less profit by the issuer or producer in the short term
-- less solvability by the issuer or producer in the long term</rdfs:comment>
        <rdfs:comment xml:lang="en">Risk that the management represents through:
- incompetency on management level;
- ignorance in the field of activity of the issuer;
- remuneration and departure premiums out of proportion to the results;
- focus on short term results</rdfs:comment>
    </owl:Class>
    


    <!-- http://www.fadyart.com/Finance.owl#ManagementRiskSymptom -->

    <owl:Class rdf:about="http://www.fadyart.com/Finance.owl#ManagementRiskSymptom">
        <rdfs:label xml:lang="en">Management risk symptom</rdfs:label>
        <rdfs:subClassOf rdf:resource="http://www.fadyart.com/Finance.owl#RiskSymptom"/>
        <rdfs:comment xml:lang="en">Management symptoms on which a risk profile is based.</rdfs:comment>
    </owl:Class>
    


    <!-- http://www.fadyart.com/Finance.owl#MandatoryCorporateAction -->

    <owl:Class rdf:about="http://www.fadyart.com/Finance.owl#MandatoryCorporateAction">
        <rdfs:label xml:lang="en">Mandatory corporate action</rdfs:label>
        <rdfs:subClassOf rdf:resource="http://www.fadyart.com/Finance.owl#ServiceLinkedToCorporateAction"/>
        <rdfs:comment xml:lang="en">Service of executing mandatory corporate actions: coupon payments, reimbursements,...</rdfs:comment>
    </owl:Class>
    


    <!-- http://www.fadyart.com/Finance.owl#MediumProfitabilityImpact -->

    <owl:Class rdf:about="http://www.fadyart.com/Finance.owl#MediumProfitabilityImpact">
        <rdfs:label xml:lang="en">Medium profitability impact</rdfs:label>
        <rdfs:subClassOf rdf:resource="http://www.fadyart.com/Finance.owl#ProfitabilityImpact"/>
    </owl:Class>
    


    <!-- http://www.fadyart.com/Finance.owl#MediumRiskProbability -->

    <owl:Class rdf:about="http://www.fadyart.com/Finance.owl#MediumRiskProbability">
        <rdfs:label xml:lang="en">Medium risk probability</rdfs:label>
        <rdfs:subClassOf rdf:resource="http://www.fadyart.com/Finance.owl#ProbabilityOfRiskOccurence"/>
    </owl:Class>
    


    <!-- http://www.fadyart.com/Finance.owl#MediumSolvabilityImpact -->

    <owl:Class rdf:about="http://www.fadyart.com/Finance.owl#MediumSolvabilityImpact">
        <rdfs:label xml:lang="en">Medium solvability impact</rdfs:label>
        <rdfs:subClassOf rdf:resource="http://www.fadyart.com/Finance.owl#SolvabilityImpact"/>
    </owl:Class>
    


    <!-- http://www.fadyart.com/Finance.owl#MediumStockPriceImpact -->

    <owl:Class rdf:about="http://www.fadyart.com/Finance.owl#MediumStockPriceImpact">
        <rdfs:label xml:lang="en">Medium impact on the stock price</rdfs:label>
        <rdfs:subClassOf rdf:resource="http://www.fadyart.com/Finance.owl#StockPriceImpact"/>
    </owl:Class>
    


    <!-- http://www.fadyart.com/Finance.owl#MerchantBanking -->

    <owl:Class rdf:about="http://www.fadyart.com/Finance.owl#MerchantBanking">
        <rdfs:label xml:lang="en">Merchant banking</rdfs:label>
        <rdfs:subClassOf rdf:resource="http://www.fadyart.com/Finance.owl#CommercialNetwork"/>
        <rdfs:comment xml:lang="en">Contact points for corporations and wealthy customers</rdfs:comment>
    </owl:Class>
    


    <!-- http://www.fadyart.com/Finance.owl#NOSTRO -->

    <owl:Class rdf:about="http://www.fadyart.com/Finance.owl#NOSTRO">
        <rdfs:label xml:lang="en">NOSTRO account</rdfs:label>
        <owl:equivalentClass>
            <owl:Class>
                <owl:unionOf rdf:parseType="Collection">
                    <rdf:Description rdf:about="http://www.fadyart.com/Finance.owl#NostroCashAccount"/>
                    <rdf:Description rdf:about="http://www.fadyart.com/Finance.owl#NostroSecuritiesAccount"/>
                </owl:unionOf>
            </owl:Class>
        </owl:equivalentClass>
        <rdfs:subClassOf rdf:resource="http://www.fadyart.com/Finance.owl#AccountsReceivable"/>
        <rdfs:comment xml:lang="en">The account in the principal&apos;s books of holdings of another financial institution.</rdfs:comment>
    </owl:Class>
    


    <!-- http://www.fadyart.com/Finance.owl#NonResidentCapitalOwner -->

    <owl:Class rdf:about="http://www.fadyart.com/Finance.owl#NonResidentCapitalOwner">
        <rdfs:label xml:lang="en">Non-resident capital owner</rdfs:label>
        <rdfs:subClassOf rdf:resource="http://www.fadyart.com/Finance.owl#BeneficialOwnerCapital"/>
        <rdfs:comment xml:lang="en">Capital owner is a fiscal non-resident in the fiscal country of the principal. His fiscal country is different from the principal&apos;s.</rdfs:comment>
    </owl:Class>
    


    <!-- http://www.fadyart.com/Finance.owl#NonResidentIncomeOwner -->

    <owl:Class rdf:about="http://www.fadyart.com/Finance.owl#NonResidentIncomeOwner">
        <rdfs:label xml:lang="en">Non resident income owner</rdfs:label>
        <rdfs:subClassOf rdf:resource="http://www.fadyart.com/Finance.owl#BeneficialOwnerIncome"/>
        <rdfs:comment xml:lang="en">Income owner is a fiscal non-resident in the fiscal country of the principal. His fiscal country is different from the principal&apos;s.</rdfs:comment>
    </owl:Class>
    


    <!-- http://www.fadyart.com/Finance.owl#NostroAccountPosition -->

    <owl:Class rdf:about="http://www.fadyart.com/Finance.owl#NostroAccountPosition">
        <rdfs:label xml:lang="en">NOSTRO account position</rdfs:label>
        <rdfs:subClassOf rdf:resource="http://www.fadyart.com/Finance.owl#NostroSecuritiesAccount"/>
        <rdfs:subClassOf>
            <owl:Class>
                <owl:intersectionOf rdf:parseType="Collection">
                    <owl:Restriction>
                        <owl:onProperty rdf:resource="http://www.fadyart.com/Finance.owl#concernsFinancialInstrument"/>
                        <owl:someValuesFrom rdf:resource="http://www.fadyart.com/Finance.owl#FinancialInstrument"/>
                    </owl:Restriction>
                    <owl:Restriction>
                        <owl:onProperty rdf:resource="http://www.fadyart.com/Finance.owl#concernsFinancialInstrument"/>
                        <owl:allValuesFrom rdf:resource="http://www.fadyart.com/Finance.owl#FinancialInstrument"/>
                    </owl:Restriction>
                </owl:intersectionOf>
            </owl:Class>
        </rdfs:subClassOf>
        <rdfs:subClassOf>
            <owl:Class>
                <owl:intersectionOf rdf:parseType="Collection">
                    <owl:Restriction>
                        <owl:onProperty rdf:resource="http://www.fadyart.com/Finance.owl#hasValidityInstant"/>
                        <owl:someValuesFrom rdf:resource="http://www.fadyart.com/Finance.owl#ValidInstant"/>
                    </owl:Restriction>
                    <owl:Restriction>
                        <owl:onProperty rdf:resource="http://www.fadyart.com/Finance.owl#hasValidityInstant"/>
                        <owl:allValuesFrom rdf:resource="http://www.fadyart.com/Finance.owl#ValidInstant"/>
                    </owl:Restriction>
                </owl:intersectionOf>
            </owl:Class>
        </rdfs:subClassOf>
        <rdfs:comment xml:lang="en">The position in financial instruments of the account</rdfs:comment>
    </owl:Class>
    


    <!-- http://www.fadyart.com/Finance.owl#NostroCashAccount -->

    <owl:Class rdf:about="http://www.fadyart.com/Finance.owl#NostroCashAccount">
        <rdfs:label xml:lang="en">NOSTRO cash account</rdfs:label>
        <rdfs:subClassOf rdf:resource="http://www.fadyart.com/Finance.owl#NOSTRO"/>
    </owl:Class>
    


    <!-- http://www.fadyart.com/Finance.owl#NostroSecuritiesAccount -->

    <owl:Class rdf:about="http://www.fadyart.com/Finance.owl#NostroSecuritiesAccount">
        <rdfs:label xml:lang="en">NOSTRO securities account</rdfs:label>
        <rdfs:subClassOf rdf:resource="http://www.fadyart.com/Finance.owl#NOSTRO"/>
    </owl:Class>
    


    <!-- http://www.fadyart.com/Finance.owl#OperationalRiskProfile -->

    <owl:Class rdf:about="http://www.fadyart.com/Finance.owl#OperationalRiskProfile">
        <rdfs:label xml:lang="en">Risk profile of business operations</rdfs:label>
        <rdfs:subClassOf rdf:resource="http://www.fadyart.com/Finance.owl#RiskProfile"/>
        <rdfs:subClassOf>
            <owl:Restriction>
                <owl:onProperty rdf:resource="http://www.fadyart.com/Finance.owl#hasRiskSymptom"/>
                <owl:someValuesFrom rdf:resource="http://www.fadyart.com/Finance.owl#OperationalRiskSymptom"/>
            </owl:Restriction>
        </rdfs:subClassOf>
        <rdfs:comment xml:lang="en">Example of operational risk:

- Producer area
Deliveries delayed, image damaged, poorer quality:
-- less sales by the producer
-- less profit by the issuer in the short term
-- less solvability by the issuer in the long term</rdfs:comment>
        <rdfs:comment xml:lang="en">The risk bared by the operations of the issuer or the elements in the production chain.</rdfs:comment>
    </owl:Class>
    


    <!-- http://www.fadyart.com/Finance.owl#OperationalRiskSymptom -->

    <owl:Class rdf:about="http://www.fadyart.com/Finance.owl#OperationalRiskSymptom">
        <rdfs:label xml:lang="en">Operational risk symptom</rdfs:label>
        <rdfs:subClassOf rdf:resource="http://www.fadyart.com/Finance.owl#RiskSymptom"/>
        <rdfs:comment xml:lang="en">Operational symptoms on which a risk profile is based.</rdfs:comment>
    </owl:Class>
    


    <!-- http://www.fadyart.com/Finance.owl#Operations -->

    <owl:Class rdf:about="http://www.fadyart.com/Finance.owl#Operations">
        <rdfs:label xml:lang="en">Operational organisation</rdfs:label>
        <rdfs:subClassOf rdf:resource="http://www.fadyart.com/Finance.owl#Organization"/>
        <rdfs:subClassOf>
            <owl:Class>
                <owl:intersectionOf rdf:parseType="Collection">
                    <owl:Restriction>
                        <owl:onProperty rdf:resource="http://www.fadyart.com/Finance.owl#hasAccessToChannel"/>
                        <owl:someValuesFrom rdf:resource="http://www.fadyart.com/Finance.owl#AdministrationChannel"/>
                    </owl:Restriction>
                    <owl:Restriction>
                        <owl:onProperty rdf:resource="http://www.fadyart.com/Finance.owl#hasAccessToChannel"/>
                        <owl:allValuesFrom rdf:resource="http://www.fadyart.com/Finance.owl#AdministrationChannel"/>
                    </owl:Restriction>
                </owl:intersectionOf>
            </owl:Class>
        </rdfs:subClassOf>
        <rdfs:comment xml:lang="en">Organization of operational entities</rdfs:comment>
    </owl:Class>
    


    <!-- http://www.fadyart.com/Finance.owl#Organization -->

    <owl:Class rdf:about="http://www.fadyart.com/Finance.owl#Organization">
        <rdfs:label xml:lang="en">Organizational structure of the principals</rdfs:label>
        <owl:equivalentClass>
            <owl:Class>
                <owl:unionOf rdf:parseType="Collection">
                    <rdf:Description rdf:about="http://www.fadyart.com/Finance.owl#CommercialNetwork"/>
                    <rdf:Description rdf:about="http://www.fadyart.com/Finance.owl#Operations"/>
                </owl:unionOf>
            </owl:Class>
        </owl:equivalentClass>
        <rdfs:comment xml:lang="en">Reference to the organisational structure of the principal is made for:
- indication of the performer of procedure steps
- commission calculations
- common income- and cost attributions
- authorizations
- destination for files and reports
- contactpoints for questions and issues
- ...</rdfs:comment>
    </owl:Class>
    


    <!-- http://www.fadyart.com/Finance.owl#OtherDebtors -->

    <owl:Class rdf:about="http://www.fadyart.com/Finance.owl#OtherDebtors">
        <rdfs:label xml:lang="en">Other debtors</rdfs:label>
        <rdfs:subClassOf rdf:resource="http://www.fadyart.com/Finance.owl#AccountsReceivable"/>
    </owl:Class>
    


    <!-- http://www.fadyart.com/Finance.owl#PcsClientComplianceEvaluationFinal -->

    <owl:Class rdf:about="http://www.fadyart.com/Finance.owl#PcsClientComplianceEvaluationFinal">
        <rdfs:label xml:lang="en">Final step in the customer compliance evaluation process</rdfs:label>
        <rdfs:subClassOf rdf:resource="&parties;PcsClientComplianceEvaluation"/>
    </owl:Class>
    


    <!-- http://www.fadyart.com/Finance.owl#PoliticalRiskProfile -->

    <owl:Class rdf:about="http://www.fadyart.com/Finance.owl#PoliticalRiskProfile">
        <rdfs:label xml:lang="en">Risk profile of the political situation.</rdfs:label>
        <rdfs:subClassOf rdf:resource="http://www.fadyart.com/Finance.owl#RiskProfile"/>
        <rdfs:subClassOf>
            <owl:Restriction>
                <owl:onProperty rdf:resource="http://www.fadyart.com/Finance.owl#hasRiskArea"/>
                <owl:someValuesFrom rdf:resource="&ctry;ISO3166-CountryCode"/>
            </owl:Restriction>
        </rdfs:subClassOf>
        <rdfs:subClassOf>
            <owl:Restriction>
                <owl:onProperty rdf:resource="http://www.fadyart.com/Finance.owl#hasRiskSymptom"/>
                <owl:someValuesFrom rdf:resource="http://www.fadyart.com/Finance.owl#PoliticalRiskSymptom"/>
            </owl:Restriction>
        </rdfs:subClassOf>
        <rdfs:comment xml:lang="en">Examples of political risk occurences:

- Customer area
If the products are subject to e.g. an import embargo:
-- less sales by the producer
-- less profit by the issuer in the short term
-- less solvability by the issuer in the long term

- Producer area
If the products cannot be exported to certain customers, this means:
-- less sales by the producer
-- less profit by the issuer in the short term
-- less solvability by the issuer in the long term

- Issuer/Producer area
If the issuer or producers are nationalized, this means:
-- profits are going down in the general interest
-- less profit by the issuer in the short term
-- less solvability by the issuer in the long term

- Customer area
Political dictatures have a decreasing purchase power as consequence:
-- less demand for the products
-- less profit by the issuer in the short term
-- less solvability by the issuer in the long term</rdfs:comment>
        <rdfs:comment xml:lang="en">Risk incured by political decisions.</rdfs:comment>
    </owl:Class>
    


    <!-- http://www.fadyart.com/Finance.owl#PoliticalRiskSymptom -->

    <owl:Class rdf:about="http://www.fadyart.com/Finance.owl#PoliticalRiskSymptom">
        <rdfs:label xml:lang="en">Political risk symptom</rdfs:label>
        <rdfs:subClassOf rdf:resource="http://www.fadyart.com/Finance.owl#RiskSymptom"/>
        <rdfs:comment xml:lang="en">Political symptoms on which a risk profile is based.</rdfs:comment>
    </owl:Class>
    


    <!-- http://www.fadyart.com/Finance.owl#PrimaryMarket -->

    <owl:Class rdf:about="http://www.fadyart.com/Finance.owl#PrimaryMarket">
        <rdfs:label xml:lang="en">Primary markets</rdfs:label>
        <rdfs:subClassOf rdf:resource="http://www.fadyart.com/Finance.owl#SecuritiesHandling"/>
        <rdfs:comment xml:lang="en">Entity in charge of handling the primary market orders.
These orders include 
- new issues of financial instruments: equities and bonds;
- continuous issues of financial instruments: open investment funds like SICAV&apos;s, saving bonds,...</rdfs:comment>
    </owl:Class>
    


    <!-- http://www.fadyart.com/Finance.owl#PrimaryMarketOrderFee -->

    <owl:Class rdf:about="http://www.fadyart.com/Finance.owl#PrimaryMarketOrderFee">
        <rdfs:label xml:lang="en">Primary market order fee</rdfs:label>
        <rdfs:subClassOf rdf:resource="http://www.fadyart.com/Finance.owl#ServiceLinkedToMarketOrders"/>
        <rdfs:comment xml:lang="en">Service of executing orders on the primary market</rdfs:comment>
    </owl:Class>
    


    <!-- http://www.fadyart.com/Finance.owl#PrivateBanking -->

    <owl:Class rdf:about="http://www.fadyart.com/Finance.owl#PrivateBanking">
        <rdfs:label xml:lang="en">Private banking</rdfs:label>
        <rdfs:subClassOf rdf:resource="http://www.fadyart.com/Finance.owl#CommercialNetwork"/>
        <rdfs:comment xml:lang="en">Private banking customer&apos;s contact points</rdfs:comment>
    </owl:Class>
    


    <!-- http://www.fadyart.com/Finance.owl#ProbabilityOfRiskOccurence -->

    <owl:Class rdf:about="http://www.fadyart.com/Finance.owl#ProbabilityOfRiskOccurence">
        <rdfs:label xml:lang="en">Probability of the risk occuring</rdfs:label>
        <owl:equivalentClass>
            <owl:Class>
                <owl:unionOf rdf:parseType="Collection">
                    <rdf:Description rdf:about="http://www.fadyart.com/Finance.owl#HighRiskProbability"/>
                    <rdf:Description rdf:about="http://www.fadyart.com/Finance.owl#LowRiskProbability"/>
                    <rdf:Description rdf:about="http://www.fadyart.com/Finance.owl#MediumRiskProbability"/>
                </owl:unionOf>
            </owl:Class>
        </owl:equivalentClass>
        <rdfs:subClassOf rdf:resource="http://www.fadyart.com/Finance.owl#ExternalRisk"/>
        <rdfs:seeAlso xml:lang="en">http://www.fadyart.com/externalrisks.html</rdfs:seeAlso>
    </owl:Class>
    


    <!-- http://www.fadyart.com/Finance.owl#ProcessAndProcedure -->

    <owl:Class rdf:about="http://www.fadyart.com/Finance.owl#ProcessAndProcedure">
        <rdfs:label xml:lang="en">Processes and procedures</rdfs:label>
        <rdfs:comment xml:lang="en">This class is the actual open wharf.
The processes and subprocesses are represented by classes.
Their prefix is Pcs.
The procedures are represented by individuals in the class, their prefix is pcd.</rdfs:comment>
    </owl:Class>
    


    <!-- http://www.fadyart.com/Finance.owl#ProcessTrigger -->

    <owl:Class rdf:about="http://www.fadyart.com/Finance.owl#ProcessTrigger">
        <rdfs:label xml:lang="en">Process triggers</rdfs:label>
        <rdfs:subClassOf rdf:resource="http://www.fadyart.com/Finance.owl#ProcessValue"/>
        <rdfs:comment xml:lang="en">The triggers to start a process</rdfs:comment>
    </owl:Class>
    


    <!-- http://www.fadyart.com/Finance.owl#ProcessValue -->

    <owl:Class rdf:about="http://www.fadyart.com/Finance.owl#ProcessValue">
        <rdfs:subClassOf rdf:resource="http://www.fadyart.com/Finance.owl#ValuePartition"/>
    </owl:Class>
    


    <!-- http://www.fadyart.com/Finance.owl#ProfitAndLoss -->

    <owl:Class rdf:about="http://www.fadyart.com/Finance.owl#ProfitAndLoss">
        <rdfs:label xml:lang="en">Demonstrates the construction of the result according to the nature of the profits and costs.
This nature combined with the cost- and profitcenters found in the analytical accounting form a management information system.
In the European normalized sheme, the first digit of an account number corresponds to an accounts class.
Class 6 stands for the costs, class 7 for the costs.</rdfs:label>
        <rdfs:label xml:lang="en">Profit and loss</rdfs:label>
        <rdfs:subClassOf rdf:resource="http://www.fadyart.com/Finance.owl#YearlyAccount"/>
    </owl:Class>
    


    <!-- http://www.fadyart.com/Finance.owl#ProfitabilityImpact -->

    <owl:Class rdf:about="http://www.fadyart.com/Finance.owl#ProfitabilityImpact">
        <rdfs:label xml:lang="en">Profitability impact</rdfs:label>
        <owl:equivalentClass>
            <owl:Class>
                <owl:unionOf rdf:parseType="Collection">
                    <rdf:Description rdf:about="http://www.fadyart.com/Finance.owl#HighProfitabilityImpact"/>
                    <rdf:Description rdf:about="http://www.fadyart.com/Finance.owl#LowProfitabilityImpact"/>
                    <rdf:Description rdf:about="http://www.fadyart.com/Finance.owl#MediumProfitabilityImpact"/>
                </owl:unionOf>
            </owl:Class>
        </owl:equivalentClass>
        <rdfs:subClassOf rdf:resource="http://www.fadyart.com/Finance.owl#ImpactOfRiskOccurence"/>
        <rdfs:comment xml:lang="en">Impact on the profitability of the producer or the issuer.</rdfs:comment>
    </owl:Class>
    


    <!-- http://www.fadyart.com/Finance.owl#Proposition -->

    <owl:Class rdf:about="http://www.fadyart.com/Finance.owl#Proposition">
        <rdfs:subClassOf rdf:resource="http://www.fadyart.com/Finance.owl#Temporal"/>
    </owl:Class>
    


    <!-- http://www.fadyart.com/Finance.owl#PublicBanking -->

    <owl:Class rdf:about="http://www.fadyart.com/Finance.owl#PublicBanking">
        <rdfs:label xml:lang="en">Public banking</rdfs:label>
        <rdfs:subClassOf rdf:resource="http://www.fadyart.com/Finance.owl#MerchantBanking"/>
        <rdfs:comment xml:lang="en">Contact points for public customers</rdfs:comment>
    </owl:Class>
    


    <!-- http://www.fadyart.com/Finance.owl#ReasonForAccountFreeze -->

    <owl:Class rdf:about="http://www.fadyart.com/Finance.owl#ReasonForAccountFreeze">
        <rdfs:label xml:lang="en">Reasons for account freeze.</rdfs:label>
        <rdfs:subClassOf rdf:resource="http://www.fadyart.com/Finance.owl#AccountValues"/>
        <rdfs:comment xml:lang="en">The reasons why an account is frozen.
This means all positions on the account as well as the relationships with persons.</rdfs:comment>
    </owl:Class>
    


    <!-- http://www.fadyart.com/Finance.owl#ReasonForPositionFreeze -->

    <owl:Class rdf:about="http://www.fadyart.com/Finance.owl#ReasonForPositionFreeze">
        <rdfs:label xml:lang="en">Reason for position freeze</rdfs:label>
        <rdfs:subClassOf rdf:resource="http://www.fadyart.com/Finance.owl#AccountValues"/>
        <rdfs:comment xml:lang="en">Reason why a position in account is frozen</rdfs:comment>
    </owl:Class>
    


    <!-- http://www.fadyart.com/Finance.owl#ReferentialSystem -->

    <owl:Class rdf:about="http://www.fadyart.com/Finance.owl#ReferentialSystem">
        <rdfs:label xml:lang="en">Referential systems</rdfs:label>
        <rdfs:subClassOf rdf:resource="http://www.fadyart.com/Finance.owl#SecuritiesHandling"/>
        <rdfs:comment xml:lang="en">Entities in charge of securities and securities accounts referential systems.
When used exclusively for securities handling, this might include the customer referential systems.</rdfs:comment>
    </owl:Class>
    


    <!-- http://www.fadyart.com/Finance.owl#RegulatoryRiskProfile -->

    <owl:Class rdf:about="http://www.fadyart.com/Finance.owl#RegulatoryRiskProfile">
        <rdfs:label xml:lang="en">Risk profile of regulations</rdfs:label>
        <rdfs:subClassOf rdf:resource="http://www.fadyart.com/Finance.owl#RiskProfile"/>
        <rdfs:subClassOf>
            <owl:Restriction>
                <owl:onProperty rdf:resource="http://www.fadyart.com/Finance.owl#hasRiskArea"/>
                <owl:someValuesFrom rdf:resource="&ctry;ISO3166-CountryCode"/>
            </owl:Restriction>
        </rdfs:subClassOf>
        <rdfs:subClassOf>
            <owl:Restriction>
                <owl:onProperty rdf:resource="http://www.fadyart.com/Finance.owl#hasRiskSymptom"/>
                <owl:someValuesFrom rdf:resource="http://www.fadyart.com/Finance.owl#RegulatoryRiskSymptom"/>
            </owl:Restriction>
        </rdfs:subClassOf>
        <rdfs:comment xml:lang="en">Examples of risk occurences:

- Customer area
The markets in the scope are the export markets of the issuer or the producers.
If the products are subject to e.g. an import restriction, the target is to reduce the share of imported products on the local market with as a consequence:
-- less sales by the producer
-- less profit by the issuer in the short term
-- less solvability by the issuer in the long term

- Producer area
If the products are subject to e.g. stringent technical specifications, the consequence in first instance will be:
-- less sales by the producer
-- less profit by the issuer in the short term
-- less solvability by the issuer in the long term

- Holder area
Due to stricter regulatory measures, liquidity decreases, with higher risk premiums as consequence:
-- less demand for the stock
-- prices, thus valuation falling</rdfs:comment>
        <rdfs:comment xml:lang="en">The risk incurred by regulations.</rdfs:comment>
    </owl:Class>
    


    <!-- http://www.fadyart.com/Finance.owl#RegulatoryRiskSymptom -->

    <owl:Class rdf:about="http://www.fadyart.com/Finance.owl#RegulatoryRiskSymptom">
        <rdfs:label xml:lang="en">Regulatory risk symptom</rdfs:label>
        <rdfs:subClassOf rdf:resource="http://www.fadyart.com/Finance.owl#RiskSymptom"/>
        <rdfs:comment xml:lang="en">Regulatory symptoms on which a risk profile is based.</rdfs:comment>
    </owl:Class>
    


    <!-- http://www.fadyart.com/Finance.owl#ReputationalRiskProfile -->

    <owl:Class rdf:about="http://www.fadyart.com/Finance.owl#ReputationalRiskProfile">
        <rdfs:label xml:lang="en">Risk profile of the reputation</rdfs:label>
        <rdfs:subClassOf rdf:resource="http://www.fadyart.com/Finance.owl#RiskProfile"/>
        <rdfs:subClassOf>
            <owl:Restriction>
                <owl:onProperty rdf:resource="http://www.fadyart.com/Finance.owl#hasRiskSymptom"/>
                <owl:someValuesFrom rdf:resource="http://www.fadyart.com/Finance.owl#ReputationalRiskSymptom"/>
            </owl:Restriction>
        </rdfs:subClassOf>
        <rdfs:comment xml:lang="en">Examples of risk occurences:

- Customer area
If customers have to be excluded from sales due to reputational risk, e.g. armement deliveries to dictatures, this means:
-- less sales by the producer
-- less profit by the issuer in the short term
-- less solvability by the issuer in the long term

- Producer area
If the reputation of the producer is at risk, e.g. child labour in shoe manufacturies, this means:
-- less sales by the producer
-- less profit by the issuer in the short term
-- less solvability by the issuer in the long term

- Issuer area
If the reputation of the issuer is at risk, e.g. anti-trust investigations, this means:
-- less profit by the issuer in the short term
-- less solvability by the issuer in the long term

- Holder area
If the reputation of the holder is at risk, e.g. mafia connections of major shareholders, this means:
-- less demand for the stock
-- prices, thus valuation falling</rdfs:comment>
        <rdfs:comment xml:lang="en">Risk incurred by the public reputation.</rdfs:comment>
    </owl:Class>
    


    <!-- http://www.fadyart.com/Finance.owl#ReputationalRiskSymptom -->

    <owl:Class rdf:about="http://www.fadyart.com/Finance.owl#ReputationalRiskSymptom">
        <rdfs:label xml:lang="en">Reputational risk symptom</rdfs:label>
        <rdfs:subClassOf rdf:resource="http://www.fadyart.com/Finance.owl#RiskSymptom"/>
        <rdfs:comment xml:lang="en">Reputational symptoms on which a risk profile is based.</rdfs:comment>
    </owl:Class>
    


    <!-- http://www.fadyart.com/Finance.owl#ResidentCapitalOwner -->

    <owl:Class rdf:about="http://www.fadyart.com/Finance.owl#ResidentCapitalOwner">
        <rdfs:label xml:lang="en">Resident capital owner</rdfs:label>
        <rdfs:subClassOf rdf:resource="http://www.fadyart.com/Finance.owl#BeneficialOwnerCapital"/>
        <rdfs:comment xml:lang="en">Capital owner is a fiscal resident in the fiscal residence country of the principal.</rdfs:comment>
    </owl:Class>
    


    <!-- http://www.fadyart.com/Finance.owl#ResidentIncomeOwner -->

    <owl:Class rdf:about="http://www.fadyart.com/Finance.owl#ResidentIncomeOwner">
        <rdfs:label xml:lang="en">Resident income owner</rdfs:label>
        <rdfs:subClassOf rdf:resource="http://www.fadyart.com/Finance.owl#BeneficialOwnerIncome"/>
        <rdfs:comment xml:lang="en">Income owner is a fiscal resident in the fiscal residence country of the principal.</rdfs:comment>
    </owl:Class>
    


    <!-- http://www.fadyart.com/Finance.owl#RetailBanking -->

    <owl:Class rdf:about="http://www.fadyart.com/Finance.owl#RetailBanking">
        <rdfs:label xml:lang="en">Retail branches</rdfs:label>
        <rdfs:subClassOf rdf:resource="http://www.fadyart.com/Finance.owl#CommercialNetwork"/>
        <rdfs:comment xml:lang="en">Retail customers contact points</rdfs:comment>
    </owl:Class>
    


    <!-- http://www.fadyart.com/Finance.owl#Risk -->

    <owl:Class rdf:about="http://www.fadyart.com/Finance.owl#Risk">
        <rdfs:label xml:lang="en">Risk</rdfs:label>
        <owl:equivalentClass>
            <owl:Class>
                <owl:unionOf rdf:parseType="Collection">
                    <rdf:Description rdf:about="http://www.fadyart.com/Finance.owl#ExternalRisk"/>
                    <rdf:Description rdf:about="http://www.fadyart.com/Finance.owl#InternalRisk"/>
                </owl:unionOf>
            </owl:Class>
        </owl:equivalentClass>
        <rdfs:comment xml:lang="en">Risk monitoring</rdfs:comment>
        <rdfs:seeAlso xml:lang="en">http://www.fadyart.com/externalrisks.html</rdfs:seeAlso>
    </owl:Class>
    


    <!-- http://www.fadyart.com/Finance.owl#RiskProfile -->

    <owl:Class rdf:about="http://www.fadyart.com/Finance.owl#RiskProfile">
        <rdfs:label xml:lang="en">Risk profile</rdfs:label>
        <owl:equivalentClass>
            <owl:Class>
                <owl:intersectionOf rdf:parseType="Collection">
                    <owl:Restriction>
                        <owl:onProperty rdf:resource="http://www.fadyart.com/Finance.owl#hasRiskSymptom"/>
                        <owl:someValuesFrom rdf:resource="http://www.fadyart.com/Finance.owl#RiskSymptom"/>
                    </owl:Restriction>
                    <owl:Restriction>
                        <owl:onProperty rdf:resource="http://www.fadyart.com/Finance.owl#hasRiskSymptom"/>
                        <owl:allValuesFrom rdf:resource="http://www.fadyart.com/Finance.owl#RiskSymptom"/>
                    </owl:Restriction>
                </owl:intersectionOf>
            </owl:Class>
        </owl:equivalentClass>
        <owl:equivalentClass>
            <owl:Class>
                <owl:intersectionOf rdf:parseType="Collection">
                    <owl:Restriction>
                        <owl:onProperty rdf:resource="http://www.fadyart.com/Finance.owl#hasRiskImpact"/>
                        <owl:someValuesFrom rdf:resource="http://www.fadyart.com/Finance.owl#ImpactOfRiskOccurence"/>
                    </owl:Restriction>
                    <owl:Restriction>
                        <owl:onProperty rdf:resource="http://www.fadyart.com/Finance.owl#hasRiskImpact"/>
                        <owl:allValuesFrom rdf:resource="http://www.fadyart.com/Finance.owl#ImpactOfRiskOccurence"/>
                    </owl:Restriction>
                </owl:intersectionOf>
            </owl:Class>
        </owl:equivalentClass>
        <owl:equivalentClass>
            <owl:Class>
                <owl:intersectionOf rdf:parseType="Collection">
                    <owl:Restriction>
                        <owl:onProperty rdf:resource="http://www.fadyart.com/Finance.owl#hasProfileValidityPeriod"/>
                        <owl:someValuesFrom rdf:resource="http://www.fadyart.com/Finance.owl#ValidPeriod"/>
                    </owl:Restriction>
                    <owl:Restriction>
                        <owl:onProperty rdf:resource="http://www.fadyart.com/Finance.owl#hasProfileValidityPeriod"/>
                        <owl:allValuesFrom rdf:resource="http://www.fadyart.com/Finance.owl#ValidPeriod"/>
                    </owl:Restriction>
                </owl:intersectionOf>
            </owl:Class>
        </owl:equivalentClass>
        <owl:equivalentClass>
            <owl:Class>
                <owl:unionOf rdf:parseType="Collection">
                    <rdf:Description rdf:about="http://www.fadyart.com/Finance.owl#ClientRiskProfile"/>
                    <rdf:Description rdf:about="http://www.fadyart.com/Finance.owl#CommodityCostRiskProfile"/>
                    <rdf:Description rdf:about="http://www.fadyart.com/Finance.owl#EconomicSectorRiskProfile"/>
                    <rdf:Description rdf:about="http://www.fadyart.com/Finance.owl#EnergyCostRiskProfile"/>
                    <rdf:Description rdf:about="http://www.fadyart.com/Finance.owl#ExchangeRateRiskProfile"/>
                    <rdf:Description rdf:about="http://www.fadyart.com/Finance.owl#FiscalRiskProfile"/>
                    <rdf:Description rdf:about="http://www.fadyart.com/Finance.owl#InterestRateRiskProfile"/>
                    <rdf:Description rdf:about="http://www.fadyart.com/Finance.owl#LegalRestrictionRiskProfile"/>
                    <rdf:Description rdf:about="http://www.fadyart.com/Finance.owl#LiquidityRiskProfile"/>
                    <rdf:Description rdf:about="http://www.fadyart.com/Finance.owl#ManagementRiskProfile"/>
                    <rdf:Description rdf:about="http://www.fadyart.com/Finance.owl#OperationalRiskProfile"/>
                    <rdf:Description rdf:about="http://www.fadyart.com/Finance.owl#PoliticalRiskProfile"/>
                    <rdf:Description rdf:about="http://www.fadyart.com/Finance.owl#RegulatoryRiskProfile"/>
                    <rdf:Description rdf:about="http://www.fadyart.com/Finance.owl#ReputationalRiskProfile"/>
                    <rdf:Description rdf:about="http://www.fadyart.com/Finance.owl#Underlying-CollateralRiskProfile"/>
                </owl:unionOf>
            </owl:Class>
        </owl:equivalentClass>
        <owl:equivalentClass>
            <owl:Class>
                <owl:intersectionOf rdf:parseType="Collection">
                    <owl:Restriction>
                        <owl:onProperty rdf:resource="http://www.fadyart.com/Finance.owl#hasRiskProbability"/>
                        <owl:someValuesFrom rdf:resource="http://www.fadyart.com/Finance.owl#ProbabilityOfRiskOccurence"/>
                    </owl:Restriction>
                    <owl:Restriction>
                        <owl:onProperty rdf:resource="http://www.fadyart.com/Finance.owl#hasRiskProbability"/>
                        <owl:allValuesFrom rdf:resource="http://www.fadyart.com/Finance.owl#ProbabilityOfRiskOccurence"/>
                    </owl:Restriction>
                </owl:intersectionOf>
            </owl:Class>
        </owl:equivalentClass>
        <rdfs:subClassOf rdf:resource="http://www.fadyart.com/Finance.owl#ExternalRisk"/>
        <rdfs:seeAlso rdf:datatype="&xsd;anyURI">http://www.fadyart.com/externalrisks.html</rdfs:seeAlso>
        <rdfs:comment xml:lang="en">The risk profile is the core of the risk monitoring.
The risk profile can be represented in an X/Y graph.

Taxonomy of the risk profiles: 1 level of subclasses.
The level is represented by different risk subclasses: commodity cost, customer risk, energy cost, exhange rate,...
All profiles are stored at the level of the subclass.

Each risk profile can have 3 possible impact evaluations:
1. Impact on the profitability position of the issuer of the stock.
2. Impact on the solvability position of the issuer of the stock.
3. Straight or indirect decrease of the stock price.
That impactevaluation can be an individual of the subclasses of the impact class: High, Medium or Low. Example LowProfitabilityImpact.
If we represent the impact evaluation on the Y-axis, we divide the Y-axis into 3 parts. 
The part starting at the intersection represents a low impact, the second part a medium impact and the upper part a high impact.

On the X-axis we evaluate the probability of the risk occurring.
The evaluation is done on both axis in 3 categories: low, medium and high.
The low probability is represented on the 1/3 part starting at the intersection, the medium probability in the second part and the higher probabilities in the third part of the X-axis.

Each individual profile of the subclasses refers to:
1. an impact subject and assessment of the impact
2. a probability assessment
Further necessary information:
1. the area impacted by the risk: where is the source of the risk
2. the symptom which leads to a risk assessment
3. the source for the symptom: a press release, annual accounts statement, internet article,...
4. the validity period for the profile</rdfs:comment>
    </owl:Class>
    


    <!-- http://www.fadyart.com/Finance.owl#RiskSymptom -->

    <owl:Class rdf:about="http://www.fadyart.com/Finance.owl#RiskSymptom">
        <rdfs:label xml:lang="en">Risk symptom</rdfs:label>
        <owl:equivalentClass>
            <owl:Class>
                <owl:unionOf rdf:parseType="Collection">
                    <rdf:Description rdf:about="http://www.fadyart.com/Finance.owl#ClientRiskSymptom"/>
                    <rdf:Description rdf:about="http://www.fadyart.com/Finance.owl#CommodityCostRiskSymptom"/>
                    <rdf:Description rdf:about="http://www.fadyart.com/Finance.owl#EconomicSectorRiskSymptom"/>
                    <rdf:Description rdf:about="http://www.fadyart.com/Finance.owl#EnergyCostRiskSymptom"/>
                    <rdf:Description rdf:about="http://www.fadyart.com/Finance.owl#ExchangeRateRiskSymptom"/>
                    <rdf:Description rdf:about="http://www.fadyart.com/Finance.owl#FiscalRiskSymptom"/>
                    <rdf:Description rdf:about="http://www.fadyart.com/Finance.owl#InterestRateRiskSymptom"/>
                    <rdf:Description rdf:about="http://www.fadyart.com/Finance.owl#LegalRestrictionRiskSymptom"/>
                    <rdf:Description rdf:about="http://www.fadyart.com/Finance.owl#LiquidityRiskSymptom"/>
                    <rdf:Description rdf:about="http://www.fadyart.com/Finance.owl#ManagementRiskSymptom"/>
                    <rdf:Description rdf:about="http://www.fadyart.com/Finance.owl#OperationalRiskSymptom"/>
                    <rdf:Description rdf:about="http://www.fadyart.com/Finance.owl#PoliticalRiskSymptom"/>
                    <rdf:Description rdf:about="http://www.fadyart.com/Finance.owl#RegulatoryRiskSymptom"/>
                    <rdf:Description rdf:about="http://www.fadyart.com/Finance.owl#ReputationalRiskSymptom"/>
                    <rdf:Description rdf:about="http://www.fadyart.com/Finance.owl#Underlying-CollateralRiskSymptom"/>
                </owl:unionOf>
            </owl:Class>
        </owl:equivalentClass>
        <rdfs:subClassOf rdf:resource="http://www.fadyart.com/Finance.owl#ExternalRisk"/>
        <rdfs:comment xml:lang="en">Symptom on which a risk assesment is based, so that a profile is obtained.</rdfs:comment>
        <rdfs:seeAlso xml:lang="en">http://www.fadyart.com/externalrisks.html</rdfs:seeAlso>
    </owl:Class>
    


    <!-- http://www.fadyart.com/Finance.owl#SafekeepingFee -->

    <owl:Class rdf:about="http://www.fadyart.com/Finance.owl#SafekeepingFee">
        <rdfs:label xml:lang="en">Safekeeping fee</rdfs:label>
        <rdfs:subClassOf rdf:resource="http://www.fadyart.com/Finance.owl#ServiceLinkedToSecuritiesAccount"/>
        <rdfs:comment xml:lang="en">The service of safekeeping and monitoring physical or inmaterial financial instruments.</rdfs:comment>
    </owl:Class>
    


    <!-- http://www.fadyart.com/Finance.owl#SecundaryMarket -->

    <owl:Class rdf:about="http://www.fadyart.com/Finance.owl#SecundaryMarket">
        <rdfs:label xml:lang="en">Secundary markets</rdfs:label>
        <rdfs:subClassOf rdf:resource="http://www.fadyart.com/Finance.owl#SecuritiesHandling"/>
        <rdfs:comment xml:lang="en">Entities in charge of secundary market order handling.
The secundary markets handling include orders on:
- official markets;
- over the counter markets (OTC);
- public auctions for existing issues</rdfs:comment>
    </owl:Class>
    


    <!-- http://www.fadyart.com/Finance.owl#SecundaryMarketOrderFee -->

    <owl:Class rdf:about="http://www.fadyart.com/Finance.owl#SecundaryMarketOrderFee">
        <rdfs:label xml:lang="en">Secundary market order fee</rdfs:label>
        <rdfs:subClassOf rdf:resource="http://www.fadyart.com/Finance.owl#ServiceLinkedToMarketOrders"/>
        <rdfs:comment xml:lang="en">Service of execution of purchase- or salesorders on the secundary markets</rdfs:comment>
    </owl:Class>
    


    <!-- http://www.fadyart.com/Finance.owl#SecuritiesHandling -->

    <owl:Class rdf:about="http://www.fadyart.com/Finance.owl#SecuritiesHandling">
        <rdfs:label xml:lang="en">Securities handling</rdfs:label>
        <rdfs:subClassOf rdf:resource="http://www.fadyart.com/Finance.owl#Operations"/>
        <rdfs:comment xml:lang="en">Entities managing securities handling.</rdfs:comment>
    </owl:Class>
    


    <!-- http://www.fadyart.com/Finance.owl#Service -->

    <owl:Class rdf:about="http://www.fadyart.com/Finance.owl#Service">
        <rdfs:label xml:lang="en">Services</rdfs:label>
        <rdfs:comment xml:lang="en">Services rendered to the customers of and for account of our principals.
The services can be rendered in own name or in name of the principals.</rdfs:comment>
    </owl:Class>
    


    <!-- http://www.fadyart.com/Finance.owl#ServiceLinkedToClientPortolio -->

    <owl:Class rdf:about="http://www.fadyart.com/Finance.owl#ServiceLinkedToClientPortolio">
        <rdfs:label xml:lang="en">Servuices linked to client portfolios</rdfs:label>
        <rdfs:subClassOf rdf:resource="http://www.fadyart.com/Finance.owl#Service"/>
        <rdfs:comment xml:lang="en">Services rendered on the level of the client portfolio</rdfs:comment>
    </owl:Class>
    


    <!-- http://www.fadyart.com/Finance.owl#ServiceLinkedToCorporateAction -->

    <owl:Class rdf:about="http://www.fadyart.com/Finance.owl#ServiceLinkedToCorporateAction">
        <rdfs:label xml:lang="en">Service linked to corporate action</rdfs:label>
        <rdfs:subClassOf rdf:resource="http://www.fadyart.com/Finance.owl#Service"/>
        <rdfs:comment xml:lang="en">Service of executing corporate actions</rdfs:comment>
    </owl:Class>
    


    <!-- http://www.fadyart.com/Finance.owl#ServiceLinkedToMarketOrders -->

    <owl:Class rdf:about="http://www.fadyart.com/Finance.owl#ServiceLinkedToMarketOrders">
        <rdfs:label xml:lang="en">Service linked to market orders</rdfs:label>
        <rdfs:subClassOf rdf:resource="http://www.fadyart.com/Finance.owl#Service"/>
        <rdfs:comment xml:lang="en">Service of execution of primary and secundary market orders</rdfs:comment>
    </owl:Class>
    


    <!-- http://www.fadyart.com/Finance.owl#ServiceLinkedToSecuritiesAccount -->

    <owl:Class rdf:about="http://www.fadyart.com/Finance.owl#ServiceLinkedToSecuritiesAccount">
        <rdfs:label xml:lang="en">Service linked to securities accounts</rdfs:label>
        <rdfs:subClassOf rdf:resource="http://www.fadyart.com/Finance.owl#Service"/>
        <rdfs:comment xml:lang="en">Service rendered with regard to holdings in securities account.</rdfs:comment>
    </owl:Class>
    


    <!-- http://www.fadyart.com/Finance.owl#ShortTermLiabilities -->

    <owl:Class rdf:about="http://www.fadyart.com/Finance.owl#ShortTermLiabilities">
        <rdfs:label xml:lang="en">Short term passif</rdfs:label>
        <rdfs:subClassOf rdf:resource="http://www.fadyart.com/Finance.owl#Liabilities"/>
        <rdfs:comment xml:lang="en">Debts which are frozen for max 1 year.</rdfs:comment>
    </owl:Class>
    


    <!-- http://www.fadyart.com/Finance.owl#SolvabilityImpact -->

    <owl:Class rdf:about="http://www.fadyart.com/Finance.owl#SolvabilityImpact">
        <rdfs:label xml:lang="en">Solvability impact</rdfs:label>
        <owl:equivalentClass>
            <owl:Class>
                <owl:unionOf rdf:parseType="Collection">
                    <rdf:Description rdf:about="http://www.fadyart.com/Finance.owl#HighSolvabilityImpact"/>
                    <rdf:Description rdf:about="http://www.fadyart.com/Finance.owl#LowSolvabilityImpact"/>
                    <rdf:Description rdf:about="http://www.fadyart.com/Finance.owl#MediumSolvabilityImpact"/>
                </owl:unionOf>
            </owl:Class>
        </owl:equivalentClass>
        <rdfs:subClassOf rdf:resource="http://www.fadyart.com/Finance.owl#ImpactOfRiskOccurence"/>
        <rdfs:comment xml:lang="en">Impact on the solvability of the producer or issuer</rdfs:comment>
    </owl:Class>
    


    <!-- http://www.fadyart.com/Finance.owl#StockPriceImpact -->

    <owl:Class rdf:about="http://www.fadyart.com/Finance.owl#StockPriceImpact">
        <rdfs:label xml:lang="en">Direct impact on the stock price</rdfs:label>
        <owl:equivalentClass>
            <owl:Class>
                <owl:unionOf rdf:parseType="Collection">
                    <rdf:Description rdf:about="http://www.fadyart.com/Finance.owl#HighStockPriceImpact"/>
                    <rdf:Description rdf:about="http://www.fadyart.com/Finance.owl#LowStockPriceImpact"/>
                    <rdf:Description rdf:about="http://www.fadyart.com/Finance.owl#MediumStockPriceImpact"/>
                </owl:unionOf>
            </owl:Class>
        </owl:equivalentClass>
        <rdfs:subClassOf rdf:resource="http://www.fadyart.com/Finance.owl#ImpactOfRiskOccurence"/>
        <rdfs:comment xml:lang="en">Stock price impact, direct or indirect.</rdfs:comment>
    </owl:Class>
    


    <!-- http://www.fadyart.com/Finance.owl#Supplier -->

    <owl:Class rdf:about="http://www.fadyart.com/Finance.owl#Supplier">
        <rdfs:label xml:lang="en">Suppliers</rdfs:label>
        <rdfs:subClassOf rdf:resource="http://www.fadyart.com/Finance.owl#AccountsPayable"/>
    </owl:Class>
    


    <!-- http://www.fadyart.com/Finance.owl#Template -->

    <owl:Class rdf:about="http://www.fadyart.com/Finance.owl#Template">
        <rdfs:subClassOf rdf:resource="&spin;Templates"/>
    </owl:Class>
    


    <!-- http://www.fadyart.com/Finance.owl#Temporal -->

    <owl:Class rdf:about="http://www.fadyart.com/Finance.owl#Temporal">
        <rdfs:label xml:lang="en">Temporal information</rdfs:label>
        <owl:equivalentClass>
            <owl:Class>
                <owl:unionOf rdf:parseType="Collection">
                    <rdf:Description rdf:about="http://www.fadyart.com/Finance.owl#Granularity"/>
                    <rdf:Description rdf:about="http://www.fadyart.com/Finance.owl#Proposition"/>
                    <rdf:Description rdf:about="http://www.fadyart.com/Finance.owl#ValidTime"/>
                </owl:unionOf>
            </owl:Class>
        </owl:equivalentClass>
        <rdfs:comment xml:lang="en">Time indicators</rdfs:comment>
    </owl:Class>
    


    <!-- http://www.fadyart.com/Finance.owl#Underlying-CollateralRiskProfile -->

    <owl:Class rdf:about="http://www.fadyart.com/Finance.owl#Underlying-CollateralRiskProfile">
        <rdfs:label xml:lang="en">Risk profile of the underlying assets or the collateral of a security</rdfs:label>
        <rdfs:subClassOf rdf:resource="http://www.fadyart.com/Finance.owl#RiskProfile"/>
        <rdfs:subClassOf>
            <owl:Restriction>
                <owl:onProperty rdf:resource="http://www.fadyart.com/Finance.owl#hasRiskSymptom"/>
                <owl:someValuesFrom rdf:resource="http://www.fadyart.com/Finance.owl#Underlying-CollateralRiskSymptom"/>
            </owl:Restriction>
        </rdfs:subClassOf>
        <rdfs:subClassOf>
            <owl:Restriction>
                <owl:onProperty rdf:resource="http://www.fadyart.com/Finance.owl#hasRiskArea"/>
                <owl:someValuesFrom rdf:resource="&fi;ClassificationOfFinancialInstruments"/>
            </owl:Restriction>
        </rdfs:subClassOf>
        <rdfs:comment xml:lang="en">Examples of risk occurences:

- Issuer area
If the underlying assets become less worth, this means:
-- less profit by the issuer in the short term
-- less solvability by the issuer in the long term

- Holder area
If the underlying values become less worth, this means:
-- prices, thus valuation is lowered</rdfs:comment>
        <rdfs:comment xml:lang="en">The underlying for derivatives or the collateral for debt instruments can be negatively influenced.</rdfs:comment>
    </owl:Class>
    


    <!-- http://www.fadyart.com/Finance.owl#Underlying-CollateralRiskSymptom -->

    <owl:Class rdf:about="http://www.fadyart.com/Finance.owl#Underlying-CollateralRiskSymptom">
        <rdfs:label xml:lang="en">Underlying or collateral risk symptom</rdfs:label>
        <rdfs:subClassOf rdf:resource="http://www.fadyart.com/Finance.owl#RiskSymptom"/>
        <rdfs:comment xml:lang="en">Underlying-Collateral symptoms on which a risk profile is based.</rdfs:comment>
    </owl:Class>
    


    <!-- http://www.fadyart.com/Finance.owl#VOSTRO -->

    <owl:Class rdf:about="http://www.fadyart.com/Finance.owl#VOSTRO">
        <rdfs:label xml:lang="en">VOSTRO account</rdfs:label>
        <owl:equivalentClass>
            <owl:Class>
                <owl:unionOf rdf:parseType="Collection">
                    <rdf:Description rdf:about="http://www.fadyart.com/Finance.owl#VostroCashAccount"/>
                    <rdf:Description rdf:about="http://www.fadyart.com/Finance.owl#VostroSecuritiesAccount"/>
                </owl:unionOf>
            </owl:Class>
        </owl:equivalentClass>
        <rdfs:subClassOf rdf:resource="http://www.fadyart.com/Finance.owl#AccountsPayable"/>
        <rdfs:subClassOf>
            <owl:Class>
                <owl:intersectionOf rdf:parseType="Collection">
                    <owl:Restriction>
                        <owl:onProperty rdf:resource="http://www.fadyart.com/Finance.owl#hasValidityPeriod"/>
                        <owl:someValuesFrom rdf:resource="http://www.fadyart.com/Finance.owl#ValidPeriod"/>
                    </owl:Restriction>
                    <owl:Restriction>
                        <owl:onProperty rdf:resource="http://www.fadyart.com/Finance.owl#hasValidityPeriod"/>
                        <owl:allValuesFrom rdf:resource="http://www.fadyart.com/Finance.owl#ValidPeriod"/>
                    </owl:Restriction>
                </owl:intersectionOf>
            </owl:Class>
        </rdfs:subClassOf>
        <rdfs:subClassOf>
            <owl:Class>
                <owl:intersectionOf rdf:parseType="Collection">
                    <owl:Restriction>
                        <owl:onProperty rdf:resource="http://www.fadyart.com/Finance.owl#isAccessibleViaChannel"/>
                        <owl:someValuesFrom rdf:resource="http://www.fadyart.com/Finance.owl#AdministrationChannel"/>
                    </owl:Restriction>
                    <owl:Restriction>
                        <owl:onProperty rdf:resource="http://www.fadyart.com/Finance.owl#isAccessibleViaChannel"/>
                        <owl:allValuesFrom rdf:resource="http://www.fadyart.com/Finance.owl#AdministrationChannel"/>
                    </owl:Restriction>
                </owl:intersectionOf>
            </owl:Class>
        </rdfs:subClassOf>
        <rdfs:subClassOf>
            <owl:Class>
                <owl:intersectionOf rdf:parseType="Collection">
                    <owl:Restriction>
                        <owl:onProperty rdf:resource="http://www.fadyart.com/Finance.owl#hasContactPerson"/>
                        <owl:someValuesFrom rdf:resource="http://www.fadyart.com/Finance.owl#InvolvedParty"/>
                    </owl:Restriction>
                    <owl:Restriction>
                        <owl:onProperty rdf:resource="http://www.fadyart.com/Finance.owl#hasContactPerson"/>
                        <owl:allValuesFrom rdf:resource="http://www.fadyart.com/Finance.owl#InvolvedParty"/>
                    </owl:Restriction>
                </owl:intersectionOf>
            </owl:Class>
        </rdfs:subClassOf>
        <rdfs:comment xml:lang="en">The account of the principal for his holdings in another financial institution&apos;s books.</rdfs:comment>
    </owl:Class>
    


    <!-- http://www.fadyart.com/Finance.owl#ValidInstant -->

    <owl:Class rdf:about="http://www.fadyart.com/Finance.owl#ValidInstant">
        <rdfs:label xml:lang="en">Valid instant</rdfs:label>
        <rdfs:subClassOf rdf:resource="http://www.fadyart.com/Finance.owl#ValidTime"/>
        <rdfs:comment xml:lang="en">Instant at which the information of an individual is valid.</rdfs:comment>
    </owl:Class>
    


    <!-- http://www.fadyart.com/Finance.owl#ValidPeriod -->

    <owl:Class rdf:about="http://www.fadyart.com/Finance.owl#ValidPeriod">
        <rdfs:label xml:lang="en">Valid period</rdfs:label>
        <rdfs:subClassOf rdf:resource="http://www.fadyart.com/Finance.owl#ValidTime"/>
        <rdfs:comment xml:lang="en">Period during which the information on an individual is valid.</rdfs:comment>
    </owl:Class>
    


    <!-- http://www.fadyart.com/Finance.owl#ValidTime -->

    <owl:Class rdf:about="http://www.fadyart.com/Finance.owl#ValidTime">
        <rdfs:label xml:lang="en">Valid time</rdfs:label>
        <rdfs:subClassOf rdf:resource="http://www.fadyart.com/Finance.owl#Temporal"/>
        <rdfs:comment xml:lang="en">Valid time instants or periods</rdfs:comment>
    </owl:Class>
    


    <!-- http://www.fadyart.com/Finance.owl#ValuePartition -->

    <owl:Class rdf:about="http://www.fadyart.com/Finance.owl#ValuePartition">
        <rdfs:label xml:lang="en">Value partition</rdfs:label>
        <rdfs:comment xml:lang="en">Partition with reference data.
Values in this partition are referenced by the core concepts as there are: financial instrument, party, ... to value their properties.</rdfs:comment>
    </owl:Class>
    


    <!-- http://www.fadyart.com/Finance.owl#VoluntaryCorporateAction -->

    <owl:Class rdf:about="http://www.fadyart.com/Finance.owl#VoluntaryCorporateAction">
        <rdfs:label xml:lang="en">Voluntary corporate action</rdfs:label>
        <rdfs:subClassOf rdf:resource="http://www.fadyart.com/Finance.owl#ServiceLinkedToCorporateAction"/>
        <rdfs:comment xml:lang="en">Service of executing voluntary corporate actions like management buy outs, public purchase offers,...</rdfs:comment>
    </owl:Class>
    


    <!-- http://www.fadyart.com/Finance.owl#VostroAccountPosition -->

    <owl:Class rdf:about="http://www.fadyart.com/Finance.owl#VostroAccountPosition">
        <rdfs:label xml:lang="en">Vostro account position</rdfs:label>
        <rdfs:subClassOf rdf:resource="http://www.fadyart.com/Finance.owl#VostroSecuritiesAccount"/>
        <rdfs:subClassOf>
            <owl:Class>
                <owl:intersectionOf rdf:parseType="Collection">
                    <owl:Restriction>
                        <owl:onProperty rdf:resource="http://www.fadyart.com/Finance.owl#concernsFinancialInstrument"/>
                        <owl:someValuesFrom rdf:resource="http://www.fadyart.com/Finance.owl#FinancialInstrument"/>
                    </owl:Restriction>
                    <owl:Restriction>
                        <owl:onProperty rdf:resource="http://www.fadyart.com/Finance.owl#concernsFinancialInstrument"/>
                        <owl:allValuesFrom rdf:resource="http://www.fadyart.com/Finance.owl#FinancialInstrument"/>
                    </owl:Restriction>
                </owl:intersectionOf>
            </owl:Class>
        </rdfs:subClassOf>
        <rdfs:subClassOf>
            <owl:Class>
                <owl:intersectionOf rdf:parseType="Collection">
                    <owl:Restriction>
                        <owl:onProperty rdf:resource="http://www.fadyart.com/Finance.owl#hasValidityInstant"/>
                        <owl:someValuesFrom rdf:resource="http://www.fadyart.com/Finance.owl#ValidInstant"/>
                    </owl:Restriction>
                    <owl:Restriction>
                        <owl:onProperty rdf:resource="http://www.fadyart.com/Finance.owl#hasValidityInstant"/>
                        <owl:allValuesFrom rdf:resource="http://www.fadyart.com/Finance.owl#ValidInstant"/>
                    </owl:Restriction>
                </owl:intersectionOf>
            </owl:Class>
        </rdfs:subClassOf>
        <rdfs:comment xml:lang="en">The position of financial instruments in the account</rdfs:comment>
    </owl:Class>
    


    <!-- http://www.fadyart.com/Finance.owl#VostroCashAccount -->

    <owl:Class rdf:about="http://www.fadyart.com/Finance.owl#VostroCashAccount">
        <rdfs:label xml:lang="en">Vostro cash account</rdfs:label>
        <rdfs:subClassOf rdf:resource="http://www.fadyart.com/Finance.owl#VOSTRO"/>
    </owl:Class>
    


    <!-- http://www.fadyart.com/Finance.owl#VostroSecuritiesAccount -->

    <owl:Class rdf:about="http://www.fadyart.com/Finance.owl#VostroSecuritiesAccount">
        <rdfs:label xml:lang="en">Vostro securities account</rdfs:label>
        <rdfs:subClassOf rdf:resource="http://www.fadyart.com/Finance.owl#VOSTRO"/>
    </owl:Class>
    


    <!-- http://www.fadyart.com/Finance.owl#XNStatus -->

    <owl:Class rdf:about="http://www.fadyart.com/Finance.owl#XNStatus">
        <rdfs:subClassOf rdf:resource="http://www.fadyart.com/Finance.owl#ValuePartition"/>
        <rdfs:comment xml:lang="en">The X/N status is determined at 2 levels: the customer securities account&apos; beneficial owners and the financial instrument.

Debt instruments eligible to the X/N status are instruments for which the Belgian National Bank is acting as settlement party and custodian.

An instrument with status X can only be held by beneficial owners with X status.
An instument with N or X/N status can be held by beneficial owners having the X or the N status.
When an instrument is of X or X/N status, and the beneficial owners are of X status, the income is exempted from Belgian prepaid taxes.</rdfs:comment>
    </owl:Class>
    


    <!-- http://www.fadyart.com/Finance.owl#YearlyAccount -->

    <owl:Class rdf:about="http://www.fadyart.com/Finance.owl#YearlyAccount">
        <rdfs:label xml:lang="en">Yearly account</rdfs:label>
        <owl:equivalentClass>
            <owl:Class>
                <owl:unionOf rdf:parseType="Collection">
                    <rdf:Description rdf:about="http://www.fadyart.com/Finance.owl#AccountComments"/>
                    <rdf:Description rdf:about="http://www.fadyart.com/Finance.owl#BalanceSheet"/>
                    <rdf:Description rdf:about="http://www.fadyart.com/Finance.owl#ProfitAndLoss"/>
                </owl:unionOf>
            </owl:Class>
        </owl:equivalentClass>
        <rdfs:subClassOf rdf:resource="http://www.fadyart.com/Finance.owl#Account"/>
        <rdfs:comment xml:lang="en">The accounts which have to be published at least once a year according to the national legislation.</rdfs:comment>
    </owl:Class>
    


    <!-- http://www.fadyart.com/countries#ISO3166-CountryCode -->

    <rdf:Description rdf:about="&ctry;ISO3166-CountryCode">
        <rdfs:subClassOf rdf:resource="http://www.fadyart.com/Finance.owl#ISOCodes"/>
    </rdf:Description>
    


    <!-- http://www.fadyart.com/currencies#ISO4217-Currencycodes -->

    <rdf:Description rdf:about="http://www.fadyart.com/currencies#ISO4217-Currencycodes">
        <rdfs:subClassOf rdf:resource="http://www.fadyart.com/Finance.owl#ISOCodes"/>
    </rdf:Description>
    


    <!-- http://www.fadyart.com/financialInstruments#AccountIdentification -->

    <rdf:Description rdf:about="&fi;AccountIdentification">
        <rdfs:subClassOf rdf:resource="http://www.fadyart.com/Finance.owl#Account"/>
    </rdf:Description>
    


    <!-- http://www.fadyart.com/financialInstruments#AlternateInstrumentIdentification -->

    <rdf:Description rdf:about="&fi;AlternateInstrumentIdentification">
        <rdfs:subClassOf rdf:resource="http://www.fadyart.com/Finance.owl#FinancialInstrument"/>
    </rdf:Description>
    


    <!-- http://www.fadyart.com/financialInstruments#Instrument -->

    <rdf:Description rdf:about="&fi;Instrument">
        <rdfs:subClassOf rdf:resource="http://www.fadyart.com/Finance.owl#FinancialInstrument"/>
    </rdf:Description>
    


    <!-- http://www.fadyart.com/financialInstruments#InvolvedParty -->

    <rdf:Description rdf:about="&fi;InvolvedParty">
        <rdfs:subClassOf rdf:resource="http://www.fadyart.com/Finance.owl#FinancialInstrument"/>
    </rdf:Description>
    


    <!-- http://www.fadyart.com/financialInstruments#ValuePartition -->

    <rdf:Description rdf:about="&fi;ValuePartition">
        <rdfs:subClassOf rdf:resource="http://www.fadyart.com/Finance.owl#FinancialInstrument"/>
    </rdf:Description>
    


    <!-- http://www.fadyart.com/iso20022.owl#MessageDefinition -->

    <rdf:Description rdf:about="&iso20022;MessageDefinition">
        <rdfs:subClassOf rdf:resource="http://www.fadyart.com/Finance.owl#ISO20022-UNIFIMessages"/>
    </rdf:Description>
    


    <!-- http://www.fadyart.com/iso20022.owl#MessageFlow -->

    <rdf:Description rdf:about="&iso20022;MessageFlow">
        <rdfs:subClassOf rdf:resource="http://www.fadyart.com/Finance.owl#ISO20022-UNIFIMessages"/>
    </rdf:Description>
    


    <!-- http://www.fadyart.com/markets#ISO10383-MarketIdentifierCodes -->

    <rdf:Description rdf:about="&mic;ISO10383-MarketIdentifierCodes">
        <rdfs:subClassOf rdf:resource="http://www.fadyart.com/Finance.owl#ISOCodes"/>
    </rdf:Description>
    


    <!-- http://www.fadyart.com/parties#Blacklists -->

    <rdf:Description rdf:about="&parties;Blacklists">
        <rdfs:subClassOf rdf:resource="http://www.fadyart.com/Finance.owl#InvolvedParty"/>
    </rdf:Description>
    


    <!-- http://www.fadyart.com/parties#Citizenship -->

    <rdf:Description rdf:about="&parties;Citizenship">
        <rdfs:subClassOf rdf:resource="http://www.fadyart.com/Finance.owl#InvolvedParty"/>
    </rdf:Description>
    


    <!-- http://www.fadyart.com/parties#ClearingSystemMemberIdentification -->

    <rdf:Description rdf:about="&parties;ClearingSystemMemberIdentification">
        <rdfs:subClassOf rdf:resource="http://www.fadyart.com/Finance.owl#FinancialInstrument"/>
    </rdf:Description>
    


    <!-- http://www.fadyart.com/parties#ComplianceQuestionnaire -->

    <rdf:Description rdf:about="&parties;ComplianceQuestionnaire">
        <rdfs:subClassOf rdf:resource="http://www.fadyart.com/Finance.owl#InvolvedParty"/>
    </rdf:Description>
    


    <!-- http://www.fadyart.com/parties#ComplianceValidationProfile -->

    <rdf:Description rdf:about="&parties;ComplianceValidationProfile">
        <rdfs:subClassOf rdf:resource="http://www.fadyart.com/Finance.owl#InvolvedParty"/>
    </rdf:Description>
    


    <!-- http://www.fadyart.com/parties#Contact -->

    <rdf:Description rdf:about="&parties;Contact">
        <rdfs:label xml:lang="en">Address</rdfs:label>
    </rdf:Description>
    


    <!-- http://www.fadyart.com/parties#ContactInformation -->

    <rdf:Description rdf:about="&parties;ContactInformation">
        <rdfs:subClassOf rdf:resource="http://www.fadyart.com/Finance.owl#InvolvedParty"/>
    </rdf:Description>
    


    <!-- http://www.fadyart.com/parties#CountryAndResidentialStatus -->

    <rdf:Description rdf:about="&parties;CountryAndResidentialStatus">
        <rdfs:subClassOf rdf:resource="http://www.fadyart.com/Finance.owl#InvolvedParty"/>
    </rdf:Description>
    


    <!-- http://www.fadyart.com/parties#GenericIdentification -->

    <rdf:Description rdf:about="&parties;GenericIdentification">
        <rdfs:subClassOf rdf:resource="http://www.fadyart.com/Finance.owl#InvolvedParty"/>
    </rdf:Description>
    


    <!-- http://www.fadyart.com/parties#OrganisationIdentification -->

    <rdf:Description rdf:about="&parties;OrganisationIdentification">
        <rdfs:subClassOf rdf:resource="http://www.fadyart.com/Finance.owl#InvolvedParty"/>
    </rdf:Description>
    


    <!-- http://www.fadyart.com/parties#Party -->

    <rdf:Description rdf:about="&parties;Party">
        <rdfs:subClassOf rdf:resource="http://www.fadyart.com/Finance.owl#InvolvedParty"/>
    </rdf:Description>
    


    <!-- http://www.fadyart.com/parties#PcsClientRelated -->

    <rdf:Description rdf:about="&parties;PcsClientRelated">
        <rdfs:subClassOf rdf:resource="http://www.fadyart.com/Finance.owl#InvolvedParty"/>
    </rdf:Description>
    


    <!-- http://www.fadyart.com/parties#ProprietaryIdentification -->

    <rdf:Description rdf:about="&parties;ProprietaryIdentification">
        <rdfs:subClassOf rdf:resource="http://www.fadyart.com/Finance.owl#InvolvedParty"/>
    </rdf:Description>
    


    <!-- http://www.fadyart.com/parties#ValuePartition -->

    <rdf:Description rdf:about="&parties;ValuePartition">
        <rdfs:subClassOf rdf:resource="http://www.fadyart.com/Finance.owl#InvolvedParty"/>
    </rdf:Description>
    


    <!-- http://www.w3.org/2002/07/owl#Thing -->

    <owl:Class rdf:about="&owl;Thing">
        <rdfs:label rdf:datatype="&xsd;string">Finance</rdfs:label>
        <dc:rights rdf:datatype="&xsd;string">The finance ontology and the website pages of Eddy Vanderlinden are licensed according 
Creative Commons Attribution-Share alike 2.0 Belgium license.</dc:rights>
    </owl:Class>
    


    <!-- 
    ///////////////////////////////////////////////////////////////////////////////////////
    //
    // Individuals
    //
    ///////////////////////////////////////////////////////////////////////////////////////
     -->

    


    <!-- http://www.fadyart.com/Finance.owl#Template -->

    <owl:NamedIndividual rdf:about="http://www.fadyart.com/Finance.owl#Template">
        <rdf:type rdf:resource="&spin;Template"/>
    </owl:NamedIndividual>
    


    <!-- http://www.fadyart.com/Finance.owl#UsedCountriesAsFiscalResidence -->

    <owl:NamedIndividual rdf:about="http://www.fadyart.com/Finance.owl#UsedCountriesAsFiscalResidence">
        <rdf:type rdf:resource="&sp;Select"/>
        <rdfs:label rdf:datatype="&xsd;string">Used countries as fiscal residence</rdfs:label>
    </owl:NamedIndividual>
    


    <!-- http://www.fadyart.com/Finance.owl#XNStatusN -->

    <owl:NamedIndividual rdf:about="http://www.fadyart.com/Finance.owl#XNStatusN">
        <rdf:type rdf:resource="http://www.fadyart.com/Finance.owl#XNStatus"/>
    </owl:NamedIndividual>
    


    <!-- http://www.fadyart.com/Finance.owl#XNStatusX -->

    <owl:NamedIndividual rdf:about="http://www.fadyart.com/Finance.owl#XNStatusX">
        <rdf:type rdf:resource="http://www.fadyart.com/Finance.owl#XNStatus"/>
    </owl:NamedIndividual>
    


    <!-- http://www.fadyart.com/Finance.owl#acctFreezeDecease -->

    <owl:NamedIndividual rdf:about="http://www.fadyart.com/Finance.owl#acctFreezeDecease">
        <rdf:type rdf:resource="http://www.fadyart.com/Finance.owl#ReasonForAccountFreeze"/>
        <rdfs:label xml:lang="en">Decease</rdfs:label>
        <rdfs:comment xml:lang="en">The account is frozen due to the decease of one of the account-holders.</rdfs:comment>
    </owl:NamedIndividual>
    


    <!-- http://www.fadyart.com/Finance.owl#acctFreezeDescent -->

    <owl:NamedIndividual rdf:about="http://www.fadyart.com/Finance.owl#acctFreezeDescent">
        <rdf:type rdf:resource="http://www.fadyart.com/Finance.owl#ReasonForAccountFreeze"/>
        <rdfs:label xml:lang="en">Descent</rdfs:label>
        <rdfs:comment xml:lang="en">The account is frozen until a descent dispute is settled</rdfs:comment>
    </owl:NamedIndividual>
    


    <!-- http://www.fadyart.com/Finance.owl#acctFreezeDivorce -->

    <owl:NamedIndividual rdf:about="http://www.fadyart.com/Finance.owl#acctFreezeDivorce">
        <rdf:type rdf:resource="http://www.fadyart.com/Finance.owl#ReasonForAccountFreeze"/>
        <rdfs:label xml:lang="en">Divorce</rdfs:label>
        <rdfs:comment xml:lang="en">The reason for freezing the account is a divorce settlement</rdfs:comment>
    </owl:NamedIndividual>
    


    <!-- http://www.fadyart.com/Finance.owl#acctFreezeFiscalDispute -->

    <owl:NamedIndividual rdf:about="http://www.fadyart.com/Finance.owl#acctFreezeFiscalDispute">
        <rdf:type rdf:resource="http://www.fadyart.com/Finance.owl#ReasonForAccountFreeze"/>
        <rdfs:label xml:lang="en">Fiscal dispute</rdfs:label>
        <rdfs:comment xml:lang="en">The account is frozen until a dispute with the fiscal administration is settled.</rdfs:comment>
    </owl:NamedIndividual>
    


    <!-- http://www.fadyart.com/Finance.owl#acctFreezeFiscalInvestigation -->

    <owl:NamedIndividual rdf:about="http://www.fadyart.com/Finance.owl#acctFreezeFiscalInvestigation">
        <rdf:type rdf:resource="http://www.fadyart.com/Finance.owl#ReasonForAccountFreeze"/>
        <rdfs:label xml:lang="en">Fiscal investigation</rdfs:label>
        <rdfs:comment xml:lang="en">The account is frozen due to a fiscal investigation</rdfs:comment>
    </owl:NamedIndividual>
    


    <!-- http://www.fadyart.com/Finance.owl#acctFreezeIncapacities -->

    <owl:NamedIndividual rdf:about="http://www.fadyart.com/Finance.owl#acctFreezeIncapacities">
        <rdf:type rdf:resource="http://www.fadyart.com/Finance.owl#ReasonForAccountFreeze"/>
        <rdfs:label xml:lang="en">Incapacities</rdfs:label>
        <rdfs:comment xml:lang="en">The account is frozen due to incapacity occurances with the holders or mandated persons.</rdfs:comment>
    </owl:NamedIndividual>
    


    <!-- http://www.fadyart.com/Finance.owl#acctFreezeInheritance -->

    <owl:NamedIndividual rdf:about="http://www.fadyart.com/Finance.owl#acctFreezeInheritance">
        <rdf:type rdf:resource="http://www.fadyart.com/Finance.owl#ReasonForAccountFreeze"/>
        <rdfs:label xml:lang="en">Inheritance dispute</rdfs:label>
        <rdfs:comment xml:lang="en">The account is frozen to solve an inheritance dispute.</rdfs:comment>
    </owl:NamedIndividual>
    


    <!-- http://www.fadyart.com/Finance.owl#acctFreezeJuridicalInvestigation -->

    <owl:NamedIndividual rdf:about="http://www.fadyart.com/Finance.owl#acctFreezeJuridicalInvestigation">
        <rdf:type rdf:resource="http://www.fadyart.com/Finance.owl#ReasonForAccountFreeze"/>
        <rdfs:label xml:lang="en">Juridical investigation</rdfs:label>
        <rdfs:comment xml:lang="en">The account is frozen due to a juridical investigation</rdfs:comment>
    </owl:NamedIndividual>
    


    <!-- http://www.fadyart.com/Finance.owl#acctFreezeJusticeOfThePeace -->

    <owl:NamedIndividual rdf:about="http://www.fadyart.com/Finance.owl#acctFreezeJusticeOfThePeace">
        <rdf:type rdf:resource="http://www.fadyart.com/Finance.owl#ReasonForAccountFreeze"/>
        <rdfs:label xml:lang="en">justice of the peace</rdfs:label>
        <rdfs:comment xml:lang="en">The account is frozen until a dispute before the justice of peace is settled.</rdfs:comment>
    </owl:NamedIndividual>
    


    <!-- http://www.fadyart.com/Finance.owl#acctFreezeSeizure -->

    <owl:NamedIndividual rdf:about="http://www.fadyart.com/Finance.owl#acctFreezeSeizure">
        <rdf:type rdf:resource="http://www.fadyart.com/Finance.owl#ReasonForAccountFreeze"/>
        <rdfs:label xml:lang="en">Seizure</rdfs:label>
        <rdfs:comment xml:lang="en">The account is frozen due to a seizure by a juridical administration.</rdfs:comment>
    </owl:NamedIndividual>
    


    <!-- http://www.fadyart.com/Finance.owl#acctFreezeWidowship -->

    <owl:NamedIndividual rdf:about="http://www.fadyart.com/Finance.owl#acctFreezeWidowship">
        <rdf:type rdf:resource="http://www.fadyart.com/Finance.owl#ReasonForAccountFreeze"/>
        <rdfs:label xml:lang="en">widow(er)</rdfs:label>
        <rdfs:comment xml:lang="en">In some countries, if the holder becomes widow(er) the account has to be frozen until the legacy is settled according to the matrimonial status of the deceased.</rdfs:comment>
    </owl:NamedIndividual>
    


    <!-- http://www.fadyart.com/Finance.owl#channelBackOfficeInterfaces -->

    <owl:NamedIndividual rdf:about="http://www.fadyart.com/Finance.owl#channelBackOfficeInterfaces">
        <rdf:type rdf:resource="http://www.fadyart.com/Finance.owl#AdministrationChannel"/>
    </owl:NamedIndividual>
    


    <!-- http://www.fadyart.com/Finance.owl#channelInstitutionalBanking -->

    <owl:NamedIndividual rdf:about="http://www.fadyart.com/Finance.owl#channelInstitutionalBanking">
        <rdf:type rdf:resource="http://www.fadyart.com/Finance.owl#AdministrationChannel"/>
    </owl:NamedIndividual>
    


    <!-- http://www.fadyart.com/Finance.owl#channelMerchantBanking -->

    <owl:NamedIndividual rdf:about="http://www.fadyart.com/Finance.owl#channelMerchantBanking">
        <rdf:type rdf:resource="http://www.fadyart.com/Finance.owl#AdministrationChannel"/>
    </owl:NamedIndividual>
    


    <!-- http://www.fadyart.com/Finance.owl#channelPhoneBanking -->

    <owl:NamedIndividual rdf:about="http://www.fadyart.com/Finance.owl#channelPhoneBanking">
        <rdf:type rdf:resource="http://www.fadyart.com/Finance.owl#AdministrationChannel"/>
    </owl:NamedIndividual>
    


    <!-- http://www.fadyart.com/Finance.owl#channelPrivateBanking -->

    <owl:NamedIndividual rdf:about="http://www.fadyart.com/Finance.owl#channelPrivateBanking">
        <rdf:type rdf:resource="http://www.fadyart.com/Finance.owl#AdministrationChannel"/>
    </owl:NamedIndividual>
    


    <!-- http://www.fadyart.com/Finance.owl#channelRetailOffices -->

    <owl:NamedIndividual rdf:about="http://www.fadyart.com/Finance.owl#channelRetailOffices">
        <rdf:type rdf:resource="http://www.fadyart.com/Finance.owl#AdministrationChannel"/>
    </owl:NamedIndividual>
    


    <!-- http://www.fadyart.com/Finance.owl#channelWebBanking -->

    <owl:NamedIndividual rdf:about="http://www.fadyart.com/Finance.owl#channelWebBanking">
        <rdf:type rdf:resource="http://www.fadyart.com/Finance.owl#AdministrationChannel"/>
    </owl:NamedIndividual>
    


    <!-- http://www.fadyart.com/Finance.owl#extremelyHighDirectStockPriceImpact -->

    <owl:NamedIndividual rdf:about="http://www.fadyart.com/Finance.owl#extremelyHighDirectStockPriceImpact">
        <rdf:type rdf:resource="http://www.fadyart.com/Finance.owl#HighStockPriceImpact"/>
        <rdfs:label rdf:datatype="&xsd;string">Extremely high direct stock price impact</rdfs:label>
    </owl:NamedIndividual>
    


    <!-- http://www.fadyart.com/Finance.owl#extremelyHighIndirectStockPriceImpact -->

    <owl:NamedIndividual rdf:about="http://www.fadyart.com/Finance.owl#extremelyHighIndirectStockPriceImpact">
        <rdf:type rdf:resource="http://www.fadyart.com/Finance.owl#HighStockPriceImpact"/>
        <rdfs:label rdf:datatype="&xsd;string">Extremely high indirect stcok price impact</rdfs:label>
    </owl:NamedIndividual>
    


    <!-- http://www.fadyart.com/Finance.owl#extremelyHighProfitabilityImpact -->

    <owl:NamedIndividual rdf:about="http://www.fadyart.com/Finance.owl#extremelyHighProfitabilityImpact">
        <rdf:type rdf:resource="http://www.fadyart.com/Finance.owl#HighProfitabilityImpact"/>
        <rdfs:label rdf:datatype="&xsd;string">Extremely high profitability impact</rdfs:label>
    </owl:NamedIndividual>
    


    <!-- http://www.fadyart.com/Finance.owl#extremelyHighSolvabilityImpact -->

    <owl:NamedIndividual rdf:about="http://www.fadyart.com/Finance.owl#extremelyHighSolvabilityImpact">
        <rdf:type rdf:resource="http://www.fadyart.com/Finance.owl#HighSolvabilityImpact"/>
        <rdfs:label rdf:datatype="&xsd;string">Extremely high solvability impact</rdfs:label>
    </owl:NamedIndividual>
    


    <!-- http://www.fadyart.com/Finance.owl#genericAntiMoneyLaunderingUnit -->

    <owl:NamedIndividual rdf:about="http://www.fadyart.com/Finance.owl#genericAntiMoneyLaunderingUnit">
        <rdf:type rdf:resource="http://www.fadyart.com/Finance.owl#Compliance"/>
        <rdfs:label xml:lang="en">generic Anti-Money Laundering Unit</rdfs:label>
        <rdfs:comment xml:lang="en">The unit which performs investigations on client integrity risks and provides advice to the requestors on the opportunity of client relations.</rdfs:comment>
    </owl:NamedIndividual>
    


    <!-- http://www.fadyart.com/Finance.owl#genericBranchInstitutionalBanking -->

    <owl:NamedIndividual rdf:about="http://www.fadyart.com/Finance.owl#genericBranchInstitutionalBanking">
        <rdf:type rdf:resource="http://www.fadyart.com/Finance.owl#InstitutionalBanking"/>
        <hasAccessToChannel rdf:resource="http://www.fadyart.com/Finance.owl#channelInstitutionalBanking"/>
    </owl:NamedIndividual>
    


    <!-- http://www.fadyart.com/Finance.owl#genericBranchMerchantBanking -->

    <owl:NamedIndividual rdf:about="http://www.fadyart.com/Finance.owl#genericBranchMerchantBanking">
        <rdf:type rdf:resource="http://www.fadyart.com/Finance.owl#MerchantBanking"/>
        <hasAccessToChannel rdf:resource="http://www.fadyart.com/Finance.owl#channelMerchantBanking"/>
    </owl:NamedIndividual>
    


    <!-- http://www.fadyart.com/Finance.owl#genericBranchPrivateBanking -->

    <owl:NamedIndividual rdf:about="http://www.fadyart.com/Finance.owl#genericBranchPrivateBanking">
        <rdf:type rdf:resource="http://www.fadyart.com/Finance.owl#PrivateBanking"/>
        <hasAccessToChannel rdf:resource="http://www.fadyart.com/Finance.owl#channelPrivateBanking"/>
    </owl:NamedIndividual>
    


    <!-- http://www.fadyart.com/Finance.owl#genericBranchRetailBanking -->

    <owl:NamedIndividual rdf:about="http://www.fadyart.com/Finance.owl#genericBranchRetailBanking">
        <rdf:type rdf:resource="http://www.fadyart.com/Finance.owl#RetailBanking"/>
        <hasAccessToChannel rdf:resource="http://www.fadyart.com/Finance.owl#channelRetailOffices"/>
    </owl:NamedIndividual>
    


    <!-- http://www.fadyart.com/Finance.owl#genericClientPortfolio1 -->

    <owl:NamedIndividual rdf:about="http://www.fadyart.com/Finance.owl#genericClientPortfolio1">
        <rdf:type rdf:resource="http://www.fadyart.com/Finance.owl#ClientPortfolio"/>
        <isAccessibleViaChannel rdf:resource="http://www.fadyart.com/Finance.owl#channelBackOfficeInterfaces"/>
        <isAccessibleViaChannel rdf:resource="http://www.fadyart.com/Finance.owl#channelRetailOffices"/>
        <hasValidityPeriod rdf:resource="http://www.fadyart.com/Finance.owl#period1"/>
        <hasClientPortfolioBeneficialOwnerCapital rdf:resource="&parties;genericPartyHolder1"/>
        <hasClientPortfolioBeneficialOwnerIncome rdf:resource="&parties;genericPartyHolder1"/>
        <hasContactPerson rdf:resource="&parties;genericPartyHolder1"/>
        <hasAsPrincipal rdf:resource="&parties;genericPrincipal1"/>
    </owl:NamedIndividual>
    


    <!-- http://www.fadyart.com/Finance.owl#genericClientPortfolio2 -->

    <owl:NamedIndividual rdf:about="http://www.fadyart.com/Finance.owl#genericClientPortfolio2">
        <rdf:type rdf:resource="http://www.fadyart.com/Finance.owl#ClientPortfolio"/>
        <isAccessibleViaChannel rdf:resource="http://www.fadyart.com/Finance.owl#channelBackOfficeInterfaces"/>
        <isAccessibleViaChannel rdf:resource="http://www.fadyart.com/Finance.owl#channelRetailOffices"/>
        <hasValidityPeriod rdf:resource="http://www.fadyart.com/Finance.owl#period1"/>
        <hasClientPortfolioBeneficialOwnerIncome rdf:resource="&parties;genericPartyHolder1"/>
        <hasContactPerson rdf:resource="&parties;genericPartyHolder1"/>
        <hasClientPortfolioBeneficialOwnerCapital rdf:resource="&parties;genericPartyHolder2"/>
        <hasAsPrincipal rdf:resource="&parties;genericPrincipal1"/>
    </owl:NamedIndividual>
    


    <!-- http://www.fadyart.com/Finance.owl#genericClientPortfolio3 -->

    <owl:NamedIndividual rdf:about="http://www.fadyart.com/Finance.owl#genericClientPortfolio3">
        <rdf:type rdf:resource="http://www.fadyart.com/Finance.owl#ClientPortfolio"/>
        <isAccessibleViaChannel rdf:resource="http://www.fadyart.com/Finance.owl#channelBackOfficeInterfaces"/>
        <isAccessibleViaChannel rdf:resource="http://www.fadyart.com/Finance.owl#channelRetailOffices"/>
        <hasValidityPeriod rdf:resource="http://www.fadyart.com/Finance.owl#period1"/>
        <hasClientPortfolioBeneficialOwnerCapital rdf:resource="&parties;genericPartyHolder2"/>
        <hasContactPerson rdf:resource="&parties;genericPartyHolder2"/>
        <hasClientPortfolioBeneficialOwnerIncome rdf:resource="&parties;genericPartyHolder2"/>
        <hasAsPrincipal rdf:resource="&parties;genericPrincipal2"/>
    </owl:NamedIndividual>
    


    <!-- http://www.fadyart.com/Finance.owl#genericEntityAccounting -->

    <owl:NamedIndividual rdf:about="http://www.fadyart.com/Finance.owl#genericEntityAccounting">
        <rdf:type rdf:resource="http://www.fadyart.com/Finance.owl#Accounting"/>
        <hasAccessToChannel rdf:resource="http://www.fadyart.com/Finance.owl#channelBackOfficeInterfaces"/>
    </owl:NamedIndividual>
    


    <!-- http://www.fadyart.com/Finance.owl#genericEntityCashAccountsAndCards -->

    <owl:NamedIndividual rdf:about="http://www.fadyart.com/Finance.owl#genericEntityCashAccountsAndCards">
        <rdf:type rdf:resource="http://www.fadyart.com/Finance.owl#CashAccountsAndCards"/>
        <hasAccessToChannel rdf:resource="http://www.fadyart.com/Finance.owl#channelBackOfficeInterfaces"/>
    </owl:NamedIndividual>
    


    <!-- http://www.fadyart.com/Finance.owl#genericEntityCorporateAction -->

    <owl:NamedIndividual rdf:about="http://www.fadyart.com/Finance.owl#genericEntityCorporateAction">
        <rdf:type rdf:resource="http://www.fadyart.com/Finance.owl#CorporateAction"/>
        <hasAccessToChannel rdf:resource="http://www.fadyart.com/Finance.owl#channelBackOfficeInterfaces"/>
    </owl:NamedIndividual>
    


    <!-- http://www.fadyart.com/Finance.owl#genericEntityCredit -->

    <owl:NamedIndividual rdf:about="http://www.fadyart.com/Finance.owl#genericEntityCredit">
        <rdf:type rdf:resource="http://www.fadyart.com/Finance.owl#Credit"/>
        <hasAccessToChannel rdf:resource="http://www.fadyart.com/Finance.owl#channelBackOfficeInterfaces"/>
    </owl:NamedIndividual>
    


    <!-- http://www.fadyart.com/Finance.owl#genericEntityCustomerReferential -->

    <owl:NamedIndividual rdf:about="http://www.fadyart.com/Finance.owl#genericEntityCustomerReferential">
        <rdf:type rdf:resource="http://www.fadyart.com/Finance.owl#CustomerReferential"/>
        <hasAccessToChannel rdf:resource="http://www.fadyart.com/Finance.owl#channelBackOfficeInterfaces"/>
    </owl:NamedIndividual>
    


    <!-- http://www.fadyart.com/Finance.owl#genericEntityGlobalMarkets -->

    <owl:NamedIndividual rdf:about="http://www.fadyart.com/Finance.owl#genericEntityGlobalMarkets">
        <rdf:type rdf:resource="http://www.fadyart.com/Finance.owl#GlobalMarkets"/>
        <hasAccessToChannel rdf:resource="http://www.fadyart.com/Finance.owl#channelBackOfficeInterfaces"/>
    </owl:NamedIndividual>
    


    <!-- http://www.fadyart.com/Finance.owl#genericEntityPrimaryMarket -->

    <owl:NamedIndividual rdf:about="http://www.fadyart.com/Finance.owl#genericEntityPrimaryMarket">
        <rdf:type rdf:resource="http://www.fadyart.com/Finance.owl#PrimaryMarket"/>
        <hasAccessToChannel rdf:resource="http://www.fadyart.com/Finance.owl#channelBackOfficeInterfaces"/>
    </owl:NamedIndividual>
    


    <!-- http://www.fadyart.com/Finance.owl#genericEntityReferentialSystems -->

    <owl:NamedIndividual rdf:about="http://www.fadyart.com/Finance.owl#genericEntityReferentialSystems">
        <rdf:type rdf:resource="http://www.fadyart.com/Finance.owl#ReferentialSystem"/>
        <hasAccessToChannel rdf:resource="http://www.fadyart.com/Finance.owl#channelBackOfficeInterfaces"/>
    </owl:NamedIndividual>
    


    <!-- http://www.fadyart.com/Finance.owl#genericEntitySecundaryMarkets -->

    <owl:NamedIndividual rdf:about="http://www.fadyart.com/Finance.owl#genericEntitySecundaryMarkets">
        <rdf:type rdf:resource="http://www.fadyart.com/Finance.owl#SecundaryMarket"/>
        <hasAccessToChannel rdf:resource="http://www.fadyart.com/Finance.owl#channelBackOfficeInterfaces"/>
    </owl:NamedIndividual>
    


    <!-- http://www.fadyart.com/Finance.owl#genericNostroCashAccount1 -->

    <owl:NamedIndividual rdf:about="http://www.fadyart.com/Finance.owl#genericNostroCashAccount1">
        <rdf:type rdf:resource="http://www.fadyart.com/Finance.owl#NostroCashAccount"/>
        <isAccessibleViaChannel rdf:resource="http://www.fadyart.com/Finance.owl#channelBackOfficeInterfaces"/>
        <isAccessibleViaChannel rdf:resource="http://www.fadyart.com/Finance.owl#channelInstitutionalBanking"/>
        <hasValidityPeriod rdf:resource="http://www.fadyart.com/Finance.owl#period1"/>
        <hasClientPortfolioBeneficialOwnerIncome rdf:resource="&parties;genericPartyHolder1"/>
        <hasClientPortfolioBeneficialOwnerCapital rdf:resource="&parties;genericPartyHolder1"/>
        <hasContactPerson rdf:resource="&parties;genericPartyHolder1"/>
        <hasAsPrincipal rdf:resource="&parties;genericPrincipal1"/>
    </owl:NamedIndividual>
    


    <!-- http://www.fadyart.com/Finance.owl#genericNostroCashAccount2 -->

    <owl:NamedIndividual rdf:about="http://www.fadyart.com/Finance.owl#genericNostroCashAccount2">
        <rdf:type rdf:resource="http://www.fadyart.com/Finance.owl#NostroCashAccount"/>
        <isAccessibleViaChannel rdf:resource="http://www.fadyart.com/Finance.owl#channelBackOfficeInterfaces"/>
        <isAccessibleViaChannel rdf:resource="http://www.fadyart.com/Finance.owl#channelInstitutionalBanking"/>
        <hasValidityPeriod rdf:resource="http://www.fadyart.com/Finance.owl#period1"/>
        <hasContactPerson rdf:resource="&parties;genericPartyHolder2"/>
        <hasClientPortfolioBeneficialOwnerCapital rdf:resource="&parties;genericPartyHolder2"/>
        <hasClientPortfolioBeneficialOwnerIncome rdf:resource="&parties;genericPartyHolder2"/>
        <hasAsPrincipal rdf:resource="&parties;genericPrincipal2"/>
    </owl:NamedIndividual>
    


    <!-- http://www.fadyart.com/Finance.owl#genericNostroSecuritiesAccount1 -->

    <owl:NamedIndividual rdf:about="http://www.fadyart.com/Finance.owl#genericNostroSecuritiesAccount1">
        <rdf:type rdf:resource="http://www.fadyart.com/Finance.owl#NostroSecuritiesAccount"/>
        <isAccessibleViaChannel rdf:resource="http://www.fadyart.com/Finance.owl#channelBackOfficeInterfaces"/>
        <isAccessibleViaChannel rdf:resource="http://www.fadyart.com/Finance.owl#channelInstitutionalBanking"/>
        <hasValidityPeriod rdf:resource="http://www.fadyart.com/Finance.owl#period1"/>
        <hasClientPortfolioBeneficialOwnerIncome rdf:resource="&parties;genericPartyHolder1"/>
        <hasContactPerson rdf:resource="&parties;genericPartyHolder1"/>
        <hasClientPortfolioBeneficialOwnerCapital rdf:resource="&parties;genericPartyHolder1"/>
        <hasAsPrincipal rdf:resource="&parties;genericPrincipal1"/>
    </owl:NamedIndividual>
    


    <!-- http://www.fadyart.com/Finance.owl#genericNostroSecuritiesAccount2 -->

    <owl:NamedIndividual rdf:about="http://www.fadyart.com/Finance.owl#genericNostroSecuritiesAccount2">
        <rdf:type rdf:resource="http://www.fadyart.com/Finance.owl#NostroSecuritiesAccount"/>
        <isAccessibleViaChannel rdf:resource="http://www.fadyart.com/Finance.owl#channelBackOfficeInterfaces"/>
        <isAccessibleViaChannel rdf:resource="http://www.fadyart.com/Finance.owl#channelInstitutionalBanking"/>
        <hasValidityPeriod rdf:resource="http://www.fadyart.com/Finance.owl#period1"/>
        <hasContactPerson rdf:resource="&parties;genericPartyHolder2"/>
        <hasClientPortfolioBeneficialOwnerIncome rdf:resource="&parties;genericPartyHolder2"/>
        <hasClientPortfolioBeneficialOwnerCapital rdf:resource="&parties;genericPartyHolder2"/>
        <hasAsPrincipal rdf:resource="&parties;genericPrincipal2"/>
    </owl:NamedIndividual>
    


    <!-- http://www.fadyart.com/Finance.owl#genericProfile0 -->

    <owl:NamedIndividual rdf:about="http://www.fadyart.com/Finance.owl#genericProfile0">
        <rdf:type rdf:resource="http://www.fadyart.com/Finance.owl#Underlying-CollateralRiskProfile"/>
        <hasRiskSymptomSource rdf:datatype="&xsd;string">WSJ 2008-03-01</hasRiskSymptomSource>
        <hasRiskImpact rdf:resource="http://www.fadyart.com/Finance.owl#highIndirectStockPriceImpact"/>
        <hasRiskImpact rdf:resource="http://www.fadyart.com/Finance.owl#highProfitabilityImpact"/>
        <hasRiskImpact rdf:resource="http://www.fadyart.com/Finance.owl#highSolvabilityImpact"/>
        <hasRiskProbability rdf:resource="http://www.fadyart.com/Finance.owl#nearToCertaintyRiskProbability"/>
        <hasProfileValidityPeriod rdf:resource="http://www.fadyart.com/Finance.owl#period0"/>
        <hasRiskSymptom rdf:resource="http://www.fadyart.com/Finance.owl#rskSymptomUnderlying-CollateralWorthLoss"/>
        <hasRiskArea rdf:resource="http://www.fadyart.com/iso10962#B-MortgageBackedDebt"/>
    </owl:NamedIndividual>
    


    <!-- http://www.fadyart.com/Finance.owl#genericVostroCashAccount1 -->

    <owl:NamedIndividual rdf:about="http://www.fadyart.com/Finance.owl#genericVostroCashAccount1">
        <rdf:type rdf:resource="http://www.fadyart.com/Finance.owl#VostroCashAccount"/>
        <isAccessibleViaChannel rdf:resource="http://www.fadyart.com/Finance.owl#channelBackOfficeInterfaces"/>
        <isAccessibleViaChannel rdf:resource="http://www.fadyart.com/Finance.owl#channelInstitutionalBanking"/>
        <hasValidityPeriod rdf:resource="http://www.fadyart.com/Finance.owl#period1"/>
        <hasClientPortfolioBeneficialOwnerCapital rdf:resource="&parties;genericPartyHolder1"/>
        <hasContactPerson rdf:resource="&parties;genericPartyHolder1"/>
        <hasClientPortfolioBeneficialOwnerIncome rdf:resource="&parties;genericPartyHolder1"/>
        <hasAsPrincipal rdf:resource="&parties;genericPrincipal1"/>
    </owl:NamedIndividual>
    


    <!-- http://www.fadyart.com/Finance.owl#genericVostroCashAccount2 -->

    <owl:NamedIndividual rdf:about="http://www.fadyart.com/Finance.owl#genericVostroCashAccount2">
        <rdf:type rdf:resource="http://www.fadyart.com/Finance.owl#VostroCashAccount"/>
        <isAccessibleViaChannel rdf:resource="http://www.fadyart.com/Finance.owl#channelBackOfficeInterfaces"/>
        <isAccessibleViaChannel rdf:resource="http://www.fadyart.com/Finance.owl#channelInstitutionalBanking"/>
        <hasValidityPeriod rdf:resource="http://www.fadyart.com/Finance.owl#period1"/>
        <hasContactPerson rdf:resource="&parties;genericPartyHolder2"/>
        <hasClientPortfolioBeneficialOwnerIncome rdf:resource="&parties;genericPartyHolder2"/>
        <hasClientPortfolioBeneficialOwnerCapital rdf:resource="&parties;genericPartyHolder2"/>
        <hasAsPrincipal rdf:resource="&parties;genericPrincipal2"/>
    </owl:NamedIndividual>
    


    <!-- http://www.fadyart.com/Finance.owl#genericVostroSecuritiesAccount1 -->

    <owl:NamedIndividual rdf:about="http://www.fadyart.com/Finance.owl#genericVostroSecuritiesAccount1">
        <rdf:type rdf:resource="http://www.fadyart.com/Finance.owl#VostroSecuritiesAccount"/>
        <isAccessibleViaChannel rdf:resource="http://www.fadyart.com/Finance.owl#channelBackOfficeInterfaces"/>
        <isAccessibleViaChannel rdf:resource="http://www.fadyart.com/Finance.owl#channelInstitutionalBanking"/>
        <hasValidityPeriod rdf:resource="http://www.fadyart.com/Finance.owl#period1"/>
        <hasClientPortfolioBeneficialOwnerCapital rdf:resource="&parties;genericPartyHolder1"/>
        <hasContactPerson rdf:resource="&parties;genericPartyHolder1"/>
        <hasClientPortfolioBeneficialOwnerIncome rdf:resource="&parties;genericPartyHolder1"/>
        <hasAsPrincipal rdf:resource="&parties;genericPrincipal1"/>
    </owl:NamedIndividual>
    


    <!-- http://www.fadyart.com/Finance.owl#genericVostroSecuritiesAccount2 -->

    <owl:NamedIndividual rdf:about="http://www.fadyart.com/Finance.owl#genericVostroSecuritiesAccount2">
        <rdf:type rdf:resource="http://www.fadyart.com/Finance.owl#VostroSecuritiesAccount"/>
        <isAccessibleViaChannel rdf:resource="http://www.fadyart.com/Finance.owl#channelBackOfficeInterfaces"/>
        <isAccessibleViaChannel rdf:resource="http://www.fadyart.com/Finance.owl#channelInstitutionalBanking"/>
        <hasValidityPeriod rdf:resource="http://www.fadyart.com/Finance.owl#period1"/>
        <hasClientPortfolioBeneficialOwnerCapital rdf:resource="&parties;genericPartyHolder2"/>
        <hasClientPortfolioBeneficialOwnerIncome rdf:resource="&parties;genericPartyHolder2"/>
        <hasContactPerson rdf:resource="&parties;genericPartyHolder2"/>
        <hasAsPrincipal rdf:resource="&parties;genericPrincipal2"/>
    </owl:NamedIndividual>
    


    <!-- http://www.fadyart.com/Finance.owl#granularityDays -->

    <owl:NamedIndividual rdf:about="http://www.fadyart.com/Finance.owl#granularityDays">
        <rdf:type rdf:resource="http://www.fadyart.com/Finance.owl#Granularity"/>
    </owl:NamedIndividual>
    


    <!-- http://www.fadyart.com/Finance.owl#granularityHours -->

    <owl:NamedIndividual rdf:about="http://www.fadyart.com/Finance.owl#granularityHours">
        <rdf:type rdf:resource="http://www.fadyart.com/Finance.owl#Granularity"/>
    </owl:NamedIndividual>
    


    <!-- http://www.fadyart.com/Finance.owl#granularityMilliseconds -->

    <owl:NamedIndividual rdf:about="http://www.fadyart.com/Finance.owl#granularityMilliseconds">
        <rdf:type rdf:resource="http://www.fadyart.com/Finance.owl#Granularity"/>
    </owl:NamedIndividual>
    


    <!-- http://www.fadyart.com/Finance.owl#granularityMinutes -->

    <owl:NamedIndividual rdf:about="http://www.fadyart.com/Finance.owl#granularityMinutes">
        <rdf:type rdf:resource="http://www.fadyart.com/Finance.owl#Granularity"/>
    </owl:NamedIndividual>
    


    <!-- http://www.fadyart.com/Finance.owl#granularityMonths -->

    <owl:NamedIndividual rdf:about="http://www.fadyart.com/Finance.owl#granularityMonths">
        <rdf:type rdf:resource="http://www.fadyart.com/Finance.owl#Granularity"/>
    </owl:NamedIndividual>
    


    <!-- http://www.fadyart.com/Finance.owl#granularitySeconds -->

    <owl:NamedIndividual rdf:about="http://www.fadyart.com/Finance.owl#granularitySeconds">
        <rdf:type rdf:resource="http://www.fadyart.com/Finance.owl#Granularity"/>
    </owl:NamedIndividual>
    


    <!-- http://www.fadyart.com/Finance.owl#granularityWeeks -->

    <owl:NamedIndividual rdf:about="http://www.fadyart.com/Finance.owl#granularityWeeks">
        <rdf:type rdf:resource="http://www.fadyart.com/Finance.owl#Granularity"/>
    </owl:NamedIndividual>
    


    <!-- http://www.fadyart.com/Finance.owl#granularityYears -->

    <owl:NamedIndividual rdf:about="http://www.fadyart.com/Finance.owl#granularityYears">
        <rdf:type rdf:resource="http://www.fadyart.com/Finance.owl#Granularity"/>
    </owl:NamedIndividual>
    


    <!-- http://www.fadyart.com/Finance.owl#highDirectStockPriceImpact -->

    <owl:NamedIndividual rdf:about="http://www.fadyart.com/Finance.owl#highDirectStockPriceImpact">
        <rdf:type rdf:resource="http://www.fadyart.com/Finance.owl#HighStockPriceImpact"/>
        <rdfs:label rdf:datatype="&xsd;string">High direct stock price impact</rdfs:label>
    </owl:NamedIndividual>
    


    <!-- http://www.fadyart.com/Finance.owl#highIndirectStockPriceImpact -->

    <owl:NamedIndividual rdf:about="http://www.fadyart.com/Finance.owl#highIndirectStockPriceImpact">
        <rdf:type rdf:resource="http://www.fadyart.com/Finance.owl#HighStockPriceImpact"/>
        <rdfs:label rdf:datatype="&xsd;string">High indirect stock price impact</rdfs:label>
    </owl:NamedIndividual>
    


    <!-- http://www.fadyart.com/Finance.owl#highProfitabilityImpact -->

    <owl:NamedIndividual rdf:about="http://www.fadyart.com/Finance.owl#highProfitabilityImpact">
        <rdf:type rdf:resource="http://www.fadyart.com/Finance.owl#HighProfitabilityImpact"/>
        <rdfs:label rdf:datatype="&xsd;string">High profitability impact</rdfs:label>
    </owl:NamedIndividual>
    


    <!-- http://www.fadyart.com/Finance.owl#highRiskProbability -->

    <owl:NamedIndividual rdf:about="http://www.fadyart.com/Finance.owl#highRiskProbability">
        <rdf:type rdf:resource="http://www.fadyart.com/Finance.owl#HighRiskProbability"/>
        <rdfs:label rdf:datatype="&xsd;string">High risk probability</rdfs:label>
    </owl:NamedIndividual>
    


    <!-- http://www.fadyart.com/Finance.owl#highSolvabilityImpact -->

    <owl:NamedIndividual rdf:about="http://www.fadyart.com/Finance.owl#highSolvabilityImpact">
        <rdf:type rdf:resource="http://www.fadyart.com/Finance.owl#HighSolvabilityImpact"/>
        <rdfs:label rdf:datatype="&xsd;string">High solvability impact</rdfs:label>
    </owl:NamedIndividual>
    


    <!-- http://www.fadyart.com/Finance.owl#instant0 -->

    <owl:NamedIndividual rdf:about="http://www.fadyart.com/Finance.owl#instant0">
        <rdf:type rdf:resource="http://www.fadyart.com/Finance.owl#ValidInstant"/>
        <rdfs:label rdf:datatype="&xsd;string">Unknown instant</rdfs:label>
        <hasTime rdf:datatype="&xsd;dateTime">1902-01-01T09:00:08</hasTime>
    </owl:NamedIndividual>
    


    <!-- http://www.fadyart.com/Finance.owl#lowDirectStockPriceImpact -->

    <owl:NamedIndividual rdf:about="http://www.fadyart.com/Finance.owl#lowDirectStockPriceImpact">
        <rdf:type rdf:resource="http://www.fadyart.com/Finance.owl#LowStockPriceImpact"/>
        <rdfs:label rdf:datatype="&xsd;string">Low direct stock price impact</rdfs:label>
    </owl:NamedIndividual>
    


    <!-- http://www.fadyart.com/Finance.owl#lowIndirectStockPriceImpact -->

    <owl:NamedIndividual rdf:about="http://www.fadyart.com/Finance.owl#lowIndirectStockPriceImpact">
        <rdf:type rdf:resource="http://www.fadyart.com/Finance.owl#LowStockPriceImpact"/>
        <rdfs:label rdf:datatype="&xsd;string">Low indirect stock price impact</rdfs:label>
    </owl:NamedIndividual>
    


    <!-- http://www.fadyart.com/Finance.owl#lowProfitabilityImpact -->

    <owl:NamedIndividual rdf:about="http://www.fadyart.com/Finance.owl#lowProfitabilityImpact">
        <rdf:type rdf:resource="http://www.fadyart.com/Finance.owl#LowProfitabilityImpact"/>
        <rdfs:label rdf:datatype="&xsd;string">Low profitability impact</rdfs:label>
    </owl:NamedIndividual>
    


    <!-- http://www.fadyart.com/Finance.owl#lowRiskProbability -->

    <owl:NamedIndividual rdf:about="http://www.fadyart.com/Finance.owl#lowRiskProbability">
        <rdf:type rdf:resource="http://www.fadyart.com/Finance.owl#LowRiskProbability"/>
        <rdfs:label rdf:datatype="&xsd;string">Low risk probability</rdfs:label>
    </owl:NamedIndividual>
    


    <!-- http://www.fadyart.com/Finance.owl#lowSolvabilityImpact -->

    <owl:NamedIndividual rdf:about="http://www.fadyart.com/Finance.owl#lowSolvabilityImpact">
        <rdf:type rdf:resource="http://www.fadyart.com/Finance.owl#LowSolvabilityImpact"/>
        <rdfs:label rdf:datatype="&xsd;string">Low solvability impact</rdfs:label>
    </owl:NamedIndividual>
    


    <!-- http://www.fadyart.com/Finance.owl#mediumDirectStockPriceImpact -->

    <owl:NamedIndividual rdf:about="http://www.fadyart.com/Finance.owl#mediumDirectStockPriceImpact">
        <rdf:type rdf:resource="http://www.fadyart.com/Finance.owl#MediumStockPriceImpact"/>
        <rdfs:label rdf:datatype="&xsd;string">Medium direct stock price impact</rdfs:label>
    </owl:NamedIndividual>
    


    <!-- http://www.fadyart.com/Finance.owl#mediumIndirectStockPriceImpact -->

    <owl:NamedIndividual rdf:about="http://www.fadyart.com/Finance.owl#mediumIndirectStockPriceImpact">
        <rdf:type rdf:resource="http://www.fadyart.com/Finance.owl#MediumStockPriceImpact"/>
        <rdfs:label rdf:datatype="&xsd;string">Medium indirect stock price impact</rdfs:label>
    </owl:NamedIndividual>
    


    <!-- http://www.fadyart.com/Finance.owl#mediumProfitabilityImpact -->

    <owl:NamedIndividual rdf:about="http://www.fadyart.com/Finance.owl#mediumProfitabilityImpact">
        <rdf:type rdf:resource="http://www.fadyart.com/Finance.owl#MediumProfitabilityImpact"/>
        <rdfs:label rdf:datatype="&xsd;string">Medium profitability impact</rdfs:label>
    </owl:NamedIndividual>
    


    <!-- http://www.fadyart.com/Finance.owl#mediumRiskProbability -->

    <owl:NamedIndividual rdf:about="http://www.fadyart.com/Finance.owl#mediumRiskProbability">
        <rdf:type rdf:resource="http://www.fadyart.com/Finance.owl#MediumRiskProbability"/>
        <rdfs:label rdf:datatype="&xsd;string">Medium risk probability</rdfs:label>
    </owl:NamedIndividual>
    


    <!-- http://www.fadyart.com/Finance.owl#mediumSolvabilityImpact -->

    <owl:NamedIndividual rdf:about="http://www.fadyart.com/Finance.owl#mediumSolvabilityImpact">
        <rdf:type rdf:resource="http://www.fadyart.com/Finance.owl#MediumSolvabilityImpact"/>
        <rdfs:label rdf:datatype="&xsd;string">Medium solvability impact</rdfs:label>
    </owl:NamedIndividual>
    


    <!-- http://www.fadyart.com/Finance.owl#nearToCertaintyRiskProbability -->

    <owl:NamedIndividual rdf:about="http://www.fadyart.com/Finance.owl#nearToCertaintyRiskProbability">
        <rdf:type rdf:resource="http://www.fadyart.com/Finance.owl#HighRiskProbability"/>
        <rdfs:label rdf:datatype="&xsd;string">Near to certainty</rdfs:label>
    </owl:NamedIndividual>
    


    <!-- http://www.fadyart.com/Finance.owl#nearToNoRiskProbability -->

    <owl:NamedIndividual rdf:about="http://www.fadyart.com/Finance.owl#nearToNoRiskProbability">
        <rdf:type rdf:resource="http://www.fadyart.com/Finance.owl#LowRiskProbability"/>
        <rdfs:label rdf:datatype="&xsd;string">Near to no risk</rdfs:label>
    </owl:NamedIndividual>
    


    <!-- http://www.fadyart.com/Finance.owl#pcsTrgAbnormalTransaction -->

    <owl:NamedIndividual rdf:about="http://www.fadyart.com/Finance.owl#pcsTrgAbnormalTransaction">
        <rdf:type rdf:resource="http://www.fadyart.com/Finance.owl#ProcessTrigger"/>
        <rdfs:label xml:lang="en">Abnormal transaction</rdfs:label>
        <rdfs:comment xml:lang="en">Some exemples of abnormal transactions:
- the information provided arround the transaction is incorrect or irrealistic;
- the bank has no knowledge about the source of the funds;
- the customer requests parial transfers so that the global amount of the transaction remains hidden;
- client is interested only in speed of the transaction, not in the costs related to the transaction, including exchange costs;
- the client questions about the obligations of financial institutions in matthers of money laundering;</rdfs:comment>
        <isTriggerFor rdf:resource="&parties;pcdCERegisterBirthAndDeceaseInformation"/>
    </owl:NamedIndividual>
    


    <!-- http://www.fadyart.com/Finance.owl#pcsTrgNewClientRelation -->

    <owl:NamedIndividual rdf:about="http://www.fadyart.com/Finance.owl#pcsTrgNewClientRelation">
        <rdf:type rdf:resource="http://www.fadyart.com/Finance.owl#ProcessTrigger"/>
        <rdfs:label xml:lang="en">New client relation</rdfs:label>
        <rdfs:comment xml:lang="en">A new client relation is a trigger to make a client assesment from compliance point of view.</rdfs:comment>
        <isTriggerFor rdf:resource="&parties;pcdCECreateIndividualParty"/>
    </owl:NamedIndividual>
    


    <!-- http://www.fadyart.com/Finance.owl#pcsTrgTransactionAmount -->

    <owl:NamedIndividual rdf:about="http://www.fadyart.com/Finance.owl#pcsTrgTransactionAmount">
        <rdf:type rdf:resource="http://www.fadyart.com/Finance.owl#ProcessTrigger"/>
        <rdfs:label xml:lang="en">Transaction amount</rdfs:label>
        <rdfs:comment xml:lang="en">The treshold for an eventual evaluation lies following the recommendations of FATF on 15 000 EUR/USD.
This does not mean an investigation will take place for each transaction of 15 000 EUR/USD.</rdfs:comment>
        <isTriggerFor rdf:resource="&parties;pcdCERegisterBirthAndDeceaseInformation"/>
    </owl:NamedIndividual>
    


    <!-- http://www.fadyart.com/Finance.owl#pcsTrgUnusualTransaction -->

    <owl:NamedIndividual rdf:about="http://www.fadyart.com/Finance.owl#pcsTrgUnusualTransaction">
        <rdf:type rdf:resource="http://www.fadyart.com/Finance.owl#ProcessTrigger"/>
        <rdfs:label xml:lang="en">Unusual transaction</rdfs:label>
        <rdfs:comment xml:lang="en">Some exemples of unusual transactions:
- the transaction is unusual in respect of the known standing of the client;
- the transaction is unusual in respect of the activities performed by the client;
- the transaction is unusual in respect of the known turn-over on the client&apos;s account;
- there is no justification nor documentation on the trasnaction;
- the client&apos;s transactions are not for own account</rdfs:comment>
        <isTriggerFor rdf:resource="&parties;pcdCERegisterBirthAndDeceaseInformation"/>
    </owl:NamedIndividual>
    


    <!-- http://www.fadyart.com/Finance.owl#period0 -->

    <owl:NamedIndividual rdf:about="http://www.fadyart.com/Finance.owl#period0">
        <rdf:type rdf:resource="http://www.fadyart.com/Finance.owl#ValidPeriod"/>
        <rdfs:label rdf:datatype="&xsd;string">Unknown begin- and end date</rdfs:label>
        <hasStartTime rdf:datatype="&xsd;dateTime">1902-01-01T09:00:08</hasStartTime>
        <hasFinishTime rdf:datatype="&xsd;dateTime">2999-12-31T09:00:08</hasFinishTime>
    </owl:NamedIndividual>
    


    <!-- http://www.fadyart.com/Finance.owl#period1 -->

    <owl:NamedIndividual rdf:about="http://www.fadyart.com/Finance.owl#period1">
        <rdf:type rdf:resource="http://www.fadyart.com/Finance.owl#ValidPeriod"/>
        <hasStartTime rdf:datatype="&xsd;dateTime">2009-01-02T09:00:08</hasStartTime>
        <hasFinishTime rdf:datatype="&xsd;dateTime">2999-12-31T09:00:08</hasFinishTime>
    </owl:NamedIndividual>
    


    <!-- http://www.fadyart.com/Finance.owl#posFreezeCorporateAction -->

    <owl:NamedIndividual rdf:about="http://www.fadyart.com/Finance.owl#posFreezeCorporateAction">
        <rdf:type rdf:resource="http://www.fadyart.com/Finance.owl#ReasonForPositionFreeze"/>
        <rdfs:label xml:lang="en">Position frozen for corporate action</rdfs:label>
        <rdfs:comment xml:lang="en">A corporate action is ongoing.
E.g. coupon payment, equity exchange operation, convertion, rename, ...</rdfs:comment>
    </owl:NamedIndividual>
    


    <!-- http://www.fadyart.com/Finance.owl#posFreezeGuaranteeForThirdParty -->

    <owl:NamedIndividual rdf:about="http://www.fadyart.com/Finance.owl#posFreezeGuaranteeForThirdParty">
        <rdf:type rdf:resource="http://www.fadyart.com/Finance.owl#ReasonForPositionFreeze"/>
        <rdfs:label xml:lang="en">Posiition frozen as guarantee for third party</rdfs:label>
        <rdfs:comment xml:lang="en">The position serves as guarantee for a third party.
E.g. as guarantee for a rental contract of real estate, guarantee as member of board of directors, guarantee for public works,...</rdfs:comment>
    </owl:NamedIndividual>
    


    <!-- http://www.fadyart.com/Finance.owl#posFreezeIrregularForm -->

    <owl:NamedIndividual rdf:about="http://www.fadyart.com/Finance.owl#posFreezeIrregularForm">
        <rdf:type rdf:resource="http://www.fadyart.com/Finance.owl#ReasonForPositionFreeze"/>
        <rdfs:label xml:lang="en">Position froze due to irregular form of the instrument</rdfs:label>
        <rdfs:comment xml:lang="en">The financial instruments are damaged, unreadable, inidentifyable, ...</rdfs:comment>
    </owl:NamedIndividual>
    


    <!-- http://www.fadyart.com/Finance.owl#posFreezeNominative -->

    <owl:NamedIndividual rdf:about="http://www.fadyart.com/Finance.owl#posFreezeNominative">
        <rdf:type rdf:resource="http://www.fadyart.com/Finance.owl#ReasonForPositionFreeze"/>
        <rdfs:label xml:lang="en">Position frozen because the instument is nominative</rdfs:label>
        <rdfs:comment xml:lang="en">Nominative certificates, ADR/ADS,...</rdfs:comment>
    </owl:NamedIndividual>
    


    <!-- http://www.fadyart.com/Finance.owl#posFreezePledge -->

    <owl:NamedIndividual rdf:about="http://www.fadyart.com/Finance.owl#posFreezePledge">
        <rdf:type rdf:resource="http://www.fadyart.com/Finance.owl#ReasonForPositionFreeze"/>
        <rdfs:label xml:lang="en">Position frozen due to pledge</rdfs:label>
        <rdfs:comment xml:lang="en">Position serves as pledge for a loan by the principal.</rdfs:comment>
    </owl:NamedIndividual>
    


    <!-- http://www.fadyart.com/Finance.owl#posFreezeSalesOrder -->

    <owl:NamedIndividual rdf:about="http://www.fadyart.com/Finance.owl#posFreezeSalesOrder">
        <rdf:type rdf:resource="http://www.fadyart.com/Finance.owl#ReasonForPositionFreeze"/>
        <rdfs:label xml:lang="en">Position frozen  because a sales order is issued</rdfs:label>
        <rdfs:comment xml:lang="en">A sales order is still valid for the position.</rdfs:comment>
    </owl:NamedIndividual>
    


    <!-- http://www.fadyart.com/Finance.owl#posFreezeShareholdersMeeting -->

    <owl:NamedIndividual rdf:about="http://www.fadyart.com/Finance.owl#posFreezeShareholdersMeeting">
        <rdf:type rdf:resource="http://www.fadyart.com/Finance.owl#ReasonForPositionFreeze"/>
        <rdfs:label xml:lang="en">Position is frozen until after the shareholders meeting</rdfs:label>
        <rdfs:comment xml:lang="en">The accountholders registered their shares to exercise their voting rights.</rdfs:comment>
    </owl:NamedIndividual>
    


    <!-- http://www.fadyart.com/Finance.owl#posFreezeUnderInjunction -->

    <owl:NamedIndividual rdf:about="http://www.fadyart.com/Finance.owl#posFreezeUnderInjunction">
        <rdf:type rdf:resource="http://www.fadyart.com/Finance.owl#ReasonForPositionFreeze"/>
        <rdfs:label xml:lang="en">Position frozen due to injunction measures</rdfs:label>
        <rdfs:comment xml:lang="en">There is an injunction on the financial instruments due to fraud, theft, loss,...</rdfs:comment>
    </owl:NamedIndividual>
    


    <!-- http://www.fadyart.com/Finance.owl#rskSymptomAbnormalRemuneration -->

    <owl:NamedIndividual rdf:about="http://www.fadyart.com/Finance.owl#rskSymptomAbnormalRemuneration">
        <rdf:type rdf:resource="http://www.fadyart.com/Finance.owl#ManagementRiskSymptom"/>
        <rdfs:label rdf:datatype="&xsd;string">Abnormal remuneration</rdfs:label>
        <rdfs:comment rdf:datatype="&xsd;string">Abnormal high remunerations of the management team, linked to abnormal high departure indemnities in case of early break of the contract form an additional threath for the issuer.</rdfs:comment>
    </owl:NamedIndividual>
    


    <!-- http://www.fadyart.com/Finance.owl#rskSymptomAppreciation -->

    <owl:NamedIndividual rdf:about="http://www.fadyart.com/Finance.owl#rskSymptomAppreciation">
        <rdf:type rdf:resource="http://www.fadyart.com/Finance.owl#ExchangeRateRiskSymptom"/>
        <rdfs:label rdf:datatype="&xsd;string">The currency appreciation</rdfs:label>
        <rdfs:comment rdf:datatype="&xsd;string">The risk the value of the producers currency appreciates against the customers currency, this means :
- a more expensive product 
- less sales by the producer
- less profit by the issuer in the short term
- less solvability by the issuer in the long term

If the value of the holders currency appreciates against the holders currency, this means :
- less revenues in holders currency
- lower stock quotes because of the needed rentability uplift</rdfs:comment>
    </owl:NamedIndividual>
    


    <!-- http://www.fadyart.com/Finance.owl#rskSymptomBusinessIgnorance -->

    <owl:NamedIndividual rdf:about="http://www.fadyart.com/Finance.owl#rskSymptomBusinessIgnorance">
        <rdf:type rdf:resource="http://www.fadyart.com/Finance.owl#ManagementRiskSymptom"/>
        <rdfs:label rdf:datatype="&xsd;string">Ignorance about the business</rdfs:label>
        <rdfs:comment rdf:datatype="&xsd;string">Ignorance of the underlying business model and technicality of the producer or issuer.
Decisions are taken without sufficient knowledge of the context.</rdfs:comment>
    </owl:NamedIndividual>
    


    <!-- http://www.fadyart.com/Finance.owl#rskSymptomCommodityCostDecrease -->

    <owl:NamedIndividual rdf:about="http://www.fadyart.com/Finance.owl#rskSymptomCommodityCostDecrease">
        <rdf:type rdf:resource="http://www.fadyart.com/Finance.owl#CommodityCostRiskSymptom"/>
        <rdfs:label rdf:datatype="&xsd;string">Commodity cost decrease</rdfs:label>
        <rdfs:comment rdf:datatype="&xsd;string">If the commodity costs decrease, the costs of collaterals increase and the underlying assets of derivatives become less worth, thus:
- less profit by the issuer in the short term
- less solvability by the issuer in the long term

If the commodity costs decrease, the underlying values become less worth, thus:
- prices, thus valuation is lowered</rdfs:comment>
    </owl:NamedIndividual>
    


    <!-- http://www.fadyart.com/Finance.owl#rskSymptomCommodityCostIncrease -->

    <owl:NamedIndividual rdf:about="http://www.fadyart.com/Finance.owl#rskSymptomCommodityCostIncrease">
        <rdf:type rdf:resource="http://www.fadyart.com/Finance.owl#CommodityCostRiskSymptom"/>
        <rdfs:label rdf:datatype="&xsd;string">Comodity cost increase</rdfs:label>
        <rdfs:comment rdf:datatype="&xsd;string">If the commodity costs increase, the costs of production are increasing, thus:
- less sales by the producer
- less profit by the issuer in the short term
- less solvability by the issuer in the long term</rdfs:comment>
    </owl:NamedIndividual>
    


    <!-- http://www.fadyart.com/Finance.owl#rskSymptomConceited -->

    <owl:NamedIndividual rdf:about="http://www.fadyart.com/Finance.owl#rskSymptomConceited">
        <rdf:type rdf:resource="http://www.fadyart.com/Finance.owl#ManagementRiskSymptom"/>
        <rdfs:label rdf:datatype="&xsd;string">Conceited management</rdfs:label>
        <rdfs:comment rdf:datatype="&xsd;string">The management did not learn from errors in the past since there were no lessons to learn.</rdfs:comment>
    </owl:NamedIndividual>
    


    <!-- http://www.fadyart.com/Finance.owl#rskSymptomDecreasedDemocracy -->

    <owl:NamedIndividual rdf:about="http://www.fadyart.com/Finance.owl#rskSymptomDecreasedDemocracy">
        <rdf:type rdf:resource="http://www.fadyart.com/Finance.owl#PoliticalRiskSymptom"/>
        <rdfs:label rdf:datatype="&xsd;string">Democracy level is decreased</rdfs:label>
        <rdfs:comment rdf:datatype="&xsd;string">Political dictatures have a decreasing purchase power as consequence:
- less demand for the products
- less profit by the issuer in the short term
- less solvability by the issuer in the long term</rdfs:comment>
    </owl:NamedIndividual>
    


    <!-- http://www.fadyart.com/Finance.owl#rskSymptomDelayedDeliveries -->

    <owl:NamedIndividual rdf:about="http://www.fadyart.com/Finance.owl#rskSymptomDelayedDeliveries">
        <rdf:type rdf:resource="http://www.fadyart.com/Finance.owl#OperationalRiskSymptom"/>
        <rdfs:label rdf:datatype="&xsd;string">Delayed deliveries</rdfs:label>
        <rdfs:comment rdf:datatype="&xsd;string">Delayed deliveries damage the image of the producer/issuer with as consequence:
- less sales by the producer
- less profit by the issuer in the short term
- less solvability by the issuer in the long term</rdfs:comment>
    </owl:NamedIndividual>
    


    <!-- http://www.fadyart.com/Finance.owl#rskSymptomDepreciation -->

    <owl:NamedIndividual rdf:about="http://www.fadyart.com/Finance.owl#rskSymptomDepreciation">
        <rdf:type rdf:resource="http://www.fadyart.com/Finance.owl#ExchangeRateRiskSymptom"/>
        <rdfs:label rdf:datatype="&xsd;string">The currency depreciation</rdfs:label>
        <rdfs:comment rdf:datatype="&xsd;string">If the value of the customers currency depreciates against the producers currency, this means: 
- a more expensive product 
- less sales by the producer
- less profit by the issuer in the short term
- less solvability by the issuer in the long term

If the value of the issuers currency depreciates against the holders currency, this means :
- less revenues in holders currency
- lower stock quotes because of the needed rentability uplift</rdfs:comment>
    </owl:NamedIndividual>
    


    <!-- http://www.fadyart.com/Finance.owl#rskSymptomEnergyCostIncrease -->

    <owl:NamedIndividual rdf:about="http://www.fadyart.com/Finance.owl#rskSymptomEnergyCostIncrease">
        <rdf:type rdf:resource="http://www.fadyart.com/Finance.owl#EnergyCostRiskSymptom"/>
        <rdfs:label rdf:datatype="&xsd;string">Energy cost increase</rdfs:label>
        <rdfs:comment rdf:datatype="&xsd;string">If the energy costs increase, the costs of production are increasing, thus:
- less sales by the producer
- less profit by the issuer in the short term
- less solvability by the issuer in the long term</rdfs:comment>
    </owl:NamedIndividual>
    


    <!-- http://www.fadyart.com/Finance.owl#rskSymptomExportEmbargo -->

    <owl:NamedIndividual rdf:about="http://www.fadyart.com/Finance.owl#rskSymptomExportEmbargo">
        <rdf:type rdf:resource="http://www.fadyart.com/Finance.owl#PoliticalRiskSymptom"/>
        <rdfs:label rdf:datatype="&xsd;string">Export embargo</rdfs:label>
        <rdfs:comment rdf:datatype="&xsd;string">If the products cannot be exported to certain customers, this means:
- less sales by the producer
- less profit by the issuer in the short term
- less solvability by the issuer in the long term</rdfs:comment>
    </owl:NamedIndividual>
    


    <!-- http://www.fadyart.com/Finance.owl#rskSymptomHigherFiscalPressure -->

    <owl:NamedIndividual rdf:about="http://www.fadyart.com/Finance.owl#rskSymptomHigherFiscalPressure">
        <rdf:type rdf:resource="http://www.fadyart.com/Finance.owl#FiscalRiskSymptom"/>
        <rdfs:label rdf:datatype="&xsd;string">Higher fiscal pressure</rdfs:label>
        <rdfs:comment rdf:datatype="&xsd;string">If the customer has to pay more taxes, his consumption is reduced with those directly or indirectly :
- less sales by the producer
- less profit by the issuer in the short term
- less solvability by the issuer in the long term

If there are tax increases on the profits of producers, e.g. ruling is abolished:
- less profit by the producer
- less profit by the issuer in the short term
- less solvability by the issuer in the long term

If there are tax increases on the activities of issuers, e.g. stock market tax:
- less profit by the issuer in the short term
- less solvability by the issuer in the long term

If the fiscal pressure on stock increases, e.g. through higher prepaid tax rates, this means:
- less net profit for the holder
- less demand for the stock
- prices, thus valuation falling</rdfs:comment>
    </owl:NamedIndividual>
    


    <!-- http://www.fadyart.com/Finance.owl#rskSymptomIdeology -->

    <owl:NamedIndividual rdf:about="http://www.fadyart.com/Finance.owl#rskSymptomIdeology">
        <rdf:type rdf:resource="http://www.fadyart.com/Finance.owl#PoliticalRiskSymptom"/>
        <rdfs:label rdf:datatype="&xsd;string">Ideology with tradition of failing economy</rdfs:label>
        <rdfs:comment rdf:datatype="&xsd;string">Political parties can have a tradition in halting economic development of the nation:
- less demand for the products
- less profit by the issuer in the short term
- less solvability by the issuer in the long term</rdfs:comment>
    </owl:NamedIndividual>
    


    <!-- http://www.fadyart.com/Finance.owl#rskSymptomImportEmbargo -->

    <owl:NamedIndividual rdf:about="http://www.fadyart.com/Finance.owl#rskSymptomImportEmbargo">
        <rdf:type rdf:resource="http://www.fadyart.com/Finance.owl#PoliticalRiskSymptom"/>
        <rdfs:label rdf:datatype="&xsd;string">Import embargo</rdfs:label>
        <rdfs:comment rdf:datatype="&xsd;string">If the products are subject to e.g. an import embargo:
- less sales by the producer
- less profit by the issuer in the short term
- less solvability by the issuer in the long term</rdfs:comment>
    </owl:NamedIndividual>
    


    <!-- http://www.fadyart.com/Finance.owl#rskSymptomImportRestriction -->

    <owl:NamedIndividual rdf:about="http://www.fadyart.com/Finance.owl#rskSymptomImportRestriction">
        <rdf:type rdf:resource="http://www.fadyart.com/Finance.owl#RegulatoryRiskSymptom"/>
        <rdfs:label rdf:datatype="&xsd;string">Import restriction</rdfs:label>
        <rdfs:comment rdf:datatype="&xsd;string">The markets in the scope are the export markets of the issuer or the producers.
If the products are subject to e.g. an import restriction, the target is to reduce the share of imported products on the local market with as a consequence:
- less sales by the producer
- less profit by the issuer in the short term
- less solvability by the issuer in the long term</rdfs:comment>
    </owl:NamedIndividual>
    


    <!-- http://www.fadyart.com/Finance.owl#rskSymptomInterestRateRise -->

    <owl:NamedIndividual rdf:about="http://www.fadyart.com/Finance.owl#rskSymptomInterestRateRise">
        <rdf:type rdf:resource="http://www.fadyart.com/Finance.owl#InterestRateRiskSymptom"/>
        <rdfs:label rdf:datatype="&xsd;string">Rise of interest rates</rdfs:label>
        <rdfs:comment rdf:datatype="&xsd;string">If the customer has to pay more interests for credits, his consumption is reduced with direct or indirect :
- less sales by the producer
- less profit by the issuer in the short term
- less solvability by the issuer in the long term

If the producer has to pay more interests for credits, his profitability is reduced, meaning:
- less profit by the issuer in the short term
- less solvability by the issuer in the long term

If the market interests rise in the issuers area, the issuer has to provide a higher rentability too, meaning:
- less solvability by the issuer in the long term

If the market interests rise in the holders area, the rentability of the current investments lowers.
To keep the rentability uplevel, the underlying value is lowered.</rdfs:comment>
    </owl:NamedIndividual>
    


    <!-- http://www.fadyart.com/Finance.owl#rskSymptomLegalRestrictionOnProduction -->

    <owl:NamedIndividual rdf:about="http://www.fadyart.com/Finance.owl#rskSymptomLegalRestrictionOnProduction">
        <rdf:type rdf:resource="http://www.fadyart.com/Finance.owl#LegalRestrictionRiskSymptom"/>
        <rdfs:label rdf:datatype="&xsd;string">Legal restriction on production</rdfs:label>
        <rdfs:comment rdf:datatype="&xsd;string">If there are legal restrictions on the production by the producers, e.g. cars with high carbon dioxide emission:
- less sales by the producer
- less profit by the issuer in the short term
- less solvability by the issuer in the long term</rdfs:comment>
    </owl:NamedIndividual>
    


    <!-- http://www.fadyart.com/Finance.owl#rskSymptomLegalRestrictionOnStockTrade -->

    <owl:NamedIndividual rdf:about="http://www.fadyart.com/Finance.owl#rskSymptomLegalRestrictionOnStockTrade">
        <rdf:type rdf:resource="http://www.fadyart.com/Finance.owl#LegalRestrictionRiskSymptom"/>
        <rdfs:label rdf:datatype="&xsd;string">Legal restriction on stock trade</rdfs:label>
        <rdfs:comment rdf:datatype="&xsd;string">If there are legal restrictions on the issuance of stock, e.g. stock with mortgages as collateral are evaluated less than 100%, this means:
- need more collaterals as guarantee for loans
- increased costs for borrowing
- less profit by the issuer in the short term
- less solvability by the issuer in the long term

If the purchase of stock is legally restricted, e.g. of so-called fiscal paradises, this means:
- less demand for the stock
- prices, thus valuation falling</rdfs:comment>
    </owl:NamedIndividual>
    


    <!-- http://www.fadyart.com/Finance.owl#rskSymptomLegalRestrictionsOnSales -->

    <owl:NamedIndividual rdf:about="http://www.fadyart.com/Finance.owl#rskSymptomLegalRestrictionsOnSales">
        <rdf:type rdf:resource="http://www.fadyart.com/Finance.owl#LegalRestrictionRiskSymptom"/>
        <rdfs:label rdf:datatype="&xsd;string">Legal restriction on sales</rdfs:label>
        <rdfs:comment rdf:datatype="&xsd;string">If there are legal restrictions on the purchases by the customers, e.g. alcohol by young persons:
- less sales by the producer
- less profit by the issuer in the short term
- less solvability by the issuer in the long term</rdfs:comment>
    </owl:NamedIndividual>
    


    <!-- http://www.fadyart.com/Finance.owl#rskSymptomNationalization -->

    <owl:NamedIndividual rdf:about="http://www.fadyart.com/Finance.owl#rskSymptomNationalization">
        <rdf:type rdf:resource="http://www.fadyart.com/Finance.owl#PoliticalRiskSymptom"/>
        <rdfs:label rdf:datatype="&xsd;string">Nationalization</rdfs:label>
        <rdfs:comment rdf:datatype="&xsd;string">If the issuer or producers are nationalized, this means:
- profits are going down in the general interest
- less profit by the issuer in the short term
- less solvability by the issuer in the long term</rdfs:comment>
    </owl:NamedIndividual>
    


    <!-- http://www.fadyart.com/Finance.owl#rskSymptomPoorQuality -->

    <owl:NamedIndividual rdf:about="http://www.fadyart.com/Finance.owl#rskSymptomPoorQuality">
        <rdf:type rdf:resource="http://www.fadyart.com/Finance.owl#OperationalRiskSymptom"/>
        <rdfs:label rdf:datatype="&xsd;string">Poor quality</rdfs:label>
        <rdfs:comment rdf:datatype="&xsd;string">Poor quality damages the image of the producer/issuer with as consequence:
- less sales by the producer
- less profit by the issuer in the short term
- less solvability by the issuer in the long term</rdfs:comment>
    </owl:NamedIndividual>
    


    <!-- http://www.fadyart.com/Finance.owl#rskSymptomReducedPurchasePower -->

    <owl:NamedIndividual rdf:about="http://www.fadyart.com/Finance.owl#rskSymptomReducedPurchasePower">
        <rdf:type rdf:resource="http://www.fadyart.com/Finance.owl#ClientRiskSymptom"/>
        <rdfs:label rdf:datatype="&xsd;string">Reduced purchase power</rdfs:label>
        <rdfs:comment rdf:datatype="&xsd;string">If the customers are subject to purchase power reductions, the consequence is:
- less sales by the producer
- less profit by the issuer in the short term
- less solvability by the issuer in the long term

If the producers are subject to reduced purchase power, the purchases become more expensive:
- less sales by the producer
- less profit by the issuer in the short term
- less solvability by the issuer in the long term</rdfs:comment>
    </owl:NamedIndividual>
    


    <!-- http://www.fadyart.com/Finance.owl#rskSymptomReducedStockLiquidity -->

    <owl:NamedIndividual rdf:about="http://www.fadyart.com/Finance.owl#rskSymptomReducedStockLiquidity">
        <rdf:type rdf:resource="http://www.fadyart.com/Finance.owl#LiquidityRiskSymptom"/>
        <rdfs:label rdf:datatype="&xsd;string">Reduced stock liquidity</rdfs:label>
        <rdfs:comment rdf:datatype="&xsd;string">If the stock is less liquid then investors will require a compensation for it.</rdfs:comment>
    </owl:NamedIndividual>
    


    <!-- http://www.fadyart.com/Finance.owl#rskSymptomReputationDamage -->

    <owl:NamedIndividual rdf:about="http://www.fadyart.com/Finance.owl#rskSymptomReputationDamage">
        <rdf:type rdf:resource="http://www.fadyart.com/Finance.owl#ReputationalRiskSymptom"/>
        <rdfs:label rdf:datatype="&xsd;string">Damage to the reputation</rdfs:label>
        <rdfs:comment rdf:datatype="&xsd;string">If the reputation of the producer is at risk, e.g. child labour in shoe manufacturies, this means:
- less sales by the producer
- less profit by the issuer in the short term
- less solvability by the issuer in the long term

If the reputation of the issuer is at risk, e.g. anti-trust investigations, this means:
- less profit by the issuer in the short term
- less solvability by the issuer in the long term

If the reputation of the holder is at risk, e.g. mafia connections of major shareholders, this means:
- less demand for the stock
- prices, thus valuation falling</rdfs:comment>
    </owl:NamedIndividual>
    


    <!-- http://www.fadyart.com/Finance.owl#rskSymptomStockTradeRestrictions -->

    <owl:NamedIndividual rdf:about="http://www.fadyart.com/Finance.owl#rskSymptomStockTradeRestrictions">
        <rdf:type rdf:resource="http://www.fadyart.com/Finance.owl#LiquidityRiskSymptom"/>
        <rdfs:label rdf:datatype="&xsd;string">Stock trade restrictions</rdfs:label>
        <rdfs:comment rdf:datatype="&xsd;string">If some capital markets would become unaccessible:
- less capital gathering possibilities
- less profit by the issuer in the short term
- less solvability by the issuer in the long term</rdfs:comment>
    </owl:NamedIndividual>
    


    <!-- http://www.fadyart.com/Finance.owl#rskSymptomStringentTechnicalSpecification -->

    <owl:NamedIndividual rdf:about="http://www.fadyart.com/Finance.owl#rskSymptomStringentTechnicalSpecification">
        <rdf:type rdf:resource="http://www.fadyart.com/Finance.owl#RegulatoryRiskSymptom"/>
        <rdfs:label rdf:datatype="&xsd;string">Stringent technical specification</rdfs:label>
        <rdfs:comment rdf:datatype="&xsd;string">If the products are subject to e.g. stringent technical specifications, the consequence in first instance will be:
- less sales by the producer
- less profit by the issuer in the short term
- less solvability by the issuer in the long term</rdfs:comment>
    </owl:NamedIndividual>
    


    <!-- http://www.fadyart.com/Finance.owl#rskSymptomUnderlying-CollateralWorthLoss -->

    <owl:NamedIndividual rdf:about="http://www.fadyart.com/Finance.owl#rskSymptomUnderlying-CollateralWorthLoss">
        <rdf:type rdf:resource="http://www.fadyart.com/Finance.owl#Underlying-CollateralRiskSymptom"/>
        <rdfs:label rdf:datatype="&xsd;string">Loss of worth of the underlying or collateral</rdfs:label>
        <rdfs:comment rdf:datatype="&xsd;string">If the underlying assets become less worth, this means:
- less profit by the issuer in the short term
- less solvability by the issuer in the long term

If the underlying values become less worth, this means:
- prices, thus valuation is lowered</rdfs:comment>
    </owl:NamedIndividual>
    


    <!-- http://www.fadyart.com/Finance.owl#rskSymptomUnexperiencedManagement -->

    <owl:NamedIndividual rdf:about="http://www.fadyart.com/Finance.owl#rskSymptomUnexperiencedManagement">
        <rdf:type rdf:resource="http://www.fadyart.com/Finance.owl#ManagementRiskSymptom"/>
        <rdfs:label rdf:datatype="&xsd;string">Unexperienced management</rdfs:label>
        <rdfs:comment rdf:datatype="&xsd;string">The management did not learn from errors in the past since there were no errors commitet</rdfs:comment>
    </owl:NamedIndividual>
    


    <!-- http://www.fadyart.com/Finance.owl#rskSymptomUnprofessionalApproach -->

    <owl:NamedIndividual rdf:about="http://www.fadyart.com/Finance.owl#rskSymptomUnprofessionalApproach">
        <rdf:type rdf:resource="http://www.fadyart.com/Finance.owl#ManagementRiskSymptom"/>
        <rdfs:label rdf:datatype="&xsd;string">Unprofessional approach</rdfs:label>
        <rdfs:comment rdf:datatype="&xsd;string">In stead of thorough case studies, the management uses vague criteria to justify decisions:
- from the stomac
- by intuition
- based on &quot;feeling&quot;</rdfs:comment>
    </owl:NamedIndividual>
    


    <!-- http://www.fadyart.com/Finance.owl#rskSymptomsManagementErrors -->

    <owl:NamedIndividual rdf:about="http://www.fadyart.com/Finance.owl#rskSymptomsManagementErrors">
        <rdf:type rdf:resource="http://www.fadyart.com/Finance.owl#ManagementRiskSymptom"/>
        <rdfs:label rdf:datatype="&xsd;string">Management errors</rdfs:label>
        <rdfs:comment rdf:datatype="&xsd;string">Pure but mainly judgement errors from members of the management team.</rdfs:comment>
    </owl:NamedIndividual>
    


    <!-- http://www.fadyart.com/Finance.owl#veryLowDirectStockPriceImpact -->

    <owl:NamedIndividual rdf:about="http://www.fadyart.com/Finance.owl#veryLowDirectStockPriceImpact">
        <rdf:type rdf:resource="http://www.fadyart.com/Finance.owl#LowStockPriceImpact"/>
        <rdfs:label rdf:datatype="&xsd;string">Very low direct stock price impact</rdfs:label>
    </owl:NamedIndividual>
    


    <!-- http://www.fadyart.com/Finance.owl#veryLowIndirectStockPriceImpact -->

    <owl:NamedIndividual rdf:about="http://www.fadyart.com/Finance.owl#veryLowIndirectStockPriceImpact">
        <rdf:type rdf:resource="http://www.fadyart.com/Finance.owl#LowStockPriceImpact"/>
        <rdfs:label rdf:datatype="&xsd;string">Very low indirect stock price impact</rdfs:label>
    </owl:NamedIndividual>
    


    <!-- http://www.fadyart.com/Finance.owl#veryLowProfitabilityImpact -->

    <owl:NamedIndividual rdf:about="http://www.fadyart.com/Finance.owl#veryLowProfitabilityImpact">
        <rdf:type rdf:resource="http://www.fadyart.com/Finance.owl#LowProfitabilityImpact"/>
        <rdfs:label rdf:datatype="&xsd;string">Very low profitability impact</rdfs:label>
    </owl:NamedIndividual>
    


    <!-- http://www.fadyart.com/Finance.owl#veryLowSolvabilityImpact -->

    <owl:NamedIndividual rdf:about="http://www.fadyart.com/Finance.owl#veryLowSolvabilityImpact">
        <rdf:type rdf:resource="http://www.fadyart.com/Finance.owl#LowSolvabilityImpact"/>
        <rdfs:label rdf:datatype="&xsd;string">Very low solvability impact</rdfs:label>
    </owl:NamedIndividual>
    


    <!-- http://www.fadyart.com/iso10962#B-MortgageBackedDebt -->

    <owl:NamedIndividual rdf:about="http://www.fadyart.com/iso10962#B-MortgageBackedDebt"/>
    


    <!-- http://www.fadyart.com/parties#genericPartyDataProvider -->

    <owl:NamedIndividual rdf:about="&parties;genericPartyDataProvider">
        <rdf:type rdf:resource="&parties;Organisation"/>
    </owl:NamedIndividual>
    


    <!-- 
    ///////////////////////////////////////////////////////////////////////////////////////
    //
    // Annotations
    //
    ///////////////////////////////////////////////////////////////////////////////////////
     -->

    <rdf:Description rdf:about="&isic;Code">
        <dc:source rdf:datatype="&xsd;string">http://unstats.un.org/unsd/cr/registry/regdnld.asp?Lg=1</dc:source>
    </rdf:Description>
</rdf:RDF>



<!-- Generated by the OWL API (version 3.4.2) http://owlapi.sourceforge.net -->

